<?xml version="1.0"?>


<!DOCTYPE rdf:RDF [
    <!ENTITY owl "http://www.w3.org/2002/07/owl#" >
    <!ENTITY xsd "http://www.w3.org/2001/XMLSchema#" >
    <!ENTITY owl2xml "http://www.w3.org/2006/12/owl2-xml#" >
    <!ENTITY rdfs "http://www.w3.org/2000/01/rdf-schema#" >
    <!ENTITY rdf "http://www.w3.org/1999/02/22-rdf-syntax-ns#" >
    <!ENTITY XCLOntology1 "http://www.semanticweb.org/ontologies/2008/7/XCLOntology1.5.owl#" >
    <!ENTITY PDF "http://www.semanticweb.org/ontologies/2008/7/XCLOntology1.5.owl#PDF/" >
    <!ENTITY XCLOntology12 "http://www.semanticweb.org/ontologies/2008/7/XCLOntology1.5.owl#1931" >
    <!ENTITY b "http://www.semanticweb.org/ontologies/2008/7/XCLOntology1.5.owl#L*a*b*" >
    <!ENTITY Times "http://www.semanticweb.org/ontologies/2008/7/XCLOntology1.5.owl#Times&#8722;" >
    <!ENTITY Courier "http://www.semanticweb.org/ontologies/2008/7/XCLOntology1.5.owl#Courier&#8722;" >
    <!ENTITY package "http://www.semanticweb.org/ontologies/2008/7/XCLOntology1.5.owl#package&#39;" >
    <!ENTITY Helvetica "http://www.semanticweb.org/ontologies/2008/7/XCLOntology1.5.owl#Helvetica&#8722;" >
    <!ENTITY YphysScanResolution "http://www.semanticweb.org/ontologies/2008/7/XCLOntology1.5.owl#YphysScanResolution&#8211;" >
    <!ENTITY PrimaryChromaticities_GreenY "http://www.semanticweb.org/ontologies/2008/7/XCLOntology1.5.owl#PrimaryChromaticities_GreenY&#8211;" >
]>


<rdf:RDF xmlns="http://www.semanticweb.org/ontologies/2008/7/XCLOntology1.5.owl#"
     xml:base="http://www.semanticweb.org/ontologies/2008/7/XCLOntology1.5.owl"
     xmlns:owl2xml="http://www.w3.org/2006/12/owl2-xml#"
     xmlns:Helvetica="&XCLOntology1;Helvetica&#8722;"
     xmlns:YphysScanResolution="&XCLOntology1;YphysScanResolution&#8211;"
     xmlns:PrimaryChromaticities_GreenY="&XCLOntology1;PrimaryChromaticities_GreenY&#8211;"
     xmlns:Times="&XCLOntology1;Times&#8722;"
     xmlns:xsd="http://www.w3.org/2001/XMLSchema#"
     xmlns:XCLOntology12="&XCLOntology1;1931"
     xmlns:rdfs="http://www.w3.org/2000/01/rdf-schema#"
     xmlns:b="&XCLOntology1;L*a*b*"
     xmlns:owl="http://www.w3.org/2002/07/owl#"
     xmlns:PDF="&XCLOntology1;PDF/"
     xmlns:XCLOntology1="http://www.semanticweb.org/ontologies/2008/7/XCLOntology1.5.owl#"
     xmlns:rdf="http://www.w3.org/1999/02/22-rdf-syntax-ns#"
     xmlns:package="&XCLOntology1;package&#39;"
     xmlns:Courier="&XCLOntology1;Courier&#8722;">
    <owl:Ontology rdf:about=""/>
    


    <!-- 
    ///////////////////////////////////////////////////////////////////////////////////////
    //
    // Annotation properties
    //
    ///////////////////////////////////////////////////////////////////////////////////////
     -->

    <owl:AnnotationProperty rdf:about="#Datatype"/>
    <owl:AnnotationProperty rdf:about="#Restriction"/>
    <owl:AnnotationProperty rdf:about="#ID"/>
    <owl:AnnotationProperty rdf:about="#Unit"/>
    


    <!-- 
    ///////////////////////////////////////////////////////////////////////////////////////
    //
    // Object Properties
    //
    ///////////////////////////////////////////////////////////////////////////////////////
     -->

    


    <!-- http://www.semanticweb.org/ontologies/2008/7/XCLOntology1.5.owl#devideBy10 -->

    <owl:ObjectProperty rdf:about="#devideBy10"/>
    


    <!-- http://www.semanticweb.org/ontologies/2008/7/XCLOntology1.5.owl#enumToRealValues -->

    <owl:ObjectProperty rdf:about="#enumToRealValues">
        <rdfs:comment
            >requires specific algorithms</rdfs:comment>
    </owl:ObjectProperty>
    


    <!-- http://www.semanticweb.org/ontologies/2008/7/XCLOntology1.5.owl#has_specificationProperties -->

    <owl:ObjectProperty rdf:about="#has_specificationProperties"/>
    


    <!-- http://www.semanticweb.org/ontologies/2008/7/XCLOntology1.5.owl#has_specificationPropertiesBMP -->

    <owl:ObjectProperty rdf:about="#has_specificationPropertiesBMP">
        <rdfs:domain rdf:resource="#BMP"/>
        <rdfs:range rdf:resource="#BMP_Properties"/>
        <rdfs:subPropertyOf rdf:resource="#has_specificationProperties"/>
    </owl:ObjectProperty>
    


    <!-- http://www.semanticweb.org/ontologies/2008/7/XCLOntology1.5.owl#has_specificationPropertiesJPEG -->

    <owl:ObjectProperty rdf:about="#has_specificationPropertiesJPEG">
        <rdfs:domain rdf:resource="#JPEG_JFIF"/>
        <rdfs:range rdf:resource="#JPEG_Properties"/>
        <rdfs:subPropertyOf rdf:resource="#has_specificationProperties"/>
    </owl:ObjectProperty>
    


    <!-- http://www.semanticweb.org/ontologies/2008/7/XCLOntology1.5.owl#has_specificationPropertiesJPEG2000 -->

    <owl:ObjectProperty rdf:about="#has_specificationPropertiesJPEG2000">
        <rdfs:range rdf:resource="#JPEG2000_Properties"/>
        <rdfs:domain rdf:resource="#JPEG_2000"/>
        <rdfs:subPropertyOf rdf:resource="#has_specificationProperties"/>
    </owl:ObjectProperty>
    


    <!-- http://www.semanticweb.org/ontologies/2008/7/XCLOntology1.5.owl#has_specificationPropertiesMPEG1 -->

    <owl:ObjectProperty rdf:about="#has_specificationPropertiesMPEG1">
        <rdfs:subPropertyOf rdf:resource="#has_specificationProperties"/>
    </owl:ObjectProperty>
    


    <!-- http://www.semanticweb.org/ontologies/2008/7/XCLOntology1.5.owl#has_specificationPropertiesMPEG2 -->

    <owl:ObjectProperty rdf:about="#has_specificationPropertiesMPEG2">
        <rdfs:subPropertyOf rdf:resource="#has_specificationProperties"/>
    </owl:ObjectProperty>
    


    <!-- http://www.semanticweb.org/ontologies/2008/7/XCLOntology1.5.owl#has_specificationPropertiesMPEG4 -->

    <owl:ObjectProperty rdf:about="#has_specificationPropertiesMPEG4">
        <rdfs:domain rdf:resource="#MP4"/>
        <rdfs:range rdf:resource="#MPEG4_Properties"/>
        <rdfs:subPropertyOf rdf:resource="#has_specificationProperties"/>
    </owl:ObjectProperty>
    


    <!-- http://www.semanticweb.org/ontologies/2008/7/XCLOntology1.5.owl#has_specificationPropertiesMsWord97 -->

    <owl:ObjectProperty rdf:about="#has_specificationPropertiesMsWord97">
        <rdfs:range rdf:resource="#MsWord97_Properties"/>
        <rdfs:domain rdf:resource="#Word_1997"/>
        <rdfs:subPropertyOf rdf:resource="#has_specificationProperties"/>
    </owl:ObjectProperty>
    


    <!-- http://www.semanticweb.org/ontologies/2008/7/XCLOntology1.5.owl#has_specificationPropertiesTiff -->

    <owl:ObjectProperty rdf:about="#has_specificationPropertiesTiff">
        <rdfs:domain rdf:resource="#TIFF6"/>
        <rdfs:range rdf:resource="#Tiff_Properties"/>
        <rdfs:subPropertyOf rdf:resource="#has_specificationProperties"/>
    </owl:ObjectProperty>
    


    <!-- http://www.semanticweb.org/ontologies/2008/7/XCLOntology1.5.owl#has_specificationProperties_DOCX -->

    <owl:ObjectProperty rdf:about="#has_specificationProperties_DOCX">
        <rdfs:domain rdf:resource="#DOCX"/>
        <rdfs:range rdf:resource="#DOCX_Properties"/>
        <rdfs:subPropertyOf rdf:resource="#has_specificationProperties"/>
    </owl:ObjectProperty>
    


    <!-- http://www.semanticweb.org/ontologies/2008/7/XCLOntology1.5.owl#has_specificationProperties_Gif -->

    <owl:ObjectProperty rdf:about="#has_specificationProperties_Gif">
        <rdfs:domain rdf:resource="#GIF"/>
        <rdfs:range rdf:resource="#GIF_Properties"/>
        <rdfs:subPropertyOf rdf:resource="#has_specificationProperties"/>
    </owl:ObjectProperty>
    


    <!-- http://www.semanticweb.org/ontologies/2008/7/XCLOntology1.5.owl#has_specificationProperties_PNG -->

    <owl:ObjectProperty rdf:about="#has_specificationProperties_PNG">
        <rdfs:domain rdf:resource="#PNG"/>
        <rdfs:range rdf:resource="#PNG_Properties"/>
        <rdfs:subPropertyOf rdf:resource="#has_specificationProperties"/>
    </owl:ObjectProperty>
    


    <!-- http://www.semanticweb.org/ontologies/2008/7/XCLOntology1.5.owl#has_specificationProperties_Pdf1.3 -->

    <owl:ObjectProperty rdf:about="#has_specificationProperties_Pdf1.3">
        <rdfs:range rdf:resource="#PDF1.3_Properties"/>
        <rdfs:domain rdf:resource="#PDF_1.3"/>
        <rdfs:subPropertyOf rdf:resource="#has_specificationProperties"/>
    </owl:ObjectProperty>
    


    <!-- http://www.semanticweb.org/ontologies/2008/7/XCLOntology1.5.owl#is_same_as -->

    <owl:ObjectProperty rdf:about="#is_same_as">
        <rdf:type rdf:resource="&owl;SymmetricProperty"/>
        <rdfs:comment
            >for equivalent properties</rdfs:comment>
    </owl:ObjectProperty>
    


    <!-- 
    ///////////////////////////////////////////////////////////////////////////////////////
    //
    // Classes
    //
    ///////////////////////////////////////////////////////////////////////////////////////
     -->

    


    <!-- http://www.semanticweb.org/ontologies/2008/7/XCLOntology1.5.owl#AIFF -->

    <owl:Class rdf:about="#AIFF">
        <rdfs:subClassOf rdf:resource="#Audiofile"/>
        <owl:disjointWith rdf:resource="#WMA"/>
    </owl:Class>
    


    <!-- http://www.semanticweb.org/ontologies/2008/7/XCLOntology1.5.owl#AI_CS -->

    <owl:Class rdf:about="#AI_CS">
        <rdfs:subClassOf rdf:resource="#Vector_Image"/>
    </owl:Class>
    


    <!-- http://www.semanticweb.org/ontologies/2008/7/XCLOntology1.5.owl#AI_until_Version_9 -->

    <owl:Class rdf:about="#AI_until_Version_9">
        <rdfs:subClassOf rdf:resource="#Vector_Image"/>
    </owl:Class>
    


    <!-- http://www.semanticweb.org/ontologies/2008/7/XCLOntology1.5.owl#AMV -->

    <owl:Class rdf:about="#AMV">
        <rdfs:subClassOf rdf:resource="#Videofile"/>
    </owl:Class>
    


    <!-- http://www.semanticweb.org/ontologies/2008/7/XCLOntology1.5.owl#AVC -->

    <owl:Class rdf:about="#AVC">
        <owl:equivalentClass rdf:resource="#MPEG4_Part15"/>
        <rdfs:subClassOf rdf:resource="#Videofile"/>
    </owl:Class>
    


    <!-- http://www.semanticweb.org/ontologies/2008/7/XCLOntology1.5.owl#Arial -->

    <owl:Class rdf:about="#Arial">
        <rdfs:subClassOf rdf:resource="#Fonts"/>
    </owl:Class>
    


    <!-- http://www.semanticweb.org/ontologies/2008/7/XCLOntology1.5.owl#Arial_Bold -->

    <owl:Class rdf:about="#Arial_Bold">
        <rdfs:subClassOf rdf:resource="#Fonts"/>
    </owl:Class>
    


    <!-- http://www.semanticweb.org/ontologies/2008/7/XCLOntology1.5.owl#Arial_Bold_Italic -->

    <owl:Class rdf:about="#Arial_Bold_Italic">
        <rdfs:subClassOf rdf:resource="#Fonts"/>
    </owl:Class>
    


    <!-- http://www.semanticweb.org/ontologies/2008/7/XCLOntology1.5.owl#Arial_Italic -->

    <owl:Class rdf:about="#Arial_Italic">
        <rdfs:subClassOf rdf:resource="#Fonts"/>
    </owl:Class>
    


    <!-- http://www.semanticweb.org/ontologies/2008/7/XCLOntology1.5.owl#Audiofile -->

    <owl:Class rdf:about="#Audiofile">
        <rdfs:subClassOf rdf:resource="#fileObjects"/>
        <rdfs:comment
            >includes all Audiofiletypes</rdfs:comment>
    </owl:Class>
    


    <!-- http://www.semanticweb.org/ontologies/2008/7/XCLOntology1.5.owl#BMP -->

    <owl:Class rdf:about="#BMP">
        <rdfs:subClassOf rdf:resource="#Raster_Image"/>
    </owl:Class>
    


    <!-- http://www.semanticweb.org/ontologies/2008/7/XCLOntology1.5.owl#BMP_Properties -->

    <owl:Class rdf:about="#BMP_Properties">
        <rdfs:subClassOf rdf:resource="#specificationPropertyNames"/>
    </owl:Class>
    


    <!-- http://www.semanticweb.org/ontologies/2008/7/XCLOntology1.5.owl#Courier(PC) -->

    <owl:Class rdf:about="#Courier(PC)">
        <rdfs:subClassOf rdf:resource="#Fonts"/>
    </owl:Class>
    


    <!-- http://www.semanticweb.org/ontologies/2008/7/XCLOntology1.5.owl#Courier_New -->

    <owl:Class rdf:about="#Courier_New">
        <rdfs:subClassOf rdf:resource="#Fonts"/>
    </owl:Class>
    


    <!-- http://www.semanticweb.org/ontologies/2008/7/XCLOntology1.5.owl#Courier_New_Bold -->

    <owl:Class rdf:about="#Courier_New_Bold">
        <rdfs:subClassOf rdf:resource="#Fonts"/>
    </owl:Class>
    


    <!-- http://www.semanticweb.org/ontologies/2008/7/XCLOntology1.5.owl#Courier_New_Bold_Italic -->

    <owl:Class rdf:about="#Courier_New_Bold_Italic">
        <rdfs:subClassOf rdf:resource="#Fonts"/>
    </owl:Class>
    


    <!-- http://www.semanticweb.org/ontologies/2008/7/XCLOntology1.5.owl#Courier_New_Italic -->

    <owl:Class rdf:about="#Courier_New_Italic">
        <rdfs:subClassOf rdf:resource="#Fonts"/>
    </owl:Class>
    


    <!-- http://www.semanticweb.org/ontologies/2008/7/XCLOntology1.5.owl#DOCX -->

    <owl:Class rdf:about="#DOCX">
        <rdfs:subClassOf rdf:resource="#OOXML"/>
    </owl:Class>
    


    <!-- http://www.semanticweb.org/ontologies/2008/7/XCLOntology1.5.owl#DOCX_Properties -->

    <owl:Class rdf:about="#DOCX_Properties">
        <rdfs:subClassOf rdf:resource="#specificationPropertyNames"/>
    </owl:Class>
    


    <!-- http://www.semanticweb.org/ontologies/2008/7/XCLOntology1.5.owl#EPS -->

    <owl:Class rdf:about="#EPS">
        <rdfs:subClassOf rdf:resource="#Vector_Image"/>
    </owl:Class>
    


    <!-- http://www.semanticweb.org/ontologies/2008/7/XCLOntology1.5.owl#FLV -->

    <owl:Class rdf:about="#FLV">
        <rdfs:subClassOf rdf:resource="#Videofile"/>
    </owl:Class>
    


    <!-- http://www.semanticweb.org/ontologies/2008/7/XCLOntology1.5.owl#Fonts -->

    <owl:Class rdf:about="#Fonts">
        <rdfs:subClassOf rdf:resource="#Mixed_File"/>
        <rdfs:comment xml:lang="en"
            >font_systemfiles</rdfs:comment>
    </owl:Class>
    


    <!-- http://www.semanticweb.org/ontologies/2008/7/XCLOntology1.5.owl#GIF -->

    <owl:Class rdf:about="#GIF">
        <rdfs:subClassOf rdf:resource="#Raster_Image"/>
    </owl:Class>
    


    <!-- http://www.semanticweb.org/ontologies/2008/7/XCLOntology1.5.owl#GIF_Properties -->

    <owl:Class rdf:about="#GIF_Properties">
        <rdfs:subClassOf rdf:resource="#specificationPropertyNames"/>
    </owl:Class>
    


    <!-- http://www.semanticweb.org/ontologies/2008/7/XCLOntology1.5.owl#GIS_Formats -->

    <owl:Class rdf:about="#GIS_Formats">
        <rdfs:subClassOf rdf:resource="#Mixed_File"/>
    </owl:Class>
    


    <!-- http://www.semanticweb.org/ontologies/2008/7/XCLOntology1.5.owl#Html -->

    <owl:Class rdf:about="#Html">
        <rdfs:subClassOf rdf:resource="#Mixed_File"/>
    </owl:Class>
    


    <!-- http://www.semanticweb.org/ontologies/2008/7/XCLOntology1.5.owl#ID -->

    <owl:Class rdf:about="#ID">
        <rdfs:subClassOf rdf:resource="#concepts"/>
    </owl:Class>
    


    <!-- http://www.semanticweb.org/ontologies/2008/7/XCLOntology1.5.owl#Imagefile -->

    <owl:Class rdf:about="#Imagefile">
        <rdfs:subClassOf rdf:resource="#fileObjects"/>
        <rdfs:comment
            >includes all Imagefiletypes</rdfs:comment>
    </owl:Class>
    


    <!-- http://www.semanticweb.org/ontologies/2008/7/XCLOntology1.5.owl#JHOVE -->

    <owl:Class rdf:about="#JHOVE">
        <rdfs:subClassOf rdf:resource="#metadataStandards"/>
    </owl:Class>
    


    <!-- http://www.semanticweb.org/ontologies/2008/7/XCLOntology1.5.owl#JPEG2000_Properties -->

    <owl:Class rdf:about="#JPEG2000_Properties">
        <rdfs:subClassOf rdf:resource="#specificationPropertyNames"/>
    </owl:Class>
    


    <!-- http://www.semanticweb.org/ontologies/2008/7/XCLOntology1.5.owl#JPEG_2000 -->

    <owl:Class rdf:about="#JPEG_2000">
        <rdfs:subClassOf rdf:resource="#Raster_Image"/>
    </owl:Class>
    


    <!-- http://www.semanticweb.org/ontologies/2008/7/XCLOntology1.5.owl#JPEG_JFIF -->

    <owl:Class rdf:about="#JPEG_JFIF">
        <rdfs:subClassOf rdf:resource="#Raster_Image"/>
    </owl:Class>
    


    <!-- http://www.semanticweb.org/ontologies/2008/7/XCLOntology1.5.owl#JPEG_Properties -->

    <owl:Class rdf:about="#JPEG_Properties">
        <rdfs:subClassOf rdf:resource="#specificationPropertyNames"/>
    </owl:Class>
    


    <!-- http://www.semanticweb.org/ontologies/2008/7/XCLOntology1.5.owl#M4A -->

    <owl:Class rdf:about="#M4A">
        <rdfs:subClassOf rdf:resource="#Audiofile"/>
    </owl:Class>
    


    <!-- http://www.semanticweb.org/ontologies/2008/7/XCLOntology1.5.owl#MOV -->

    <owl:Class rdf:about="#MOV">
        <rdfs:subClassOf rdf:resource="#Videofile"/>
    </owl:Class>
    


    <!-- http://www.semanticweb.org/ontologies/2008/7/XCLOntology1.5.owl#MP1 -->

    <owl:Class rdf:about="#MP1">
        <owl:equivalentClass rdf:resource="#MPEG1_Layer1"/>
        <rdfs:subClassOf rdf:resource="#Audiofile"/>
    </owl:Class>
    


    <!-- http://www.semanticweb.org/ontologies/2008/7/XCLOntology1.5.owl#MP2 -->

    <owl:Class rdf:about="#MP2">
        <owl:equivalentClass rdf:resource="#MPEG1_Layer2"/>
        <rdfs:subClassOf rdf:resource="#Audiofile"/>
    </owl:Class>
    


    <!-- http://www.semanticweb.org/ontologies/2008/7/XCLOntology1.5.owl#MP3 -->

    <owl:Class rdf:about="#MP3">
        <owl:equivalentClass rdf:resource="#MPEG1_Layer3"/>
        <rdfs:subClassOf rdf:resource="#Audiofile"/>
    </owl:Class>
    


    <!-- http://www.semanticweb.org/ontologies/2008/7/XCLOntology1.5.owl#MP4 -->

    <owl:Class rdf:about="#MP4">
        <owl:equivalentClass rdf:resource="#MPEG4_Part14"/>
        <rdfs:subClassOf rdf:resource="#Videofile"/>
    </owl:Class>
    


    <!-- http://www.semanticweb.org/ontologies/2008/7/XCLOntology1.5.owl#MPEG -->

    <owl:Class rdf:about="#MPEG">
        <rdfs:subClassOf rdf:resource="#Mixed_File"/>
    </owl:Class>
    


    <!-- http://www.semanticweb.org/ontologies/2008/7/XCLOntology1.5.owl#MPEG1 -->

    <owl:Class rdf:about="#MPEG1">
        <rdfs:subClassOf rdf:resource="#MPEG"/>
    </owl:Class>
    


    <!-- http://www.semanticweb.org/ontologies/2008/7/XCLOntology1.5.owl#MPEG1_Layer1 -->

    <owl:Class rdf:about="#MPEG1_Layer1">
        <rdfs:subClassOf rdf:resource="#MPEG1_Part3"/>
    </owl:Class>
    


    <!-- http://www.semanticweb.org/ontologies/2008/7/XCLOntology1.5.owl#MPEG1_Layer2 -->

    <owl:Class rdf:about="#MPEG1_Layer2">
        <rdfs:subClassOf rdf:resource="#MPEG1_Part3"/>
        <rdfs:comment xml:lang="en">for Audio</rdfs:comment>
    </owl:Class>
    


    <!-- http://www.semanticweb.org/ontologies/2008/7/XCLOntology1.5.owl#MPEG1_Layer3 -->

    <owl:Class rdf:about="#MPEG1_Layer3">
        <rdfs:subClassOf rdf:resource="#MPEG1_Part3"/>
        <rdfs:comment xml:lang="en"
            >Also known as MP3</rdfs:comment>
    </owl:Class>
    


    <!-- http://www.semanticweb.org/ontologies/2008/7/XCLOntology1.5.owl#MPEG1_Part1 -->

    <owl:Class rdf:about="#MPEG1_Part1">
        <rdfs:subClassOf rdf:resource="#MPEG1"/>
    </owl:Class>
    


    <!-- http://www.semanticweb.org/ontologies/2008/7/XCLOntology1.5.owl#MPEG1_Part2 -->

    <owl:Class rdf:about="#MPEG1_Part2">
        <owl:equivalentClass rdf:resource="#MPG1"/>
        <rdfs:subClassOf rdf:resource="#MPEG1"/>
    </owl:Class>
    


    <!-- http://www.semanticweb.org/ontologies/2008/7/XCLOntology1.5.owl#MPEG1_Part3 -->

    <owl:Class rdf:about="#MPEG1_Part3">
        <rdfs:subClassOf rdf:resource="#MPEG1"/>
    </owl:Class>
    


    <!-- http://www.semanticweb.org/ontologies/2008/7/XCLOntology1.5.owl#MPEG1_Properties -->

    <owl:Class rdf:about="#MPEG1_Properties">
        <rdfs:subClassOf rdf:resource="#specificationPropertyNames"/>
        <rdfs:comment xml:lang="en"
            >Properties and Metrics of MPEG1-files from the fileformat-specification</rdfs:comment>
    </owl:Class>
    


    <!-- http://www.semanticweb.org/ontologies/2008/7/XCLOntology1.5.owl#MPEG2 -->

    <owl:Class rdf:about="#MPEG2">
        <rdfs:subClassOf rdf:resource="#MPEG"/>
        <rdfs:comment xml:lang="en"
            >MPEG-2 is a standard for &quot;the generic coding of moving pictures and associated audio information&quot;</rdfs:comment>
    </owl:Class>
    


    <!-- http://www.semanticweb.org/ontologies/2008/7/XCLOntology1.5.owl#MPEG2_Part1 -->

    <owl:Class rdf:about="#MPEG2_Part1">
        <rdfs:subClassOf rdf:resource="#MPEG2"/>
    </owl:Class>
    


    <!-- http://www.semanticweb.org/ontologies/2008/7/XCLOntology1.5.owl#MPEG2_Part10 -->

    <owl:Class rdf:about="#MPEG2_Part10">
        <rdfs:subClassOf rdf:resource="#MPEG2"/>
    </owl:Class>
    


    <!-- http://www.semanticweb.org/ontologies/2008/7/XCLOntology1.5.owl#MPEG2_Part2 -->

    <owl:Class rdf:about="#MPEG2_Part2">
        <rdfs:subClassOf rdf:resource="#MPEG2"/>
    </owl:Class>
    


    <!-- http://www.semanticweb.org/ontologies/2008/7/XCLOntology1.5.owl#MPEG2_Part3 -->

    <owl:Class rdf:about="#MPEG2_Part3">
        <rdfs:subClassOf rdf:resource="#MPEG2"/>
    </owl:Class>
    


    <!-- http://www.semanticweb.org/ontologies/2008/7/XCLOntology1.5.owl#MPEG2_Part4 -->

    <owl:Class rdf:about="#MPEG2_Part4">
        <rdfs:subClassOf rdf:resource="#MPEG2"/>
    </owl:Class>
    


    <!-- http://www.semanticweb.org/ontologies/2008/7/XCLOntology1.5.owl#MPEG2_Part5 -->

    <owl:Class rdf:about="#MPEG2_Part5">
        <rdfs:subClassOf rdf:resource="#MPEG2"/>
    </owl:Class>
    


    <!-- http://www.semanticweb.org/ontologies/2008/7/XCLOntology1.5.owl#MPEG2_Part6 -->

    <owl:Class rdf:about="#MPEG2_Part6">
        <rdfs:subClassOf rdf:resource="#MPEG2"/>
    </owl:Class>
    


    <!-- http://www.semanticweb.org/ontologies/2008/7/XCLOntology1.5.owl#MPEG2_Part7 -->

    <owl:Class rdf:about="#MPEG2_Part7">
        <rdfs:subClassOf rdf:resource="#MPEG2"/>
    </owl:Class>
    


    <!-- http://www.semanticweb.org/ontologies/2008/7/XCLOntology1.5.owl#MPEG2_Part8 -->

    <owl:Class rdf:about="#MPEG2_Part8">
        <rdfs:subClassOf rdf:resource="#MPEG2"/>
    </owl:Class>
    


    <!-- http://www.semanticweb.org/ontologies/2008/7/XCLOntology1.5.owl#MPEG2_Part9 -->

    <owl:Class rdf:about="#MPEG2_Part9">
        <rdfs:subClassOf rdf:resource="#MPEG2"/>
    </owl:Class>
    


    <!-- http://www.semanticweb.org/ontologies/2008/7/XCLOntology1.5.owl#MPEG2_Properties -->

    <owl:Class rdf:about="#MPEG2_Properties">
        <rdfs:subClassOf rdf:resource="#specificationPropertyNames"/>
    </owl:Class>
    


    <!-- http://www.semanticweb.org/ontologies/2008/7/XCLOntology1.5.owl#MPEG4 -->

    <owl:Class rdf:about="#MPEG4">
        <rdfs:subClassOf rdf:resource="#MPEG"/>
    </owl:Class>
    


    <!-- http://www.semanticweb.org/ontologies/2008/7/XCLOntology1.5.owl#MPEG4_Part1 -->

    <owl:Class rdf:about="#MPEG4_Part1">
        <rdfs:subClassOf rdf:resource="#MPEG4"/>
    </owl:Class>
    


    <!-- http://www.semanticweb.org/ontologies/2008/7/XCLOntology1.5.owl#MPEG4_Part10 -->

    <owl:Class rdf:about="#MPEG4_Part10">
        <rdfs:subClassOf rdf:resource="#MPEG4"/>
    </owl:Class>
    


    <!-- http://www.semanticweb.org/ontologies/2008/7/XCLOntology1.5.owl#MPEG4_Part11 -->

    <owl:Class rdf:about="#MPEG4_Part11">
        <rdfs:subClassOf rdf:resource="#MPEG4"/>
    </owl:Class>
    


    <!-- http://www.semanticweb.org/ontologies/2008/7/XCLOntology1.5.owl#MPEG4_Part12 -->

    <owl:Class rdf:about="#MPEG4_Part12">
        <rdfs:subClassOf rdf:resource="#MPEG4"/>
    </owl:Class>
    


    <!-- http://www.semanticweb.org/ontologies/2008/7/XCLOntology1.5.owl#MPEG4_Part13 -->

    <owl:Class rdf:about="#MPEG4_Part13">
        <rdfs:subClassOf rdf:resource="#MPEG4"/>
    </owl:Class>
    


    <!-- http://www.semanticweb.org/ontologies/2008/7/XCLOntology1.5.owl#MPEG4_Part14 -->

    <owl:Class rdf:about="#MPEG4_Part14">
        <rdfs:subClassOf rdf:resource="#MPEG4"/>
    </owl:Class>
    


    <!-- http://www.semanticweb.org/ontologies/2008/7/XCLOntology1.5.owl#MPEG4_Part15 -->

    <owl:Class rdf:about="#MPEG4_Part15">
        <rdfs:subClassOf rdf:resource="#MPEG4"/>
    </owl:Class>
    


    <!-- http://www.semanticweb.org/ontologies/2008/7/XCLOntology1.5.owl#MPEG4_Part16 -->

    <owl:Class rdf:about="#MPEG4_Part16">
        <rdfs:subClassOf rdf:resource="#MPEG4"/>
    </owl:Class>
    


    <!-- http://www.semanticweb.org/ontologies/2008/7/XCLOntology1.5.owl#MPEG4_Part17 -->

    <owl:Class rdf:about="#MPEG4_Part17">
        <rdfs:subClassOf rdf:resource="#MPEG4"/>
    </owl:Class>
    


    <!-- http://www.semanticweb.org/ontologies/2008/7/XCLOntology1.5.owl#MPEG4_Part18 -->

    <owl:Class rdf:about="#MPEG4_Part18">
        <rdfs:subClassOf rdf:resource="#MPEG4"/>
    </owl:Class>
    


    <!-- http://www.semanticweb.org/ontologies/2008/7/XCLOntology1.5.owl#MPEG4_Part19 -->

    <owl:Class rdf:about="#MPEG4_Part19">
        <rdfs:subClassOf rdf:resource="#MPEG4"/>
    </owl:Class>
    


    <!-- http://www.semanticweb.org/ontologies/2008/7/XCLOntology1.5.owl#MPEG4_Part2 -->

    <owl:Class rdf:about="#MPEG4_Part2">
        <rdfs:subClassOf rdf:resource="#MPEG4"/>
        <rdfs:comment xml:lang="en"
            >Codec for visual data (video, still textures, synthetic images, etc.)</rdfs:comment>
    </owl:Class>
    


    <!-- http://www.semanticweb.org/ontologies/2008/7/XCLOntology1.5.owl#MPEG4_Part20 -->

    <owl:Class rdf:about="#MPEG4_Part20">
        <rdfs:subClassOf rdf:resource="#MPEG4"/>
    </owl:Class>
    


    <!-- http://www.semanticweb.org/ontologies/2008/7/XCLOntology1.5.owl#MPEG4_Part21 -->

    <owl:Class rdf:about="#MPEG4_Part21">
        <rdfs:subClassOf rdf:resource="#MPEG4"/>
    </owl:Class>
    


    <!-- http://www.semanticweb.org/ontologies/2008/7/XCLOntology1.5.owl#MPEG4_Part22 -->

    <owl:Class rdf:about="#MPEG4_Part22">
        <rdfs:subClassOf rdf:resource="#MPEG4"/>
        <rdfs:comment xml:lang="en"
            >Open Font Format Specification (OFFS) based on OpenType...</rdfs:comment>
    </owl:Class>
    


    <!-- http://www.semanticweb.org/ontologies/2008/7/XCLOntology1.5.owl#MPEG4_Part23 -->

    <owl:Class rdf:about="#MPEG4_Part23">
        <rdfs:subClassOf rdf:resource="#MPEG4"/>
    </owl:Class>
    


    <!-- http://www.semanticweb.org/ontologies/2008/7/XCLOntology1.5.owl#MPEG4_Part3 -->

    <owl:Class rdf:about="#MPEG4_Part3">
        <rdfs:subClassOf rdf:resource="#MPEG4"/>
    </owl:Class>
    


    <!-- http://www.semanticweb.org/ontologies/2008/7/XCLOntology1.5.owl#MPEG4_Part4 -->

    <owl:Class rdf:about="#MPEG4_Part4">
        <rdfs:subClassOf rdf:resource="#MPEG4"/>
        <rdfs:comment xml:lang="en"
            >reference software specification</rdfs:comment>
    </owl:Class>
    


    <!-- http://www.semanticweb.org/ontologies/2008/7/XCLOntology1.5.owl#MPEG4_Part5 -->

    <owl:Class rdf:about="#MPEG4_Part5">
        <rdfs:subClassOf rdf:resource="#MPEG4"/>
        <rdfs:comment xml:lang="en"
            >conformance bit-streams specification</rdfs:comment>
    </owl:Class>
    


    <!-- http://www.semanticweb.org/ontologies/2008/7/XCLOntology1.5.owl#MPEG4_Part6 -->

    <owl:Class rdf:about="#MPEG4_Part6">
        <rdfs:subClassOf rdf:resource="#MPEG4"/>
    </owl:Class>
    


    <!-- http://www.semanticweb.org/ontologies/2008/7/XCLOntology1.5.owl#MPEG4_Part7 -->

    <owl:Class rdf:about="#MPEG4_Part7">
        <rdfs:subClassOf rdf:resource="#MPEG4"/>
    </owl:Class>
    


    <!-- http://www.semanticweb.org/ontologies/2008/7/XCLOntology1.5.owl#MPEG4_Part8 -->

    <owl:Class rdf:about="#MPEG4_Part8">
        <rdfs:subClassOf rdf:resource="#MPEG4"/>
    </owl:Class>
    


    <!-- http://www.semanticweb.org/ontologies/2008/7/XCLOntology1.5.owl#MPEG4_Part9 -->

    <owl:Class rdf:about="#MPEG4_Part9">
        <rdfs:subClassOf rdf:resource="#MPEG4"/>
    </owl:Class>
    


    <!-- http://www.semanticweb.org/ontologies/2008/7/XCLOntology1.5.owl#MPEG4_Properties -->

    <owl:Class rdf:about="#MPEG4_Properties">
        <rdfs:subClassOf rdf:resource="#specificationPropertyNames"/>
    </owl:Class>
    


    <!-- http://www.semanticweb.org/ontologies/2008/7/XCLOntology1.5.owl#MPG1 -->

    <owl:Class rdf:about="#MPG1">
        <rdfs:subClassOf rdf:resource="#Videofile"/>
    </owl:Class>
    


    <!-- http://www.semanticweb.org/ontologies/2008/7/XCLOntology1.5.owl#Mixed_File -->

    <owl:Class rdf:about="#Mixed_File">
        <rdfs:subClassOf rdf:resource="#fileObjects"/>
        <rdfs:comment
            >includes all complex filetypes, which are composed of different mediatypes</rdfs:comment>
    </owl:Class>
    


    <!-- http://www.semanticweb.org/ontologies/2008/7/XCLOntology1.5.owl#MsWord97_Properties -->

    <owl:Class rdf:about="#MsWord97_Properties">
        <rdfs:subClassOf rdf:resource="#specificationPropertyNames"/>
    </owl:Class>
    


    <!-- http://www.semanticweb.org/ontologies/2008/7/XCLOntology1.5.owl#NISO -->

    <owl:Class rdf:about="#NISO">
        <rdfs:subClassOf rdf:resource="#metadataStandards"/>
    </owl:Class>
    


    <!-- http://www.semanticweb.org/ontologies/2008/7/XCLOntology1.5.owl#ODF -->

    <owl:Class rdf:about="#ODF">
        <rdfs:subClassOf rdf:resource="#Textfile"/>
    </owl:Class>
    


    <!-- http://www.semanticweb.org/ontologies/2008/7/XCLOntology1.5.owl#OOXML -->

    <owl:Class rdf:about="#OOXML">
        <rdfs:subClassOf rdf:resource="#OfficeFormats"/>
    </owl:Class>
    


    <!-- http://www.semanticweb.org/ontologies/2008/7/XCLOntology1.5.owl#OfficeFormats -->

    <owl:Class rdf:about="#OfficeFormats">
        <rdfs:subClassOf rdf:resource="#Textfile"/>
    </owl:Class>
    


    <!-- http://www.semanticweb.org/ontologies/2008/7/XCLOntology1.5.owl#OpenDocument_Properties -->

    <owl:Class rdf:about="#OpenDocument_Properties">
        <rdfs:subClassOf rdf:resource="#specificationPropertyNames"/>
    </owl:Class>
    


    <!-- http://www.semanticweb.org/ontologies/2008/7/XCLOntology1.5.owl#PDF/a_Properties -->

    <owl:Class rdf:about="#PDF/a_Properties">
        <rdfs:subClassOf rdf:resource="#specificationPropertyNames"/>
    </owl:Class>
    


    <!-- http://www.semanticweb.org/ontologies/2008/7/XCLOntology1.5.owl#PDF1.3_Properties -->

    <owl:Class rdf:about="#PDF1.3_Properties">
        <rdfs:subClassOf rdf:resource="#specificationPropertyNames"/>
    </owl:Class>
    


    <!-- http://www.semanticweb.org/ontologies/2008/7/XCLOntology1.5.owl#PDFFormats -->

    <owl:Class rdf:about="#PDFFormats">
        <rdfs:subClassOf rdf:resource="#Textfile"/>
    </owl:Class>
    


    <!-- http://www.semanticweb.org/ontologies/2008/7/XCLOntology1.5.owl#PDF_1.0 -->

    <owl:Class rdf:about="#PDF_1.0">
        <rdfs:subClassOf rdf:resource="#PDFFormats"/>
    </owl:Class>
    


    <!-- http://www.semanticweb.org/ontologies/2008/7/XCLOntology1.5.owl#PDF_1.3 -->

    <owl:Class rdf:about="#PDF_1.3">
        <rdfs:subClassOf rdf:resource="#PDFFormats"/>
    </owl:Class>
    


    <!-- http://www.semanticweb.org/ontologies/2008/7/XCLOntology1.5.owl#PDF_1.4 -->

    <owl:Class rdf:about="#PDF_1.4">
        <rdfs:subClassOf rdf:resource="#PDFFormats"/>
    </owl:Class>
    


    <!-- http://www.semanticweb.org/ontologies/2008/7/XCLOntology1.5.owl#PDF_1.5 -->

    <owl:Class rdf:about="#PDF_1.5">
        <rdfs:subClassOf rdf:resource="#PDFFormats"/>
    </owl:Class>
    


    <!-- http://www.semanticweb.org/ontologies/2008/7/XCLOntology1.5.owl#PDF_1.6 -->

    <owl:Class rdf:about="#PDF_1.6">
        <rdfs:subClassOf rdf:resource="#PDFFormats"/>
    </owl:Class>
    


    <!-- http://www.semanticweb.org/ontologies/2008/7/XCLOntology1.5.owl#PDF_X -->

    <owl:Class rdf:about="#PDF_X">
        <rdfs:subClassOf rdf:resource="#PDFFormats"/>
    </owl:Class>
    


    <!-- http://www.semanticweb.org/ontologies/2008/7/XCLOntology1.5.owl#PNG -->

    <owl:Class rdf:about="#PNG">
        <rdfs:subClassOf rdf:resource="#Raster_Image"/>
    </owl:Class>
    


    <!-- http://www.semanticweb.org/ontologies/2008/7/XCLOntology1.5.owl#PNG_Properties -->

    <owl:Class rdf:about="#PNG_Properties">
        <rdfs:subClassOf rdf:resource="#specificationPropertyNames"/>
    </owl:Class>
    


    <!-- http://www.semanticweb.org/ontologies/2008/7/XCLOntology1.5.owl#PPTX -->

    <owl:Class rdf:about="#PPTX">
        <rdfs:subClassOf rdf:resource="#OOXML"/>
    </owl:Class>
    


    <!-- http://www.semanticweb.org/ontologies/2008/7/XCLOntology1.5.owl#RTF -->

    <owl:Class rdf:about="#RTF">
        <rdfs:subClassOf rdf:resource="#Textfile"/>
    </owl:Class>
    


    <!-- http://www.semanticweb.org/ontologies/2008/7/XCLOntology1.5.owl#Raster_Image -->

    <owl:Class rdf:about="#Raster_Image">
        <rdfs:subClassOf rdf:resource="#Imagefile"/>
    </owl:Class>
    


    <!-- http://www.semanticweb.org/ontologies/2008/7/XCLOntology1.5.owl#SVG -->

    <owl:Class rdf:about="#SVG">
        <rdfs:subClassOf rdf:resource="#Vector_Image"/>
    </owl:Class>
    


    <!-- http://www.semanticweb.org/ontologies/2008/7/XCLOntology1.5.owl#SVG_Properties -->

    <owl:Class rdf:about="#SVG_Properties">
        <rdfs:subClassOf rdf:resource="#specificationPropertyNames"/>
    </owl:Class>
    


    <!-- http://www.semanticweb.org/ontologies/2008/7/XCLOntology1.5.owl#Symbol(PC) -->

    <owl:Class rdf:about="#Symbol(PC)">
        <rdfs:subClassOf rdf:resource="#Fonts"/>
    </owl:Class>
    


    <!-- http://www.semanticweb.org/ontologies/2008/7/XCLOntology1.5.owl#TIFF6 -->

    <owl:Class rdf:about="#TIFF6">
        <rdfs:subClassOf rdf:resource="#Raster_Image"/>
    </owl:Class>
    


    <!-- http://www.semanticweb.org/ontologies/2008/7/XCLOntology1.5.owl#TextMD -->

    <owl:Class rdf:about="#TextMD">
        <rdfs:subClassOf rdf:resource="#metadataStandards"/>
    </owl:Class>
    


    <!-- http://www.semanticweb.org/ontologies/2008/7/XCLOntology1.5.owl#Textfile -->

    <owl:Class rdf:about="#Textfile">
        <rdfs:subClassOf rdf:resource="#fileObjects"/>
        <rdfs:comment
            >includes all Textfiletypes</rdfs:comment>
    </owl:Class>
    


    <!-- http://www.semanticweb.org/ontologies/2008/7/XCLOntology1.5.owl#Tiff_Properties -->

    <owl:Class rdf:about="#Tiff_Properties">
        <rdfs:subClassOf rdf:resource="#specificationPropertyNames"/>
    </owl:Class>
    


    <!-- http://www.semanticweb.org/ontologies/2008/7/XCLOntology1.5.owl#Times_New_Roman -->

    <owl:Class rdf:about="#Times_New_Roman">
        <rdfs:subClassOf rdf:resource="#Fonts"/>
    </owl:Class>
    


    <!-- http://www.semanticweb.org/ontologies/2008/7/XCLOntology1.5.owl#Times_New_Roman_Bold -->

    <owl:Class rdf:about="#Times_New_Roman_Bold">
        <rdfs:subClassOf rdf:resource="#Fonts"/>
    </owl:Class>
    


    <!-- http://www.semanticweb.org/ontologies/2008/7/XCLOntology1.5.owl#Times_New_Roman_Bold_Italic -->

    <owl:Class rdf:about="#Times_New_Roman_Bold_Italic">
        <rdfs:subClassOf rdf:resource="#Fonts"/>
    </owl:Class>
    


    <!-- http://www.semanticweb.org/ontologies/2008/7/XCLOntology1.5.owl#Times_New_Roman_Italic -->

    <owl:Class rdf:about="#Times_New_Roman_Italic">
        <rdfs:subClassOf rdf:resource="#Fonts"/>
    </owl:Class>
    


    <!-- http://www.semanticweb.org/ontologies/2008/7/XCLOntology1.5.owl#Vector_Image -->

    <owl:Class rdf:about="#Vector_Image">
        <rdfs:subClassOf rdf:resource="#Imagefile"/>
        <rdfs:comment xml:lang="en"
            >Can eather be subclass of Imagefile or subclass of Mixed_File because vectorfiles can also contain text</rdfs:comment>
    </owl:Class>
    


    <!-- http://www.semanticweb.org/ontologies/2008/7/XCLOntology1.5.owl#Videofile -->

    <owl:Class rdf:about="#Videofile">
        <rdfs:subClassOf rdf:resource="#fileObjects"/>
    </owl:Class>
    


    <!-- http://www.semanticweb.org/ontologies/2008/7/XCLOntology1.5.owl#WAV -->

    <owl:Class rdf:about="#WAV">
        <rdfs:subClassOf rdf:resource="#Videofile"/>
    </owl:Class>
    


    <!-- http://www.semanticweb.org/ontologies/2008/7/XCLOntology1.5.owl#WMA -->

    <owl:Class rdf:about="#WMA">
        <rdfs:subClassOf rdf:resource="#Audiofile"/>
    </owl:Class>
    


    <!-- http://www.semanticweb.org/ontologies/2008/7/XCLOntology1.5.owl#WMV -->

    <owl:Class rdf:about="#WMV">
        <rdfs:subClassOf rdf:resource="#Videofile"/>
    </owl:Class>
    


    <!-- http://www.semanticweb.org/ontologies/2008/7/XCLOntology1.5.owl#WingDings -->

    <owl:Class rdf:about="#WingDings">
        <rdfs:subClassOf rdf:resource="#Fonts"/>
    </owl:Class>
    


    <!-- http://www.semanticweb.org/ontologies/2008/7/XCLOntology1.5.owl#Word_1997 -->

    <owl:Class rdf:about="#Word_1997">
        <rdfs:subClassOf rdf:resource="#OfficeFormats"/>
    </owl:Class>
    


    <!-- http://www.semanticweb.org/ontologies/2008/7/XCLOntology1.5.owl#Word_2000 -->

    <owl:Class rdf:about="#Word_2000">
        <rdfs:subClassOf rdf:resource="#OfficeFormats"/>
    </owl:Class>
    


    <!-- http://www.semanticweb.org/ontologies/2008/7/XCLOntology1.5.owl#Word_2004 -->

    <owl:Class rdf:about="#Word_2004">
        <rdfs:subClassOf rdf:resource="#OfficeFormats"/>
    </owl:Class>
    


    <!-- http://www.semanticweb.org/ontologies/2008/7/XCLOntology1.5.owl#Word_X_Mac -->

    <owl:Class rdf:about="#Word_X_Mac">
        <rdfs:subClassOf rdf:resource="#DOCX"/>
        <owl:disjointWith rdf:resource="#Word_X_Windows"/>
    </owl:Class>
    


    <!-- http://www.semanticweb.org/ontologies/2008/7/XCLOntology1.5.owl#Word_X_Windows -->

    <owl:Class rdf:about="#Word_X_Windows">
        <rdfs:subClassOf rdf:resource="#DOCX"/>
    </owl:Class>
    


    <!-- http://www.semanticweb.org/ontologies/2008/7/XCLOntology1.5.owl#XCL_Properties -->

    <owl:Class rdf:about="#XCL_Properties">
        <rdfs:subClassOf rdf:resource="&owl;Thing"/>
    </owl:Class>
    


    <!-- http://www.semanticweb.org/ontologies/2008/7/XCLOntology1.5.owl#XLSX -->

    <owl:Class rdf:about="#XLSX">
        <rdfs:subClassOf rdf:resource="#OOXML"/>
    </owl:Class>
    


    <!-- http://www.semanticweb.org/ontologies/2008/7/XCLOntology1.5.owl#Zapf_Dingbats -->

    <owl:Class rdf:about="#Zapf_Dingbats">
        <rdfs:subClassOf rdf:resource="#Fonts"/>
    </owl:Class>
    


    <!-- http://www.semanticweb.org/ontologies/2008/7/XCLOntology1.5.owl#audioInformation -->

    <owl:Class rdf:about="#audioInformation">
        <rdfs:subClassOf rdf:resource="#XCL_Properties"/>
    </owl:Class>
    


    <!-- http://www.semanticweb.org/ontologies/2008/7/XCLOntology1.5.owl#block -->

    <owl:Class rdf:about="#block">
        <rdfs:subClassOf rdf:resource="#MPEG1_Properties"/>
        <rdfs:comment xml:lang="en"
            >An 8-row by 8-column orthogonal block of pels</rdfs:comment>
    </owl:Class>
    


    <!-- http://www.semanticweb.org/ontologies/2008/7/XCLOntology1.5.owl#concepts -->

    <owl:Class rdf:about="#concepts">
        <rdfs:subClassOf rdf:resource="&owl;Thing"/>
    </owl:Class>
    


    <!-- http://www.semanticweb.org/ontologies/2008/7/XCLOntology1.5.owl#fileObjects -->

    <owl:Class rdf:about="#fileObjects">
        <rdfs:subClassOf rdf:resource="&owl;Thing"/>
    </owl:Class>
    


    <!-- http://www.semanticweb.org/ontologies/2008/7/XCLOntology1.5.owl#fontDescriptor -->

    <owl:Class rdf:about="#fontDescriptor">
        <rdfs:subClassOf rdf:resource="#PDF1.3_Properties"/>
        <rdfs:comment xml:lang="en"
            >A font descriptor describing the font&#8217;s metrics other than its glyph widths (see Section 5.7, &#8220;Font Descriptors&#8221;). 
Note: For the standard 14 fonts, the entries FirstChar, LastChar, Widths, and
FontDescriptor must either all be present or all be absent. [cit. PDF 1.7]</rdfs:comment>
    </owl:Class>
    


    <!-- http://www.semanticweb.org/ontologies/2008/7/XCLOntology1.5.owl#fontFlag -->

    <owl:Class rdf:about="#fontFlag">
        <rdfs:subClassOf rdf:resource="#PDF1.3_Properties"/>
        <rdfs:comment xml:lang="en"
            >The value of the Flags entry in a font descriptor is an unsigned 32-bit integer containing flags specifying various characteristics of the font. Bit positions within the flag word are numbered from 1 (low-order) to 32 (high-order). Table 5.20 shows the meanings of the flags; all undefined flag bits are reserved and must be set to 0.</rdfs:comment>
    </owl:Class>
    


    <!-- http://www.semanticweb.org/ontologies/2008/7/XCLOntology1.5.owl#generalInformation -->

    <owl:Class rdf:about="#generalInformation">
        <rdfs:subClassOf rdf:resource="#XCL_Properties"/>
    </owl:Class>
    


    <!-- http://www.semanticweb.org/ontologies/2008/7/XCLOntology1.5.owl#imageInformation -->

    <owl:Class rdf:about="#imageInformation">
        <rdfs:subClassOf rdf:resource="#XCL_Properties"/>
    </owl:Class>
    


    <!-- http://www.semanticweb.org/ontologies/2008/7/XCLOntology1.5.owl#layers -->

    <owl:Class rdf:about="#layers">
        <rdfs:subClassOf rdf:resource="#MPEG1_Properties"/>
        <rdfs:comment xml:lang="en"
            >Layer descriptions for MPEG</rdfs:comment>
    </owl:Class>
    


    <!-- http://www.semanticweb.org/ontologies/2008/7/XCLOntology1.5.owl#metadataStandards -->

    <owl:Class rdf:about="#metadataStandards">
        <rdfs:subClassOf rdf:resource="&owl;Thing"/>
    </owl:Class>
    


    <!-- http://www.semanticweb.org/ontologies/2008/7/XCLOntology1.5.owl#otherInformation -->

    <owl:Class rdf:about="#otherInformation">
        <rdfs:subClassOf rdf:resource="#XCL_Properties"/>
    </owl:Class>
    


    <!-- http://www.semanticweb.org/ontologies/2008/7/XCLOntology1.5.owl#property_restriction -->

    <owl:Class rdf:about="#property_restriction">
        <rdfs:subClassOf rdf:resource="#concepts"/>
    </owl:Class>
    


    <!-- http://www.semanticweb.org/ontologies/2008/7/XCLOntology1.5.owl#rasterInformation -->

    <owl:Class rdf:about="#rasterInformation">
        <rdfs:subClassOf rdf:resource="#imageInformation"/>
    </owl:Class>
    


    <!-- http://www.semanticweb.org/ontologies/2008/7/XCLOntology1.5.owl#specificationPropertyNames -->

    <owl:Class rdf:about="#specificationPropertyNames">
        <rdfs:subClassOf rdf:resource="&owl;Thing"/>
    </owl:Class>
    


    <!-- http://www.semanticweb.org/ontologies/2008/7/XCLOntology1.5.owl#textInformation -->

    <owl:Class rdf:about="#textInformation">
        <rdfs:subClassOf rdf:resource="#XCL_Properties"/>
    </owl:Class>
    


    <!-- http://www.semanticweb.org/ontologies/2008/7/XCLOntology1.5.owl#vectorInformation -->

    <owl:Class rdf:about="#vectorInformation">
        <rdfs:subClassOf rdf:resource="#imageInformation"/>
    </owl:Class>
    


    <!-- http://www.semanticweb.org/ontologies/2008/7/XCLOntology1.5.owl#videoinformation -->

    <owl:Class rdf:about="#videoinformation">
        <rdfs:subClassOf rdf:resource="#XCL_Properties"/>
    </owl:Class>
    


    <!-- http://www.semanticweb.org/ontologies/2008/7/XCLOntology1.5.owl#wordProcessingML -->

    <owl:Class rdf:about="#wordProcessingML">
        <rdfs:subClassOf rdf:resource="#DOCX_Properties"/>
    </owl:Class>
    


    <!-- http://www.semanticweb.org/ontologies/2008/7/XCLOntology1.5.owl#xcl_propertyDatatypes -->

    <owl:Class rdf:about="#xcl_propertyDatatypes">
        <rdfs:subClassOf rdf:resource="#concepts"/>
    </owl:Class>
    


    <!-- http://www.semanticweb.org/ontologies/2008/7/XCLOntology1.5.owl#xcl_units -->

    <owl:Class rdf:about="#xcl_units">
        <rdfs:subClassOf rdf:resource="#concepts"/>
        <rdfs:comment
            >defines selfdefined Units</rdfs:comment>
    </owl:Class>
    


    <!-- http://www.w3.org/2002/07/owl#Thing -->

    <owl:Class rdf:about="&owl;Thing"/>
    


    <!-- 
    ///////////////////////////////////////////////////////////////////////////////////////
    //
    // Individuals
    //
    ///////////////////////////////////////////////////////////////////////////////////////
     -->

    


    <!-- http://www.semanticweb.org/ontologies/2008/7/XCLOntology1.5.owl#1931CIE_ChromaticityBlueX -->

    <imageInformation rdf:about="#1931CIE_ChromaticityBlueX">
        <ID>id130</ID>
        <rdfs:comment xml:lang="en"
            >value x of pair xy specifying blue colour according to 1931 CIE colour space</rdfs:comment>
        <rdfs:isDefinedBy rdf:resource="#uint16"/>
    </imageInformation>
    


    <!-- http://www.semanticweb.org/ontologies/2008/7/XCLOntology1.5.owl#1931CIE_ChromaticityBlueY -->

    <imageInformation rdf:about="#1931CIE_ChromaticityBlueY">
        <ID>id131</ID>
        <rdfs:comment xml:lang="en"
            >value y of pair xy specifying green colour according to 1931 CIE colour space</rdfs:comment>
        <Datatype rdf:resource="#uint16"/>
    </imageInformation>
    


    <!-- http://www.semanticweb.org/ontologies/2008/7/XCLOntology1.5.owl#1931CIE_ChromaticityGreenX -->

    <imageInformation rdf:about="#1931CIE_ChromaticityGreenX">
        <ID>id128</ID>
        <rdfs:comment xml:lang="en"
            >value x of pair xy specifying green colour according to 1931 CIE colour space</rdfs:comment>
        <Datatype rdf:resource="#uint16"/>
    </imageInformation>
    


    <!-- http://www.semanticweb.org/ontologies/2008/7/XCLOntology1.5.owl#1931CIE_ChromaticityGreenY -->

    <imageInformation rdf:about="#1931CIE_ChromaticityGreenY">
        <ID>id129</ID>
        <rdfs:comment xml:lang="en"
            >value y of pair xy specifying green colour according to 1931 CIE colour space</rdfs:comment>
        <Datatype rdf:resource="#uint16"/>
    </imageInformation>
    


    <!-- http://www.semanticweb.org/ontologies/2008/7/XCLOntology1.5.owl#1931CIE_ChromaticityRedX -->

    <imageInformation rdf:about="#1931CIE_ChromaticityRedX">
        <ID>id126</ID>
        <rdfs:comment xml:lang="en"
            >value x of pair xy specifying red colour according to 1931 CIE colour space</rdfs:comment>
        <Datatype rdf:resource="#uint16"/>
    </imageInformation>
    


    <!-- http://www.semanticweb.org/ontologies/2008/7/XCLOntology1.5.owl#1931CIE_ChromaticityRedY -->

    <imageInformation rdf:about="#1931CIE_ChromaticityRedY">
        <ID>id127</ID>
        <rdfs:comment xml:lang="en"
            >value y of pair xy specifying red colour according to 1931 CIE colour space</rdfs:comment>
        <Datatype rdf:resource="#uint16"/>
    </imageInformation>
    


    <!-- http://www.semanticweb.org/ontologies/2008/7/XCLOntology1.5.owl#AAC -->

    <audioInformation rdf:about="#AAC">
        <rdfs:comment xml:lang="en"
            >Audio-CompressionAlgorithm== MPEG4Part3</rdfs:comment>
        <Datatype rdf:resource="#XCLLabel"/>
    </audioInformation>
    


    <!-- http://www.semanticweb.org/ontologies/2008/7/XCLOntology1.5.owl#ASCII85Decode -->

    <PDF1.3_Properties rdf:about="#ASCII85Decode">
        <rdfs:comment
            >Stream Filter for decoding a Stream as ASCII 85 Data in PDF 1.3</rdfs:comment>
    </PDF1.3_Properties>
    


    <!-- http://www.semanticweb.org/ontologies/2008/7/XCLOntology1.5.owl#ASCIIHexDecode -->

    <PDF1.3_Properties rdf:about="#ASCIIHexDecode">
        <rdfs:comment
            >ASCIIHexDecode &#64257;lter fo PDF-Streams: 
An application reading the data in that stream will transform the ASCII hexadecimal-encoded data in the stream into binary data [cit. PDF 1.3]</rdfs:comment>
    </PDF1.3_Properties>
    


    <!-- http://www.semanticweb.org/ontologies/2008/7/XCLOntology1.5.owl#AVC_Codec -->

    <audioInformation rdf:about="#AVC_Codec">
        <rdfs:comment xml:lang="en"
            >Audio CompressionAlgorithm, equals MPEG4 Part 10</rdfs:comment>
        <Datatype rdf:resource="#XCLLabel"/>
    </audioInformation>
    


    <!-- http://www.semanticweb.org/ontologies/2008/7/XCLOntology1.5.owl#AbsoluteColormetric -->

    <PDF1.3_Properties rdf:about="#AbsoluteColormetric">
        <Datatype rdf:resource="#XCLLabel"/>
    </PDF1.3_Properties>
    


    <!-- http://www.semanticweb.org/ontologies/2008/7/XCLOntology1.5.owl#Adobe_98_RGB -->

    <imageInformation rdf:about="#Adobe_98_RGB">
        <ID>id234</ID>
        <Datatype rdf:resource="#XCLLabel"/>
    </imageInformation>
    


    <!-- http://www.semanticweb.org/ontologies/2008/7/XCLOntology1.5.owl#AllCap -->

    <fontFlag rdf:about="#AllCap">
        <rdfs:comment xml:lang="en">Bit:17</rdfs:comment>
        <Datatype rdf:resource="#bit"/>
    </fontFlag>
    


    <!-- http://www.semanticweb.org/ontologies/2008/7/XCLOntology1.5.owl#Alternate_ICC -->

    <PDF1.3_Properties rdf:about="#Alternate_ICC">
        <rdfs:comment xml:lang="en"
            >(Optional) An alternate color space to be used in case the one specified in the stream data is not supported (for example, by applications designed for earlier versions of PDF). The alternate space may be any valid color space (except a Pattern color space) that has the number of components specified by N. If this entry is omitted and the application does not understand the ICC profile data, the color space used is DeviceGray, DeviceRGB, or DeviceCMYK, depending on whether the value of N is 1, 3, or 4, respectively. [cit.]</rdfs:comment>
        <Datatype rdf:resource="#string"/>
    </PDF1.3_Properties>
    


    <!-- http://www.semanticweb.org/ontologies/2008/7/XCLOntology1.5.owl#AntiAlias -->

    <PDF1.3_Properties rdf:about="#AntiAlias">
        <rdfs:comment
            >(Optional) A &#64258;ag indicating whether to &#64257;lter the shading function to prevent aliasing artifacts. The shading operators sample shading functions at a rate determined by the resolution of the output device. Aliasing can occur if the function is not smooth&#8212;that is, if it has a high spatial frequency relative to the sampling rate. Anti-aliasing can be computationally expensive and is usually unnecessary, since most shading functions are smooth enough, or are sampled at a high enough frequency, to avoid aliasing effects. Anti-aliasing may not be implemented on some output devices, in which case this &#64258;ag is ignored. Default value: false. [cit. Pdf 1.3]</rdfs:comment>
        <Datatype rdf:resource="#bool"/>
    </PDF1.3_Properties>
    


    <!-- http://www.semanticweb.org/ontologies/2008/7/XCLOntology1.5.owl#ArtBox -->

    <PDF1.3_Properties rdf:about="#ArtBox">
        <rdfs:comment
            >(Optional; PDF 1.3) A rectangle, expressed in default user space units, de&#64257;ning the extent of the page&#8217;s meaningful content (including potential white space) as intended by the page&#8217;s creator (see Section 8.6.1, &#8220;Page Boundaries&#8221;). Default value: the value of CropBox. [cit. PDf 1.3]</rdfs:comment>
        <Datatype rdf:resource="#floatArray"/>
    </PDF1.3_Properties>
    


    <!-- http://www.semanticweb.org/ontologies/2008/7/XCLOntology1.5.owl#Artist_Tiff -->

    <Tiff_Properties rdf:about="#Artist_Tiff">
        <rdfs:comment
            >Used for ImageProducer</rdfs:comment>
        <is_same_as rdf:resource="#artist"/>
        <Datatype rdf:resource="#string"/>
    </Tiff_Properties>
    


    <!-- http://www.semanticweb.org/ontologies/2008/7/XCLOntology1.5.owl#Ascent -->

    <fontDescriptor rdf:about="#Ascent">
        <rdfs:comment xml:lang="en"
            >(Required, except for Type 3 fonts) The maximum height above the baseline reached by glyphs in this font, excluding the height of glyphs for accented characters.</rdfs:comment>
        <Datatype rdf:resource="#int"/>
    </fontDescriptor>
    


    <!-- http://www.semanticweb.org/ontologies/2008/7/XCLOntology1.5.owl#Author -->

    <wordProcessingML rdf:about="#Author"/>
    


    <!-- http://www.semanticweb.org/ontologies/2008/7/XCLOntology1.5.owl#AutoFocus_NISO -->

    <NISO rdf:about="#AutoFocus_NISO">
        <rdfs:comment
            >This specifies the status of the capture device&#8217;s focus at the time of capture. 
Auto Focus Used = &#8220;The camera successfully focused on the subject.&#8221;

Auto Focus Interrupted = &#8220;The image was captured before the camera had successfully focused on the subject.&#8221;

Near Focused = &#8220;The camera deliberately focused at a distance closer than the subject to allow for the super-imposition of a focused foreground subject.&#8221;

Soft Focused = &#8220;The camera deliberately did not focus exactly at the subject distance to create a softer image (commonly used in portraits).&#8221;

Manual = &#8220;The camera was focused manually.&#8221;
[cit. NISO]</rdfs:comment>
    </NISO>
    


    <!-- http://www.semanticweb.org/ontologies/2008/7/XCLOntology1.5.owl#AvgWidth -->

    <fontDescriptor rdf:about="#AvgWidth">
        <rdfs:comment xml:lang="en"
            >The average width of glyphs in the font</rdfs:comment>
        <Datatype rdf:resource="#uint32"/>
    </fontDescriptor>
    


    <!-- http://www.semanticweb.org/ontologies/2008/7/XCLOntology1.5.owl#BBox -->

    <PDF1.3_Properties rdf:about="#BBox">
        <rdfs:comment xml:lang="en"
            >(Required) An array of four numbers in the pattern coordinate system giving
the coordinates of the left, bottom, right, and top edges, respectively, of the pattern cell&#8217;s bounding box. These boundaries are used to clip the pattern cell. [cit.]</rdfs:comment>
        <Datatype rdf:resource="#floatArray"/>
    </PDF1.3_Properties>
    


    <!-- http://www.semanticweb.org/ontologies/2008/7/XCLOntology1.5.owl#BackLight_NISO -->

    <NISO rdf:about="#BackLight_NISO">
        <rdfs:comment
            >This specifies the lighting conditions at the time of exposure. [cit. NISO]
Front light  = &#8220;Subject is illuminated from the front side.&#8221;

Backlight_1 =  &#8220;The brightness value difference between the subject center and the surrounding area is greater than one full stop (APEX).  The frame is exposed for the subject center.&#8221;

Backlight_2 = &#8220;The brightness value difference between the subject center and the surrounding area is greater than one full stop (APEX).  The frame is exposed for the surrounding area.&#8221;</rdfs:comment>
    </NISO>
    


    <!-- http://www.semanticweb.org/ontologies/2008/7/XCLOntology1.5.owl#Background -->

    <PDF1.3_Properties rdf:about="#Background">
        <rdfs:comment
            >(Optional) An array of color components appropriate to the color space, specifying a single background color value. If present, this color is used before any painting operation involving the shading, to &#64257;ll the entire area to be painted. The effect is as if the painting operation were performed twice: &#64257;rst with the background color and then again with the shading. 
[cit. Pdf 1.3]</rdfs:comment>
        <Datatype rdf:resource="#int"/>
    </PDF1.3_Properties>
    


    <!-- http://www.semanticweb.org/ontologies/2008/7/XCLOntology1.5.owl#Backgroundcolour_Gif -->

    <GIF_Properties rdf:about="#Backgroundcolour_Gif">
        <is_same_as rdf:resource="#Background"/>
        <is_same_as rdf:resource="#backgroundColour_PNG"/>
        <Datatype rdf:resource="#uint32Rational"/>
    </GIF_Properties>
    


    <!-- http://www.semanticweb.org/ontologies/2008/7/XCLOntology1.5.owl#Backslash_Pdf -->

    <PDF1.3_Properties rdf:about="#Backslash_Pdf">
        <rdfs:comment>\\</rdfs:comment>
        <Datatype rdf:resource="#string"/>
    </PDF1.3_Properties>
    


    <!-- http://www.semanticweb.org/ontologies/2008/7/XCLOntology1.5.owl#Backspace_Pdf -->

    <PDF1.3_Properties rdf:about="#Backspace_Pdf">
        <rdfs:comment>\b</rdfs:comment>
        <Datatype rdf:resource="#string"/>
    </PDF1.3_Properties>
    


    <!-- http://www.semanticweb.org/ontologies/2008/7/XCLOntology1.5.owl#BitDepth -->

    <rasterInformation rdf:about="#BitDepth">
        <rdfs:comment
            >Number of bits per sample component</rdfs:comment>
        <ID>id11</ID>
        <Unit rdf:resource="#bit"/>
        <is_same_as rdf:resource="#colourResolution"/>
        <Datatype rdf:resource="#int"/>
        <Restriction rdf:resource="#mandatory"/>
    </rasterInformation>
    


    <!-- http://www.semanticweb.org/ontologies/2008/7/XCLOntology1.5.owl#BitsPerComponent -->

    <PDF1.3_Properties rdf:about="#BitsPerComponent">
        <rdfs:comment
            >(Used only if Predictor is greater than 1) The number of bits used to represent each color component in a sample. Valid values are 1, 2, 4, and 8. Default value: 8. [cit. Pdf 1.3]</rdfs:comment>
        <Datatype rdf:resource="#int"/>
    </PDF1.3_Properties>
    


    <!-- http://www.semanticweb.org/ontologies/2008/7/XCLOntology1.5.owl#BitsPerCoordinate -->

    <PDF1.3_Properties rdf:about="#BitsPerCoordinate">
        <rdfs:comment
            >(Required) The number of bits used to represent each vertex coordinate. 
Valid values are 1, 2, 4, 8, 12, 16, 24, and 32. 
(Additional entries speci&#64257;c to a type 4 shading dictionary) [cit. Pdf 1.3]</rdfs:comment>
        <Datatype rdf:resource="#int"/>
    </PDF1.3_Properties>
    


    <!-- http://www.semanticweb.org/ontologies/2008/7/XCLOntology1.5.owl#BitsPerSample_NISO -->

    <NISO rdf:about="#BitsPerSample_NISO">
        <rdfs:comment
            >The number of bits per component for each pixel.  This field provides N values depending upon SamplesPerPixel present. Values:
1= 1-bit (bitonal)
4= 4-bit grayscale
8= 8-bit grayscale or palletizedcolor
8,8,8= RGB
16,16,16= TIFF, HDR (high dynamic range)
8,8,8,8= CMYK	
[cit. NISO]</rdfs:comment>
        <Unit rdf:resource="#bit"/>
        <is_same_as rdf:resource="#bitsPerSample"/>
        <is_same_as rdf:resource="#bitsPerSampleTiff"/>
        <Datatype rdf:resource="#int"/>
    </NISO>
    


    <!-- http://www.semanticweb.org/ontologies/2008/7/XCLOntology1.5.owl#BitsPerSample_Pdf -->

    <PDF1.3_Properties rdf:about="#BitsPerSample_Pdf">
        <rdfs:comment
            >(Required) The number of bits used to represent each sample. (If the function 
has multiple output values, each one occupies BitsPerSample bits.) Valid 
values are 1, 2, 4, 8, 12, 16, 24, and 32. [cit. Pdf 1.3]</rdfs:comment>
        <Datatype rdf:resource="#int"/>
    </PDF1.3_Properties>
    


    <!-- http://www.semanticweb.org/ontologies/2008/7/XCLOntology1.5.owl#BlackPointCalGray -->

    <PDF1.3_Properties rdf:about="#BlackPointCalGray">
        <rdfs:comment xml:lang="en"
            >(Optional) An array of three numbers [ X B YB ZB ] specifying the tristimulus value, in the CIE 1931 XYZ space, of the diffuse black point; see &#8220;CalRGB 
Color Spaces,&#8221; below, for further discussion. All three of these numbers must be non-negative. Default value: [ 0.0 0.0 0.0 ].[cit.]</rdfs:comment>
        <Datatype rdf:resource="#int"/>
    </PDF1.3_Properties>
    


    <!-- http://www.semanticweb.org/ontologies/2008/7/XCLOntology1.5.owl#BlackPointCalRGB -->

    <PDF1.3_Properties rdf:about="#BlackPointCalRGB">
        <rdfs:comment xml:lang="en"
            >(Optional) An array of three numbers [ X B YB ZB ] specifying the tristimulus value, in the CIE 1931 XYZ space, of the diffuse black point; see below for further discussion. All three of these numbers must be non-negative. Default value: [ 0.0 0.0 0.0 ]. [cit.]</rdfs:comment>
        <Datatype rdf:resource="#int"/>
    </PDF1.3_Properties>
    


    <!-- http://www.semanticweb.org/ontologies/2008/7/XCLOntology1.5.owl#BlackPointLab -->

    <PDF1.3_Properties rdf:about="#BlackPointLab">
        <rdfs:comment xml:lang="en"
            >(Optional) An array of three numbers [ X B YB ZB ] specifying the tristimulus value, in the CIE 1931 XYZ space, of the diffuse black point; see &#8220;CalRGB Color Spaces&#8221; on page 247 for further discussion. All three of these numbers must be non-negative. Default value: [ 0.0 0.0 0.0 ]. [cit.]</rdfs:comment>
        <Datatype rdf:resource="#int"/>
    </PDF1.3_Properties>
    


    <!-- http://www.semanticweb.org/ontologies/2008/7/XCLOntology1.5.owl#BleedBox -->

    <PDF1.3_Properties rdf:about="#BleedBox">
        <rdfs:comment
            >(Optional; PDF 1.3) A rectangle, expressed in default user space units, de&#64257;ning the region to which the contents of the page should be clipped when output in a production environment (see Section 8.6.1, &#8220;Page Boundaries&#8221;). Default value: the value of CropBox. [cit. Pdf 1.3]</rdfs:comment>
        <Datatype rdf:resource="#floatArray"/>
    </PDF1.3_Properties>
    


    <!-- http://www.semanticweb.org/ontologies/2008/7/XCLOntology1.5.owl#Brightness_NISO -->

    <NISO rdf:about="#Brightness_NISO">
        <rdfs:comment
            >This specifies the Brightness values measured when the image was captured, using APEX values. [cit. NISO]</rdfs:comment>
        <Datatype rdf:resource="#rational"/>
    </NISO>
    


    <!-- http://www.semanticweb.org/ontologies/2008/7/XCLOntology1.5.owl#ByteOrder_NISO -->

    <NISO rdf:about="#ByteOrder_NISO">
        <rdfs:comment
            >Virtually all computer architectures are byte addressable.  The bytes of a multi-byte data value can be stored in memory in different orders. &quot;Little_endian&quot; means that the low-order byte of the number is stored in memory at the lowest address, and the high-order byte at the highest address. &#8220;Big_endian&quot; means that the high-order byte of the number is stored in memory at the lowest address, and the low-order byte at the highest address.[cit. NISO standard]</rdfs:comment>
        <is_same_as rdf:resource="#byteOrder"/>
        <Datatype rdf:resource="#string"/>
    </NISO>
    


    <!-- http://www.semanticweb.org/ontologies/2008/7/XCLOntology1.5.owl#CCITT3 -->

    <rasterInformation rdf:about="#CCITT3">
        <rdfs:comment xml:lang="en"
            >compressionAlgorithm for monocoloured 2 Bit-images</rdfs:comment>
        <ID>id226</ID>
        <Datatype rdf:resource="#XCLLabel"/>
    </rasterInformation>
    


    <!-- http://www.semanticweb.org/ontologies/2008/7/XCLOntology1.5.owl#CCITT4 -->

    <rasterInformation rdf:about="#CCITT4">
        <ID>id227</ID>
        <rdfs:comment xml:lang="en"
            >Image Compression Algorithm for bipolar Images</rdfs:comment>
        <Datatype rdf:resource="#XCLLabel"/>
    </rasterInformation>
    


    <!-- http://www.semanticweb.org/ontologies/2008/7/XCLOntology1.5.owl#CCITTFaxDecode -->

    <PDF1.3_Properties rdf:about="#CCITTFaxDecode">
        <rdfs:comment
            >Decompresses data encoded using the CCITT facsimile standard, 
reproducing the original data (typically monochrome image data at 1 
bit per pixel). [cit. PDF 1.3]</rdfs:comment>
    </PDF1.3_Properties>
    


    <!-- http://www.semanticweb.org/ontologies/2008/7/XCLOntology1.5.owl#CIDFontType0 -->

    <PDF1.3_Properties rdf:about="#CIDFontType0">
        <rdfs:comment
            >(PDF 1.2) A CIDFont whose glyph descriptions are based on Type 1 font technology (see Section 5.6.3, &#8220;CIDFonts&#8221;)  [cit. Pdf 1.3]</rdfs:comment>
    </PDF1.3_Properties>
    


    <!-- http://www.semanticweb.org/ontologies/2008/7/XCLOntology1.5.owl#CIDFontType2 -->

    <PDF1.3_Properties rdf:about="#CIDFontType2">
        <rdfs:comment
            >(PDF 1.2) A CIDFont whose glyph descriptions are based on TrueType font technology (see Section 5.6.3, &#8220;CIDFonts&#8221;). [cit. Pdf 1.3]</rdfs:comment>
    </PDF1.3_Properties>
    


    <!-- http://www.semanticweb.org/ontologies/2008/7/XCLOntology1.5.owl#CMYK_ICC -->

    <PDF1.3_Properties rdf:about="#CMYK_ICC">
        <rdfs:comment
            >Ranges for typical ICC color spaces [Cit. Pdf 1.3].
Component Ranges: [0.01.0]</rdfs:comment>
        <is_same_as rdf:resource="#cmyk"/>
    </PDF1.3_Properties>
    


    <!-- http://www.semanticweb.org/ontologies/2008/7/XCLOntology1.5.owl#CTM -->

    <PDF1.3_Properties rdf:about="#CTM">
        <rdfs:comment
            >The current transformation matrix, which maps positions from user coordinates to device coordinates (see Section 4.2, &#8220;Coordinate Systems&#8221;). This matrix is modi&#64257;ed by each application of the coordinate transformation operator, cm. Initial value: a matrix that transforms default user coordinates to device coordinates. [cit. Pdf 1.3]</rdfs:comment>
        <Datatype rdf:resource="#matrix"/>
    </PDF1.3_Properties>
    


    <!-- http://www.semanticweb.org/ontologies/2008/7/XCLOntology1.5.owl#CalGray -->

    <PDF1.3_Properties rdf:about="#CalGray"/>
    


    <!-- http://www.semanticweb.org/ontologies/2008/7/XCLOntology1.5.owl#CalRGB -->

    <PDF1.3_Properties rdf:about="#CalRGB"/>
    


    <!-- http://www.semanticweb.org/ontologies/2008/7/XCLOntology1.5.owl#CarriageReturn_Pdf -->

    <PDF1.3_Properties rdf:about="#CarriageReturn_Pdf">
        <rdfs:comment>\r</rdfs:comment>
        <Datatype rdf:resource="#string"/>
    </PDF1.3_Properties>
    


    <!-- http://www.semanticweb.org/ontologies/2008/7/XCLOntology1.5.owl#CharSet -->

    <fontDescriptor rdf:about="#CharSet">
        <rdfs:comment xml:lang="en"
            >(Optional; meaningful only in Type 1 fonts; PDF 1.1)
A string listing the character names defined in a font subset. The names in this string must be in PDF syntax&#8212;that is, each name preceded by a slash (/). The names can appear in any order. The name . notdef should be omitted; it is assumed to exist in the font subset. If this entry is absent, the only indication of a font subset is the subset tag in the FontName entry (see Section 5.5.3, &#8220;Font Subsets&#8221;). 
[cit.]</rdfs:comment>
    </fontDescriptor>
    


    <!-- http://www.semanticweb.org/ontologies/2008/7/XCLOntology1.5.owl#CheckSum -->

    <PDF1.3_Properties rdf:about="#CheckSum">
        <rdfs:comment
            >(Optional) A 16-byte string that is the checksum of the bytes of the uncompressed embedded &#64257;le. The checksum is calculated by applying the standard MD5 message-digest algorithm (described in Internet RFC 1321, The MD5 Message-Digest Algorithm; see the Bibliography) to the bytes of the embedded &#64257;le stream. [cit. Pdf 1.3]</rdfs:comment>
        <Datatype rdf:resource="#string"/>
    </PDF1.3_Properties>
    


    <!-- http://www.semanticweb.org/ontologies/2008/7/XCLOntology1.5.owl#ChecksumMethod_NISO -->

    <NISO rdf:about="#ChecksumMethod_NISO">
        <rdfs:comment
            >Local repository policies regarding file integrity metadata should govern implementation of this field.  The enumerated type values should be defined locally, as should the rule regarding when the checksum is generated:  prior to deposit, at the time of deposit, or both.

Depending upon local implementation, this field may be used to list the specific type of error detection technique used (e.g., checksum, CRC, MNP, etc.) and the subsequent value would then be recorded in 2.2.3.1 ChecksumValue.
[cit. NISO]</rdfs:comment>
    </NISO>
    


    <!-- http://www.semanticweb.org/ontologies/2008/7/XCLOntology1.5.owl#ChecksumValue_NISO -->

    <NISO rdf:about="#ChecksumValue_NISO">
        <rdfs:comment
            >Linked to ChecksumMethod</rdfs:comment>
        <Datatype rdf:resource="#int"/>
    </NISO>
    


    <!-- http://www.semanticweb.org/ontologies/2008/7/XCLOntology1.5.owl#CieColorSpace -->

    <PDF1.3_Properties rdf:about="#CieColorSpace"/>
    


    <!-- http://www.semanticweb.org/ontologies/2008/7/XCLOntology1.5.owl#ClipPath_Tiff -->

    <Tiff_Properties rdf:about="#ClipPath_Tiff">
        <rdfs:comment
            >Mirrors the essentials of PostScript&#39;s path creation functionality.
Most operators can be easily translated into PostScript, and, conversely, any PostScript path can be represented as a TIFF ClipPath. However, the TIFF ClipPath list of operators is not identical to the current list of PostScript operators; for simplicity, some of the PostScript variants have been dropped, and a few operators, such as polyto and rpolyto have been added. polyto and rpolyto were added in order to make complex TIFF polygonal clip paths more compact. [cit. Tiff]</rdfs:comment>
        <is_same_as rdf:resource="#clipPath"/>
        <Datatype rdf:resource="#int"/>
    </Tiff_Properties>
    


    <!-- http://www.semanticweb.org/ontologies/2008/7/XCLOntology1.5.owl#ClippingPath -->

    <PDF1.3_Properties rdf:about="#ClippingPath">
        <rdfs:comment
            >A path de&#64257;ning the current clipping boundary against which all output is to be cropped (see Section 4.4.3, &#8220;Clipping Path Operators&#8221;). Initial value: the boundary of the entire imageable portion of the output page.[cit. Pdf 1.3]</rdfs:comment>
    </PDF1.3_Properties>
    


    <!-- http://www.semanticweb.org/ontologies/2008/7/XCLOntology1.5.owl#CodecCompliance_NISO -->

    <NISO rdf:about="#CodecCompliance_NISO">
        <rdfs:comment
            >a container of information detailing JPEG 2000 Codec compliance; comprised of four data elements (7.2.1.1.1 codec, 7.2.1.1.2 codecVersion, 7.2.1.1.3 codestreamProfile, and 7.2.1.1.4 complianceClass) 
[cit. NISO MIX]</rdfs:comment>
        <Datatype rdf:resource="#int"/>
    </NISO>
    


    <!-- http://www.semanticweb.org/ontologies/2008/7/XCLOntology1.5.owl#ColorSpaceDeviceN -->

    <PDF1.3_Properties rdf:about="#ColorSpaceDeviceN">
        <rdfs:comment xml:lang="en"
            >(Required) A name or array identifying the process color space, which may be any device or CIE-based color space. If an ICCBased color space is specified, it must provide calibration information appropriate for the process color components specified in the names array of the DeviceN color space. [cit.]</rdfs:comment>
        <is_same_as rdf:resource="#colourSpaceName"/>
        <Datatype rdf:resource="#string"/>
    </PDF1.3_Properties>
    


    <!-- http://www.semanticweb.org/ontologies/2008/7/XCLOntology1.5.owl#ColorSpace_NISO -->

    <NISO rdf:about="#ColorSpace_NISO">
        <rdfs:comment
            >0 = WhiteIsZero.  For bilevel and grayscale images: 0 is imaged as white.  2**BitsPerSample-1 is imaged as black.  This is the normal value for Compression=2.

1 =BlackIsZero.  For bilevel and grayscale images: 0 is imaged as black.  2**BitsPerSample-1 is imaged as white.  If this value is specified for Compression=2, the image should display and print reversed.

2 =RGB.  In the RGB model, a color is described as a combination of the three primary colors of light (red, green, and blue) in particular concentrations.  For each of the three components, 0 represents minimum intensity, and 2**BitsPerSample - 1 represents maximum intensity.  Thus an RGB value of (0,0,0) represents black, and (255,255,255) represents white, assuming 8-bit components.  For PlanarConfiguration = 1, the components are stored in the indicated order: first Red, then Green, then Blue.  For PlanarConfiguration = 2, the StripOffsets for the component planes are stored in the indicated order: first the Red component plane StripOffsets, then the Green plane StripOffsets, then the Blue plane StripOffsets.

3 =Palette color.  In this model, a color is described with a single component.  The value of the component is used as an index into the red, green and blue curves in the ColorMap field to retrieve an RGB triplet that defines the color.  When PhotometricInterpretation=3 is used, ColorMap must be present and SamplesPerPixel must be 1.

4 =Transparency Mask.  This means that the image is used to define an irregularly shaped region of another image in the same TIFF file.  SamplesPerPixel and BitsPerSample must be 1.  PackBits compression is recommended.  The 1-bits define the interior of the region; the 0-bits define the exterior of the region.
5 = CMYK
6 = YCbCr 
8 = CIELab [cit. Niso Standard]</rdfs:comment>
        <is_same_as rdf:resource="#YCbCrSubSampling_NISO"/>
        <Datatype rdf:resource="#int"/>
    </NISO>
    


    <!-- http://www.semanticweb.org/ontologies/2008/7/XCLOntology1.5.owl#ColorTemp_NISO -->

    <NISO rdf:about="#ColorTemp_NISO">
        <rdfs:comment
            >This specifies the actual color temperature value of the scene illuminant in units of Kelvin. [cit. NISO]</rdfs:comment>
        <Datatype rdf:resource="#rational"/>
    </NISO>
    


    <!-- http://www.semanticweb.org/ontologies/2008/7/XCLOntology1.5.owl#ColorTransform -->

    <PDF1.3_Properties rdf:about="#ColorTransform">
        <rdfs:comment
            >Optional parameter for the DCTDecode &#64257;lter.
A code specifying the transformation to be performed on the sample values:
0 No transformation. 
1 If the image has three color components, transform RGB values to 
YUV before encoding and from YUV to RGB after decoding. If the 
image has four components, transform CMYK values to YUVK be- 
fore encoding and from YUVK to CMYK after decoding. This option 
is ignored if the image has one or two color components. 
[cit. 1.3]</rdfs:comment>
        <Datatype rdf:resource="#int"/>
    </PDF1.3_Properties>
    


    <!-- http://www.semanticweb.org/ontologies/2008/7/XCLOntology1.5.owl#Colorants -->

    <PDF1.3_Properties rdf:about="#Colorants">
        <rdfs:comment xml:lang="en"
            >(Required if Subtype is NChannel and the color space includes spot colorants; otherwise optional) A dictionary describing the individual colorants used in the DeviceN color space. For each entry in this dictionary, the key is a colorant name and the value is an array defining a Separation color space for that colorant (see &#8220;Separation Color Spaces&#8221; on page 264). For each entry in this dictionary, the key is a colorant name and the 
value is an array de&#64257;ning a Separation color space for that colorant [cit. Pdf 1.3]</rdfs:comment>
    </PDF1.3_Properties>
    


    <!-- http://www.semanticweb.org/ontologies/2008/7/XCLOntology1.5.owl#Colormap_BitCodeValue_NISO -->

    <NISO rdf:about="#Colormap_BitCodeValue_NISO">
        <rdfs:comment
            >This field provides the Bit Code Value or reference point for a particular RGB triplet of the Colormap (often called a lookup table) for palette-color images. Possible Values between 0-255.
[cit. NISO]</rdfs:comment>
        <Datatype rdf:resource="#int"/>
    </NISO>
    


    <!-- http://www.semanticweb.org/ontologies/2008/7/XCLOntology1.5.owl#Colormap_BlueValue_NISO -->

    <NISO rdf:about="#Colormap_BlueValue_NISO">
        <rdfs:comment
            >This field provides the Blue Value within a particular RGB triplet of the Colormap (often called a lookup table) for palette-color images.  Particular triplet is reference in 4.2.4.1 Colormap_BitCodeValue. possible values between 0-255.
[cit. NISO]</rdfs:comment>
        <Datatype rdf:resource="#int"/>
    </NISO>
    


    <!-- http://www.semanticweb.org/ontologies/2008/7/XCLOntology1.5.owl#Colormap_GreenValue_NISO -->

    <NISO rdf:about="#Colormap_GreenValue_NISO">
        <rdfs:comment
            >This field provides the Green Value within a particular RGB triplet of the Colormap (often called a lookup table) for palette-color images.  Particular triplet is reference in 4.2.4.1 Colormap_BitCodeValue. possible values between 0-255.
[cit. NISO]</rdfs:comment>
        <Datatype rdf:resource="#int"/>
    </NISO>
    


    <!-- http://www.semanticweb.org/ontologies/2008/7/XCLOntology1.5.owl#Colormap_RedValue_NISO -->

    <NISO rdf:about="#Colormap_RedValue_NISO">
        <rdfs:comment
            >This field provides the Red Value within a particular RGB triplet of the Colormap (often called a lookup table) for palette-color images.  Particular triplet is reference in 4.2.4.1 Colormap_BitCodeValue. possible values between 0-255.
[cit. NISO]</rdfs:comment>
        <Datatype rdf:resource="#int"/>
    </NISO>
    


    <!-- http://www.semanticweb.org/ontologies/2008/7/XCLOntology1.5.owl#Colors -->

    <PDF1.3_Properties rdf:about="#Colors">
        <rdfs:comment
            >(Used only if Predictor is greater than 1) The number of interleaved color components per sample. Valid values are 1 to 4 in PDF 1.2 or earlier, and 1 or greater in PDF 1.3. Default value: 1. [cit. PDF 1.3]</rdfs:comment>
        <Datatype rdf:resource="#int"/>
    </PDF1.3_Properties>
    


    <!-- http://www.semanticweb.org/ontologies/2008/7/XCLOntology1.5.owl#Columns -->

    <PDF1.3_Properties rdf:about="#Columns">
        <rdfs:comment
            >(Used only if Predictor is greater than 1) The number of samples in each row. Default value: 1. [Cit. PDF 1.3]</rdfs:comment>
        <Datatype rdf:resource="#int"/>
    </PDF1.3_Properties>
    


    <!-- http://www.semanticweb.org/ontologies/2008/7/XCLOntology1.5.owl#Components -->

    <PDF1.3_Properties rdf:about="#Components">
        <rdfs:comment xml:lang="en"
            >(Required) An array of component names that correspond, in order, to the components of the process color space specified in ColorSpace. For example, an RGB color space must have three names corresponding to red, green, and blue. The names may be arbitrary (that is, not the same as the standard names for the color space components) and must match those specified in the names array of the DeviceN color space, even if all components are not present in the names array. [cit.]</rdfs:comment>
    </PDF1.3_Properties>
    


    <!-- http://www.semanticweb.org/ontologies/2008/7/XCLOntology1.5.owl#CompressionLevel_NISO -->

    <NISO rdf:about="#CompressionLevel_NISO">
        <rdfs:comment
            >Designates the level of compression in the compressionScheme</rdfs:comment>
        <Datatype rdf:resource="#int"/>
    </NISO>
    


    <!-- http://www.semanticweb.org/ontologies/2008/7/XCLOntology1.5.owl#CompressionRatio_NISO -->

    <NISO rdf:about="#CompressionRatio_NISO">
        <Datatype rdf:resource="#int"/>
    </NISO>
    


    <!-- http://www.semanticweb.org/ontologies/2008/7/XCLOntology1.5.owl#CompressionScheme_NISO -->

    <NISO rdf:about="#CompressionScheme_NISO">
        <rdfs:comment
            >1= Uncompressed
2= CCITT 1D
3= CCITT Group 3
4= CCITT Group 4
5= LZW
6= JPEG 
32773= PackBits (simple byte-oriented run-length scheme)</rdfs:comment>
        <Datatype rdf:resource="#uint32"/>
    </NISO>
    


    <!-- http://www.semanticweb.org/ontologies/2008/7/XCLOntology1.5.owl#Compression_NISO -->

    <NISO rdf:about="#Compression_NISO"/>
    


    <!-- http://www.semanticweb.org/ontologies/2008/7/XCLOntology1.5.owl#Courier -->

    <textInformation rdf:about="#Courier">
        <ID>id311</ID>
        <is_same_as rdf:resource="#F9"/>
    </textInformation>
    


    <!-- http://www.semanticweb.org/ontologies/2008/7/XCLOntology1.5.owl#CourierBold -->

    <textInformation rdf:about="#CourierBold">
        <ID>id313</ID>
        <is_same_as rdf:resource="#F11"/>
    </textInformation>
    


    <!-- http://www.semanticweb.org/ontologies/2008/7/XCLOntology1.5.owl#CourierBoldOblique -->

    <textInformation rdf:about="#CourierBoldOblique">
        <ID>id312</ID>
        <is_same_as rdf:resource="#F12"/>
    </textInformation>
    


    <!-- http://www.semanticweb.org/ontologies/2008/7/XCLOntology1.5.owl#CourierOblique -->

    <textInformation rdf:about="#CourierOblique">
        <ID>id314</ID>
        <is_same_as rdf:resource="#F10"/>
    </textInformation>
    


    <!-- http://www.semanticweb.org/ontologies/2008/7/XCLOntology1.5.owl#CreationDate -->

    <PDF1.3_Properties rdf:about="#CreationDate">
        <rdfs:comment
            >(Optional) The date and time when the embedded &#64257;le was created. [cit. Pdf 1.3]</rdfs:comment>
        <is_same_as rdf:resource="#DateTimeCreated_NISO"/>
        <is_same_as rdf:resource="#documentCreationDate"/>
        <Datatype rdf:resource="#timeISO8601"/>
    </PDF1.3_Properties>
    


    <!-- http://www.semanticweb.org/ontologies/2008/7/XCLOntology1.5.owl#Creator -->

    <PDF1.3_Properties rdf:about="#Creator">
        <rdfs:comment
            >Entries in a Macintosh-speci&#64257;c &#64257;le information dictionary:
(Optional) The embedded &#64257;le&#8217;s creator signature. [cit. Pdf 1.3]</rdfs:comment>
        <Datatype rdf:resource="#string"/>
    </PDF1.3_Properties>
    


    <!-- http://www.semanticweb.org/ontologies/2008/7/XCLOntology1.5.owl#CropBox -->

    <PDF1.3_Properties rdf:about="#CropBox">
        <rdfs:comment
            >(Optional; inheritable) A rectangle, expressed in default user space units, 
de&#64257;ning the region to which the contents of the page are to be clipped 
(cropped) when displayed or printed (see Section 8.6.1, &#8220;Page Bound- 
aries&#8221;). Default value: the value of MediaBox. 
[cit. Pdf 1.3]</rdfs:comment>
    </PDF1.3_Properties>
    


    <!-- http://www.semanticweb.org/ontologies/2008/7/XCLOntology1.5.owl#DCTDecode -->

    <PDF1.3_Properties rdf:about="#DCTDecode">
        <rdfs:comment
            >Decompresses data encoded using a DCT (discrete cosine transform) 
technique based on the JPEG standard, reproducing image sample 
data that approximates the original data. 
[cit. Pdf 1.3]</rdfs:comment>
    </PDF1.3_Properties>
    


    <!-- http://www.semanticweb.org/ontologies/2008/7/XCLOntology1.5.owl#DateTime -->

    <Tiff_Properties rdf:about="#DateTime">
        <rdfs:comment
            >Date and Time image was scanned</rdfs:comment>
        <Datatype rdf:resource="#timeISO8601"/>
    </Tiff_Properties>
    


    <!-- http://www.semanticweb.org/ontologies/2008/7/XCLOntology1.5.owl#DateTimeCreated_NISO -->

    <NISO rdf:about="#DateTimeCreated_NISO">
        <rdfs:comment
            >Date or DateTime image was created. [cit. NISO]</rdfs:comment>
        <is_same_as rdf:resource="#documentCreationDate"/>
        <Datatype rdf:resource="#timeISO8601"/>
    </NISO>
    


    <!-- http://www.semanticweb.org/ontologies/2008/7/XCLOntology1.5.owl#DateTimeProcessed_NISO -->

    <NISO rdf:about="#DateTimeProcessed_NISO">
        <Datatype rdf:resource="#timeISO8601"/>
    </NISO>
    


    <!-- http://www.semanticweb.org/ontologies/2008/7/XCLOntology1.5.owl#Decode -->

    <PDF1.3_Properties rdf:about="#Decode">
        <rdfs:comment
            >(Optional) An array of 2 &#215; n numbers specifying the linear mapping of sample values into the range appropriate for the function&#8217;s output values. Default value: Same as the value of Range. [cit. Pdf 1.3]</rdfs:comment>
        <Datatype rdf:resource="#matrix"/>
    </PDF1.3_Properties>
    


    <!-- http://www.semanticweb.org/ontologies/2008/7/XCLOntology1.5.owl#DefaultCMYK -->

    <PDF1.3_Properties rdf:about="#DefaultCMYK"/>
    


    <!-- http://www.semanticweb.org/ontologies/2008/7/XCLOntology1.5.owl#DefaultGray -->

    <PDF1.3_Properties rdf:about="#DefaultGray"/>
    


    <!-- http://www.semanticweb.org/ontologies/2008/7/XCLOntology1.5.owl#DefaultRGB -->

    <PDF1.3_Properties rdf:about="#DefaultRGB"/>
    


    <!-- http://www.semanticweb.org/ontologies/2008/7/XCLOntology1.5.owl#Descent -->

    <fontDescriptor rdf:about="#Descent">
        <rdfs:comment xml:lang="en"
            >(Required, except for Type 3 fonts) The maximum depth below the baseline reached by glyphs in this font. The value is a negative number.</rdfs:comment>
    </fontDescriptor>
    


    <!-- http://www.semanticweb.org/ontologies/2008/7/XCLOntology1.5.owl#DeviceCMYK -->

    <PDF1.3_Properties rdf:about="#DeviceCMYK"/>
    


    <!-- http://www.semanticweb.org/ontologies/2008/7/XCLOntology1.5.owl#DeviceGray -->

    <PDF1.3_Properties rdf:about="#DeviceGray"/>
    


    <!-- http://www.semanticweb.org/ontologies/2008/7/XCLOntology1.5.owl#DeviceN -->

    <PDF1.3_Properties rdf:about="#DeviceN">
        <rdfs:comment xml:lang="en"
            >DeviceN color spaces (PDF 1.3) can contain an arbitrary number of color components. They provide greater flexibility than is possible with standard device color spaces such as DeviceCMYK or with individual Separation color spaces. For example, it is possible to create a DeviceN color space consisting of only the cyan, magenta, and yellow color components, with the black component excluded. [cit.]</rdfs:comment>
    </PDF1.3_Properties>
    


    <!-- http://www.semanticweb.org/ontologies/2008/7/XCLOntology1.5.owl#DeviceRGB -->

    <PDF1.3_Properties rdf:about="#DeviceRGB"/>
    


    <!-- http://www.semanticweb.org/ontologies/2008/7/XCLOntology1.5.owl#DeviceSource_NISO -->

    <NISO rdf:about="#DeviceSource_NISO">
        <rdfs:comment
            >Classification of device used to create the image data. [cit. NISO]</rdfs:comment>
        <Datatype rdf:resource="#string"/>
    </NISO>
    


    <!-- http://www.semanticweb.org/ontologies/2008/7/XCLOntology1.5.owl#DigitalCameraManufacturer_NISO -->

    <NISO rdf:about="#DigitalCameraManufacturer_NISO">
        <rdfs:comment
            >The manufacturer of the digital camera used to create the image. [cit. NISO]</rdfs:comment>
        <Datatype rdf:resource="#string"/>
    </NISO>
    


    <!-- http://www.semanticweb.org/ontologies/2008/7/XCLOntology1.5.owl#DigitalCameraModel_NISO -->

    <NISO rdf:about="#DigitalCameraModel_NISO">
        <rdfs:comment
            >The model of the digital camera used to create the image. [cit. NISO]</rdfs:comment>
        <Datatype rdf:resource="#string"/>
    </NISO>
    


    <!-- http://www.semanticweb.org/ontologies/2008/7/XCLOntology1.5.owl#DisplayOrientation_NISO -->

    <NISO rdf:about="#DisplayOrientation_NISO">
        <rdfs:comment
            >0 = portrait
1 = landscape
This value is important to record when the preferred orientation of the image sent to a 3:2 aspect ratio computer monitor is different from Orientation. 

While Orientation refers to the placement of pixels in the digital image file, DisplayOrientation refers to the preferred orientation in which to display the content (text, picture, table, etc.) within the file.

This field will likely become obsolete when &#8220;standard&#8221; delivery applications, such as web browsers, incorporate an image rotation tool.
[cit. NISO]</rdfs:comment>
        <Datatype rdf:resource="#bool"/>
    </NISO>
    


    <!-- http://www.semanticweb.org/ontologies/2008/7/XCLOntology1.5.owl#DotGain -->

    <PDF1.3_Properties rdf:about="#DotGain"/>
    


    <!-- http://www.semanticweb.org/ontologies/2008/7/XCLOntology1.5.owl#DotRange_Tiff -->

    <Tiff_Properties rdf:about="#DotRange_Tiff">
        <rdfs:comment
            >Type		BYTE or SHORT
Count		2, or 2*SamplesPerPixel
Default		[0,2**BitsPerSample-1]
Description

The component values that correspond to a 0% dot and 100% dot.
DotRange[0] corresponds to a 0% dot, and DotRange[1] corresponds to a 100% dot.
It is possible, though strongly discouraged, to have a pair of DotRange values per component. [cit.Tiff]</rdfs:comment>
        <Datatype rdf:resource="#int"/>
    </Tiff_Properties>
    


    <!-- http://www.semanticweb.org/ontologies/2008/7/XCLOntology1.5.owl#EarlyChange -->

    <PDF1.3_Properties rdf:about="#EarlyChange">
        <rdfs:comment
            >(LZWDecode only) An indication of when to increase the code length. If the 
value of this entry is 0, code length increases are postponed as long as possible. If it is 1, they occur one code early. This parameter is included because LZW sample code distributed by some vendors increases the code length one code earlier than necessary. Default value: 1. [cit. Pdf 1.3]</rdfs:comment>
        <Datatype rdf:resource="#int"/>
    </PDF1.3_Properties>
    


    <!-- http://www.semanticweb.org/ontologies/2008/7/XCLOntology1.5.owl#Encode -->

    <PDF1.3_Properties rdf:about="#Encode">
        <rdfs:comment
            >(Optional) An array of 2 &#215; m numbers specifying the linear mapping of input values into the domain of the function&#8217;s sample table. Default value: 
[0  (Size  &#8722; 1)  0  (Size &#8722; 1) [cit. Pdf 1.3]</rdfs:comment>
        <Datatype rdf:resource="#matrix"/>
    </PDF1.3_Properties>
    


    <!-- http://www.semanticweb.org/ontologies/2008/7/XCLOntology1.5.owl#EncodingOptions_NISO -->

    <NISO rdf:about="#EncodingOptions_NISO">
        <rdfs:comment
            >a container of information detailing JPEG 2000 encoding options; comprisedof three data elements (7.2.1.2.1 tiles, 7.2.1.2.2 qualityLayers, and 7.2.1.2.3 resolutionLevels) [cit NISO MIX]</rdfs:comment>
        <Datatype rdf:resource="#int"/>
    </NISO>
    


    <!-- http://www.semanticweb.org/ontologies/2008/7/XCLOntology1.5.owl#EncodingType -->

    <PDF1.3_Properties rdf:about="#EncodingType">
        <is_same_as rdf:resource="#fontEncodingType"/>
    </PDF1.3_Properties>
    


    <!-- http://www.semanticweb.org/ontologies/2008/7/XCLOntology1.5.owl#ExposureBias_NISO -->

    <NISO rdf:about="#ExposureBias_NISO">
        <rdfs:comment
            >This specifies the actual exposure bias (the amount of under or over-exposure relative to a normal exposure, as determined by the camera&#39;s exposure system) used when capturing the image, using APEX units.[cit. NISO]</rdfs:comment>
        <Datatype rdf:resource="#rational"/>
    </NISO>
    


    <!-- http://www.semanticweb.org/ontologies/2008/7/XCLOntology1.5.owl#ExposureIndex_NISO -->

    <NISO rdf:about="#ExposureIndex_NISO">
        <rdfs:comment
            >This specifies the exposure index setting used. [cit. NISO]</rdfs:comment>
        <Datatype rdf:resource="#rational"/>
    </NISO>
    


    <!-- http://www.semanticweb.org/ontologies/2008/7/XCLOntology1.5.owl#ExposureTime_NISO -->

    <NISO rdf:about="#ExposureTime_NISO">
        <rdfs:comment
            >This specifies the exposure time used when the image was captured.  The value is to be recorded in seconds. [cit. NISO]</rdfs:comment>
        <Datatype rdf:resource="#rational"/>
    </NISO>
    


    <!-- http://www.semanticweb.org/ontologies/2008/7/XCLOntology1.5.owl#Extrasamples_NISO -->

    <NISO rdf:about="#Extrasamples_NISO">
        <rdfs:comment
            >Specifies that each pixel has M extra components whose interpretation is defined by one of the values listed below.   Values:
0 = unspecified data
1 = associated alpha data (with pre-multiplied color)
2 = unassociated alpha data
3 = range or depth data
[cit. NISO]</rdfs:comment>
        <is_same_as rdf:resource="#extraSamples_Tiff"/>
        <Datatype rdf:resource="#int"/>
    </NISO>
    


    <!-- http://www.semanticweb.org/ontologies/2008/7/XCLOntology1.5.owl#F1 -->

    <PDF1.3_Properties rdf:about="#F1">
        <rdfs:comment>PDF Base14 Font</rdfs:comment>
        <is_same_as rdf:resource="#Helvetica"/>
    </PDF1.3_Properties>
    


    <!-- http://www.semanticweb.org/ontologies/2008/7/XCLOntology1.5.owl#F10 -->

    <PDF1.3_Properties rdf:about="#F10">
        <rdfs:comment>PDF Base14 Font</rdfs:comment>
        <is_same_as rdf:resource="#CourierOblique"/>
    </PDF1.3_Properties>
    


    <!-- http://www.semanticweb.org/ontologies/2008/7/XCLOntology1.5.owl#F11 -->

    <PDF1.3_Properties rdf:about="#F11">
        <rdfs:comment>PDF Base14 Font</rdfs:comment>
        <is_same_as rdf:resource="#CourierBold"/>
    </PDF1.3_Properties>
    


    <!-- http://www.semanticweb.org/ontologies/2008/7/XCLOntology1.5.owl#F12 -->

    <PDF1.3_Properties rdf:about="#F12">
        <rdfs:comment>PDF Base14 Font</rdfs:comment>
        <is_same_as rdf:resource="#CourierBoldOblique"/>
    </PDF1.3_Properties>
    


    <!-- http://www.semanticweb.org/ontologies/2008/7/XCLOntology1.5.owl#F13 -->

    <PDF1.3_Properties rdf:about="#F13">
        <rdfs:comment>PDF Base14 Font</rdfs:comment>
        <is_same_as rdf:resource="#Symbol"/>
    </PDF1.3_Properties>
    


    <!-- http://www.semanticweb.org/ontologies/2008/7/XCLOntology1.5.owl#F14 -->

    <PDF1.3_Properties rdf:about="#F14">
        <rdfs:comment>PDF Base14 Font</rdfs:comment>
        <is_same_as rdf:resource="#ZapfDingbats"/>
    </PDF1.3_Properties>
    


    <!-- http://www.semanticweb.org/ontologies/2008/7/XCLOntology1.5.owl#F2 -->

    <PDF1.3_Properties rdf:about="#F2">
        <rdfs:comment>PDF Base14 Font</rdfs:comment>
        <is_same_as rdf:resource="#HelveticaOblique"/>
    </PDF1.3_Properties>
    


    <!-- http://www.semanticweb.org/ontologies/2008/7/XCLOntology1.5.owl#F3 -->

    <PDF1.3_Properties rdf:about="#F3">
        <rdfs:comment>PDF Base14 Font</rdfs:comment>
        <is_same_as rdf:resource="#HelveticaBold"/>
    </PDF1.3_Properties>
    


    <!-- http://www.semanticweb.org/ontologies/2008/7/XCLOntology1.5.owl#F4 -->

    <PDF1.3_Properties rdf:about="#F4">
        <rdfs:comment>PDF Base14 Font</rdfs:comment>
        <is_same_as rdf:resource="#HelveticaBoldOblique"/>
    </PDF1.3_Properties>
    


    <!-- http://www.semanticweb.org/ontologies/2008/7/XCLOntology1.5.owl#F5 -->

    <PDF1.3_Properties rdf:about="#F5">
        <is_same_as rdf:resource="#TimesRoman"/>
    </PDF1.3_Properties>
    


    <!-- http://www.semanticweb.org/ontologies/2008/7/XCLOntology1.5.owl#F6 -->

    <PDF1.3_Properties rdf:about="#F6">
        <rdfs:comment>PDF Base14 Font</rdfs:comment>
        <is_same_as rdf:resource="#TimesItalic"/>
    </PDF1.3_Properties>
    


    <!-- http://www.semanticweb.org/ontologies/2008/7/XCLOntology1.5.owl#F7 -->

    <PDF1.3_Properties rdf:about="#F7">
        <rdfs:comment>PDF Base14 Font</rdfs:comment>
        <is_same_as rdf:resource="#TimesBold"/>
    </PDF1.3_Properties>
    


    <!-- http://www.semanticweb.org/ontologies/2008/7/XCLOntology1.5.owl#F8 -->

    <PDF1.3_Properties rdf:about="#F8">
        <rdfs:comment>PDF Base14 Font</rdfs:comment>
        <is_same_as rdf:resource="#TimesBoldItalic"/>
    </PDF1.3_Properties>
    


    <!-- http://www.semanticweb.org/ontologies/2008/7/XCLOntology1.5.owl#F9 -->

    <PDF1.3_Properties rdf:about="#F9">
        <rdfs:comment>PDF Base14 Font</rdfs:comment>
        <is_same_as rdf:resource="#Courier"/>
    </PDF1.3_Properties>
    


    <!-- http://www.semanticweb.org/ontologies/2008/7/XCLOntology1.5.owl#FNumber_NISO -->

    <NISO rdf:about="#FNumber_NISO">
        <rdfs:comment
            >This specifies the lens f-number (ratio of lens aperture to focal length) used when the image was captured. [cit. NISO]</rdfs:comment>
        <Datatype rdf:resource="#rational"/>
    </NISO>
    


    <!-- http://www.semanticweb.org/ontologies/2008/7/XCLOntology1.5.owl#FileSpeci&#64257;cation -->

    <PDF1.3_Properties rdf:about="#FileSpeci&#64257;cation">
        <rdfs:comment
            >A simple &#64257;le speci&#64257;cation that begins with a slash is an absolute &#64257;le speci&#64257;cation. 
The last component is the &#64257;le name; the preceding components specify its context. In some &#64257;le speci&#64257;cations, the &#64257;le name may be empty; for example, URL (uniform resource locator) speci&#64257;cations can specify directories instead of &#64257;les. A &#64257;le speci&#64257;cation that does not begin with a slash is a relative &#64257;le speci&#64257;cation giving the location of the &#64257;le relative to that of the PDF &#64257;le containing it. [cit. Pdf 1.3]
Examples Values:
Mac string (Optional) A &#64257;le speci&#64257;cation string (see Section 3.10.1, &#8220;File Speci&#64257;cation Strings&#8221;) 
representing a Macintosh &#64257;le name. 
DOS string (Optional) A &#64257;le speci&#64257;cation string (see Section 3.10.1, &#8220;File Speci&#64257;cation Strings&#8221;) 
representing a DOS &#64257;le name. 
Unix string (Optional) A &#64257;le speci&#64257;cation string (see Section 3.10.1, &#8220;File Speci&#64257;cation Strings&#8221;) 
representing a UNIX &#64257;le name.</rdfs:comment>
        <Datatype rdf:resource="#string"/>
    </PDF1.3_Properties>
    


    <!-- http://www.semanticweb.org/ontologies/2008/7/XCLOntology1.5.owl#File_ID_Part -->

    <PDF1.3_Properties rdf:about="#File_ID_Part">
        <rdfs:comment xml:lang="en"
            >External file references can be made more reliable by including a file identifier (PDF 1.1) in the file and using it in addition to the normal platform-based file designation. Matching the identifier in the file reference with the one in the file confirms whether the correct file was found.</rdfs:comment>
    </PDF1.3_Properties>
    


    <!-- http://www.semanticweb.org/ontologies/2008/7/XCLOntology1.5.owl#Filter -->

    <PDF1.3_Properties rdf:about="#Filter">
        <rdfs:comment
            >(Required) The name of the security handler for this document; see below. Default value: 
Standard, for the built-in security handler. (Names for nonstandard security handlers can be registered using the procedure described in Appendix E.)</rdfs:comment>
    </PDF1.3_Properties>
    


    <!-- http://www.semanticweb.org/ontologies/2008/7/XCLOntology1.5.owl#FixedPitched -->

    <fontFlag rdf:about="#FixedPitched">
        <rdfs:comment xml:lang="en"
            >Bit:1. All Glyphs have the same width (monospaced)</rdfs:comment>
    </fontFlag>
    


    <!-- http://www.semanticweb.org/ontologies/2008/7/XCLOntology1.5.owl#Fixity_NISO -->

    <NISO rdf:about="#Fixity_NISO">
        <Datatype rdf:resource="#int"/>
    </NISO>
    


    <!-- http://www.semanticweb.org/ontologies/2008/7/XCLOntology1.5.owl#FlashEnergy_NISO -->

    <NISO rdf:about="#FlashEnergy_NISO">
        <rdfs:comment
            >This specifies the amount of flash energy that was used in Beam Candle Power Seconds (BCPS). [cit. NISO]</rdfs:comment>
        <Datatype rdf:resource="#rational"/>
    </NISO>
    


    <!-- http://www.semanticweb.org/ontologies/2008/7/XCLOntology1.5.owl#FlashReturn_NISO -->

    <NISO rdf:about="#FlashReturn_NISO">
        <rdfs:comment
            >This specifies whether the camera judged that the flash was not effective at the time of exposure. [cit. NISO]</rdfs:comment>
        <Datatype rdf:resource="#bool"/>
    </NISO>
    


    <!-- http://www.semanticweb.org/ontologies/2008/7/XCLOntology1.5.owl#Flash_NISO -->

    <NISO rdf:about="#Flash_NISO">
        <rdfs:comment
            >This specifies whether a flash was used in image capture. [cit. NISO]</rdfs:comment>
        <Datatype rdf:resource="#bool"/>
    </NISO>
    


    <!-- http://www.semanticweb.org/ontologies/2008/7/XCLOntology1.5.owl#FlateDecode -->

    <PDF1.3_Properties rdf:about="#FlateDecode">
        <rdfs:comment
            >(PDF 1.2) Decompresses data encoded using the public-domain zlib/ 
de&#64258;ate compression method, reproducing the original text or binary 
data. (See implementation note 9 in Appendix H.) 
[cit. PDF 1.3]</rdfs:comment>
    </PDF1.3_Properties>
    


    <!-- http://www.semanticweb.org/ontologies/2008/7/XCLOntology1.5.owl#FocalLength_NISO -->

    <NISO rdf:about="#FocalLength_NISO">
        <rdfs:comment
            >This specifies the lens focal length in meters used to capture the image. [cit. NISO]</rdfs:comment>
        <Datatype rdf:resource="#rational"/>
    </NISO>
    


    <!-- http://www.semanticweb.org/ontologies/2008/7/XCLOntology1.5.owl#FontFamily -->

    <fontDescriptor rdf:about="#FontFamily">
        <Datatype rdf:resource="#string"/>
    </fontDescriptor>
    


    <!-- http://www.semanticweb.org/ontologies/2008/7/XCLOntology1.5.owl#FontFile -->

    <fontDescriptor rdf:about="#FontFile">
        <rdfs:comment xml:lang="en"
            >Type 1 font program, in the original (noncompact) format described in Adobe Type 1 Font Format. This entry can appear in the font descriptor for 
a Type1 or MMType1 font dictionary. [cit. Pdf 1.3]</rdfs:comment>
        <Datatype rdf:resource="#string"/>
    </fontDescriptor>
    


    <!-- http://www.semanticweb.org/ontologies/2008/7/XCLOntology1.5.owl#FontFile2 -->

    <fontDescriptor rdf:about="#FontFile2">
        <rdfs:comment xml:lang="en"
            >(PDF 1.1) TrueType font program, as described in the TrueType Reference Manual. This entry can appear in the font descriptor for a TrueType font dictionary or (in PDF 1.3) for a CIDFontType2 CIDFont dictionary. 
[cit. Pdf 1.3]</rdfs:comment>
        <Datatype rdf:resource="#string"/>
    </fontDescriptor>
    


    <!-- http://www.semanticweb.org/ontologies/2008/7/XCLOntology1.5.owl#FontFile3 -->

    <fontDescriptor rdf:about="#FontFile3">
        <rdfs:comment xml:lang="en"
            >Type1C (PDF 1.2) 
Type 1&#8211;equivalent font program represented in the Compact File Format (CFF), as described in Adobe Technical Note #5176, Compact File Format Speci&#64257;cation. This entry can appear in the font descriptor for a Type1 or MMType1 font dictionary. 
CIDFontType0C (PDF 1.3) 
Type 0 CIDFont program represented in the Compact File Format (CFF), as described in Adobe Technical Note #5176, Compact File Format Speci&#64257;cation. This entry can appear in the font descriptor for a CIDFontType0 CIDFont dictionary. 
other name 
Font or CIDFont program represented in some future format, identi&#64257;ed by other name as the font &#64257;le subtype.[cit.]</rdfs:comment>
        <Datatype rdf:resource="#string"/>
    </fontDescriptor>
    


    <!-- http://www.semanticweb.org/ontologies/2008/7/XCLOntology1.5.owl#FontMatrix -->

    <PDF1.3_Properties rdf:about="#FontMatrix">
        <rdfs:comment
            >(Required) An array of six numbers specifying the transformation from glyph space to text space (see Section 5.1.3, &#8220;Glyph Positioning and Metrics&#8221;). A common practice is to de&#64257;ne glyphs in terms of a 1000-unit glyph coordinate system, so the font matrix is [0.001  0  0  0.001  0  0]. 
[cit. Pdf 1.3]</rdfs:comment>
        <Datatype rdf:resource="#matrix"/>
    </PDF1.3_Properties>
    


    <!-- http://www.semanticweb.org/ontologies/2008/7/XCLOntology1.5.owl#FontName_PDF -->

    <fontDescriptor rdf:about="#FontName_PDF">
        <rdfs:comment xml:lang="en"
            >(Required) The PostScript name of the font. This name should be the same as the value of BaseFont in the font or CIDFont dictionary that refers to this 
font descriptor.[cit.]</rdfs:comment>
        <is_same_as rdf:resource="#fontName"/>
    </fontDescriptor>
    


    <!-- http://www.semanticweb.org/ontologies/2008/7/XCLOntology1.5.owl#FontSize_Pdf -->

    <PDF1.3_Properties rdf:about="#FontSize_Pdf">
        <is_same_as rdf:resource="#fontSize"/>
        <Datatype rdf:resource="#int"/>
    </PDF1.3_Properties>
    


    <!-- http://www.semanticweb.org/ontologies/2008/7/XCLOntology1.5.owl#FontStretch -->

    <fontDescriptor rdf:about="#FontStretch"/>
    


    <!-- http://www.semanticweb.org/ontologies/2008/7/XCLOntology1.5.owl#FontWeight -->

    <fontDescriptor rdf:about="#FontWeight"/>
    


    <!-- http://www.semanticweb.org/ontologies/2008/7/XCLOntology1.5.owl#ForceBold -->

    <fontFlag rdf:about="#ForceBold">
        <rdfs:comment xml:lang="en">Bit:19</rdfs:comment>
    </fontFlag>
    


    <!-- http://www.semanticweb.org/ontologies/2008/7/XCLOntology1.5.owl#FormFeed_Pdf -->

    <PDF1.3_Properties rdf:about="#FormFeed_Pdf">
        <rdfs:comment>\f</rdfs:comment>
        <Datatype rdf:resource="#string"/>
    </PDF1.3_Properties>
    


    <!-- http://www.semanticweb.org/ontologies/2008/7/XCLOntology1.5.owl#FunctionType -->

    <PDF1.3_Properties rdf:about="#FunctionType">
        <rdfs:comment
            >(Required) The function type: 
0 Sampled function 
2 Exponential interpolation function 
3 Stitching function 
4 PostScript calculator function 
[cit. Pdf 1.3]</rdfs:comment>
        <Datatype rdf:resource="#int"/>
    </PDF1.3_Properties>
    


    <!-- http://www.semanticweb.org/ontologies/2008/7/XCLOntology1.5.owl#GCM -->

    <GIF_Properties rdf:about="#GCM">
        <rdfs:comment xml:lang="en"
            >GlobalColourMap.
1=Global Colour Map exists
0=Local Colour Map exists</rdfs:comment>
    </GIF_Properties>
    


    <!-- http://www.semanticweb.org/ontologies/2008/7/XCLOntology1.5.owl#GDALMetadata -->

    <imageInformation rdf:about="#GDALMetadata">
        <rdfs:comment
            >Used by the GDAL library, holds an XML list of name=value pairs</rdfs:comment>
        <ID>id63</ID>
        <Datatype rdf:resource="#string"/>
    </imageInformation>
    


    <!-- http://www.semanticweb.org/ontologies/2008/7/XCLOntology1.5.owl#GIF_Signature -->

    <GIF_Properties rdf:about="#GIF_Signature">
        <is_same_as rdf:resource="#signature"/>
    </GIF_Properties>
    


    <!-- http://www.semanticweb.org/ontologies/2008/7/XCLOntology1.5.owl#GammaCalGray -->

    <PDF1.3_Properties rdf:about="#GammaCalGray">
        <rdfs:comment xml:lang="en"
            >(Optional) A number G defining the gamma for the gray (A) component. G 
must be positive and is generally greater than or equal to 1. Default value: 1. [cit.]</rdfs:comment>
        <Datatype rdf:resource="#int"/>
    </PDF1.3_Properties>
    


    <!-- http://www.semanticweb.org/ontologies/2008/7/XCLOntology1.5.owl#GammaCalRGB -->

    <PDF1.3_Properties rdf:about="#GammaCalRGB">
        <rdfs:comment xml:lang="en"
            >(Optional) An array of three numbers [ G R GG GB ] specifying the gamma for the red, green, and blue (A, B, and C) components of the color space. Default value: [ 1.0 1.0 1.0 ]. [cit.]</rdfs:comment>
        <Datatype rdf:resource="#int"/>
    </PDF1.3_Properties>
    


    <!-- http://www.semanticweb.org/ontologies/2008/7/XCLOntology1.5.owl#GlyphBoundingBox -->

    <PDF1.3_Properties rdf:about="#GlyphBoundingBox">
        <rdfs:comment
            >The glyph bounding box is the smallest rectangle (oriented with the axes of the glyph coordinate system) that will just enclose the entire glyph shape. The bounding box is expressed in terms of its left, bottom, right, and top coordinates relative to the glyph origin in the glyph coordinate system. 
[cit. Pdf 1.3]</rdfs:comment>
        <Datatype rdf:resource="#matrix"/>
    </PDF1.3_Properties>
    


    <!-- http://www.semanticweb.org/ontologies/2008/7/XCLOntology1.5.owl#GlyphDisplacmentVector -->

    <PDF1.3_Properties rdf:about="#GlyphDisplacmentVector">
        <rdfs:comment
            >The glyph displacement is the distance from the glyph&#8217;s origin to the point at which the origin of the next glyph should normally be placed when painting the consecutive glyphs of a line of text. This distance is a vector (called the displacement vector) in the glyph coordinate system; it has x and y components. (A displacement that is horizontal is usually called a width.) Most Indo-European alphabets, including the Latin alphabet, have a positive x displacement and a zero y displacement; some Asian writing systems have a nonzero y displacement. [cit. Pdf 1.3]</rdfs:comment>
    </PDF1.3_Properties>
    


    <!-- http://www.semanticweb.org/ontologies/2008/7/XCLOntology1.5.owl#GlyphWidth -->

    <PDF1.3_Properties rdf:about="#GlyphWidth">
        <rdfs:comment>Fontmetric</rdfs:comment>
        <Datatype rdf:resource="#int"/>
    </PDF1.3_Properties>
    


    <!-- http://www.semanticweb.org/ontologies/2008/7/XCLOntology1.5.owl#GrayResponseCurve_NISO -->

    <NISO rdf:about="#GrayResponseCurve_NISO">
        <rdfs:comment
            >For grayscale data, the optical density of each possible pixel value. [cit. NISO]</rdfs:comment>
        <is_same_as rdf:resource="#grayResponseCurve"/>
        <is_same_as rdf:resource="#grayResponseCurveTiff"/>
        <Datatype rdf:resource="#int"/>
    </NISO>
    


    <!-- http://www.semanticweb.org/ontologies/2008/7/XCLOntology1.5.owl#GrayResponseUnit_NISO -->

    <NISO rdf:about="#GrayResponseUnit_NISO">
        <rdfs:comment
            >The precision of the information contained in the GrayResponseCurve.
1 = Number represents tenths of a unit.
2 = Number represents hundredths of a unit.
3 = Number represents thousandths of a unit.
4 = Number represents ten-thousandths of a unit.
5 = Number represents hundred-thousandths of a unit.
[CIT. NISO]</rdfs:comment>
        <is_same_as rdf:resource="#grayResponseUnit"/>
        <is_same_as rdf:resource="#grayResponseUnitTiff"/>
        <Datatype rdf:resource="#int"/>
    </NISO>
    


    <!-- http://www.semanticweb.org/ontologies/2008/7/XCLOntology1.5.owl#Gray_ICC -->

    <PDF1.3_Properties rdf:about="#Gray_ICC">
        <rdfs:comment
            >Ranges for typical ICC color spaces.
COMPONENT RANGES [0.01.0] 
[cit. Pdf 1.3]</rdfs:comment>
        <is_same_as rdf:resource="#gray"/>
    </PDF1.3_Properties>
    


    <!-- http://www.semanticweb.org/ontologies/2008/7/XCLOntology1.5.owl#HalftoneHintsTiff -->

    <Tiff_Properties rdf:about="#HalftoneHintsTiff">
        <rdfs:comment
            >Conveys to the halftone function the range of gray levels within a colorimetrically-specified image that should retain tonal detail.[cit. Tiff]</rdfs:comment>
    </Tiff_Properties>
    


    <!-- http://www.semanticweb.org/ontologies/2008/7/XCLOntology1.5.owl#Height_Gif -->

    <GIF_Properties rdf:about="#Height_Gif">
        <is_same_as rdf:resource="#imageHeight"/>
        <Datatype rdf:resource="#int"/>
    </GIF_Properties>
    


    <!-- http://www.semanticweb.org/ontologies/2008/7/XCLOntology1.5.owl#Helvetica -->

    <textInformation rdf:about="#Helvetica">
        <ID>id306</ID>
        <is_same_as rdf:resource="#F1"/>
    </textInformation>
    


    <!-- http://www.semanticweb.org/ontologies/2008/7/XCLOntology1.5.owl#HelveticaBold -->

    <textInformation rdf:about="#HelveticaBold">
        <ID>id309</ID>
        <is_same_as rdf:resource="#F3"/>
    </textInformation>
    


    <!-- http://www.semanticweb.org/ontologies/2008/7/XCLOntology1.5.owl#HelveticaBoldOblique -->

    <textInformation rdf:about="#HelveticaBoldOblique">
        <ID>id308</ID>
        <is_same_as rdf:resource="#F4"/>
    </textInformation>
    


    <!-- http://www.semanticweb.org/ontologies/2008/7/XCLOntology1.5.owl#HelveticaOblique -->

    <textInformation rdf:about="#HelveticaOblique">
        <ID>id307</ID>
        <is_same_as rdf:resource="#F2"/>
    </textInformation>
    


    <!-- http://www.semanticweb.org/ontologies/2008/7/XCLOntology1.5.owl#HorizontalTab_Pdf -->

    <PDF1.3_Properties rdf:about="#HorizontalTab_Pdf">
        <rdfs:comment>\t</rdfs:comment>
        <Datatype rdf:resource="#string"/>
    </PDF1.3_Properties>
    


    <!-- http://www.semanticweb.org/ontologies/2008/7/XCLOntology1.5.owl#HostComputer_NISO -->

    <NISO rdf:about="#HostComputer_NISO">
        <rdfs:comment
            >Computer and/or operating system in use at the time of image creation.[cit. NISO]</rdfs:comment>
        <is_same_as rdf:resource="#hostCompOS"/>
        <is_same_as rdf:resource="#hostComputer_TIff"/>
        <Datatype rdf:resource="#string"/>
    </NISO>
    


    <!-- http://www.semanticweb.org/ontologies/2008/7/XCLOntology1.5.owl#ICCBased -->

    <PDF1.3_Properties rdf:about="#ICCBased"/>
    


    <!-- http://www.semanticweb.org/ontologies/2008/7/XCLOntology1.5.owl#ICCProfileName -->

    <imageInformation rdf:about="#ICCProfileName">
        <rdfs:comment
            >Name of the description of the colour space (in the form of an International colour Consortium (ICC) profile) to which the samples in the image conform, should be something like: sRGB IEC1966-2.1, Adobe RGB &#180;98, for cmyk: ISO Coated V2 (ECI) and ISO Uncoated</rdfs:comment>
        <ID>id43</ID>
        <is_same_as rdf:resource="#ICCBased"/>
        <is_same_as rdf:resource="#ICCProfile_Tiff"/>
        <is_same_as rdf:resource="#iCCP"/>
    </imageInformation>
    


    <!-- http://www.semanticweb.org/ontologies/2008/7/XCLOntology1.5.owl#ICCProfile_Tiff -->

    <Tiff_Properties rdf:about="#ICCProfile_Tiff">
        <rdfs:comment
            >Color profile data</rdfs:comment>
        <is_same_as rdf:resource="#ICCProfileName"/>
    </Tiff_Properties>
    


    <!-- http://www.semanticweb.org/ontologies/2008/7/XCLOntology1.5.owl#ID -->

    <ID rdf:about="#ID">
        <rdf:type rdf:resource="&owl;Class"/>
    </ID>
    


    <!-- http://www.semanticweb.org/ontologies/2008/7/XCLOntology1.5.owl#ID3Tag -->

    <audioInformation rdf:about="#ID3Tag">
        <ID>id209</ID>
        <Unit rdf:resource="#NULL"/>
        <Datatype rdf:resource="#string"/>
    </audioInformation>
    


    <!-- http://www.semanticweb.org/ontologies/2008/7/XCLOntology1.5.owl#IDAT -->

    <GIF_Properties rdf:about="#IDAT">
        <rdfs:comment xml:lang="en"
            >BitmapData Chunk</rdfs:comment>
    </GIF_Properties>
    


    <!-- http://www.semanticweb.org/ontologies/2008/7/XCLOntology1.5.owl#IHDR -->

    <PNG_Properties rdf:about="#IHDR">
        <rdfs:comment xml:lang="en"
            >file-header chunk in PNG-file.
Place to store Interlacing Methods</rdfs:comment>
    </PNG_Properties>
    


    <!-- http://www.semanticweb.org/ontologies/2008/7/XCLOntology1.5.owl#IL -->

    <GIF_Properties rdf:about="#IL">
        <rdfs:comment xml:lang="en">Interlaced</rdfs:comment>
    </GIF_Properties>
    


    <!-- http://www.semanticweb.org/ontologies/2008/7/XCLOntology1.5.owl#IPTC_Metadata -->

    <audioInformation rdf:about="#IPTC_Metadata">
        <rdf:type rdf:resource="#imageInformation"/>
        <rdf:type rdf:resource="#textInformation"/>
        <rdf:type rdf:resource="#videoinformation"/>
        <rdfs:comment xml:lang="en"
            >Standards of the International Press Telecommunications Council (IPTC) and Newspaper Association of America (NAA) for annotating content of any medial kind</rdfs:comment>
        <ID>id65</ID>
        <Unit rdf:resource="#NULL"/>
        <Datatype rdf:resource="#string"/>
    </audioInformation>
    


    <!-- http://www.semanticweb.org/ontologies/2008/7/XCLOntology1.5.owl#ISO-639 -->

    <xcl_propertyDatatypes rdf:about="#ISO-639">
        <rdfs:comment
            >Language Specification</rdfs:comment>
    </xcl_propertyDatatypes>
    


    <!-- http://www.semanticweb.org/ontologies/2008/7/XCLOntology1.5.owl#ISO216 -->

    <xcl_propertyDatatypes rdf:about="#ISO216">
        <rdfs:comment
            >Din Formats for Paper</rdfs:comment>
    </xcl_propertyDatatypes>
    


    <!-- http://www.semanticweb.org/ontologies/2008/7/XCLOntology1.5.owl#ImageData_NISO -->

    <NISO rdf:about="#ImageData_NISO">
        <rdfs:comment
            >Identifies the path where the digital image of the reference target identified in 4.3.2 TargetID is located.[cit. NISO]</rdfs:comment>
        <is_same_as rdf:resource="#imageData"/>
        <Datatype rdf:resource="#string"/>
    </NISO>
    


    <!-- http://www.semanticweb.org/ontologies/2008/7/XCLOntology1.5.owl#ImageIdentifierLocation_NISO -->

    <NISO rdf:about="#ImageIdentifierLocation_NISO">
        <rdfs:comment
            >A location qualifier to be used in conjunction with ImageIdentifier [cit. NISO].</rdfs:comment>
        <Datatype rdf:resource="#string"/>
    </NISO>
    


    <!-- http://www.semanticweb.org/ontologies/2008/7/XCLOntology1.5.owl#ImageIdentifier_NISO -->

    <NISO rdf:about="#ImageIdentifier_NISO">
        <rdfs:comment
            >A unique Identifier</rdfs:comment>
        <Datatype rdf:resource="#string"/>
    </NISO>
    


    <!-- http://www.semanticweb.org/ontologies/2008/7/XCLOntology1.5.owl#ImageLength_NISO -->

    <NISO rdf:about="#ImageLength_NISO">
        <rdfs:comment
            >This specifies the length of the digital image, i.e. vertical or Y dimension,  in pixels. [cit. NISO]</rdfs:comment>
        <is_same_as rdf:resource="#Height_Gif"/>
        <is_same_as rdf:resource="#ImageLength_tiff"/>
        <is_same_as rdf:resource="#imageHeight"/>
        <Datatype rdf:resource="#int"/>
    </NISO>
    


    <!-- http://www.semanticweb.org/ontologies/2008/7/XCLOntology1.5.owl#ImageLength_tiff -->

    <Tiff_Properties rdf:about="#ImageLength_tiff">
        <rdfs:comment
            >The number of rows of pixels in the image.</rdfs:comment>
        <is_same_as rdf:resource="#ImageLength_NISO"/>
        <Datatype rdf:resource="#int"/>
    </Tiff_Properties>
    


    <!-- http://www.semanticweb.org/ontologies/2008/7/XCLOntology1.5.owl#ImageMask -->

    <PDF1.3_Properties rdf:about="#ImageMask">
        <rdfs:comment
            >(Optional) A &#64258;ag indicating whether the image is to be treated as an image mask (see Section 4.8.5, &#8220;Masked Images&#8221;). If this &#64258;ag is true, the value of BitsPerComponent must be 1 and Mask and ColorSpace should not be speci&#64257;ed; unmasked areas will be painted using the current nonstroking color. Default value: false. 
[cit. Pdf 1.3]</rdfs:comment>
        <Datatype rdf:resource="#bool"/>
    </PDF1.3_Properties>
    


    <!-- http://www.semanticweb.org/ontologies/2008/7/XCLOntology1.5.owl#ImageProducer_NISO -->

    <NISO rdf:about="#ImageProducer_NISO">
        <rdfs:comment
            >Identifies the organization level producer(s) of the image.[cit. NISO]</rdfs:comment>
        <Datatype rdf:resource="#string"/>
    </NISO>
    


    <!-- http://www.semanticweb.org/ontologies/2008/7/XCLOntology1.5.owl#ImageSeparator -->

    <GIF_Properties rdf:about="#ImageSeparator">
        <rdfs:comment xml:lang="en"
            >hexadecimalValue that separates two single pictures from another (in an animated Gif)</rdfs:comment>
    </GIF_Properties>
    


    <!-- http://www.semanticweb.org/ontologies/2008/7/XCLOntology1.5.owl#ImageWidth_NISO -->

    <NISO rdf:about="#ImageWidth_NISO">
        <rdfs:comment
            >This specifies the width of the digital image, i.e. horizontal or X dimension, in pixels. [cit. NISO]</rdfs:comment>
        <is_same_as rdf:resource="#ImageWidth_tiff"/>
        <is_same_as rdf:resource="#Width_Gif"/>
        <is_same_as rdf:resource="#imageWidth"/>
        <Datatype rdf:resource="#int"/>
    </NISO>
    


    <!-- http://www.semanticweb.org/ontologies/2008/7/XCLOntology1.5.owl#ImageWidth_tiff -->

    <Tiff_Properties rdf:about="#ImageWidth_tiff">
        <rdfs:comment
            >The number of columns in the image, i.e., the number of pixels per row.</rdfs:comment>
        <is_same_as rdf:resource="#ImageWidth_NISO"/>
        <is_same_as rdf:resource="#Width_Gif"/>
        <is_same_as rdf:resource="#imageWidth"/>
        <Datatype rdf:resource="#int"/>
    </Tiff_Properties>
    


    <!-- http://www.semanticweb.org/ontologies/2008/7/XCLOntology1.5.owl#Indexed -->

    <PDF1.3_Properties rdf:about="#Indexed">
        <rdfs:comment xml:lang="en"
            >An Indexed color space allows a PDF content stream to use small integers as indices into a color map or color table of arbitrary colors in some other space. A PDF consumer application treats each sample value as an index into the color table and uses the color value it finds there. This technique can considerably reduce the amount of data required to represent a sampled image&#8212;for example, by using 8-bit index values as samples instead of 24-bit RGB color values. An Indexed color space is defined by a four-element array: [ /Indexed base hival lookup ] 
The first element is the color space family name Indexed. The remaining elements are parameters that an Indexed color space requires. Setting the current stroking or nonstroking color space to an Indexed color space initializes the corresponding current color to 0. [cit.]</rdfs:comment>
    </PDF1.3_Properties>
    


    <!-- http://www.semanticweb.org/ontologies/2008/7/XCLOntology1.5.owl#Indexed_Tiff -->

    <Tiff_Properties rdf:about="#Indexed_Tiff">
        <rdfs:comment
            >Aims to broaden the support for indexed images to include support for any color space.
Indexed images are images where the pixels do not represent color values, but rather an index (usually 8-bit) into a separate color table, the ColorMap.
ColorMap is required for an Indexed image.
The specification supplement defines these values:
0 = not indexed
1 = indexed [cit. Tiff]</rdfs:comment>
        <Datatype rdf:resource="#bool"/>
    </Tiff_Properties>
    


    <!-- http://www.semanticweb.org/ontologies/2008/7/XCLOntology1.5.owl#IndirectObjectKey -->

    <PDF1.3_Properties rdf:about="#IndirectObjectKey"/>
    


    <!-- http://www.semanticweb.org/ontologies/2008/7/XCLOntology1.5.owl#InkNames_Tiff -->

    <Tiff_Properties rdf:about="#InkNames_Tiff">
        <rdfs:comment
            >The name of each ink used in a separated image.
These names are written as a list of concatenated, NUL-terminated ASCII strings. The number of strings must be equal to NumberOfInks.
The samples are in the same order as the ink names. [cit. Tiff]</rdfs:comment>
        <Datatype rdf:resource="#string"/>
    </Tiff_Properties>
    


    <!-- http://www.semanticweb.org/ontologies/2008/7/XCLOntology1.5.owl#InkSet_Tiff -->

    <Tiff_Properties rdf:about="#InkSet_Tiff">
        <rdfs:comment
            >The set of inks used in a separated (PhotometricInterpretation=5) image.
The specification defines these values:
1 = CMYK. The order of the components is cyan, magenta, yellow, black. Usually, a value of 0 represents 0% ink coverage and a value of 255 represents 100% ink coverage for that component, but see DotRange. The InkNames field should not exist when InkSet=1.
2 = not CMYK. See the InkNames field for a description of the inks to be used.</rdfs:comment>
        <Datatype rdf:resource="#int"/>
    </Tiff_Properties>
    


    <!-- http://www.semanticweb.org/ontologies/2008/7/XCLOntology1.5.owl#Interlace_0 -->

    <PNG_Properties rdf:about="#Interlace_0">
        <rdfs:comment xml:lang="en"
            >With interlace method 0, pixels are stored sequentially from left to right, and scanlines sequentially from top to bottom (no interlacing).</rdfs:comment>
    </PNG_Properties>
    


    <!-- http://www.semanticweb.org/ontologies/2008/7/XCLOntology1.5.owl#Interlace_1 -->

    <PNG_Properties rdf:about="#Interlace_1">
        <rdfs:comment xml:lang="en"
            >stands for interlacing-Method: adam7.
It consists of seven distinct passes over the image. Each pass transmits a subset of the pixels in the image. The pass in which each pixel is transmitted is defined by replicating the following 8-by-8 pattern over the entire image, starting at the upper left corner. Caution if the Image has less than 5 rows or columns!</rdfs:comment>
        <is_same_as rdf:resource="#interlace"/>
    </PNG_Properties>
    


    <!-- http://www.semanticweb.org/ontologies/2008/7/XCLOntology1.5.owl#Interpolate -->

    <PDF1.3_Properties rdf:about="#Interpolate">
        <rdfs:comment
            >(Optional) A &#64258;ag indicating whether image interpolation is to be performed (see &#8220;Image Interpolation&#8221; on page 255). Default value: false. [cit. Pdf 1.3]</rdfs:comment>
        <Datatype rdf:resource="#bool"/>
    </PDF1.3_Properties>
    


    <!-- http://www.semanticweb.org/ontologies/2008/7/XCLOntology1.5.owl#Italic -->

    <fontFlag rdf:about="#Italic">
        <rdfs:comment xml:lang="en">Bit:7</rdfs:comment>
    </fontFlag>
    


    <!-- http://www.semanticweb.org/ontologies/2008/7/XCLOntology1.5.owl#ItalicAngle -->

    <fontDescriptor rdf:about="#ItalicAngle">
        <rdfs:comment xml:lang="en"
            >(Required) The angle, expressed in degrees counterclockwise from the vertical, of the dominant vertical strokes of the font. (For example, the 9-o&#8217;clock position is 90 degrees, and the 3-o&#8217;clock position is &#8211;90 degrees.) The value is negative for fonts that slope to the right, as almost all italic fonts do.</rdfs:comment>
        <Datatype rdf:resource="#int"/>
    </fontDescriptor>
    


    <!-- http://www.semanticweb.org/ontologies/2008/7/XCLOntology1.5.owl#JBIG2Decode -->

    <PDF1.3_Properties rdf:about="#JBIG2Decode">
        <rdfs:comment
            >Decompresses data encoded using the JBIG2 standard, reproducing the original monochrome (1 bit per pixel) image data (or an approximation of that data). [cit. PDF 1.4]</rdfs:comment>
    </PDF1.3_Properties>
    


    <!-- http://www.semanticweb.org/ontologies/2008/7/XCLOntology1.5.owl#JBIG2Globals -->

    <PDF1.3_Properties rdf:about="#JBIG2Globals">
        <rdfs:comment
            >A stream containing the JBIG2 global (page 0) segments. Global segments must be placed in this stream even if only a single JBIG2 image XObject refers to it. 
[cit. Pdf 1.4]</rdfs:comment>
        <Datatype rdf:resource="#string"/>
    </PDF1.3_Properties>
    


    <!-- http://www.semanticweb.org/ontologies/2008/7/XCLOntology1.5.owl#JPEG-Compression -->

    <rasterInformation rdf:about="#JPEG-Compression">
        <rdfs:comment xml:lang="en"
            >Compression Algorithm for Images</rdfs:comment>
    </rasterInformation>
    


    <!-- http://www.semanticweb.org/ontologies/2008/7/XCLOntology1.5.owl#L*a*b*_ICC -->

    <PDF1.3_Properties rdf:about="#L*a*b*_ICC">
        <rdfs:comment
            >Ranges for typical ICC color spaces.
Component Range: L*: [0100]; a* and b*: [&#8722;128127] 
[cit Pdf 1.3]</rdfs:comment>
    </PDF1.3_Properties>
    


    <!-- http://www.semanticweb.org/ontologies/2008/7/XCLOntology1.5.owl#L1 -->

    <layers rdf:about="#L1"/>
    


    <!-- http://www.semanticweb.org/ontologies/2008/7/XCLOntology1.5.owl#L2 -->

    <layers rdf:about="#L2"/>
    


    <!-- http://www.semanticweb.org/ontologies/2008/7/XCLOntology1.5.owl#L3 -->

    <layers rdf:about="#L3"/>
    


    <!-- http://www.semanticweb.org/ontologies/2008/7/XCLOntology1.5.owl#LCM -->

    <GIF_Properties rdf:about="#LCM">
        <rdfs:comment xml:lang="en"
            >local colour Map,
1=Global Colour Map exists
0=Local Colour Map exists</rdfs:comment>
    </GIF_Properties>
    


    <!-- http://www.semanticweb.org/ontologies/2008/7/XCLOntology1.5.owl#LZW -->

    <rasterInformation rdf:about="#LZW">
        <ID>id229</ID>
        <rdfs:comment xml:lang="en"
            >Compression Algorithm for Images</rdfs:comment>
    </rasterInformation>
    


    <!-- http://www.semanticweb.org/ontologies/2008/7/XCLOntology1.5.owl#LZWDecode -->

    <PDF1.3_Properties rdf:about="#LZWDecode">
        <rdfs:comment
            >Stream-Filter for decoding data as LZW-compressed in PDF 1.3</rdfs:comment>
    </PDF1.3_Properties>
    


    <!-- http://www.semanticweb.org/ontologies/2008/7/XCLOntology1.5.owl#Lab -->

    <PDF1.3_Properties rdf:about="#Lab">
        <rdfs:comment xml:lang="en"
            >ICC-based LAB ColourSpace</rdfs:comment>
    </PDF1.3_Properties>
    


    <!-- http://www.semanticweb.org/ontologies/2008/7/XCLOntology1.5.owl#Lang -->

    <PDF1.3_Properties rdf:about="#Lang">
        <rdfs:comment
            >Additional font descriptor entry for CIDFonts.
Language of the Font-Programm.
EN for English, JA for japanese.
Norm ISO 639</rdfs:comment>
        <Datatype rdf:resource="#ISO-639"/>
        <is_same_as rdf:resource="#documentLanguage"/>
    </PDF1.3_Properties>
    


    <!-- http://www.semanticweb.org/ontologies/2008/7/XCLOntology1.5.owl#LastModi&#64257;ed -->

    <PDF1.3_Properties rdf:about="#LastModi&#64257;ed">
        <rdfs:comment
            >(Optional unless PieceInfo is present; PDF 1.3) The date and time (see Section 3.8.2, &#8220;Dates&#8221;) when the page&#8217;s contents were most recently modi&#64257;ed. 
[cit. Pdf 1.3]</rdfs:comment>
        <Datatype rdf:resource="#timeISO8601"/>
    </PDF1.3_Properties>
    


    <!-- http://www.semanticweb.org/ontologies/2008/7/XCLOntology1.5.owl#Leading -->

    <fontDescriptor rdf:about="#Leading">
        <rdfs:comment xml:lang="en"
            >(Optional) lIt speci&#64257;es the vertical distance between the baselines of adjacent lines of text, as shown in Figure 5.9. The leading parameter is used by the TD, T*, &#39;, and &quot; operators[...]
The spacing between baselines of consecutive lines of text. Default value: 0. [cit]</rdfs:comment>
        <Datatype rdf:resource="#int"/>
    </fontDescriptor>
    


    <!-- http://www.semanticweb.org/ontologies/2008/7/XCLOntology1.5.owl#LeftParenthesis_Pdf -->

    <PDF1.3_Properties rdf:about="#LeftParenthesis_Pdf">
        <rdfs:comment>\(</rdfs:comment>
        <Datatype rdf:resource="#string"/>
    </PDF1.3_Properties>
    


    <!-- http://www.semanticweb.org/ontologies/2008/7/XCLOntology1.5.owl#Level1 -->

    <PDF1.3_Properties rdf:about="#Level1">
        <rdfs:comment
            >(Optional) A stream whose contents are to be used in place of the PostScript XObject&#8217;s stream when the PDF viewer knows that the target PostScript interpreter supports only LanguageLevel 1. 
[cit. Pdf 1.3]</rdfs:comment>
        <Datatype rdf:resource="#string"/>
    </PDF1.3_Properties>
    


    <!-- http://www.semanticweb.org/ontologies/2008/7/XCLOntology1.5.owl#LineButtCap -->

    <vectorInformation rdf:about="#LineButtCap">
        <is_same_as rdf:resource="#LineCapStyle0"/>
    </vectorInformation>
    


    <!-- http://www.semanticweb.org/ontologies/2008/7/XCLOntology1.5.owl#LineCapStyle0 -->

    <PDF1.3_Properties rdf:about="#LineCapStyle0">
        <rdfs:comment
            >0 Butt cap. The stroke is squared off at the endpoint of 
the path. There is no projection beyond the end of 
the path.</rdfs:comment>
        <is_same_as rdf:resource="#LineButtCap"/>
        <Datatype rdf:resource="#int"/>
    </PDF1.3_Properties>
    


    <!-- http://www.semanticweb.org/ontologies/2008/7/XCLOntology1.5.owl#LineCapStyle1 -->

    <PDF1.3_Properties rdf:about="#LineCapStyle1">
        <rdfs:comment
            >1 Round cap. A semicircular arc with a diameter equal 
to the line width is drawn around the endpoint and 
&#64257;lled in.</rdfs:comment>
        <is_same_as rdf:resource="#LineRoundCap"/>
        <Datatype rdf:resource="#int"/>
    </PDF1.3_Properties>
    


    <!-- http://www.semanticweb.org/ontologies/2008/7/XCLOntology1.5.owl#LineCapStyle2 -->

    <PDF1.3_Properties rdf:about="#LineCapStyle2">
        <rdfs:comment
            >2 Projecting square cap. The stroke continues beyond 
the endpoint of the path for a distance equal to half 
the line width and is then squared off.  [cit. Pdf 1.3]</rdfs:comment>
        <is_same_as rdf:resource="#LineSquareCap"/>
        <Datatype rdf:resource="#int"/>
    </PDF1.3_Properties>
    


    <!-- http://www.semanticweb.org/ontologies/2008/7/XCLOntology1.5.owl#LineDashPattern -->

    <PDF1.3_Properties rdf:about="#LineDashPattern">
        <rdfs:comment
            >A description of the dash pattern to be used when paths are stroked (see &#8220;Line Dash Pattern&#8221; on page 141). Initial value: a solid line. 
[ ] 0 No dash; solid, unbroken lines 
[3] 0 3 units on, 3 units off, &#8230; 
[2] 1 1 on, 2 off, 2 on, 2 off, &#8230; 
[21] 0 2 on, 1 off, 2 on, 1 off, &#8230; 
[35] 6 2 off, 3 on, 5 off, 3 on, 5 off, &#8230; 
[23] 11 1 on, 3 off, 2 on, 3 off, 2 on, &#8230; 
[cit. Pdf 1.3]</rdfs:comment>
        <Datatype rdf:resource="#int"/>
        <is_same_as rdf:resource="#strokeDasharray"/>
    </PDF1.3_Properties>
    


    <!-- http://www.semanticweb.org/ontologies/2008/7/XCLOntology1.5.owl#LineFeed_PDF -->

    <PDF1.3_Properties rdf:about="#LineFeed_PDF">
        <rdfs:comment>\n</rdfs:comment>
        <Datatype rdf:resource="#string"/>
    </PDF1.3_Properties>
    


    <!-- http://www.semanticweb.org/ontologies/2008/7/XCLOntology1.5.owl#LineJoinStyle1 -->

    <PDF1.3_Properties rdf:about="#LineJoinStyle1">
        <rdfs:comment
            >Miter join. The outer edges of the strokes for the two segments are extended until they meet at an angle, as in a picture frame. If the segments meet at too sharp an angle (as de&#64257;ned by the miter limit parameter&#8212; 
see &#8220;Miter Limit,&#8221; below), a bevel join is used instead. [cit. Pdf 1.3]</rdfs:comment>
        <Datatype rdf:resource="#int"/>
        <is_same_as rdf:resource="#lineJoinMiter"/>
    </PDF1.3_Properties>
    


    <!-- http://www.semanticweb.org/ontologies/2008/7/XCLOntology1.5.owl#LineJoinStyle2 -->

    <PDF1.3_Properties rdf:about="#LineJoinStyle2">
        <rdfs:comment
            >Round join. A circle with a diameter equal to the line width is drawn around the point where the two segments meet and is &#64257;lled in, producing a rounded corner. 
Note: If path segments shorter than half the line width meet at a sharp angle, an unintended &#8220;wrong side&#8221; of the circle may appear. 
[cit. Pdf 1.3]</rdfs:comment>
        <Datatype rdf:resource="#int"/>
        <is_same_as rdf:resource="#lineJoinRound"/>
    </PDF1.3_Properties>
    


    <!-- http://www.semanticweb.org/ontologies/2008/7/XCLOntology1.5.owl#LineJoinStyle3 -->

    <PDF1.3_Properties rdf:about="#LineJoinStyle3">
        <rdfs:comment
            >Bevel join. The two segments are &#64257;nished with butt caps (see &#8220;Line Cap Style&#8221; on page 139) and the resulting notch beyond the ends of the segments is &#64257;lled with a triangle. [cit. Pdf 1.3]</rdfs:comment>
        <Datatype rdf:resource="#int"/>
        <is_same_as rdf:resource="#lineJoinBevel"/>
    </PDF1.3_Properties>
    


    <!-- http://www.semanticweb.org/ontologies/2008/7/XCLOntology1.5.owl#LineRoundCap -->

    <vectorInformation rdf:about="#LineRoundCap">
        <is_same_as rdf:resource="#LineCapStyle1"/>
        <Datatype rdf:resource="#int"/>
    </vectorInformation>
    


    <!-- http://www.semanticweb.org/ontologies/2008/7/XCLOntology1.5.owl#LineSquareCap -->

    <vectorInformation rdf:about="#LineSquareCap">
        <is_same_as rdf:resource="#LineCapStyle2"/>
        <Datatype rdf:resource="#int"/>
    </vectorInformation>
    


    <!-- http://www.semanticweb.org/ontologies/2008/7/XCLOntology1.5.owl#MMType1 -->

    <PDF1.3_Properties rdf:about="#MMType1">
        <rdfs:comment
            >A multiple master font&#8212;an extension of the Type 1 font that allows the generation of a wide variety of typeface styles from a single font (see &#8220;Multiple Master Fonts&#8221; on page 297). [cit. Pdf 1.3]</rdfs:comment>
    </PDF1.3_Properties>
    


    <!-- http://www.semanticweb.org/ontologies/2008/7/XCLOntology1.5.owl#MPEG2_Part2_Codec -->

    <videoinformation rdf:about="#MPEG2_Part2_Codec">
        <rdfs:comment xml:lang="en"
            >Compression Algorithm for video-objects</rdfs:comment>
    </videoinformation>
    


    <!-- http://www.semanticweb.org/ontologies/2008/7/XCLOntology1.5.owl#MPEG2_Part3_Codec -->

    <audioInformation rdf:about="#MPEG2_Part3_Codec">
        <rdfs:comment xml:lang="en"
            >Audio compression algorithm</rdfs:comment>
    </audioInformation>
    


    <!-- http://www.semanticweb.org/ontologies/2008/7/XCLOntology1.5.owl#MPEG4_Part2_Codec -->

    <rasterInformation rdf:about="#MPEG4_Part2_Codec">
        <rdfs:comment xml:lang="en"
            >Compression Algorithm for Images</rdfs:comment>
    </rasterInformation>
    


    <!-- http://www.semanticweb.org/ontologies/2008/7/XCLOntology1.5.owl#MUSICAM -->

    <audioInformation rdf:about="#MUSICAM">
        <rdfs:comment xml:lang="en">AudioCodec</rdfs:comment>
    </audioInformation>
    


    <!-- http://www.semanticweb.org/ontologies/2008/7/XCLOntology1.5.owl#MacExpertEncoding -->

    <PDF1.3_Properties rdf:about="#MacExpertEncoding"/>
    


    <!-- http://www.semanticweb.org/ontologies/2008/7/XCLOntology1.5.owl#MacRomanEncoding -->

    <PDF1.3_Properties rdf:about="#MacRomanEncoding"/>
    


    <!-- http://www.semanticweb.org/ontologies/2008/7/XCLOntology1.5.owl#Matrix -->

    <PDF1.3_Properties rdf:about="#Matrix">
        <rdfs:comment xml:lang="en"
            >(Optional) An array of six numbers specifying the pattern matrix (see Section 4.6.1, &#8220;General Properties of Patterns&#8221;). Default value: the identity matrix [ 1 0 0 1 0 0 ]. [cit.]</rdfs:comment>
    </PDF1.3_Properties>
    


    <!-- http://www.semanticweb.org/ontologies/2008/7/XCLOntology1.5.owl#MatrixCalRGB -->

    <PDF1.3_Properties rdf:about="#MatrixCalRGB">
        <rdfs:comment xml:lang="en"
            >(Optional) An array of nine numbers [ X A YA ZA XB YB ZB XC YC ZC ] specifying the linear interpretation of the decoded A, B, and C components of the color space with respect to the final XYZ representation. Default value: the identity matrix [ 1 0 0 0 1 0 0 0 1 ]. [cit.]</rdfs:comment>
    </PDF1.3_Properties>
    


    <!-- http://www.semanticweb.org/ontologies/2008/7/XCLOntology1.5.owl#MaxWidth -->

    <fontDescriptor rdf:about="#MaxWidth">
        <rdfs:comment xml:lang="en"
            >(Optional) The maximum width of glyphs in the font. Default value: 0. [cit.]</rdfs:comment>
    </fontDescriptor>
    


    <!-- http://www.semanticweb.org/ontologies/2008/7/XCLOntology1.5.owl#MediaBox -->

    <PDF1.3_Properties rdf:about="#MediaBox"/>
    


    <!-- http://www.semanticweb.org/ontologies/2008/7/XCLOntology1.5.owl#MeteringMode_Average_NISO -->

    <NISO rdf:about="#MeteringMode_Average_NISO">
        <rdfs:comment
            >This specifies the metering mode (the camera&#39;s method of spatially weighting the scene luminance values to determine the sensor exposure) used when capturing the image.[cit. NISO]
Average is the first value of the enumerations_list.
Every Enumeration-value is designed as individual in this ontology</rdfs:comment>
    </NISO>
    


    <!-- http://www.semanticweb.org/ontologies/2008/7/XCLOntology1.5.owl#MeteringMode_CenterWeightedAverage_NISO -->

    <NISO rdf:about="#MeteringMode_CenterWeightedAverage_NISO"/>
    


    <!-- http://www.semanticweb.org/ontologies/2008/7/XCLOntology1.5.owl#MeteringMode_Multispot_NISO -->

    <NISO rdf:about="#MeteringMode_Multispot_NISO"/>
    


    <!-- http://www.semanticweb.org/ontologies/2008/7/XCLOntology1.5.owl#MeteringMode_Partial_NISO -->

    <NISO rdf:about="#MeteringMode_Partial_NISO"/>
    


    <!-- http://www.semanticweb.org/ontologies/2008/7/XCLOntology1.5.owl#MeteringMode_Pattern_NISO -->

    <NISO rdf:about="#MeteringMode_Pattern_NISO"/>
    


    <!-- http://www.semanticweb.org/ontologies/2008/7/XCLOntology1.5.owl#MeteringMode_Spot_NISO -->

    <NISO rdf:about="#MeteringMode_Spot_NISO"/>
    


    <!-- http://www.semanticweb.org/ontologies/2008/7/XCLOntology1.5.owl#Methodology_NISO -->

    <NISO rdf:about="#Methodology_NISO">
        <rdfs:comment
            >Designates the methodology and rationale to digitize an object or collection. [cit. NISO]</rdfs:comment>
        <Datatype rdf:resource="#string"/>
    </NISO>
    


    <!-- http://www.semanticweb.org/ontologies/2008/7/XCLOntology1.5.owl#MissingWidth -->

    <fontDescriptor rdf:about="#MissingWidth">
        <rdfs:comment xml:lang="en"
            >(Optional) The width to use for character codes whose widths are not speci-
fied in a font dictionary&#8217;s Widths array. This has a predictable effect only if all such codes map to glyphs whose actual widths are the same as the value of the MissingWidth entry. Default value: 0. [cit.]</rdfs:comment>
    </fontDescriptor>
    


    <!-- http://www.semanticweb.org/ontologies/2008/7/XCLOntology1.5.owl#MixingHints -->

    <PDF1.3_Properties rdf:about="#MixingHints">
        <rdfs:comment xml:lang="en"
            >(Optional; PDF 1.6) A dictionary (see Table 4.23) that specifies optional attributes of the inks to be used in blending calculations when used as an alternative to the tint transformation function.[cit.]</rdfs:comment>
    </PDF1.3_Properties>
    


    <!-- http://www.semanticweb.org/ontologies/2008/7/XCLOntology1.5.owl#ModDate -->

    <PDF1.3_Properties rdf:about="#ModDate">
        <rdfs:comment
            >(Optional) The date and time when the embedded &#64257;le was last modi&#64257;ed. [cit. Pdf 1.3]</rdfs:comment>
        <Datatype rdf:resource="#timeISO8601"/>
    </PDF1.3_Properties>
    


    <!-- http://www.semanticweb.org/ontologies/2008/7/XCLOntology1.5.owl#N -->

    <PDF1.3_Properties rdf:about="#N">
        <rdfs:comment xml:lang="en"
            >(Required) The number of color components in the color space described by the ICC profile data. This number must match the number of components actually in the ICC profile. As of PDF 1.4, N must be 1, 3, or 4.</rdfs:comment>
        <Datatype rdf:resource="#int"/>
        <is_same_as rdf:resource="#numberOfInks"/>
    </PDF1.3_Properties>
    


    <!-- http://www.semanticweb.org/ontologies/2008/7/XCLOntology1.5.owl#NULL -->

    <xcl_units rdf:about="#NULL">
        <rdf:type rdf:resource="#xcl_propertyDatatypes"/>
    </xcl_units>
    


    <!-- http://www.semanticweb.org/ontologies/2008/7/XCLOntology1.5.owl#Nonsymbolic -->

    <fontFlag rdf:about="#Nonsymbolic">
        <rdfs:comment xml:lang="en"
            >Bit:6. Font uses Adobe standard Latin1 characterSet [cit.]</rdfs:comment>
    </fontFlag>
    


    <!-- http://www.semanticweb.org/ontologies/2008/7/XCLOntology1.5.owl#OSVersion_NISO -->

    <NISO rdf:about="#OSVersion_NISO">
        <rdfs:comment
            >Version of the operating system in use at the time of image creation.[cit. NiSO]</rdfs:comment>
    </NISO>
    


    <!-- http://www.semanticweb.org/ontologies/2008/7/XCLOntology1.5.owl#OS_NISO -->

    <NISO rdf:about="#OS_NISO">
        <rdfs:comment
            >Operating system in use at the time of image creation.[cit. NISO]</rdfs:comment>
        <Datatype rdf:resource="#string"/>
    </NISO>
    


    <!-- http://www.semanticweb.org/ontologies/2008/7/XCLOntology1.5.owl#OpenAction -->

    <PDF1.3_Properties rdf:about="#OpenAction">
        <rdfs:comment
            >(Optional; PDF 1.1) A value specifying a destination to be displayed or an action to be performed when the document is opened. The value is either an array de&#64257;ning a destination (see Section 7.2.1, &#8220;Destinations&#8221;) or an action dictionary representing an action (Section 7.5, &#8220;Actions&#8221;). 
If this entry is absent, the document should be opened to the top of the  &#64257;rst page at the default magni&#64257;cation factor. [cit. Pdf 1.3]</rdfs:comment>
    </PDF1.3_Properties>
    


    <!-- http://www.semanticweb.org/ontologies/2008/7/XCLOntology1.5.owl#Order -->

    <PDF1.3_Properties rdf:about="#Order">
        <rdfs:comment
            >(Optional) The order of interpolation between samples. Valid values are 1 
and 3, specifying linear and cubic spline interpolation, respectively. (See implementation note 23 in Appendix H.) Default value: 1. [cit. Pdf 1.3]</rdfs:comment>
        <Datatype rdf:resource="#int"/>
    </PDF1.3_Properties>
    


    <!-- http://www.semanticweb.org/ontologies/2008/7/XCLOntology1.5.owl#Orientation_NISO -->

    <NISO rdf:about="#Orientation_NISO">
        <rdfs:comment
            >Designates the orientation of the image, with respect to the placement of its rows (ImageWidth) and columns (ImageLength), as it was saved to disk.
1 = normal*
3 = normal rotated 180&#176;
6 = normal rotated cw 90&#176;
8 = normal rotated ccw 90&#176;
9 = unknown
[cit. NISO]</rdfs:comment>
        <is_same_as rdf:resource="#imageOrientation"/>
        <Datatype rdf:resource="#int"/>
        <is_same_as rdf:resource="#orientation_TIFF"/>
    </NISO>
    


    <!-- http://www.semanticweb.org/ontologies/2008/7/XCLOntology1.5.owl#P -->

    <PDF1.3_Properties rdf:about="#P">
        <rdfs:comment
            >Additional encryption dictionary entriy for the standard security handler.
A set of &#64258;ags specifying which operations are permitted when the document is opened with the user password:
1&#8211;2 Reserved; must be 0 
3 Print document 
4 Modify contents of document (other than text annotations and 
interactive form &#64257;elds) 
5 Copy text and graphics from document 
6 Add or modify text annotations and interactive form &#64257;elds 
7&#8211;32 Reserved; must be 1 
[cit. PDF 1.3]</rdfs:comment>
        <Datatype rdf:resource="#int"/>
    </PDF1.3_Properties>
    


    <!-- http://www.semanticweb.org/ontologies/2008/7/XCLOntology1.5.owl#PAR -->

    <GIF_Properties rdf:about="#PAR">
        <is_same_as rdf:resource="#pixelAspectRatio"/>
    </GIF_Properties>
    


    <!-- http://www.semanticweb.org/ontologies/2008/7/XCLOntology1.5.owl#PASC -->

    <audioInformation rdf:about="#PASC">
        <rdfs:comment xml:lang="en">AudioCodec</rdfs:comment>
    </audioInformation>
    


    <!-- http://www.semanticweb.org/ontologies/2008/7/XCLOntology1.5.owl#PLTE -->

    <PNG_Properties rdf:about="#PLTE">
        <rdfs:comment xml:lang="en"
            >Chunk that containes the Palette for truecolour-PNGs. Use is optional.
If the Image containes also an alpha-channel there should also be a bKGD Chunk.
Required for colour_type3-PNGs</rdfs:comment>
        <is_same_as rdf:resource="#colourMapTiff"/>
        <is_same_as rdf:resource="#rgbPalette"/>
    </PNG_Properties>
    


    <!-- http://www.semanticweb.org/ontologies/2008/7/XCLOntology1.5.owl#PageLayout -->

    <PDF1.3_Properties rdf:about="#PageLayout">
        <rdfs:comment
            >(Optional) A name object specifying the page layout to be used when the 
document is opened: 
SinglePage Display one page at a time. 
OneColumn Display the pages in one column. 
TwoColumnLeft Display the pages in two columns, with odd- 
numbered pages on the left. 
TwoColumnRight Display the pages in two columns, with odd- 
numbered pages on the right. 
[cit. Pdf 1.3]</rdfs:comment>
        <Datatype rdf:resource="#string"/>
    </PDF1.3_Properties>
    


    <!-- http://www.semanticweb.org/ontologies/2008/7/XCLOntology1.5.owl#PageMode -->

    <PDF1.3_Properties rdf:about="#PageMode">
        <rdfs:comment
            >(Optional) A name object specifying how the document should be displayed when opened: 
UseNone Neither document outline nor thumbnail images visible 
UseOutlines Document outline visible 
UseThumbs Thumbnail images visible 
FullScreen Full-screen mode, with no menu bar, window 
controls, or any other window visible 
Default value: UseNone. 
[cit. Pdf 1.3]</rdfs:comment>
        <Datatype rdf:resource="#string"/>
    </PDF1.3_Properties>
    


    <!-- http://www.semanticweb.org/ontologies/2008/7/XCLOntology1.5.owl#PaintType -->

    <PDF1.3_Properties rdf:about="#PaintType">
        <rdfs:comment xml:lang="en"
            >(Required) A code that determines how the color of the pattern cell is to be 
specified: 
1 Colored tiling pattern. The pattern&#8217;s content stream specifies the col- 
ors used to paint the pattern cell. When the content stream begins ex- 
ecution, the current color is the one that was initially in effect in the 
pattern&#8217;s parent content stream. (This is similar to the definition of 
the pattern matrix; see Section 4.6.1, &#8220;General Properties of Pat- 
terns.&#8221;) 
2 Uncolored tiling pattern. The pattern&#8217;s content stream does not specify 
any color information. Instead, the entire pattern cell is painted with 
a separately specified color each time the pattern is used. Essentially, 
the content stream describes a stencil through which the current col- 
or is to be poured. The content stream must not invoke operators that 
specify colors or other color-related parameters in the graphics state; 
otherwise, an error occurs (see Section 4.5.7, &#8220;Color Operators&#8221;). 
The content stream may paint an image mask, however, since it does 
not specify any color information (see &#8220;Stencil Masking&#8221; on page 
350). [cit.]</rdfs:comment>
    </PDF1.3_Properties>
    


    <!-- http://www.semanticweb.org/ontologies/2008/7/XCLOntology1.5.owl#Palette -->

    <rasterInformation rdf:about="#Palette"/>
    


    <!-- http://www.semanticweb.org/ontologies/2008/7/XCLOntology1.5.owl#PanoseEntry -->

    <PDF1.3_Properties rdf:about="#PanoseEntry">
        <rdfs:comment
            >The Panose Entry defines style-attributes and values for a CIDFont.
The value of Panose is a 12-byte string consisting of the following: 
&#8226; The font family class and subclass ID bytes, given in the sFamilyClass &#64257;eld of the &#8220;OS/2&#8221; table in a TrueType font. This &#64257;eld is documented in Microsoft&#8217;s TrueType 1.0 Font Files Technical Speci&#64257;cation. 
&#8226; Ten bytes for the PANOSE classi&#64257;cation number for the font. The PANOSE 
classi&#64257;cation system is documented in the PANOSE Classi&#64257;cation Metrics 
Guide. See the Bibliography for more information about these documents. The following is an example of a Style entry in the font descriptor: 
/Style &lt;&lt;/Panose &lt;01 05 02 02 03 00 00 00 00 00 00 00&gt;&gt;&gt; 
[cit. Pdf 1.3]</rdfs:comment>
        <Datatype rdf:resource="#int"/>
    </PDF1.3_Properties>
    


    <!-- http://www.semanticweb.org/ontologies/2008/7/XCLOntology1.5.owl#Pattern -->

    <PDF1.3_Properties rdf:about="#Pattern">
        <rdfs:comment xml:lang="en"
            >A Pattern color space (PDF 1.2) enables a PDF content stream to paint an area with a pattern rather than a single color. The pattern may be either a tiling pattern (type 1) or a shading pattern (type 2). Section 4.6, &#8220;Patterns,&#8221; discusses patterns in detail. [cit.]</rdfs:comment>
    </PDF1.3_Properties>
    


    <!-- http://www.semanticweb.org/ontologies/2008/7/XCLOntology1.5.owl#PatternType -->

    <PDF1.3_Properties rdf:about="#PatternType">
        <rdfs:comment xml:lang="en"
            >A Pattern color space (PDF 1.2) enables a PDF content stream to paint an area with a &#8220;color&#8221; de&#64257;ned as a pattern, which may be either a tiling pattern 
(PatternType 1) or a shading pattern (PatternType 2). Section 4.6, &#8220;Patterns,&#8221; discusses patterns in detail. [cit. Pdf 1.3]</rdfs:comment>
        <Datatype rdf:resource="#int"/>
    </PDF1.3_Properties>
    


    <!-- http://www.semanticweb.org/ontologies/2008/7/XCLOntology1.5.owl#Perceptual -->

    <PDF1.3_Properties rdf:about="#Perceptual"/>
    


    <!-- http://www.semanticweb.org/ontologies/2008/7/XCLOntology1.5.owl#PerformanceData_NISO -->

    <NISO rdf:about="#PerformanceData_NISO">
        <rdfs:comment
            >Identifies the path of the file that contains the image performance data relative to the target identified in 4.3.2 TargetID...
PerformanceData refers to standards-based characterizations of system performance according to measurements of spatial resolution, OECF, noise, and other attributes important to image quality.

Standards: Electronic imaging standards through the International Imaging Industry Association (I3A) (http://www.i3a.org/it10.html) provide example uses and reporting formats for proposed ISO performance data characterization.  These include, for example, GrayResponseCurve (ISO 14524) and Spatial Resolution Measurement (ISO 16067).
[cit. NISO]</rdfs:comment>
        <Datatype rdf:resource="#string"/>
    </NISO>
    


    <!-- http://www.semanticweb.org/ontologies/2008/7/XCLOntology1.5.owl#PixelBits -->

    <GIF_Properties rdf:about="#PixelBits">
        <rdfs:comment xml:lang="en"
            >BitDepth of the &quot;global colour map&quot; or &quot;local colour map&quot; + 1</rdfs:comment>
    </GIF_Properties>
    


    <!-- http://www.semanticweb.org/ontologies/2008/7/XCLOntology1.5.owl#PixelSize_NISO -->

    <NISO rdf:about="#PixelSize_NISO">
        <rdfs:comment
            >This specifies the pixel size, in meters, of the scanner. [cit. NISO]</rdfs:comment>
        <Datatype rdf:resource="#rational"/>
    </NISO>
    


    <!-- http://www.semanticweb.org/ontologies/2008/7/XCLOntology1.5.owl#PlanarConfiguration_NISO -->

    <NISO rdf:about="#PlanarConfiguration_NISO">
        <rdfs:comment
            >1 = chunky (pixel interleaved) format
2 = planar format [cit.: NISO/Tiff]</rdfs:comment>
        <Datatype rdf:resource="#int"/>
        <is_same_as rdf:resource="#planarConfiguration"/>
        <is_same_as rdf:resource="#planarConfigurationTiff"/>
    </NISO>
    


    <!-- http://www.semanticweb.org/ontologies/2008/7/XCLOntology1.5.owl#Predictor_Pdf -->

    <PDF1.3_Properties rdf:about="#Predictor_Pdf">
        <rdfs:comment
            >A code that selects the predictor algorithm, if any. If the value of this entry 
is 1, the &#64257;lter assumes that the normal algorithm was used to encode the data, without prediction. If the value is greater than 1, the &#64257;lter assumes that the data was differenced before being encoded, and Predictor selects the predictor algorithm. For more information regarding Predictor values greater than 1, see &#8220;LZW and Flate Predictor Functions,&#8221; below. Default value: 1. 
1 No prediction (the default value) 
2 TIFF Predictor 2 
10 PNG prediction (on encoding, PNG None on all rows) 
11 PNG prediction (on encoding, PNG Sub on all rows) 
12 PNG prediction (on encoding, PNG Up on all rows) 
13 PNG prediction (on encoding, PNG Average on all rows) 
14 PNG prediction (on encoding, PNG Paeth on all rows) 
15 PNG prediction (on encoding, PNG optimum) 
[Pdf 1.3]</rdfs:comment>
        <Datatype rdf:resource="#int"/>
    </PDF1.3_Properties>
    


    <!-- http://www.semanticweb.org/ontologies/2008/7/XCLOntology1.5.owl#Predictor_Tiff -->

    <Tiff_Properties rdf:about="#Predictor_Tiff">
        <rdfs:comment
            >A mathematical operator that is applied to the image data before an encoding scheme is applied.
Theoretically, the predictor step is independent from the compression step, and thus can be combined with any compression scheme. It is, however, likely to be most usefull when combined with either LZW or Deflate compression.
The specification defines these values:
1 = No prediction scheme used before coding.
2 = Horizontal differencing.
A third specification supplement from Adobe, that is not yet available on-line, defines this new value:
3 = Floating point horizontal differencing.
LibTiff defines these values:
PREDICTOR_NONE = 1;
PREDICTOR_HORIZONTAL = 2;
PREDICTOR_FLOATINGPOINT = 3; [cit. TIff]</rdfs:comment>
        <Datatype rdf:resource="#int"/>
    </Tiff_Properties>
    


    <!-- http://www.semanticweb.org/ontologies/2008/7/XCLOntology1.5.owl#PreferredPresentation_NISO -->

    <NISO rdf:about="#PreferredPresentation_NISO">
        <rdfs:comment
            >For image data that can be defined to have a &#8220;best representation,&#8221; use this free-text field to recommend the &#8220;target&#8221; device, application, medium, viewing environment (or combination thereof) presumed or proven to be meaningful to image quality.  This will be especially important as viewing devices other than the conventional 3:2 monitor become popular.  Calculation and automated optimal display from one display Aspect Ratio to another will be possible with the information from 2.2.5 DisplayOrientation and the host of measurements supported within this standard.

The Library of Congress&#8217;s presentation_profile specifies &#8220;the program (or equivalent) used to manage the presentation of this primary or intermediate object for users.&#8221; 

Standard: ISO/DIS 3664 Viewing conditions for graphic technology and photography.
[NISO]</rdfs:comment>
        <Datatype rdf:resource="#string"/>
    </NISO>
    


    <!-- http://www.semanticweb.org/ontologies/2008/7/XCLOntology1.5.owl#PrimaryChromaticities_BlueX_NISO -->

    <NISO rdf:about="#PrimaryChromaticities_BlueX_NISO">
        <rdfs:comment
            >This specifies the Blue [x} value for the chromaticities of the primary colors of the imaging process.
These values specify the 1931 CIE xy chromaticities of the capture primaries. The ordering is red [x], red [y], green[x], green[y],blue[x],blue[y].

Note: &#8220;The chromaticities of the primaries of the image are encoded using the redColorantTag, greenColorTag, and blueColorantTag values within the InterColorProfile tag value.&#8221;  (TIFF/EP 4.5 Camera Color Space Information)
[cit. NISO]</rdfs:comment>
        <Datatype rdf:resource="#int"/>
    </NISO>
    


    <!-- http://www.semanticweb.org/ontologies/2008/7/XCLOntology1.5.owl#PrimaryChromaticities_BlueY_NISO -->

    <NISO rdf:about="#PrimaryChromaticities_BlueY_NISO">
        <rdfs:comment
            >This specifies the Blue [y} value for the chromaticities of the primary colors of the imaging process.
These values specify the 1931 CIE xy chromaticities of the capture primaries. The ordering is red [x], red [y], green[x], green[y],blue[x],blue[y].

Note: &#8220;The chromaticities of the primaries of the image are encoded using the redColorantTag, greenColorTag, and blueColorantTag values within the InterColorProfile tag value.&#8221;  (TIFF/EP 4.5 Camera Color Space Information)
[cit. NISO]</rdfs:comment>
        <Datatype rdf:resource="#int"/>
    </NISO>
    


    <!-- http://www.semanticweb.org/ontologies/2008/7/XCLOntology1.5.owl#PrimaryChromaticities_GreenX_NISO -->

    <NISO rdf:about="#PrimaryChromaticities_GreenX_NISO">
        <rdfs:comment
            >This specifies the Green [x} value for the chromaticities of the primary colors of the imaging process.
These values specify the 1931 CIE xy chromaticities of the capture primaries. The ordering is red [x], red [y], green[x], green[y],blue[x],blue[y].

Note: &#8220;The chromaticities of the primaries of the image are encoded using the redColorantTag, greenColorTag, and blueColorantTag values within the InterColorProfile tag value.&#8221;  (TIFF/EP 4.5 Camera Color Space Information)
[cit. NISO]</rdfs:comment>
        <Datatype rdf:resource="#int"/>
    </NISO>
    


    <!-- http://www.semanticweb.org/ontologies/2008/7/XCLOntology1.5.owl#PrimaryChromaticities_GreenY&#8211;NISO -->

    <NISO rdf:about="#PrimaryChromaticities_GreenY&#8211;NISO">
        <rdfs:comment
            >This specifies the Green [y} value for the chromaticities of the primary colors of the imaging process.
These values specify the 1931 CIE xy chromaticities of the capture primaries. The ordering is red [x], red [y], green[x], green[y],blue[x],blue[y].

Note: &#8220;The chromaticities of the primaries of the image are encoded using the redColorantTag, greenColorTag, and blueColorantTag values within the InterColorProfile tag value.&#8221;  (TIFF/EP 4.5 Camera Color Space Information)
[cit. NISO]</rdfs:comment>
        <Datatype rdf:resource="#int"/>
    </NISO>
    


    <!-- http://www.semanticweb.org/ontologies/2008/7/XCLOntology1.5.owl#PrimaryChromaticities_RedX_NISO -->

    <NISO rdf:about="#PrimaryChromaticities_RedX_NISO">
        <rdfs:comment
            >This specifies the Red [x} value for the chromaticities of the primary colors of the imaging process.
These values specify the 1931 CIE xy chromaticities of the capture primaries. The ordering is red [x], red [y], green[x], green[y],blue[x],blue[y].

Note: &#8220;The chromaticities of the primaries of the image are encoded using the redColorantTag, greenColorTag, and blueColorantTag values within the InterColorProfile tag value.&#8221;  (TIFF/EP 4.5 Camera Color Space Information)
[cit. NISO]</rdfs:comment>
        <Datatype rdf:resource="#int"/>
    </NISO>
    


    <!-- http://www.semanticweb.org/ontologies/2008/7/XCLOntology1.5.owl#PrimaryChromaticities_RedY_NISO -->

    <NISO rdf:about="#PrimaryChromaticities_RedY_NISO">
        <rdfs:comment
            >This specifies the Red [y} value for the chromaticities of the primary colors of the imaging process.
These values specify the 1931 CIE xy chromaticities of the capture primaries. The ordering is red [x], red [y], green[x], green[y],blue[x],blue[y].

Note: &#8220;The chromaticities of the primaries of the image are encoded using the redColorantTag, greenColorTag, and blueColorantTag values within the InterColorProfile tag value.&#8221;  (TIFF/EP 4.5 Camera Color Space Information)
[cit. NISO]</rdfs:comment>
        <Datatype rdf:resource="#int"/>
    </NISO>
    


    <!-- http://www.semanticweb.org/ontologies/2008/7/XCLOntology1.5.owl#PrimaryChromaticities_TIFF -->

    <Tiff_Properties rdf:about="#PrimaryChromaticities_TIFF">
        <rdfs:comment
            >The chromaticities of the primaries of the image.

This is the chromaticity for each of the primaries when it has its ReferenceWhite value and the other primaries have their ReferenceBlack values. These values are described using the 1931 CIE xy chromaticity diagram and only the chromaticities are specified. These values can correspond to the chromaticities of the phosphors of a monitor, the filter set and light source combination of a scanner or the imaging model of a rendering package. The ordering is red[x], red[y], green[x], green[y], blue[x], and blue[y].

For example the CCIR Recommendation 709 primaries are:
640/1000,330/1000,
300/1000, 600/1000,
150/1000, 60/1000 [cit. Tiff]</rdfs:comment>
        <Datatype rdf:resource="#uint32Rational"/>
    </Tiff_Properties>
    


    <!-- http://www.semanticweb.org/ontologies/2008/7/XCLOntology1.5.owl#PrintingOrder -->

    <PDF1.3_Properties rdf:about="#PrintingOrder"/>
    


    <!-- http://www.semanticweb.org/ontologies/2008/7/XCLOntology1.5.owl#Process -->

    <PDF1.3_Properties rdf:about="#Process">
        <rdfs:comment xml:lang="en"
            >Required if Subtype is NChannel and the color space includes components of a process color space, otherwise optional; PDF 1.6) A dictionary (see Table 4.22) that describes the process color space whose components are included in this color space. [cit.]</rdfs:comment>
    </PDF1.3_Properties>
    


    <!-- http://www.semanticweb.org/ontologies/2008/7/XCLOntology1.5.owl#ProcessingActions_NISO -->

    <NISO rdf:about="#ProcessingActions_NISO">
        <rdfs:comment
            >An ordinal listing of the image processing steps performed by way of ProcessingSoftware (5.1.4). [cit. NISO]</rdfs:comment>
        <Datatype rdf:resource="#string"/>
    </NISO>
    


    <!-- http://www.semanticweb.org/ontologies/2008/7/XCLOntology1.5.owl#ProcessingAgency_NISO -->

    <NISO rdf:about="#ProcessingAgency_NISO">
        <rdfs:comment
            >Identifies the organization-level producer(s) of the processed image. [cit. NISO]</rdfs:comment>
        <Datatype rdf:resource="#string"/>
    </NISO>
    


    <!-- http://www.semanticweb.org/ontologies/2008/7/XCLOntology1.5.owl#ProcessingSoftwareName_Name -->

    <NISO rdf:about="#ProcessingSoftwareName_Name">
        <rdfs:comment
            >The name of the image processing software used to edit or transform the image data. [cit. NISO]</rdfs:comment>
        <Datatype rdf:resource="#string"/>
    </NISO>
    


    <!-- http://www.semanticweb.org/ontologies/2008/7/XCLOntology1.5.owl#ProcessingSoftwareVersion_NISO -->

    <NISO rdf:about="#ProcessingSoftwareVersion_NISO">
        <rdfs:comment
            >The version number of the image processing software used to edit or transform the image data. [cit. NISO]</rdfs:comment>
        <Datatype rdf:resource="#string"/>
    </NISO>
    


    <!-- http://www.semanticweb.org/ontologies/2008/7/XCLOntology1.5.owl#ProfileName_NISO -->

    <NISO rdf:about="#ProfileName_NISO">
        <rdfs:comment
            >Name of the ICC profile</rdfs:comment>
        <is_same_as rdf:resource="#colourSpaceName"/>
        <Datatype rdf:resource="#string"/>
    </NISO>
    


    <!-- http://www.semanticweb.org/ontologies/2008/7/XCLOntology1.5.owl#ProfileURL_NISO -->

    <NISO rdf:about="#ProfileURL_NISO">
        <rdfs:comment
            >Designates the URL/URN where the ICC profile is located.</rdfs:comment>
        <Datatype rdf:resource="#string"/>
    </NISO>
    


    <!-- http://www.semanticweb.org/ontologies/2008/7/XCLOntology1.5.owl#Profiles_NISO -->

    <NISO rdf:about="#Profiles_NISO">
        <rdfs:comment
            >Identifies the path of the file that contains the ICC color profile or other image management profiles.
The Count for this field = 1.  Each target shall be represented by its own logical metadata block.  See diagram of proposed TargetData structure (4.3). [cit. NISO]</rdfs:comment>
        <Datatype rdf:resource="#string"/>
    </NISO>
    


    <!-- http://www.semanticweb.org/ontologies/2008/7/XCLOntology1.5.owl#RGBA -->

    <PNG_Properties rdf:about="#RGBA">
        <rdfs:comment xml:lang="en"
            >Colourvalue for alphachannel-pictures, containes a 32-Bit-Value.
This means the first 3 8-Bits are between 0-255 and refer to RGB-Colour and the last 8-Bit describe the percentage-value of the Alpha-channel (where 0.0=0% and 1.0=100%)</rdfs:comment>
    </PNG_Properties>
    


    <!-- http://www.semanticweb.org/ontologies/2008/7/XCLOntology1.5.owl#RGB_ICC -->

    <PDF1.3_Properties rdf:about="#RGB_ICC">
        <rdfs:comment
            >Ranges for typical ICC color spaces.
COMPONENT RANGES  [0.01.0] 
[cit. Pdf 1.3]</rdfs:comment>
    </PDF1.3_Properties>
    


    <!-- http://www.semanticweb.org/ontologies/2008/7/XCLOntology1.5.owl#RLE -->

    <rasterInformation rdf:about="#RLE">
        <rdfs:comment
            >CompressionAlgorithm</rdfs:comment>
        <ID>id317</ID>
        <is_same_as rdf:resource="#RunLengthDecode"/>
    </rasterInformation>
    


    <!-- http://www.semanticweb.org/ontologies/2008/7/XCLOntology1.5.owl#RangeLab -->

    <PDF1.3_Properties rdf:about="#RangeLab">
        <rdfs:comment xml:lang="en"
            >(Optional) An array of four numbers [ a min amax bmin bmax ] specifying the range of valid values for the a* and b* (B and C) components of the color space&#8212;that is, and Component values falling outside the specified range are adjusted to the nearest valid value without error indication. Default value: [ &#8722;100 100 &#8722;100 100 ].
a min &#8804; a* &#8804; a max 
and
b min &#8804; b* &#8804; b max 
[cit.]</rdfs:comment>
        <Datatype rdf:resource="#int"/>
    </PDF1.3_Properties>
    


    <!-- http://www.semanticweb.org/ontologies/2008/7/XCLOntology1.5.owl#Range_ICC -->

    <PDF1.3_Properties rdf:about="#Range_ICC">
        <rdfs:comment xml:lang="en"
            >(Optional) An array of 2 &#215; N numbers [ min 0 max0 min1 max1 &#8230; ] specifying the minimum and maximum valid values of the corresponding color components. These values must match the information in the ICC profile. Default value: [ 0.0 1.0 0.0 1.0 &#8230; ]. [cit.]</rdfs:comment>
    </PDF1.3_Properties>
    


    <!-- http://www.semanticweb.org/ontologies/2008/7/XCLOntology1.5.owl#Range_Pdf -->

    <PDF1.3_Properties rdf:about="#Range_Pdf">
        <rdfs:comment
            >(Optional) An array of 2 &#215; N numbers [min 0 max0 min1 max1 &#8230;] specifying the minimum and maximum valid values of the corresponding color components. These values must match the information in the ICC pro&#64257;le. Default value: [0.0  1.0 0.0  1.0 &#8230;]. 
[cit. Pdf 1.3]</rdfs:comment>
        <Datatype rdf:resource="#int"/>
    </PDF1.3_Properties>
    


    <!-- http://www.semanticweb.org/ontologies/2008/7/XCLOntology1.5.owl#ReferenceBlackWhite_NISO -->

    <NISO rdf:about="#ReferenceBlackWhite_NISO">
        <rdfs:comment
            >Encodes a pair of headroom and footroom image data values for each pixel component. This tag is mandatory when PhotometricInterpretation = 6 (YCbCr), and there are no defaults allowed.[cit. NISO standard]</rdfs:comment>
        <Datatype rdf:resource="#rational"/>
    </NISO>
    


    <!-- http://www.semanticweb.org/ontologies/2008/7/XCLOntology1.5.owl#RelativeColorimetric -->

    <PDF1.3_Properties rdf:about="#RelativeColorimetric"/>
    


    <!-- http://www.semanticweb.org/ontologies/2008/7/XCLOntology1.5.owl#RenderingIntent_Pdf -->

    <PDF1.3_Properties rdf:about="#RenderingIntent_Pdf">
        <rdfs:comment
            >can be:
AbsoluteColorimetric.
RelativeColorimetric.
Saturation.
Perceptual.
[cit. Pdf 1.3]</rdfs:comment>
        <is_same_as rdf:resource="#renderingIntent_PNG"/>
    </PDF1.3_Properties>
    


    <!-- http://www.semanticweb.org/ontologies/2008/7/XCLOntology1.5.owl#ResFork -->

    <PDF1.3_Properties rdf:about="#ResFork">
        <rdfs:comment
            >Entries in a Macintosh-speci&#64257;c &#64257;le information dictionary:
(Optional) The binary contents of the embedded &#64257;le&#8217;s resource fork. [cit. Pdf 1.3]</rdfs:comment>
    </PDF1.3_Properties>
    


    <!-- http://www.semanticweb.org/ontologies/2008/7/XCLOntology1.5.owl#Resources -->

    <PDF1.3_Properties rdf:about="#Resources">
        <rdfs:comment xml:lang="en"
            >(Optional but strongly recommended; PDF 1.2) A dictionary specifying any 
resources (such as fonts and images) required by the form XObject (also required by patterns) 
[cit.]</rdfs:comment>
    </PDF1.3_Properties>
    


    <!-- http://www.semanticweb.org/ontologies/2008/7/XCLOntology1.5.owl#RightParenthesis_Pdf -->

    <PDF1.3_Properties rdf:about="#RightParenthesis_Pdf">
        <rdfs:comment>\)</rdfs:comment>
        <Datatype rdf:resource="#string"/>
    </PDF1.3_Properties>
    


    <!-- http://www.semanticweb.org/ontologies/2008/7/XCLOntology1.5.owl#Rotate -->

    <PDF1.3_Properties rdf:about="#Rotate">
        <rdfs:comment
            >(Optional; inheritable) The number of degrees by which the page should be rotated clockwise when displayed or printed. The value must be a multiple of 90. Default value: 0. [cit. Pdf 1.3]</rdfs:comment>
        <Datatype rdf:resource="#int"/>
        <is_same_as rdf:resource="#rotationDisplay"/>
        <is_same_as rdf:resource="#rotationPrint"/>
    </PDF1.3_Properties>
    


    <!-- http://www.semanticweb.org/ontologies/2008/7/XCLOntology1.5.owl#RowsPerStrip_NISO -->

    <NISO rdf:about="#RowsPerStrip_NISO">
        <rdfs:comment
            >&#8220;RowsPerStrip and ImageLength together tell us the number of strips in the entire image.  The equation is:&#8230;&#8221; (TIFF, p39) [cit. NISO standard]</rdfs:comment>
        <Datatype rdf:resource="#int"/>
        <is_same_as rdf:resource="#rowsPerStrip_Tiff"/>
    </NISO>
    


    <!-- http://www.semanticweb.org/ontologies/2008/7/XCLOntology1.5.owl#Run -->

    <wordProcessingML rdf:about="#Run">
        <rdfs:comment
            >Just as a paragraph can have properties, so too can a run. All of the elements inside an r element have their properties controlled by a corresponding optional rPr run properties element (&#167;2.7.8.1; &#167;2.3.2.26), which must be the first child of the r element. In turn, the rPr element is a container for a set of property elements that are applied to the rest of the children of the r element. [Note: The elements inside the rPr container element allow the consumer to control whether the content in the following run content is bold, underlined, or visible, for example. 
Example: Consider the following run within a WordprocessingML document: &lt;w:r&gt; 
  &lt;w:rPr&gt; 
    &lt;w:b/&gt; 
    &lt;w:i/&gt; 
  &lt;/w:rPr&gt; 
  &lt;w:t&gt;quick&lt;/w:t&gt; 
&lt;/w:r&gt;
The run specifies two formatting properties in its run contents: bold and italic. These properties are therefore applied to all content within this run. 
[cit. OOXML spec.]</rdfs:comment>
        <Datatype rdf:resource="#string"/>
    </wordProcessingML>
    


    <!-- http://www.semanticweb.org/ontologies/2008/7/XCLOntology1.5.owl#RunLengthDecode -->

    <PDF1.3_Properties rdf:about="#RunLengthDecode">
        <rdfs:comment
            >Decompresses data encoded using a byte-oriented run-length encod- 
ing algorithm, reproducing the original text or binary data (typically 
monochrome image data, or any data that contains frequent long 
runs of a single byte value). 
[cit. PDF 1.3]</rdfs:comment>
    </PDF1.3_Properties>
    


    <!-- http://www.semanticweb.org/ontologies/2008/7/XCLOntology1.5.owl#SamplesPerPixel_NISO -->

    <rasterInformation rdf:about="#SamplesPerPixel_NISO">
        <rdfs:comment
            >Designates the number of color components per pixel.
1 = when PhotometricInterpretation = 0 or 1 
3 = when PhotometricInterpretation = 2 (RGB), 6 (YcbCr)
4 = when PhotometricInterpretation = 5 (CMYK)
[cit. NISO]</rdfs:comment>
        <Datatype rdf:resource="#int"/>
        <is_same_as rdf:resource="#samplesPerPixel"/>
        <is_same_as rdf:resource="#samplesPerPixelTIff"/>
    </rasterInformation>
    


    <!-- http://www.semanticweb.org/ontologies/2008/7/XCLOntology1.5.owl#SamplingFrequencyPlane_NISO -->

    <NISO rdf:about="#SamplingFrequencyPlane_NISO">
        <rdfs:comment
            >The reference plane location for which XSamplingFrequency and YsamplingFrequency are designated. 
Values:
1 = camera/scanner focal plane  
2 = object plane
3 = source object plane
[cit. NISO]</rdfs:comment>
    </NISO>
    


    <!-- http://www.semanticweb.org/ontologies/2008/7/XCLOntology1.5.owl#SamplingFrequencyUnit_NISO -->

    <NISO rdf:about="#SamplingFrequencyUnit_NISO">
        <rdfs:comment
            >The unit of measurement for XSamplingFrequency and YSamplingFrequency. Values:
1 = no absolute unit of measurement.
2 = inch
3 = centimeter
[cit. NISO]</rdfs:comment>
        <Datatype rdf:resource="#int"/>
    </NISO>
    


    <!-- http://www.semanticweb.org/ontologies/2008/7/XCLOntology1.5.owl#Saturation -->

    <PDF1.3_Properties rdf:about="#Saturation"/>
    


    <!-- http://www.semanticweb.org/ontologies/2008/7/XCLOntology1.5.owl#ScannerManufacturer_NISO -->

    <NISO rdf:about="#ScannerManufacturer_NISO">
        <rdfs:comment
            >The manufacturer of the scanner used to create the image. [cit. NISO]</rdfs:comment>
        <Datatype rdf:resource="#string"/>
    </NISO>
    


    <!-- http://www.semanticweb.org/ontologies/2008/7/XCLOntology1.5.owl#ScannerModelName_NISO -->

    <NISO rdf:about="#ScannerModelName_NISO">
        <rdfs:comment
            >The model name of the scanner used to create the image. [cit. NISO]</rdfs:comment>
        <Datatype rdf:resource="#string"/>
    </NISO>
    


    <!-- http://www.semanticweb.org/ontologies/2008/7/XCLOntology1.5.owl#ScannerModelNumber_NISO -->

    <NISO rdf:about="#ScannerModelNumber_NISO">
        <rdfs:comment
            >The model number of the scanner used to create the image. [cit. NISO]</rdfs:comment>
        <Datatype rdf:resource="#string"/>
    </NISO>
    


    <!-- http://www.semanticweb.org/ontologies/2008/7/XCLOntology1.5.owl#ScannerModelSerialNo_NISO -->

    <NISO rdf:about="#ScannerModelSerialNo_NISO">
        <rdfs:comment
            >The serial number of the scanner used to create the image. [cit. NISO]</rdfs:comment>
        <Datatype rdf:resource="#string"/>
    </NISO>
    


    <!-- http://www.semanticweb.org/ontologies/2008/7/XCLOntology1.5.owl#ScanningSoftwareVersionNo_NISO -->

    <NISO rdf:about="#ScanningSoftwareVersionNo_NISO">
        <rdfs:comment
            >The version number of the capture software used to create the image. [cit. NISO]</rdfs:comment>
        <Datatype rdf:resource="#string"/>
    </NISO>
    


    <!-- http://www.semanticweb.org/ontologies/2008/7/XCLOntology1.5.owl#ScanningSoftware_NISO -->

    <NISO rdf:about="#ScanningSoftware_NISO">
        <rdfs:comment
            >The name of the capture software used to create the image. [cit. NISO]</rdfs:comment>
        <Datatype rdf:resource="#string"/>
    </NISO>
    


    <!-- http://www.semanticweb.org/ontologies/2008/7/XCLOntology1.5.owl#SceneIlluminant_NISO -->

    <NISO rdf:about="#SceneIlluminant_NISO">
        <rdfs:comment
            >This specifies the light source that was present when the image was captured.
Enumerated type (restricted to external standard)
possible values:
Daylight
Fluorescent 
Tungsten Lamp
Flash
Standard Illuminant A
Standard Illuminant B
Standard Illuminant C
D55 Illuminant
D65 Illuminant
D75 Illuminant
[cit. NISO]</rdfs:comment>
    </NISO>
    


    <!-- http://www.semanticweb.org/ontologies/2008/7/XCLOntology1.5.owl#Script -->

    <fontFlag rdf:about="#Script">
        <rdfs:comment xml:lang="en"
            >Bit:4. resemble cursive handwriting [cit.]</rdfs:comment>
    </fontFlag>
    


    <!-- http://www.semanticweb.org/ontologies/2008/7/XCLOntology1.5.owl#SegmentType_NISO -->

    <NISO rdf:about="#SegmentType_NISO">
        <rdfs:comment
            >Specifies whether image data is stored in strips or tiles. 
0 = strips
1 = tiles
[cit. NISO]</rdfs:comment>
        <Datatype rdf:resource="#bool"/>
    </NISO>
    


    <!-- http://www.semanticweb.org/ontologies/2008/7/XCLOntology1.5.owl#Sensor_NISO -->

    <NISO rdf:about="#Sensor_NISO">
        <rdfs:comment
            >Designates the type of image sensor used in the camera or image capture device.
undefined
MonochromeArea
OneChipColorArea
TwoChipColorArea
ThreeChipColorArea
ColorSequentialArea
MonochromeLinear
ColorTriLinear
ColorSequentialLinear
[cit. NISO]</rdfs:comment>
    </NISO>
    


    <!-- http://www.semanticweb.org/ontologies/2008/7/XCLOntology1.5.owl#Separation -->

    <PDF1.3_Properties rdf:about="#Separation">
        <rdfs:comment xml:lang="en"
            >Enables the Object to have more SpotColors.
&quot;A Separation color space (PDF 1.2) provides a means for specifying the use of additional colorants or for isolating the control of individual color components of a device color space for a subtractive device. When such a space is the current color space, the current color is a single-component value, called a tint, that controls the application of the given colorant or color components only.....
In other words, it is a four-element array whose first element is the color space family name Separation. The remaining elements are parameters that a Separation color space requires; their meanings are discussed below. 
A color value in a Separation color space consists of a single tint component in the range 0.0 to 1.0. The value 0.0 represents the minimum amount of colorant that can be applied; 1.0 represents the maximum. Tints are always treated as subtractive colors, even if the device produces output for the designated component by an additive method. Thus, a tint value of 0.0 denotes the lightest color that can be achieved with the given colorant, and 1.0 is the darkest.  &quot; [cit.]</rdfs:comment>
    </PDF1.3_Properties>
    


    <!-- http://www.semanticweb.org/ontologies/2008/7/XCLOntology1.5.owl#Serif -->

    <fontFlag rdf:about="#Serif">
        <rdfs:comment xml:lang="en"
            >Bit:2. Glyphs have serifs...</rdfs:comment>
    </fontFlag>
    


    <!-- http://www.semanticweb.org/ontologies/2008/7/XCLOntology1.5.owl#ShadingCoords -->

    <PDF1.3_Properties rdf:about="#ShadingCoords">
        <rdfs:comment
            >(Required) An array of four numbers [x 0 y0 x1 y1] specifying the starting and ending coordinates of the axis, expressed in the shading&#8217;s target coordinate space. 
[cit. Pdf 1.3]</rdfs:comment>
        <Datatype rdf:resource="#int"/>
    </PDF1.3_Properties>
    


    <!-- http://www.semanticweb.org/ontologies/2008/7/XCLOntology1.5.owl#ShadingDomain -->

    <PDF1.3_Properties rdf:about="#ShadingDomain">
        <rdfs:comment
            >(Optional) An array of four numbers [x min  xmax  ymin  ymax] specifying the rectangular domain of coordinates over which the color function(s) are de&#64257;ned. Default value: [0.0  1.0 0.0  1.0]. [cit. Pdf 1.3]</rdfs:comment>
        <Datatype rdf:resource="#int"/>
    </PDF1.3_Properties>
    


    <!-- http://www.semanticweb.org/ontologies/2008/7/XCLOntology1.5.owl#ShadingFunction -->

    <PDF1.3_Properties rdf:about="#ShadingFunction">
        <rdfs:comment
            >1-in, n-out function or an array of n 1-in, 1-out functions (where n 
is the number of color components in the shading dictionary&#8217;s color space). The function(s) are called with values of the parametric variable t in the domain de&#64257;ned by the shading dictionary&#8217;s Domain entry. Each function&#8217;s domain must be a superset of that of the shading dictionary. If the value returned by the function for a given color component is out of range, it will be adjusted to the nearest valid value. [cit. Pdf 1.3]</rdfs:comment>
        <Datatype rdf:resource="#int"/>
    </PDF1.3_Properties>
    


    <!-- http://www.semanticweb.org/ontologies/2008/7/XCLOntology1.5.owl#ShadingMatrix -->

    <PDF1.3_Properties rdf:about="#ShadingMatrix">
        <rdfs:comment
            >(Optional) A transformation matrix mapping the coordinate space speci&#64257;ed by the Domain entry into the shading&#8217;s target coordinate space. For example, to map the domain rectangle [0.0  1.0 0.0  1.0] to a 1-inch square with lower-left corner at coordinates (100, 100) in default user space, the Matrix value would be [72 0072 100100]. Default value: the identity matrix [100100]. [cit. Pdf 1.3]</rdfs:comment>
        <Datatype rdf:resource="#int"/>
    </PDF1.3_Properties>
    


    <!-- http://www.semanticweb.org/ontologies/2008/7/XCLOntology1.5.owl#ShadingPattern -->

    <PDF1.3_Properties rdf:about="#ShadingPattern">
        <rdfs:comment xml:lang="en"
            >PDF 1.3
...provide a smooth transition between colors across an area to be painted, independent of the resolution of any particular output device and without specifying the number of steps in the color transition. Patterns of this type are described by pattern dictionaries with a pattern type of 2. Table 4.26 shows the contents of this type of dictionary.[cit]</rdfs:comment>
    </PDF1.3_Properties>
    


    <!-- http://www.semanticweb.org/ontologies/2008/7/XCLOntology1.5.owl#Shadingtype -->

    <PDF1.3_Properties rdf:about="#Shadingtype">
        <rdfs:comment
            >dictionary&#8217;s ShadingType entry: 
1 Function-based shading 
2 Axial shading 
3 Radial shading 
4 Free-form Gouraud-shaded triangle mesh 
5 Lattice-form Gouraud-shaded triangle mesh 
6 Coons patch mesh 
7 Tensor-product patch mesh 
 [cit Pdf 1.3]
Note: for every Shading Type exist Coords, a Domain, a Function and a Matrix</rdfs:comment>
        <Datatype rdf:resource="#int"/>
    </PDF1.3_Properties>
    


    <!-- http://www.semanticweb.org/ontologies/2008/7/XCLOntology1.5.owl#Size -->

    <PDF1.3_Properties rdf:about="#Size">
        <rdfs:comment
            >(Optional) The size of the embedded &#64257;le, in bytes. 
[cit. Pdf 1.3]</rdfs:comment>
        <Unit rdf:resource="#byte"/>
        <Datatype rdf:resource="#int"/>
    </PDF1.3_Properties>
    


    <!-- http://www.semanticweb.org/ontologies/2008/7/XCLOntology1.5.owl#SmallCap -->

    <fontFlag rdf:about="#SmallCap">
        <rdfs:comment xml:lang="en">Bit:18</rdfs:comment>
    </fontFlag>
    


    <!-- http://www.semanticweb.org/ontologies/2008/7/XCLOntology1.5.owl#Software -->

    <Tiff_Properties rdf:about="#Software">
        <rdfs:comment
            >Name and version number of the software package(s) used to create the image. [cit. Tiff]</rdfs:comment>
        <is_same_as rdf:resource="#creationSoftware"/>
        <Datatype rdf:resource="#string"/>
    </Tiff_Properties>
    


    <!-- http://www.semanticweb.org/ontologies/2008/7/XCLOntology1.5.owl#Solidities -->

    <PDF1.3_Properties rdf:about="#Solidities"/>
    


    <!-- http://www.semanticweb.org/ontologies/2008/7/XCLOntology1.5.owl#SourceData_NISO -->

    <NISO rdf:about="#SourceData_NISO">
        <rdfs:comment
            >This field specifies either a reference to the source image data (digital file), or a brief description of the file, from which the processed digital image file was created. [cit. NISO]</rdfs:comment>
        <Datatype rdf:resource="#string"/>
    </NISO>
    


    <!-- http://www.semanticweb.org/ontologies/2008/7/XCLOntology1.5.owl#SourceID_NISO -->

    <NISO rdf:about="#SourceID_NISO">
        <Datatype rdf:resource="#string"/>
    </NISO>
    


    <!-- http://www.semanticweb.org/ontologies/2008/7/XCLOntology1.5.owl#SourceType_NISO -->

    <NISO rdf:about="#SourceType_NISO">
        <rdfs:comment
            >This field specifies the medium of the analog source material scanned to create a digital still image.
daguerreotype
reflection print
silver gelatin print
Acme Bronze 100
chromagenic film
35mm color negative Kodak Royal Gold 100 Emul. 3712011
monograph
microfilm</rdfs:comment>
        <Datatype rdf:resource="#string"/>
    </NISO>
    


    <!-- http://www.semanticweb.org/ontologies/2008/7/XCLOntology1.5.owl#SourceXDimension_NISO -->

    <NISO rdf:about="#SourceXDimension_NISO">
        <rdfs:comment
            >a container of information detailing the SourceXDimension (width) of the imaged object; comprised of two data elements (8.1.3.1.1 SourceXDimensionValue and 8.1.3.1.2 sourceXDimensionUnit) 
[cit. NISO]</rdfs:comment>
        <Datatype rdf:resource="#int"/>
    </NISO>
    


    <!-- http://www.semanticweb.org/ontologies/2008/7/XCLOntology1.5.owl#Source_XdimensionUnit_NISO -->

    <NISO rdf:about="#Source_XdimensionUnit_NISO">
        <rdfs:comment
            >Specifies the unit of measure used in Source_Xdimension [cit. NISO]</rdfs:comment>
        <Datatype rdf:resource="#string"/>
    </NISO>
    


    <!-- http://www.semanticweb.org/ontologies/2008/7/XCLOntology1.5.owl#Source_Xdimension_NISO -->

    <NISO rdf:about="#Source_Xdimension_NISO">
        <rdfs:comment
            >Specifies the width of the scanned object. [cit. NISO]</rdfs:comment>
        <Datatype rdf:resource="#rational"/>
    </NISO>
    


    <!-- http://www.semanticweb.org/ontologies/2008/7/XCLOntology1.5.owl#Source_YdimensionUnit_NISO -->

    <NISO rdf:about="#Source_YdimensionUnit_NISO">
        <rdfs:comment
            >Specifies the unit of measure used in Source_Ydimension [cit. NISO]</rdfs:comment>
        <Datatype rdf:resource="#rational"/>
    </NISO>
    


    <!-- http://www.semanticweb.org/ontologies/2008/7/XCLOntology1.5.owl#Source_Ydimension_NISO -->

    <NISO rdf:about="#Source_Ydimension_NISO">
        <rdfs:comment
            >Specifies the height (i.e., vertical dimension) of the scanned object. [cit. NISO]</rdfs:comment>
        <Datatype rdf:resource="#rational"/>
    </NISO>
    


    <!-- http://www.semanticweb.org/ontologies/2008/7/XCLOntology1.5.owl#StandardEncoding -->

    <PDF1.3_Properties rdf:about="#StandardEncoding"/>
    


    <!-- http://www.semanticweb.org/ontologies/2008/7/XCLOntology1.5.owl#StripByteCounts_NISO -->

    <NISO rdf:about="#StripByteCounts_NISO">
        <Datatype rdf:resource="#int"/>
        <is_same_as rdf:resource="#stripByteCount_Tiff"/>
    </NISO>
    


    <!-- http://www.semanticweb.org/ontologies/2008/7/XCLOntology1.5.owl#StripOffsets_NISO -->

    <NISO rdf:about="#StripOffsets_NISO">
        <rdfs:comment
            >&#8220;The StripOffsets field stores the offsets from the start of the image file to the start of each image data strip.&#8221; (TIFF/EP) from NISO standard</rdfs:comment>
        <is_same_as rdf:resource="#StripOffsets_Tiff"/>
        <Datatype rdf:resource="#int"/>
    </NISO>
    


    <!-- http://www.semanticweb.org/ontologies/2008/7/XCLOntology1.5.owl#StripOffsets_Tiff -->

    <Tiff_Properties rdf:about="#StripOffsets_Tiff">
        <rdfs:comment
            >For each strip, the byte offset of that strip.

The offset is specified with respect to the beginning of the TIFF file. Note that this implies that each strip has a location independent of the locations of other strips. This feature may be useful for editing applications. This required field is the only way for a reader to find the image data. (Unless TileOffsets is used; see TileOffsets.)

Note that either SHORT or LONG values may be used to specify the strip offsets. SHORT values may be used for small TIFF files. It should be noted, however, that earlier TIFF specifications required LONG strip offsets and that some software may not accept SHORT values.

For maximum compatibility with operating systems such as MS-DOS and Windows, the StripOffsets array should be less than or equal to 64K bytes in length, and the strips themselves, in both compressed and uncompressed forms, should not be larger than 64K bytes. [cit. Tiff 6]</rdfs:comment>
        <is_same_as rdf:resource="#StripOffsets_NISO"/>
        <Datatype rdf:resource="#int"/>
    </Tiff_Properties>
    


    <!-- http://www.semanticweb.org/ontologies/2008/7/XCLOntology1.5.owl#Style_ID -->

    <wordProcessingML rdf:about="#Style_ID">
        <rdfs:comment xml:lang="en"
            >Unique ID for style of text in ooxml. Simplifies the name given in UIName into an acceptable format (overwrites special characters and white spaces, that are not accepted by all software): &#220;berschrift 1=berschrift1</rdfs:comment>
        <Datatype rdf:resource="#string"/>
    </wordProcessingML>
    


    <!-- http://www.semanticweb.org/ontologies/2008/7/XCLOntology1.5.owl#SubjectDistance_NISO -->

    <NISO rdf:about="#SubjectDistance_NISO">
        <rdfs:comment
            >This specifies the distance, in meters, between the frontal plane of the camera lens and the subject on which the camera was focused. [cit. NISO]</rdfs:comment>
        <Datatype rdf:resource="#rational"/>
    </NISO>
    


    <!-- http://www.semanticweb.org/ontologies/2008/7/XCLOntology1.5.owl#SubtypeDeviceN -->

    <PDF1.3_Properties rdf:about="#SubtypeDeviceN">
        <rdfs:comment xml:lang="en"
            >(Optional; PDF 1.6) A name specifying the preferred treatment for the color 
space. Possible values are DeviceN and NChannel. Default value: DeviceN. [cit.]</rdfs:comment>
    </PDF1.3_Properties>
    


    <!-- http://www.semanticweb.org/ontologies/2008/7/XCLOntology1.5.owl#Symbol -->

    <textInformation rdf:about="#Symbol">
        <ID>id310</ID>
        <is_same_as rdf:resource="#F13"/>
    </textInformation>
    


    <!-- http://www.semanticweb.org/ontologies/2008/7/XCLOntology1.5.owl#Symbolic -->

    <fontFlag rdf:about="#Symbolic">
        <rdfs:comment xml:lang="en"
            >Bit:3.: Font contains glyphs outside the Adobe standard Latin character set. This flag and the Nonsymbolic flag cannot both be set or both be clear (see below). [cit.]</rdfs:comment>
    </fontFlag>
    


    <!-- http://www.semanticweb.org/ontologies/2008/7/XCLOntology1.5.owl#TargetIDManufacturer_NISO -->

    <NISO rdf:about="#TargetIDManufacturer_NISO">
        <rdfs:comment
            >Identifies the manufacturer or organization that created the target.</rdfs:comment>
        <Datatype rdf:resource="#string"/>
    </NISO>
    


    <!-- http://www.semanticweb.org/ontologies/2008/7/XCLOntology1.5.owl#TargetIDMedia_NISO -->

    <NISO rdf:about="#TargetIDMedia_NISO">
        <rdfs:comment
            >Identifies the media of the target. [cit. NISO]</rdfs:comment>
        <Datatype rdf:resource="#string"/>
    </NISO>
    


    <!-- http://www.semanticweb.org/ontologies/2008/7/XCLOntology1.5.owl#TargetIDName_NISO -->

    <NISO rdf:about="#TargetIDName_NISO">
        <rdfs:comment
            >Identifies the name of the target. [cit. NISO]</rdfs:comment>
        <Datatype rdf:resource="#string"/>
    </NISO>
    


    <!-- http://www.semanticweb.org/ontologies/2008/7/XCLOntology1.5.owl#TargetIDNo_NISO -->

    <NISO rdf:about="#TargetIDNo_NISO">
        <rdfs:comment
            >Identifies the version or number of the target. [cit. NISO]</rdfs:comment>
        <Datatype rdf:resource="#string"/>
    </NISO>
    


    <!-- http://www.semanticweb.org/ontologies/2008/7/XCLOntology1.5.owl#TargetPrinter -->

    <Tiff_Properties rdf:about="#TargetPrinter">
        <rdfs:comment
            >A description of the printing environment for which this separation is intended. [cit. Tiff]</rdfs:comment>
        <Datatype rdf:resource="#string"/>
    </Tiff_Properties>
    


    <!-- http://www.semanticweb.org/ontologies/2008/7/XCLOntology1.5.owl#TargetType_NISO -->

    <NISO rdf:about="#TargetType_NISO">
        <rdfs:comment
            >This element identifies the targets as either internal or external.
0 = external
1 = internal
Internal targets are targets which appear within the frame of the digitized item.  External targets do not appear within the frame with the digitized item and are separate files, usually full frame targets used for calibration purposes.

The Count for this field = 1.  Each target shall be represented by its own logical metadata block.  See diagram of proposed TargetData structure (4.3).

When value = 1, the ImageData field shall not be used.  See 4.3.3 ImageData.
[cit. NISO]</rdfs:comment>
        <Datatype rdf:resource="#bool"/>
    </NISO>
    


    <!-- http://www.semanticweb.org/ontologies/2008/7/XCLOntology1.5.owl#TextRenderingMode -->

    <PDF1.3_Properties rdf:about="#TextRenderingMode">
        <rdfs:comment
            >The text rendering mode, T mode, determines whether showing text causes glyph outlines to be stroked, &#64257;lled, used as a clipping path, or some combination of these operations. Stroking, &#64257;lling, and clipping have the same effects for a text object as they do for a path object, although they are speci&#64257;ed in an entirely different way; Default value: 0. 
0 Fill text. 
1 Stroke text. 
2 Fill, then stroke, text. 
3 Neither &#64257;ll nor stroke text (invisible). 
4 Fill text and add to path for clipping (see above). 
5 Stroke text and add to path for clipping. 
6 Fill, then stroke, text and add to path for clipping. 
7 Add text to path for clipping. 

Note:  The text rendering mode has no effect on text displayed in a Type 3 font (see Section 5.5.4, &#8220;Type 3 Fonts&#8221;). 
[cit. Pdf 1.3]</rdfs:comment>
        <Datatype rdf:resource="#int"/>
    </PDF1.3_Properties>
    


    <!-- http://www.semanticweb.org/ontologies/2008/7/XCLOntology1.5.owl#TextRise -->

    <PDF1.3_Properties rdf:about="#TextRise">
        <rdfs:comment
            >Text rise, T rise, speci&#64257;es the distance, in unscaled text space units, to move the baseline up or down from its default location. Positive values of text rise move the baseline up. Adjustments to the baseline are useful for drawing superscripts or subscripts. The default location of the baseline can be restored by setting the text rise to 0. [cit. Pdf 1.3]</rdfs:comment>
        <Datatype rdf:resource="#int"/>
    </PDF1.3_Properties>
    


    <!-- http://www.semanticweb.org/ontologies/2008/7/XCLOntology1.5.owl#TextSpace -->

    <PDF1.3_Properties rdf:about="#TextSpace">
        <rdfs:comment
            >Text space is the coordinate system in which text is shown. It is de&#64257;ned by the text matrix, T m, and the text state parameters Tfs, Th, and Trise, which together determine the transformation from text space to user space. [cit. pdf 1.3]</rdfs:comment>
        <Datatype rdf:resource="#matrix"/>
    </PDF1.3_Properties>
    


    <!-- http://www.semanticweb.org/ontologies/2008/7/XCLOntology1.5.owl#Threshholding_Tiff -->

    <Tiff_Properties rdf:about="#Threshholding_Tiff">
        <rdfs:comment
            >For black and white TIFF files that represent shades of gray, the technique used to convert from gray to black and white pixels.

The specification defines these values:

1 = No dithering or halftoning has been applied to the image data.
2 = An ordered dither or halftone technique has been applied to the image data.
3 = A randomized process such as error diffusion has been applied to the image data.

LibTiff defines these values:

THRESHHOLD_BILEVEL = 1;
THRESHHOLD_HALFTONE = 2;
THRESHHOLD_ERRORDIFFUSE = 3;  [cit. Tiff]</rdfs:comment>
        <Datatype rdf:resource="#int"/>
    </Tiff_Properties>
    


    <!-- http://www.semanticweb.org/ontologies/2008/7/XCLOntology1.5.owl#TileByteCounts_NISO -->

    <NISO rdf:about="#TileByteCounts_NISO">
        <rdfs:comment
            >= TilesPerImage for PlanarConfiguration = 1
= SamplesPerPixel * TilesPerImage for PlanarConfiguration = 2 [Tiff...NISO]</rdfs:comment>
        <Datatype rdf:resource="#int"/>
        <is_same_as rdf:resource="#tileByteCounts_Tiff"/>
    </NISO>
    


    <!-- http://www.semanticweb.org/ontologies/2008/7/XCLOntology1.5.owl#TileLength_NISO -->

    <NISO rdf:about="#TileLength_NISO">
        <Datatype rdf:resource="#int"/>
        <is_same_as rdf:resource="#tileWidth_Tiff"/>
    </NISO>
    


    <!-- http://www.semanticweb.org/ontologies/2008/7/XCLOntology1.5.owl#TileOffsets_NISO -->

    <NISO rdf:about="#TileOffsets_NISO">
        <Datatype rdf:resource="#int"/>
        <is_same_as rdf:resource="#tileOffset_Tiff"/>
    </NISO>
    


    <!-- http://www.semanticweb.org/ontologies/2008/7/XCLOntology1.5.owl#TileWidth_NISO -->

    <NISO rdf:about="#TileWidth_NISO">
        <Datatype rdf:resource="#int"/>
        <is_same_as rdf:resource="#tileWidth_Tiff"/>
    </NISO>
    


    <!-- http://www.semanticweb.org/ontologies/2008/7/XCLOntology1.5.owl#TilingType -->

    <PDF1.3_Properties rdf:about="#TilingType">
        <rdfs:comment xml:lang="en"
            >(Required) A code that controls adjustments to the spacing of tiles relative to the device pixel grid: 
1 Constant spacing. Pattern cells are spaced consistently&#8212;that is, by a 
multiple of a device pixel. To achieve this, the application may need to distort the pattern cell slightly by making small adjustments to XStep, YStep, and the transformation matrix. The amount of distortion does not exceed 1 device pixel. 
2 No distortion. The pattern cell is not distorted, but the spacing between pattern cells may vary by as much as 1 device pixel, both horizontally and vertically, when the pattern is painted. This achieves the spacing requested by XStep and YStep on average but not necessarily for each individual pattern cell. 
3 Constant spacing and faster tiling. Pattern cells are spaced consistently 
as in tiling type 1 but with additional distortion permitted to enable a more efficient implementation. 
[cit.]</rdfs:comment>
        <Datatype rdf:resource="#int"/>
    </PDF1.3_Properties>
    


    <!-- http://www.semanticweb.org/ontologies/2008/7/XCLOntology1.5.owl#TimesBold -->

    <textInformation rdf:about="#TimesBold">
        <ID>id303</ID>
        <is_same_as rdf:resource="#F7"/>
    </textInformation>
    


    <!-- http://www.semanticweb.org/ontologies/2008/7/XCLOntology1.5.owl#TimesBoldItalic -->

    <textInformation rdf:about="#TimesBoldItalic">
        <ID>id305</ID>
        <is_same_as rdf:resource="#F8"/>
    </textInformation>
    


    <!-- http://www.semanticweb.org/ontologies/2008/7/XCLOntology1.5.owl#TimesItalic -->

    <textInformation rdf:about="#TimesItalic">
        <ID>id304</ID>
        <is_same_as rdf:resource="#F6"/>
    </textInformation>
    


    <!-- http://www.semanticweb.org/ontologies/2008/7/XCLOntology1.5.owl#TimesRoman -->

    <textInformation rdf:about="#TimesRoman">
        <ID>id302</ID>
        <is_same_as rdf:resource="#F5"/>
    </textInformation>
    


    <!-- http://www.semanticweb.org/ontologies/2008/7/XCLOntology1.5.owl#Title -->

    <wordProcessingML rdf:about="#Title"/>
    


    <!-- http://www.semanticweb.org/ontologies/2008/7/XCLOntology1.5.owl#TransferFunction -->

    <Tiff_Properties rdf:about="#TransferFunction">
        <rdfs:comment
            >Type		SHORT
Count		(1 or 3) * (1 &lt;&lt; BitsPerSample)
Default		A single table corresponding to the NTSC standard gamma value of 2.2.
Description

Describes a transfer function for the image in tabular style.

Pixel components can be gamma-compensated, companded, non-uniformly quantized, or coded in some other way. The TransferFunction maps the pixel components from a non-linear BitsPerSample (e.g. 8-bit) form into a 16-bit linear form without a perceptible loss of accuracy. [cit. Tiff]</rdfs:comment>
        <Datatype rdf:resource="#int"/>
    </Tiff_Properties>
    


    <!-- http://www.semanticweb.org/ontologies/2008/7/XCLOntology1.5.owl#TrimBox -->

    <PDF1.3_Properties rdf:about="#TrimBox">
        <rdfs:comment
            >(Optional; PDF 1.3) A rectangle, expressed in default user space units, de&#64257;ning the intended dimensions of the &#64257;nished page after trimming (see Section 8.6.1, &#8220;Page Boundaries&#8221;). Default value: the value of CropBox.[cit. Pdf 1.3]</rdfs:comment>
    </PDF1.3_Properties>
    


    <!-- http://www.semanticweb.org/ontologies/2008/7/XCLOntology1.5.owl#TrueType_pdf -->

    <PDF1.3_Properties rdf:about="#TrueType_pdf">
        <rdfs:comment
            >A font based on the TrueType font format (see Section 5.5.2, &#8220;TrueType Fonts&#8221;). [cit. Pdf 1.3]</rdfs:comment>
    </PDF1.3_Properties>
    


    <!-- http://www.semanticweb.org/ontologies/2008/7/XCLOntology1.5.owl#Type0 -->

    <PDF1.3_Properties rdf:about="#Type0">
        <rdfs:comment
            >(PDF 1.2) A composite font&#8212;a font composed of other fonts, organized hierarchically (see Section 5.6, &#8220;Composite Fonts&#8221;) [cit. Pdf 1.3]</rdfs:comment>
    </PDF1.3_Properties>
    


    <!-- http://www.semanticweb.org/ontologies/2008/7/XCLOntology1.5.owl#Type1 -->

    <PDF1.3_Properties rdf:about="#Type1">
        <rdfs:comment
            >A font that de&#64257;nes glyph shapes by using a special encoded format (see Section 5.5.1, &#8220;Type 1 Fonts&#8221;. [cit. Pdf 1.3]</rdfs:comment>
    </PDF1.3_Properties>
    


    <!-- http://www.semanticweb.org/ontologies/2008/7/XCLOntology1.5.owl#Type3 -->

    <PDF1.3_Properties rdf:about="#Type3">
        <rdfs:comment
            >A font that de&#64257;nes glyphs with streams of PDF graphics operators (see Section 5.5.4, &#8220;Type 3 Fonts&#8221;). [cit. Pdf 1.3]</rdfs:comment>
    </PDF1.3_Properties>
    


    <!-- http://www.semanticweb.org/ontologies/2008/7/XCLOntology1.5.owl#UBP -->

    <GIF_Properties rdf:about="#UBP">
        <rdfs:comment xml:lang="en"
            >Number of bits per Pixel in the original picture+1</rdfs:comment>
    </GIF_Properties>
    


    <!-- http://www.semanticweb.org/ontologies/2008/7/XCLOntology1.5.owl#UserSpace -->

    <PDF1.3_Properties rdf:about="#UserSpace">
        <rdfs:comment
            >PDF de&#64257;nes a device-independent coordinate system that always bears the same relationship to the current page, regardless of the output device on which printing or displaying will occur. This device-independent coordinate system is called user space. 
The user space coordinate system is initialized to a default state for each page of a document. Initially, the origin is located at the lower-left corner of the output page or display window, with the positive x axis extending horizontally to the right and the positive y axis extending vertically upward, as in standard mathematical practice. The length of a unit along both the x and y axes is 1&#8260;72 inch. 
This coordinate system is the default user space, in which all points on a page have positive x and y coordinate values.</rdfs:comment>
    </PDF1.3_Properties>
    


    <!-- http://www.semanticweb.org/ontologies/2008/7/XCLOntology1.5.owl#V -->

    <PDF1.3_Properties rdf:about="#V">
        <rdfs:comment
            >A code specifying the algorithm to be used in encrypting and decrypting the document: 
0 An algorithm that is undocumented and no longer supported, and whose use is strongly discouraged. 
1 Algorithm 3.1 on page 73, with an encryption key length of 40 bits; see below. 
2 (PDF 1.4) Algorithm 3.1 on page 73, but allowing encryption key lengths greater than 40 bits. 
3 (PDF 1.4) An unpublished algorithm allowing encryption key lengths ranging from 40 to 128 bits. (This algorithm is unpublished as an export requirement of the U.S. Department of Commerce.)</rdfs:comment>
    </PDF1.3_Properties>
    


    <!-- http://www.semanticweb.org/ontologies/2008/7/XCLOntology1.5.owl#VerticesPerRow -->

    <PDF1.3_Properties rdf:about="#VerticesPerRow">
        <rdfs:comment
            >(Required) The number of vertices in each row of the lattice; the value must be greater than or equal to 2. The number of rows need not be speci&#64257;ed. 
[cit. Pdf 1.3]</rdfs:comment>
        <Datatype rdf:resource="#int"/>
    </PDF1.3_Properties>
    


    <!-- http://www.semanticweb.org/ontologies/2008/7/XCLOntology1.5.owl#ViewerPreferences -->

    <PDF1.3_Properties rdf:about="#ViewerPreferences"/>
    


    <!-- http://www.semanticweb.org/ontologies/2008/7/XCLOntology1.5.owl#WhitePointCalGray -->

    <PDF1.3_Properties rdf:about="#WhitePointCalGray">
        <rdfs:comment xml:lang="en"
            >(Required) An array of three numbers [ X W YW ZW ] specifying the tristimulus value, in the CIE 1931 XYZ space, of the diffuse white point; see 
&#8220;CalRGB Color Spaces,&#8221; below, for further discussion. The numbers XW and 
Z must be positive, and Y must be equal to 1.0. [cit.]</rdfs:comment>
        <Datatype rdf:resource="#int"/>
    </PDF1.3_Properties>
    


    <!-- http://www.semanticweb.org/ontologies/2008/7/XCLOntology1.5.owl#WhitePointCalRGB -->

    <PDF1.3_Properties rdf:about="#WhitePointCalRGB">
        <rdfs:comment xml:lang="en"
            >(Required) An array of three numbers [ X W YW ZW ] specifying the tristimulus value, in the CIE 1931 XYZ space, of the diffuse white point; see below for further discussion. The numbers XW and ZW must be positive, and YW must be equal to 1.0. [cit.]</rdfs:comment>
        <Datatype rdf:resource="#int"/>
    </PDF1.3_Properties>
    


    <!-- http://www.semanticweb.org/ontologies/2008/7/XCLOntology1.5.owl#WhitePointLab -->

    <PDF1.3_Properties rdf:about="#WhitePointLab">
        <rdfs:comment xml:lang="en"
            >(Required) An array of three numbers [ X W YW ZW ] specifying the tristimulus value, in the CIE 1931 XYZ space, of the diffuse white point; see &#8220;CalRGB Color Spaces&#8221; on page 247 for further discussion. The numbers XW and ZW must be positive, and YW must be equal to 1.0. [cit.]</rdfs:comment>
        <Datatype rdf:resource="#int"/>
    </PDF1.3_Properties>
    


    <!-- http://www.semanticweb.org/ontologies/2008/7/XCLOntology1.5.owl#WhitePoint_Tiff -->

    <Tiff_Properties rdf:about="#WhitePoint_Tiff">
        <rdfs:comment
            >The chromaticity of the white point of the image.

This is the chromaticity when each of the primaries has its ReferenceWhite value. The value is described using the 1931 CIE xy chromaticity diagram and only the chromaticity is specified. This value can correspond to the chromaticity of the alignment white of a monitor, the filter set and light source combination of a scanner or the imaging model of a rendering package. The ordering is white[x], white[y].

For example, the CIE Standard Illuminant D65 used by CCIR Recommendation 709 and Kodak PhotoYCC is:
3127/10000,3290/10000 [cit. Tiff]</rdfs:comment>
        <Datatype rdf:resource="#uint32Rational"/>
        <is_same_as rdf:resource="#whitePointX"/>
    </Tiff_Properties>
    


    <!-- http://www.semanticweb.org/ontologies/2008/7/XCLOntology1.5.owl#WhitePoint_Xvalue_NISO -->

    <NISO rdf:about="#WhitePoint_Xvalue_NISO">
        <rdfs:comment
            >The X value for the white point chromaticity of the effective illumination source of the capture process.
These values specify the 1931 CIE xy chromaticities of the effective illumination (i.e., filter/light source combination) at capture. They do not have any relation to location or directional coordinates. For more information about the 1931 CIE standard colorimetric observer, see http://www.color.org/profile.html.

The chromaticity of the white point of the image is encoded using the mediaWhitePointTag values within the InterColorProfile tag value.&#8221;  (TIFF/EP 4.5 Camera Color Space Information)
[CIT. NISO]</rdfs:comment>
        <Datatype rdf:resource="#int"/>
    </NISO>
    


    <!-- http://www.semanticweb.org/ontologies/2008/7/XCLOntology1.5.owl#WhitePoint_Yvalue_NISO -->

    <NISO rdf:about="#WhitePoint_Yvalue_NISO">
        <rdfs:comment
            >The Y value for the white point chromaticity of the effective illumination source of the capture process.
These values specify the 1931 CIE xy chromaticities of the effective illumination (i.e., filter/light source combination) at capture. They do not have any relation to location or directional coordinates. For more information about the 1931 CIE standard colorimetric observer, see http://www.color.org/profile.html.

The chromaticity of the white point of the image is encoded using the mediaWhitePointTag values within the InterColorProfile tag value.&#8221;  (TIFF/EP 4.5 Camera Color Space Information)
[cit. NISO]</rdfs:comment>
        <Datatype rdf:resource="#int"/>
    </NISO>
    


    <!-- http://www.semanticweb.org/ontologies/2008/7/XCLOntology1.5.owl#Width_Gif -->

    <GIF_Properties rdf:about="#Width_Gif">
        <is_same_as rdf:resource="#ImageWidth_NISO"/>
        <is_same_as rdf:resource="#ImageWidth_tiff"/>
        <is_same_as rdf:resource="#imageWidth"/>
        <Datatype rdf:resource="#int"/>
    </GIF_Properties>
    


    <!-- http://www.semanticweb.org/ontologies/2008/7/XCLOntology1.5.owl#Widths -->

    <PDF1.3_Properties rdf:about="#Widths">
        <rdfs:comment
            >(Required except for the 14 standard fonts; indirect reference preferred) An array of (LastChar &#8722; FirstChar + 1) widths, each element being the glyph width for the character whose code is FirstChar plus the array index. For character codes outside the range FirstChar to LastChar, the value of MissingWidth from the FontDescriptor entry for this font is used. 
The glyph widths are measured in units in which 1000 units corresponds to 1 unit in text space. These widths must be consistent with the actual widths given in the font program itself. For more information on glyph widths and other glyph metrics, see Section 5.1.3, &#8220;Glyph Positioning and Metrics.&#8221; 
[cit. pdf 1.3]</rdfs:comment>
    </PDF1.3_Properties>
    


    <!-- http://www.semanticweb.org/ontologies/2008/7/XCLOntology1.5.owl#WidthsArray -->

    <PDF1.3_Properties rdf:about="#WidthsArray">
        <rdfs:comment xml:lang="en"
            >(Required except for the standard 14 fonts; indirect reference preferred) An array of (LastChar &#8722; FirstChar + 1) widths, each element being the glyph width for the character code that equals FirstChar plus the array index. For character codes outside the range FirstChar to LastChar, the value of MissingWidth from the FontDescriptor entry for this font is used. The glyph widths are measured in units in which 1000 units corresponds to 1 unit in text space. These widths must be consistent with the actual widths given in the font program. (See implementation note 61 in Appendix H.) For more information on glyph widths and other glyph metrics, see Section 5.1.3, &#8220;Glyph Positioning and Metrics.&#8221; 
Note: Beginning with PDF 1.5, the special treatment given to the standard 14 fonts is deprecated. All fonts used in a PDF document should be represented using a complete font descriptor. For backwards capability, viewer applications must still provide the special treatment identified for the standard 14 fonts.</rdfs:comment>
    </PDF1.3_Properties>
    


    <!-- http://www.semanticweb.org/ontologies/2008/7/XCLOntology1.5.owl#WinAnsiEncoding -->

    <PDF1.3_Properties rdf:about="#WinAnsiEncoding"/>
    


    <!-- http://www.semanticweb.org/ontologies/2008/7/XCLOntology1.5.owl#XCLLabel -->

    <xcl_propertyDatatypes rdf:about="#XCLLabel"/>
    


    <!-- http://www.semanticweb.org/ontologies/2008/7/XCLOntology1.5.owl#XClipPathUnits -->

    <Tiff_Properties rdf:about="#XClipPathUnits">
        <rdfs:comment
            >The number of units that span the width of the image, in terms of integer ClipPath coordinates.
All horizontal ClipPath coordinates will be divided by this value in order to get a number that is (usually) between 0.0 and 1.0, where 0.0 represents the left side of the image and 1.0 represents the right side of the image.
Note that the choice of value for XClipPathUnits will influence the choice of DataType for the ClipPath commands, since SSHORT or even SBYTE values may be usable if XClipPathUnits is smaller, while SLONG will be required if XClipPathUnits is larger.
Required for every TIFF ClipPath. [cit. Tiff]</rdfs:comment>
    </Tiff_Properties>
    


    <!-- http://www.semanticweb.org/ontologies/2008/7/XCLOntology1.5.owl#XHeight -->

    <fontDescriptor rdf:about="#XHeight">
        <rdfs:comment xml:lang="en"
            >(Optional) The font&#8217;s x height: the vertical coordinate of the top of flat non-
ascending lowercase letters (like the letter x), measured from the baseline, in fonts that have Latin characters. Default value: 0. [cit]</rdfs:comment>
    </fontDescriptor>
    


    <!-- http://www.semanticweb.org/ontologies/2008/7/XCLOntology1.5.owl#XObjectImage -->

    <PDF1.3_Properties rdf:about="#XObjectImage">
        <rdfs:comment
            >An image XObject de&#64257;nes Graphics Objects a rectangular array of color samples to be painted. [cit. Pdf 1.3]</rdfs:comment>
        <is_same_as rdf:resource="#imageData"/>
        <Datatype rdf:resource="#matrix"/>
    </PDF1.3_Properties>
    


    <!-- http://www.semanticweb.org/ontologies/2008/7/XCLOntology1.5.owl#XPosition_Tiff -->

    <Tiff_Properties rdf:about="#XPosition_Tiff">
        <rdfs:comment
            >Y position of the image.

The Y offset in ResolutionUnits of the top of the image, with respect to the top of the page. In the TIFF coordinate scheme, the positive Y direction is down, so that YPosition is always positive.</rdfs:comment>
        <Datatype rdf:resource="#rational"/>
    </Tiff_Properties>
    


    <!-- http://www.semanticweb.org/ontologies/2008/7/XCLOntology1.5.owl#XPrintAspectRatio_NISO -->

    <NISO rdf:about="#XPrintAspectRatio_NISO">
        <rdfs:comment
            >This specifies the print aspect ratio selected by the user when the picture was taken - here: Unit of X ratio. [cit. NISO]</rdfs:comment>
        <Datatype rdf:resource="#rational"/>
    </NISO>
    


    <!-- http://www.semanticweb.org/ontologies/2008/7/XCLOntology1.5.owl#XSamplingFrequency_NISO -->

    <NISO rdf:about="#XSamplingFrequency_NISO">
        <rdfs:comment
            >This field specifies the number of pixels per SamplingFrequencyUnit in the image width. [cit. NISO]</rdfs:comment>
        <Datatype rdf:resource="#int"/>
    </NISO>
    


    <!-- http://www.semanticweb.org/ontologies/2008/7/XCLOntology1.5.owl#XStep -->

    <PDF1.3_Properties rdf:about="#XStep">
        <rdfs:comment xml:lang="en"
            >(Required) The desired horizontal spacing between pattern cells, measured in the pattern coordinate system.[cit.]</rdfs:comment>
        <Datatype rdf:resource="#int"/>
    </PDF1.3_Properties>
    


    <!-- http://www.semanticweb.org/ontologies/2008/7/XCLOntology1.5.owl#XTargetedDisplayAR_NISO -->

    <NISO rdf:about="#XTargetedDisplayAR_NISO">
        <rdfs:comment
            >Unit of X orientation[NISO]</rdfs:comment>
        <Datatype rdf:resource="#int"/>
    </NISO>
    


    <!-- http://www.semanticweb.org/ontologies/2008/7/XCLOntology1.5.owl#XphysScanResolution_NISO -->

    <NISO rdf:about="#XphysScanResolution_NISO">
        <rdfs:comment
            >This specifies the physical scanning resolution of the device, in meters, recording the x (width) direction.[cit. NISO]</rdfs:comment>
        <Datatype rdf:resource="#rational"/>
    </NISO>
    


    <!-- http://www.semanticweb.org/ontologies/2008/7/XCLOntology1.5.owl#YCbCrPositioning_NISO -->

    <NISO rdf:about="#YCbCrPositioning_NISO">
        <rdfs:comment
            >mandatory when PhotometricInterpretation = 6= YCbCr</rdfs:comment>
    </NISO>
    


    <!-- http://www.semanticweb.org/ontologies/2008/7/XCLOntology1.5.owl#YCbCrSubSampling_NISO -->

    <NISO rdf:about="#YCbCrSubSampling_NISO">
        <rdfs:comment
            >Tag Name = YCbCrSubSampling 
Tag = 530 (212.H) 
Type = SHORT 
N = 2 
Value = VALUE (possible values are listed below) 
Short 0:  YCbCrSubsampleHoriz: 
1 ImageWidth of this chroma image is equal to the ImageWidth of the 
associated luma image. 
2 ImageWidth of this chroma image is half the ImageWidth of the 
associated luma image. 
4 ImageWidth of this chroma image is one-quarter the ImageWidth of the 
associated luma image. 
Vertical:
1 ImageLength (height) of this chroma image is equal to the ImageLength 
of the associated luma image. 
2 ImageLength (height) of this chroma image is half the ImageLength of 
the associated luma image. 
4 ImageLength (height) of this chroma image is one-quarter the 
ImageLength of the associated luma image. 
[cit.: N4378 Standard]</rdfs:comment>
        <is_same_as rdf:resource="#YCbCrSubSampling_Tiff"/>
        <Datatype rdf:resource="#int"/>
    </NISO>
    


    <!-- http://www.semanticweb.org/ontologies/2008/7/XCLOntology1.5.owl#YCbCrSubSampling_Tiff -->

    <Tiff_Properties rdf:about="#YCbCrSubSampling_Tiff"/>
    


    <!-- http://www.semanticweb.org/ontologies/2008/7/XCLOntology1.5.owl#YCbCr_NISO -->

    <NISO rdf:about="#YCbCr_NISO">
        <Datatype rdf:resource="#int"/>
    </NISO>
    


    <!-- http://www.semanticweb.org/ontologies/2008/7/XCLOntology1.5.owl#YClipPathUnits -->

    <Tiff_Properties rdf:about="#YClipPathUnits">
        <rdfs:comment
            >The number of units that span the height of the image, in terms of integer ClipPath coordinates.
All vertical ClipPath coordinates will be divided by this value in order to get a number that is (usually) between 0.0 and 1.0, where 0.0 represents the top of the image and 1.0 represents the bottom of the image.
Use this if you want to be able to specify your ClipPath coordinates using integer values that match the aspect ratio of an image.
Unlike the XClipPathUnits field, this field is optional. If it&#39;s not present, the default YClipPathUnits = XClipPathUnits applies. [cit. Tiff]</rdfs:comment>
    </Tiff_Properties>
    


    <!-- http://www.semanticweb.org/ontologies/2008/7/XCLOntology1.5.owl#YPosition_Tiff -->

    <Tiff_Properties rdf:about="#YPosition_Tiff">
        <rdfs:comment
            >X position of the image.
The X offset in ResolutionUnits of the left side of the image, with respect to the left side of the page. [cit. Tiff]</rdfs:comment>
        <Datatype rdf:resource="#rational"/>
    </Tiff_Properties>
    


    <!-- http://www.semanticweb.org/ontologies/2008/7/XCLOntology1.5.owl#YSamplingFrequency_NISO -->

    <NISO rdf:about="#YSamplingFrequency_NISO">
        <rdfs:comment
            >This field specifies the number of pixels per SamplingFrequencyUnit in the image length. [cit. NISO]</rdfs:comment>
        <Datatype rdf:resource="#int"/>
    </NISO>
    


    <!-- http://www.semanticweb.org/ontologies/2008/7/XCLOntology1.5.owl#YStep -->

    <PDF1.3_Properties rdf:about="#YStep">
        <rdfs:comment xml:lang="en"
            >(Required) The desired vertical spacing between pattern cells, measured in 
the pattern coordinate system. Note that XStep and YStep may differ from the dimensions of the pattern cell implied by the BBox entry. This allows tiling with irregularly shaped figures. XStep and YStep may be either positive or negative but not zero. [cit.]</rdfs:comment>
        <Datatype rdf:resource="#int"/>
    </PDF1.3_Properties>
    


    <!-- http://www.semanticweb.org/ontologies/2008/7/XCLOntology1.5.owl#YTargetedDisplayAR_NISO -->

    <NISO rdf:about="#YTargetedDisplayAR_NISO">
        <rdfs:comment
            >Unit of Y orientation[cit. NISO]</rdfs:comment>
        <Datatype rdf:resource="#int"/>
    </NISO>
    


    <!-- http://www.semanticweb.org/ontologies/2008/7/XCLOntology1.5.owl#YcbCrCoefficients_NISO -->

    <NISO rdf:about="#YcbCrCoefficients_NISO">
        <rdfs:comment
            >Encodes the transformation from RGB to YCbCr image data. It is mandatory when PhotometricInterpretation = 6, and there are no defaults allowed. The transformation is specified as three rational values that represent the coefficients used to compute luminance, Y. [cit. NISO standard]</rdfs:comment>
    </NISO>
    


    <!-- http://www.semanticweb.org/ontologies/2008/7/XCLOntology1.5.owl#YphysScanResolution&#8211;NISO -->

    <NISO rdf:about="#YphysScanResolution&#8211;NISO">
        <rdfs:comment
            >This specifies the physical scanning resolution of the device, in meters, recording the Y (height) direction.[cit. NISO]</rdfs:comment>
        <Datatype rdf:resource="#rational"/>
    </NISO>
    


    <!-- http://www.semanticweb.org/ontologies/2008/7/XCLOntology1.5.owl#YprintAspectRatio_NISO -->

    <NISO rdf:about="#YprintAspectRatio_NISO">
        <rdfs:comment
            >Unit of Y ratio [cit. NISO]</rdfs:comment>
        <Datatype rdf:resource="#rational"/>
    </NISO>
    


    <!-- http://www.semanticweb.org/ontologies/2008/7/XCLOntology1.5.owl#ZapfDingbats -->

    <textInformation rdf:about="#ZapfDingbats">
        <ID>id315</ID>
        <is_same_as rdf:resource="#F14"/>
    </textInformation>
    


    <!-- http://www.semanticweb.org/ontologies/2008/7/XCLOntology1.5.owl#adjustRightInd -->

    <wordProcessingML rdf:about="#adjustRightInd">
        <rdfs:comment xml:lang="en"
            >This element specifies whether the right indent shall be automatically adjusted for the given paragraph when a document grid has been defined for the current section using the docGrid element (&#167;2.6.5), modifying of the 
current right indent used on this paragraph.[cit. OOXML spec.]</rdfs:comment>
        <Datatype rdf:resource="#bool"/>
    </wordProcessingML>
    


    <!-- http://www.semanticweb.org/ontologies/2008/7/XCLOntology1.5.owl#alphaTransparency -->

    <rasterInformation rdf:about="#alphaTransparency">
        <ID>id27</ID>
        <rdfs:comment
            >Alpha channel transpareny in value 0-255</rdfs:comment>
        <Datatype rdf:resource="#int"/>
    </rasterInformation>
    


    <!-- http://www.semanticweb.org/ontologies/2008/7/XCLOntology1.5.owl#animation -->

    <otherInformation rdf:about="#animation">
        <Datatype rdf:resource="#XCLLabel"/>
    </otherInformation>
    


    <!-- http://www.semanticweb.org/ontologies/2008/7/XCLOntology1.5.owl#artist -->

    <generalInformation rdf:about="#artist">
        <rdfs:comment xml:lang="en"
            >Person, who created the digital object</rdfs:comment>
        <ID>id31</ID>
        <is_same_as rdf:resource="#documentProducer"/>
        <Datatype rdf:resource="#string"/>
    </generalInformation>
    


    <!-- http://www.semanticweb.org/ontologies/2008/7/XCLOntology1.5.owl#aspectRatioVideo -->

    <videoinformation rdf:about="#aspectRatioVideo">
        <ID>id223</ID>
        <Datatype rdf:resource="#int"/>
    </videoinformation>
    


    <!-- http://www.semanticweb.org/ontologies/2008/7/XCLOntology1.5.owl#audioCodec -->

    <audioInformation rdf:about="#audioCodec">
        <ID>id174</ID>
        <Datatype rdf:resource="#string"/>
    </audioInformation>
    


    <!-- http://www.semanticweb.org/ontologies/2008/7/XCLOntology1.5.owl#audioData -->

    <otherInformation rdf:about="#audioData">
        <ID>id215</ID>
        <Datatype rdf:resource="#string"/>
    </otherInformation>
    


    <!-- http://www.semanticweb.org/ontologies/2008/7/XCLOntology1.5.owl#autoSpaceDE -->

    <wordProcessingML rdf:about="#autoSpaceDE">
        <rdfs:comment xml:lang="en"
            >Automatically Adjust Spacing of Latin and East Asian Text
This element specifies whether inter-character spacing shall automatically be adjusted between regions of Latin text and regions of East Asian text in the current paragraph. These regions shall be determined by the Unicode 
character values of the text content within the paragraph. [cit. OOXML spec.]</rdfs:comment>
        <Datatype rdf:resource="#bool"/>
    </wordProcessingML>
    


    <!-- http://www.semanticweb.org/ontologies/2008/7/XCLOntology1.5.owl#autoSpaceDN -->

    <wordProcessingML rdf:about="#autoSpaceDN">
        <rdfs:comment xml:lang="en"
            >Automatically Adjust Spacing of East Asian Text and Numbers
This element specifies whether inter-character spacing shall automatically be adjusted between regions of numbers and regions of East Asian text in the current paragraph. These regions shall be determined by the 
Unicode character values of the text content within the paragraph. 
[Note: This property is used to ensure that the spacing between regions of numbers and adjoining East Asian text is sufficient on each side such that the numbers can be easily read within the East Asian text. end note] 
If this element is omitted on a given paragraph, its value is determined by the setting previously set at any level of the style hierarchy (i.e. that previous setting remains unchanged). If this setting is never specified in the style hierarchy, its value is assumed to be true. 
[cit. OOXML spec.]</rdfs:comment>
        <Datatype rdf:resource="#bool"/>
    </wordProcessingML>
    


    <!-- http://www.semanticweb.org/ontologies/2008/7/XCLOntology1.5.owl#b -->

    <wordProcessingML rdf:about="#b">
        <rdfs:comment>=bold in OOXML</rdfs:comment>
        <Datatype rdf:resource="#bool"/>
    </wordProcessingML>
    


    <!-- http://www.semanticweb.org/ontologies/2008/7/XCLOntology1.5.owl#bCs -->

    <wordProcessingML rdf:about="#bCs">
        <rdfs:comment
            >Complex Script Bold
This element specifies whether the bold property shall be applied to all complex script characters in the contents of this run when displayed in a document. This formatting property is a toggle property, which specifies that its behavior differs between its use within a style definition and its use as direct formatting. When used as part of a style definition, setting this property shall toggle the current state of that property as specified up to this point in the hierarchy (i.e. applied to not applied, and vice versa). Setting it to false (or an equivalent) shall result in the current setting remaining unchanged. However, when used as direct formatting, setting this property to true or false shall set the absolute state of the resulting property.  
If this element is not present, the default value is to leave the formatting applied at previous level in the style hierarchy. If this element is never applied in the style hierarchy, then bold shall not be applied to complex script characters. 
Example: Consider a run of text which shall have the bCs property (bold) explicitly turned on for the complex  contents of the run. This constraint is specified using the following WordprocessingML: 
&lt;w:rPr&gt; 
  &lt;w:bCs w:val=&quot;true&quot;/&gt; 
&lt;/w:rPr&gt; 
This run explicitly declares that the bCs property is true , so bold is turned on for the complex script contents of this run. 
[cit. OOXML Spec.]</rdfs:comment>
        <Datatype rdf:resource="#bool"/>
    </wordProcessingML>
    


    <!-- http://www.semanticweb.org/ontologies/2008/7/XCLOntology1.5.owl#backgroundColour_PNG -->

    <PNG_Properties rdf:about="#backgroundColour_PNG">
        <rdfs:comment xml:lang="en"
            >solid colour for the background of an image to be used when presenting the image [Compatibility: PNG 1.1]</rdfs:comment>
        <is_same_as rdf:resource="#Background"/>
        <is_same_as rdf:resource="#Backgroundcolour_Gif"/>
        <Datatype rdf:resource="#uint32Rational"/>
    </PNG_Properties>
    


    <!-- http://www.semanticweb.org/ontologies/2008/7/XCLOntology1.5.owl#backgroundcolor -->

    <wordProcessingML rdf:about="#backgroundcolor">
        <rdfs:comment xml:lang="en"
            >value is the hex-value of a colour: &lt;w:background w:color=&quot;9BBB59&quot;</rdfs:comment>
        <Datatype rdf:resource="#hex"/>
    </wordProcessingML>
    


    <!-- http://www.semanticweb.org/ontologies/2008/7/XCLOntology1.5.owl#backround -->

    <wordProcessingML rdf:about="#backround">
        <rdfs:comment xml:lang="en"
            >This element specifies the background information for this document. This background shall be displayed on all pages of the document, behind all other document content. 
The child elements of the background element are in the Vector Markup Language (VML) namespace, which allows any valid VML effect to be applied to the document&#39;s background.  
For solid color fill backgrounds, however, the attributes on this element allow for the specification of use of any valid RGB or theme color value (the latter a reference to the document&#39;s themes part). 
[cit. OOXML spec.]</rdfs:comment>
    </wordProcessingML>
    


    <!-- http://www.semanticweb.org/ontologies/2008/7/XCLOntology1.5.owl#bar -->

    <wordProcessingML rdf:about="#bar">
        <rdfs:comment xml:lang="en"
            >Paragraph Border Between Facing Pages
This element specifies the border which may be displayed on the inside edge of the paragraph when the parent&#39;s section settings specify that the section shall be printed using mirrored margins using the mirrorMargins element (&#167;2.15.1.57). [Note: This information is present in the WordprocessingML for the purposes of legacy document format compatibility, and it may be removed and/or ignored as required. end note] 
If this element is omitted on a given paragraph, its value is determined by the setting previously set at any level of the style hierarchy (i.e. that previous setting remains unchanged). If this setting is never specified in the style hierarchy, then no bar border shall be applied to the current paragraph. [cit. OOXML Spec.]</rdfs:comment>
        <Datatype rdf:resource="#int"/>
    </wordProcessingML>
    


    <!-- http://www.semanticweb.org/ontologies/2008/7/XCLOntology1.5.owl#baseFont_fontAlias -->

    <PDF1.3_Properties rdf:about="#baseFont_fontAlias">
        <Datatype rdf:resource="#string"/>
    </PDF1.3_Properties>
    


    <!-- http://www.semanticweb.org/ontologies/2008/7/XCLOntology1.5.owl#bdr -->

    <wordProcessingML rdf:about="#bdr">
        <rdfs:comment
            >Text Border
This element specifies information about the border applied to the text in the current run. The first piece of information specified by the bdr element is that the current shall have a border when displayed. This information is specified simply by the presence of the bdr element in run&#39;s properties. 
The second piece of information concerns the set of runs which share the current run border. This is determined based on the attributes on the bdr element. If the set of attribute values specifies on two adjacent runs is 
identical, then those two runs shall be considered to be part of the same run border group and rendered within the same set of borders in the document. 
If this element is not present, the default value is to leave the formatting applied at previous level in the style hierarchy. If this element is never applied in the style hierarchy, then no run border shall be applied to the text in this run. 
Example: Consider a document in which the following two runs are located adjacent to one another: 
&lt;w:r&gt; 
  &lt;w:rPr&gt; 
    &lt;w:bdr w:val=&quot;single&quot; w:sz=&quot;36&quot; w:space=&quot;0&quot; w:color=&quot;B8CCE4&quot; 
w:themeColor=&quot;accent1&quot; w:themeTint=&quot;66&quot; /&gt;  
  &lt;/w:rPr&gt; 
  &lt;w:t xml:space=&quot;preserve&quot;&gt;run one&lt;/w:t&gt;  
&lt;/w:r&gt; 
&lt;w:r &gt; 
  &lt;w:rPr&gt; 
    &lt;w:b /&gt;  
    &lt;w:bdr w:val=&quot;single&quot; w:sz=&quot;36&quot; w:space=&quot;0&quot; w:color=&quot;B8CCE4&quot; 
w:themeColor=&quot;accent1&quot; w:themeTint=&quot;66&quot; /&gt;  
  &lt;/w:rPr&gt; 
  &lt;w:t&gt;run two&lt;/w:t&gt;  
&lt;/w:r&gt;
These run, although each is distinct, are combined when rendering the text border because the bdr elements are identical between the two runs.
[cit. OOXML spec.]</rdfs:comment>
        <Datatype rdf:resource="#string"/>
    </wordProcessingML>
    


    <!-- http://www.semanticweb.org/ontologies/2008/7/XCLOntology1.5.owl#between -->

    <wordProcessingML rdf:about="#between">
        <rdfs:comment xml:lang="en"
            >Paragraph Border Between Identical Paragraphs
This element specifies the border which shall be displayed between each paragraph in a set of paragraphs which have the same set of paragraph border settings.  
To determine if any two adjoining paragraphs should have a between border or an individual top and bottom border, the set of borders on the two adjoining paragraphs are compared. If the border information on those two paragraphs is identical for all possible paragraphs borders, then the between border is displayed. 
Otherwise, each paragraph shall use its bottom and top border, respectively. If this border specifies a space attribute, that value is ignored - this border is always located at the bottom of each paragraph with an identical following paragraph, taking into account any space after the line pitch. 
[cit. OOXML spec.]</rdfs:comment>
        <Datatype rdf:resource="#int"/>
    </wordProcessingML>
    


    <!-- http://www.semanticweb.org/ontologies/2008/7/XCLOntology1.5.owl#bezierCurve -->

    <vectorInformation rdf:about="#bezierCurve">
        <rdfs:comment xml:lang="en"
            >Analogue to SVG-Properties we define a curve by its angles and marker-positions. Example:
&lt;path (.....) 
d=&quot;M50,100 Q40,75 90,70Q95,60 95,50Q180,40 170,100Z&quot; /&gt; 
&lt;usexlink:href=&quot;#crvpnt&quot; x=&quot;50&quot; y=&quot;100&quot; /&gt; 
&lt;usexlink:href=&quot;#crvpnt&quot; x=&quot;90&quot; y=&quot;70&quot; /&gt; 
&lt;usexlink:href=&quot;#crvpnt&quot; x=&quot;95&quot; y=&quot;50&quot; /&gt; 
&lt;usexlink:href=&quot;#crvpnt&quot; x=&quot;170&quot; y=&quot;100&quot; /&gt; 
&lt;usexlink:href=&quot;#wheel&quot;  x=&quot;80&quot; y=&quot;100&quot; /&gt; 
&lt;usexlink:href=&quot;#wheel&quot;  x=&quot;145&quot; y=&quot;100&quot; /&gt;</rdfs:comment>
        <ID>id255</ID>
        <Datatype rdf:resource="#characterArray"/>
    </vectorInformation>
    


    <!-- http://www.semanticweb.org/ontologies/2008/7/XCLOntology1.5.owl#bidi -->

    <wordProcessingML rdf:about="#bidi">
        <rdfs:comment xml:lang="en"
            >Right to Left Paragraph Layout
This element specifies that this paragraph shall be presented using a right to left direction. This property only affects the set of paragraph-level properties, and shall not affect the layout of text within the contents of this paragraph.
[Example: Consider a paragraph with the bidi property set as follows: 
&lt;w:p&gt; 
    &lt;w:pPr&gt; 
      &lt;w:bidi/&gt; 
    &lt;/w:pPr&gt; 
    ... 
&lt;/w:p&gt; 
[cit. OOXML spec.]</rdfs:comment>
    </wordProcessingML>
    


    <!-- http://www.semanticweb.org/ontologies/2008/7/XCLOntology1.5.owl#bigEndian -->

    <generalInformation rdf:about="#bigEndian">
        <ID>id224</ID>
        <rdfs:comment xml:lang="en"
            >the kind of Byte-Order</rdfs:comment>
        <Datatype rdf:resource="#XCLLabel"/>
        <is_same_as rdf:resource="#bigEndian_NISO"/>
    </generalInformation>
    


    <!-- http://www.semanticweb.org/ontologies/2008/7/XCLOntology1.5.owl#bigEndian_NISO -->

    <NISO rdf:about="#bigEndian_NISO">
        <Unit rdf:resource="#NULL"/>
        <is_same_as rdf:resource="#bigEndian"/>
    </NISO>
    


    <!-- http://www.semanticweb.org/ontologies/2008/7/XCLOntology1.5.owl#bin -->

    <xcl_propertyDatatypes rdf:about="#bin"/>
    


    <!-- http://www.semanticweb.org/ontologies/2008/7/XCLOntology1.5.owl#bit -->

    <xcl_units rdf:about="#bit"/>
    


    <!-- http://www.semanticweb.org/ontologies/2008/7/XCLOntology1.5.owl#bitmap_1bit -->

    <imageInformation rdf:about="#bitmap_1bit">
        <ID>id230</ID>
        <rdfs:comment xml:lang="en">ColourSpaceName</rdfs:comment>
        <Datatype rdf:resource="#XCLLabel"/>
    </imageInformation>
    


    <!-- http://www.semanticweb.org/ontologies/2008/7/XCLOntology1.5.owl#bitrateVideobps -->

    <videoinformation rdf:about="#bitrateVideobps">
        <ID>id171</ID>
        <Unit rdf:resource="#bit"/>
        <Datatype rdf:resource="#uint32Rational"/>
    </videoinformation>
    


    <!-- http://www.semanticweb.org/ontologies/2008/7/XCLOntology1.5.owl#bitsPerPaletteIndex -->

    <rasterInformation rdf:about="#bitsPerPaletteIndex">
        <ID>id16</ID>
        <rdfs:comment
            >Number of bits per palette index</rdfs:comment>
        <Unit rdf:resource="#bit"/>
        <Datatype rdf:resource="#int"/>
    </rasterInformation>
    


    <!-- http://www.semanticweb.org/ontologies/2008/7/XCLOntology1.5.owl#bitsPerSample -->

    <rasterInformation rdf:about="#bitsPerSample">
        <is_same_as rdf:resource="#BitsPerSample_NISO"/>
        <Unit rdf:resource="#bit"/>
        <is_same_as rdf:resource="#bitsPerSamplePng"/>
        <is_same_as rdf:resource="#bitsPerSampleTiff"/>
        <Datatype rdf:resource="#int"/>
    </rasterInformation>
    


    <!-- http://www.semanticweb.org/ontologies/2008/7/XCLOntology1.5.owl#bitsPerSampleBlue -->

    <rasterInformation rdf:about="#bitsPerSampleBlue">
        <ID>id15</ID>
        <Unit rdf:resource="#bit"/>
        <Datatype rdf:resource="#int"/>
    </rasterInformation>
    


    <!-- http://www.semanticweb.org/ontologies/2008/7/XCLOntology1.5.owl#bitsPerSampleGreen -->

    <rasterInformation rdf:about="#bitsPerSampleGreen">
        <ID>id14</ID>
        <Unit rdf:resource="#bit"/>
        <Datatype rdf:resource="#int"/>
    </rasterInformation>
    


    <!-- http://www.semanticweb.org/ontologies/2008/7/XCLOntology1.5.owl#bitsPerSamplePng -->

    <PNG_Properties rdf:about="#bitsPerSamplePng">
        <rdfs:comment xml:lang="en"
            >Number of bits per sample component</rdfs:comment>
        <Unit rdf:resource="#bit"/>
        <Datatype rdf:resource="#int"/>
    </PNG_Properties>
    


    <!-- http://www.semanticweb.org/ontologies/2008/7/XCLOntology1.5.owl#bitsPerSampleRed -->

    <rasterInformation rdf:about="#bitsPerSampleRed">
        <ID>id12</ID>
        <Unit rdf:resource="#bit"/>
        <Datatype rdf:resource="#int"/>
    </rasterInformation>
    


    <!-- http://www.semanticweb.org/ontologies/2008/7/XCLOntology1.5.owl#bitsPerSampleTiff -->

    <Tiff_Properties rdf:about="#bitsPerSampleTiff">
        <rdfs:comment xml:lang="en"
            >Number of bits per sample component</rdfs:comment>
        <is_same_as rdf:resource="#BitsPerSample_NISO"/>
        <Unit rdf:resource="#bit"/>
        <is_same_as rdf:resource="#bitsPerSample"/>
        <Datatype rdf:resource="#int"/>
    </Tiff_Properties>
    


    <!-- http://www.semanticweb.org/ontologies/2008/7/XCLOntology1.5.owl#bitsPerSampleX_Tiff -->

    <Tiff_Properties rdf:about="#bitsPerSampleX_Tiff">
        <rdfs:comment xml:lang="en"
            >bits per Sample for sample X (=extra sample) [Compatibility: TIFF 6.0]</rdfs:comment>
        <Unit rdf:resource="#bit"/>
        <Datatype rdf:resource="#int"/>
    </Tiff_Properties>
    


    <!-- http://www.semanticweb.org/ontologies/2008/7/XCLOntology1.5.owl#blackGeneration -->

    <PDF1.3_Properties rdf:about="#blackGeneration">
        <rdfs:comment
            >(PDF 1.2) A function that calculates the level of black colorant to use when converting RGB colors to CMYK (see Section 6.2.3, &#8220;Conversion from DeviceRGB to DeviceCMYK&#8221;). Initial value: 
installation-dependent. [cit. Pdf 1.3]</rdfs:comment>
        <Datatype rdf:resource="#string"/>
    </PDF1.3_Properties>
    


    <!-- http://www.semanticweb.org/ontologies/2008/7/XCLOntology1.5.owl#blackWhiteInterpretation -->

    <rasterInformation rdf:about="#blackWhiteInterpretation">
        <ID>id17</ID>
        <Unit rdf:resource="#NULL"/>
        <Datatype rdf:resource="#XCLLabel"/>
    </rasterInformation>
    


    <!-- http://www.semanticweb.org/ontologies/2008/7/XCLOntology1.5.owl#bmpIdentifier -->

    <BMP_Properties rdf:about="#bmpIdentifier">
        <Datatype rdf:resource="#string"/>
    </BMP_Properties>
    


    <!-- http://www.semanticweb.org/ontologies/2008/7/XCLOntology1.5.owl#bodyText -->

    <wordProcessingML rdf:about="#bodyText">
        <Unit rdf:resource="#NULL"/>
        <Datatype rdf:resource="#string"/>
    </wordProcessingML>
    


    <!-- http://www.semanticweb.org/ontologies/2008/7/XCLOntology1.5.owl#bold -->

    <textInformation rdf:about="#bold">
        <ID>id161</ID>
        <rdfs:comment
            >text-property bold</rdfs:comment>
        <is_same_as rdf:resource="#b"/>
        <Datatype rdf:resource="#bool"/>
    </textInformation>
    


    <!-- http://www.semanticweb.org/ontologies/2008/7/XCLOntology1.5.owl#bool -->

    <xcl_propertyDatatypes rdf:about="#bool"/>
    


    <!-- http://www.semanticweb.org/ontologies/2008/7/XCLOntology1.5.owl#bottom -->

    <wordProcessingML rdf:about="#bottom">
        <rdfs:comment xml:lang="en"
            >Paragraph Border Between Identical Paragraphs
This element specifies the  border which shall be displayed below a set of paragraphs which have the same set of paragraph border settings. 
To determine if any two adjoining paragraphs shall have an individual top and bottom border or a between border, the set of borders on the two adjoining paragraphs are compared. If the border information on those wo paragraphs is identical for all possible paragraphs borders, then the between border is displayed. 
Otherwise, the final paragraph shall use its bottom border and the following paragraph shall use its top border, respectively. If this border specifies a space attribute, that value determines the space after the bottom of the  text (ignoring any space below) which should be left before this border is drawn, specified in points. 
If this element is omitted on a given paragraph, its value is determined by the setting previously set at any level of the style hierarchy (i.e. that previous setting remains unchanged). If this setting is never specified in the style hierarchy, then no between border shall be applied below identical paragraphs. [cit. OOXML Spec.]</rdfs:comment>
        <Datatype rdf:resource="#int"/>
    </wordProcessingML>
    


    <!-- http://www.semanticweb.org/ontologies/2008/7/XCLOntology1.5.owl#br -->

    <wordProcessingML rdf:about="#br">
        <rdfs:comment
            >br (Break) 
This element specifies that a break shall be placed at the current location in the run content. A break is a special character which is used to override the normal line breaking that would be performed based on the normal layout of the document&#8217;s contents. *Example: Normal breaking for English would occur only after a breaking space or optional hyphen character. end example]  
The behavior of this break character (the location where text shall be restarted after this break) shall be determined by its type and clear attribute values, described below. 
Example: Consider the following sentence in a WordprocessingML document: 
This is a simple sentence. 
Normally, just as shown above, this sentence would be displayed on a single line as it is not long enough to require line breaking (given the width of the current page). However, if a text wrapping break character (a typical line break) were inserted after the word is, as follows: 
&lt;w:r&gt; 
  &lt;w:t&gt;This is&lt;/w:t&gt; 
  &lt;w:br/&gt; 
  &lt;w:t xml:space=&quot;preserve&quot;&gt; a simple sentence.&lt;/w:t&gt; 
&lt;/w:r&gt; 
This would imply that this break shall be treated as a simple line break, and break the line after that word: 
This is 
 a simple sentence.
[cit. OOXML spec.]</rdfs:comment>
        <Datatype rdf:resource="#bool"/>
        <is_same_as rdf:resource="#lineBreak"/>
    </wordProcessingML>
    


    <!-- http://www.semanticweb.org/ontologies/2008/7/XCLOntology1.5.owl#byte -->

    <xcl_units rdf:about="#byte"/>
    


    <!-- http://www.semanticweb.org/ontologies/2008/7/XCLOntology1.5.owl#byteOffsetRef -->

    <Tiff_Properties rdf:about="#byteOffsetRef">
        <rdfs:comment xml:lang="en"
            >reference to byteoffset?</rdfs:comment>
    </Tiff_Properties>
    


    <!-- http://www.semanticweb.org/ontologies/2008/7/XCLOntology1.5.owl#byteOrder -->

    <generalInformation rdf:about="#byteOrder">
        <ID>id6</ID>
        <rdfs:comment
            >Ordering of bytes for multi-byte data values within a file (intel or motorola)</rdfs:comment>
        <is_same_as rdf:resource="#ByteOrder_NISO"/>
        <Unit rdf:resource="#NULL"/>
        <Datatype rdf:resource="#XCLLabel"/>
    </generalInformation>
    


    <!-- http://www.semanticweb.org/ontologies/2008/7/XCLOntology1.5.owl#caps -->

    <textInformation rdf:about="#caps">
        <ID>id168</ID>
        <rdfs:comment
            >text-property caps</rdfs:comment>
        <Datatype rdf:resource="#bool"/>
    </textInformation>
    


    <!-- http://www.semanticweb.org/ontologies/2008/7/XCLOntology1.5.owl#caps_OOXML -->

    <wordProcessingML rdf:about="#caps_OOXML">
        <rdfs:comment
            >caps (Display All Characters As Capital Letters) 
This element specifies that any lowercase characters in this text run shall be formatted for display only as their capital letter character equivalents. This property does not affect any non-alphabetic character in this run, and does not change the Unicode character for lowercase text, only the method in which it is displayed. 
This formatting property is a toggle property, which specifies that its behavior differs between its use within a style definition and its use as direct formatting. When used as part of a style definition, setting this property shall toggle the current state of that property as specified up to this point in the hierarchy (i.e. applied to not applied, and vice versa). Setting it to false (or an equivalent) shall result in the current setting remaining unchanged. However, when used as direct formatting, setting this property to true or false shall set the absolute state of the resulting property.  
If this element is not present, the default value is to leave the formatting applied at previous level in the style hierarchy. If this element is never applied in the style hierarchy, then the characters are not formatted as capital letters. 
This element shall not be present with the smallCaps (&#167;2.3.2.31) property on the same run, since they are mutually exclusive in terms of appearance. 
Example: Consider the words Hello World, which shall be displayed in all capital letters in a document. This constraint is specified as follows in the WordprocessingML: 
&lt;w:r&gt; 
  &lt;w:rPr&gt; 
    &lt;w:caps w:val=&quot;true&quot; /&gt; 
  &lt;/w:rPr&gt; 
  &lt;w:t&gt;Hello World&lt;/w:t&gt; 
&lt;/w:r&gt; 
This run will display as HELLO WORLD, even though the lowercase characters are used in the run contents due to the use of the caps element. If this property is removed, the original character forms will be displayed (they are not lost).
[cit. OOXML spec.]</rdfs:comment>
        <Unit rdf:resource="#NULL"/>
        <Datatype rdf:resource="#bool"/>
    </wordProcessingML>
    


    <!-- http://www.semanticweb.org/ontologies/2008/7/XCLOntology1.5.owl#cell -->

    <textInformation rdf:about="#cell">
        <rdfs:comment
            >defines a cell in a table</rdfs:comment>
        <ID>id275</ID>
        <Datatype rdf:resource="#int"/>
    </textInformation>
    


    <!-- http://www.semanticweb.org/ontologies/2008/7/XCLOntology1.5.owl#cellHeight -->

    <textInformation rdf:about="#cellHeight">
        <rdfs:comment
            >CellHeight of a tabel-cell in a text-document</rdfs:comment>
        <ID>id273</ID>
        <Datatype rdf:resource="#int"/>
    </textInformation>
    


    <!-- http://www.semanticweb.org/ontologies/2008/7/XCLOntology1.5.owl#cellLengthBilevel -->

    <rasterInformation rdf:about="#cellLengthBilevel">
        <ID>id133</ID>
        <rdfs:comment
            >The height of the dithering or halftoning matrix used to create a dithered or halftoned bilevel file (y-axis)</rdfs:comment>
        <is_same_as rdf:resource="#cellLengthBilevelTiff"/>
        <Datatype rdf:resource="#int"/>
    </rasterInformation>
    


    <!-- http://www.semanticweb.org/ontologies/2008/7/XCLOntology1.5.owl#cellLengthBilevelTiff -->

    <Tiff_Properties rdf:about="#cellLengthBilevelTiff">
        <rdfs:comment
            >The height of the dithering or halftoning matrix used to create a dithered or halftoned bilevel file (y-axis) [Compatibility: TIFF 6.0]</rdfs:comment>
        <is_same_as rdf:resource="#cellLengthBilevel"/>
        <Datatype rdf:resource="#int"/>
    </Tiff_Properties>
    


    <!-- http://www.semanticweb.org/ontologies/2008/7/XCLOntology1.5.owl#cellWidth -->

    <textInformation rdf:about="#cellWidth">
        <ID>id134</ID>
        <ID>id274</ID>
        <Datatype rdf:resource="#int"/>
    </textInformation>
    


    <!-- http://www.semanticweb.org/ontologies/2008/7/XCLOntology1.5.owl#cellWidthBilevelTiff -->

    <Tiff_Properties rdf:about="#cellWidthBilevelTiff">
        <rdfs:comment xml:lang="en"
            >The width of the dithering or halftoning matrix used to create a dithered or halftoned bilevel file (x-axis) [Compatibility: TIFF 6.0]</rdfs:comment>
        <Datatype rdf:resource="#int"/>
    </Tiff_Properties>
    


    <!-- http://www.semanticweb.org/ontologies/2008/7/XCLOntology1.5.owl#centerAdjustment -->

    <textInformation rdf:about="#centerAdjustment">
        <ID>id269</ID>
        <Datatype rdf:resource="#bool"/>
    </textInformation>
    


    <!-- http://www.semanticweb.org/ontologies/2008/7/XCLOntology1.5.owl#char -->

    <xcl_propertyDatatypes rdf:about="#char"/>
    


    <!-- http://www.semanticweb.org/ontologies/2008/7/XCLOntology1.5.owl#charSpace -->

    <PDF1.3_Properties rdf:about="#charSpace">
        <rdfs:comment
            >Set the character spacing, T c, to charSpace, which is a number expressed in unscaled text space units. Character spacing is used by the Tj, TJ, and &#39; operators. Default value: 0. 
[cit. Pdf 1.3]</rdfs:comment>
        <is_same_as rdf:resource="#characterSpacing"/>
        <Datatype rdf:resource="#int"/>
    </PDF1.3_Properties>
    


    <!-- http://www.semanticweb.org/ontologies/2008/7/XCLOntology1.5.owl#characterArray -->

    <xcl_propertyDatatypes rdf:about="#characterArray"/>
    


    <!-- http://www.semanticweb.org/ontologies/2008/7/XCLOntology1.5.owl#characterSpacing -->

    <textInformation rdf:about="#characterSpacing">
        <rdfs:comment
            >distance between characters if different than default values</rdfs:comment>
        <is_same_as rdf:resource="#charSpace"/>
        <Datatype rdf:resource="#int"/>
    </textInformation>
    


    <!-- http://www.semanticweb.org/ontologies/2008/7/XCLOntology1.5.owl#characterStyle -->

    <wordProcessingML rdf:about="#characterStyle"/>
    


    <!-- http://www.semanticweb.org/ontologies/2008/7/XCLOntology1.5.owl#circle -->

    <vectorInformation rdf:about="#circle">
        <rdfs:comment
            >shape of vectorGraph, diameter-value messured in vectorUnit</rdfs:comment>
        <ID>id246</ID>
        <Datatype rdf:resource="#int"/>
    </vectorInformation>
    


    <!-- http://www.semanticweb.org/ontologies/2008/7/XCLOntology1.5.owl#circleGradient -->

    <vectorInformation rdf:about="#circleGradient">
        <rdfs:comment
            >gradient-filling for vector-object from center to outer frame</rdfs:comment>
        <ID>id242</ID>
        <Datatype rdf:resource="#int"/>
    </vectorInformation>
    


    <!-- http://www.semanticweb.org/ontologies/2008/7/XCLOntology1.5.owl#circlePathShapeDiameter -->

    <vectorInformation rdf:about="#circlePathShapeDiameter">
        <rdfs:comment
            >Length of diameter of a circle-shaped vector-object</rdfs:comment>
        <Datatype rdf:resource="#matrix"/>
    </vectorInformation>
    


    <!-- http://www.semanticweb.org/ontologies/2008/7/XCLOntology1.5.owl#clipPath -->

    <rasterInformation rdf:about="#clipPath">
        <rdfs:comment
            >clipping Paths attached to image (possible in Tiff and photoshop-files), defined by markers, angels and b&#233;zier-curves</rdfs:comment>
        <ID>id200</ID>
        <Datatype rdf:resource="#int"/>
    </rasterInformation>
    


    <!-- http://www.semanticweb.org/ontologies/2008/7/XCLOntology1.5.owl#cmyk -->

    <imageInformation rdf:about="#cmyk">
        <rdfs:comment xml:lang="en">ColourSpaceName</rdfs:comment>
        <ID>id213</ID>
        <Datatype rdf:resource="#bool"/>
    </imageInformation>
    


    <!-- http://www.semanticweb.org/ontologies/2008/7/XCLOntology1.5.owl#cmykx -->

    <imageInformation rdf:about="#cmykx">
        <ID>id231</ID>
        <rdfs:comment xml:lang="en"
            >process colour (cyan, magenta, yello, black) with an additional spotcolour</rdfs:comment>
    </imageInformation>
    


    <!-- http://www.semanticweb.org/ontologies/2008/7/XCLOntology1.5.owl#cmykxy -->

    <imageInformation rdf:about="#cmykxy">
        <ID>id232</ID>
        <rdfs:comment xml:lang="en"
            >process colour (cyan, magenta, yello, black) with two additional spotcolours</rdfs:comment>
    </imageInformation>
    


    <!-- http://www.semanticweb.org/ontologies/2008/7/XCLOntology1.5.owl#cnfStyle -->

    <wordProcessingML rdf:about="#cnfStyle">
        <rdfs:comment xml:lang="en"
            >Paragraph Conditional Formatting
This element specifies the set of conditional table style formatting properties which have been applied to this paragraph, if this paragraph is contained within a table cell. [Note: This property is an optimization which may be used by consumers to determine if a given property on a paragraph is the result of the table style properties vs. direct formatting on the paragraph itself. end note] 
If this property is specified on a paragraph which is not contained within a table cell, then its contents shall be ignored when reading the contents of the document. 
Coding of the binary value:
 First Row - Is this the first row of the table?  
 Last Row - Is this the last row of the table?   
 First Column - Does this belong to the first column of the table?   
 Last Column - Does this belong to the last column of the table?   
 Band 1 Vertical - Does this belong to a column which should receive band 1 formatting? This property specifies whether the cell should receive the formatting specified for odd-numbered columns (e.g. 1,3,5,...)   
 Band 2 Vertical - Does this belong to a column which should receive band 2 formatting? This property specifies whether the cell should receive the formatting specified for even-numbered columns (e.g. 2,4,6...)   
 Band 1 Horizontal - Does this receive band 1 formatting? This property specifies whether the cell should receive the formatting specified for odd-numbered rows (e.g. 1,3,5,...)   
 Band 2 Horizontal - Does this receive band 2 formatting? This property specifies whether the cell should receive the formatting specified for even-numbered rows (e.g. 2,4,6...)   
 NE Cell - Is this part of the top-right corner of the table?   
 NW Cell - Is this part of the top-left corner of the table?   
 SE Cell - Is this part of the bottom-right corner of the table?   
 SW Cell -  Is this part of the bottom-left corner of the table?</rdfs:comment>
        <Datatype rdf:resource="#bin"/>
    </wordProcessingML>
    


    <!-- http://www.semanticweb.org/ontologies/2008/7/XCLOntology1.5.owl#color -->

    <PDF1.3_Properties rdf:about="#color">
        <rdfs:comment
            >The current color to use during painting operations. The type and interpretation of this parameter depend on the current color space; for most color spaces, a color value consists of one to four numbers. There are two separate color parameters: one for stroking and one for all other painting operations. Initial value: black. [cit. Pdf 1.3]</rdfs:comment>
    </PDF1.3_Properties>
    


    <!-- http://www.semanticweb.org/ontologies/2008/7/XCLOntology1.5.owl#color_OOXML -->

    <wordProcessingML rdf:about="#color_OOXML">
        <rdfs:comment
            >color (Run Content Color) 
This element specifies the color which shall be used to display the contents of this run in the document. 
This color may be explicitly specified, or set to allow the consumer to automatically choose an appropriate color based on the background color behind the run&#39;s content. 
If this element is not present, the default value is to leave the formatting applied at previous level in the style hierarchy. If this element is never applied in the style hierarchy, then the characters are  set to allow the consumer to automatically choose an appropriate color based on the background color behind the run&#39;s content. 
Example: Consider a run of text which should be displayed using the accent3 theme color from the document&#8217;s 
Theme part. This requirement would be specified as follows in the resulting WordprocessingML: 
&lt;w:rPr&gt; 
  &lt;w:color w:themeColor=&#8221;accent3&#8221; /&gt; 
&lt;/w:rPr&gt; 
[cit. OOXML spec.]</rdfs:comment>
        <Datatype rdf:resource="#string"/>
    </wordProcessingML>
    


    <!-- http://www.semanticweb.org/ontologies/2008/7/XCLOntology1.5.owl#colourMapTiff -->

    <Tiff_Properties rdf:about="#colourMapTiff">
        <rdfs:comment xml:lang="en"
            >A colour map for palette colour images. 
Tag = 320 (140.H) 
Type = SHORT 
N = 3 * (2**BitsPerSample) 
This field defines a Red-Green-Blue colour map (often called a lookup table) for palette-colour images. In a palette-colour image, a pixel value is used to index into an RGB lookup table. For example, a palette-colour pixel having a value of 0 would be displayed according to the 0th Red, Green, Blue triplet.</rdfs:comment>
        <is_same_as rdf:resource="#PLTE"/>
        <Datatype rdf:resource="#int"/>
        <is_same_as rdf:resource="#lookup"/>
        <is_same_as rdf:resource="#rgbPalette"/>
    </Tiff_Properties>
    


    <!-- http://www.semanticweb.org/ontologies/2008/7/XCLOntology1.5.owl#colourResolution -->

    <GIF_Properties rdf:about="#colourResolution">
        <is_same_as rdf:resource="#BitDepth"/>
        <Unit rdf:resource="#bit"/>
        <Datatype rdf:resource="#int"/>
    </GIF_Properties>
    


    <!-- http://www.semanticweb.org/ontologies/2008/7/XCLOntology1.5.owl#colourSpaceName -->

    <imageInformation rdf:about="#colourSpaceName">
        <ID>id198</ID>
        <is_same_as rdf:resource="#ColorSpaceDeviceN"/>
        <is_same_as rdf:resource="#ColorSpace_NISO"/>
        <Datatype rdf:resource="#string"/>
    </imageInformation>
    


    <!-- http://www.semanticweb.org/ontologies/2008/7/XCLOntology1.5.owl#colour_type0 -->

    <PNG_Properties rdf:about="#colour_type0">
        <rdfs:comment xml:lang="en"
            >&quot;In PNG images of colour type 0 (greyscale) each pixel is a single sample, which may have precision less than a byte (1, 2, or 4 bits). These samples are packed into bytes with the leftmost sample in the high-order bits of a byte followed by the other samples for the scanline. &quot;</rdfs:comment>
    </PNG_Properties>
    


    <!-- http://www.semanticweb.org/ontologies/2008/7/XCLOntology1.5.owl#colour_type2 -->

    <PNG_Properties rdf:about="#colour_type2">
        <rdfs:comment xml:lang="en"
            >colour type 2 (truecolour without alpha channel)</rdfs:comment>
    </PNG_Properties>
    


    <!-- http://www.semanticweb.org/ontologies/2008/7/XCLOntology1.5.owl#colour_type3 -->

    <PNG_Properties rdf:about="#colour_type3">
        <rdfs:comment xml:lang="en"
            >&quot;In PNG images of colour type 3 (indexed-colour) each pixel is a single palette index. These indices are packed into bytes in the same way as the samples for colour type 0&quot;</rdfs:comment>
    </PNG_Properties>
    


    <!-- http://www.semanticweb.org/ontologies/2008/7/XCLOntology1.5.owl#colour_type4 -->

    <PNG_Properties rdf:about="#colour_type4">
        <rdfs:comment xml:lang="en"
            >greyscale with alpha-channel</rdfs:comment>
    </PNG_Properties>
    


    <!-- http://www.semanticweb.org/ontologies/2008/7/XCLOntology1.5.owl#colour_type6 -->

    <PNG_Properties rdf:about="#colour_type6">
        <rdfs:comment xml:lang="en"
            >truecolour with alpha channel</rdfs:comment>
    </PNG_Properties>
    


    <!-- http://www.semanticweb.org/ontologies/2008/7/XCLOntology1.5.owl#colour_types -->

    <PNG_Properties rdf:about="#colour_types">
        <rdfs:comment xml:lang="en"
            >Defines the bitdepth of the PNG-File</rdfs:comment>
    </PNG_Properties>
    


    <!-- http://www.semanticweb.org/ontologies/2008/7/XCLOntology1.5.owl#colouredTilling -->

    <PDF1.3_Properties rdf:about="#colouredTilling">
        <rdfs:comment xml:lang="en"
            >PDF-Pattern property</rdfs:comment>
    </PDF1.3_Properties>
    


    <!-- http://www.semanticweb.org/ontologies/2008/7/XCLOntology1.5.owl#columnNumber -->

    <textInformation rdf:about="#columnNumber">
        <rdfs:comment
            >n-th column in a table</rdfs:comment>
        <ID>id276</ID>
        <Datatype rdf:resource="#int"/>
    </textInformation>
    


    <!-- http://www.semanticweb.org/ontologies/2008/7/XCLOntology1.5.owl#comment -->

    <textInformation rdf:about="#comment">
        <rdfs:comment xml:lang="en"
            >anchoring of a comment in a textfile (defined by its position in text and its content)</rdfs:comment>
        <ID>id185</ID>
        <Datatype rdf:resource="#string"/>
    </textInformation>
    


    <!-- http://www.semanticweb.org/ontologies/2008/7/XCLOntology1.5.owl#compressionAlgorithm -->

    <generalInformation rdf:about="#compressionAlgorithm">
        <ID>id18</ID>
        <Unit rdf:resource="#NULL"/>
        <Datatype rdf:resource="#string"/>
    </generalInformation>
    


    <!-- http://www.semanticweb.org/ontologies/2008/7/XCLOntology1.5.owl#compressionFlag -->

    <PNG_Properties rdf:about="#compressionFlag">
        <rdfs:comment xml:lang="en"
            >0=compressedText, 1=uncompressedText. For iTXt, tEXt and zTXt</rdfs:comment>
    </PNG_Properties>
    


    <!-- http://www.semanticweb.org/ontologies/2008/7/XCLOntology1.5.owl#compressionTiff -->

    <Tiff_Properties rdf:about="#compressionTiff">
        <rdfs:comment
            >Compression scheme used on image data 
1 = Uncompressed 
4 = CCITT Group 4</rdfs:comment>
        <Datatype rdf:resource="#int"/>
    </Tiff_Properties>
    


    <!-- http://www.semanticweb.org/ontologies/2008/7/XCLOntology1.5.owl#contentLengthAudio -->

    <audioInformation rdf:about="#contentLengthAudio">
        <ID>id176</ID>
        <Unit rdf:resource="#timeISO8601"/>
        <Datatype rdf:resource="#uint32Rational"/>
    </audioInformation>
    


    <!-- http://www.semanticweb.org/ontologies/2008/7/XCLOntology1.5.owl#contentLengthVideo -->

    <videoinformation rdf:about="#contentLengthVideo">
        <ID>id175</ID>
        <Unit rdf:resource="#timeISO8601"/>
        <Datatype rdf:resource="#uint32Rational"/>
    </videoinformation>
    


    <!-- http://www.semanticweb.org/ontologies/2008/7/XCLOntology1.5.owl#contextualSpacing -->

    <wordProcessingML rdf:about="#contextualSpacing">
        <rdfs:comment xml:lang="en"
            >Ignore Spacing Above and Below When Using Identical Styles
This element specifies that any space specified before or after this paragraph, specified using the spacing element (&#167;2.3.1.33), should not be applied when the preceding and following paragraphs are of the same paragraph style, affecting the top and bottom spacing respectively. [Example: This value is typically used for paragraphs in lists, in which any space between subsequent list items, even if inherited from another style, is not desirable. end example] 
If this element is omitted on a given paragraph, its value is determined by the setting previously set at any level of the style hierarchy (i.e. that previous setting remains unchanged). If this setting is never specified in the style hierarchy, then spacing is not ignored. If it is present, then the spacing above or below on this paragraph is subtracted from the spacing which would have been present if contextual spacing was off, never going below zero. 
Values: on/off:
Specifies a binary value for the property defined by the parent XML element. 
A value of on, 1, or true specifies that the property shall be explicitly applied. This is the default value for this attribute, and is implied when the parent element is present, but this attribute is omitted.  
A value of off, 0, or false specifies that the property shall be explicitly turned off.</rdfs:comment>
        <Datatype rdf:resource="#bool"/>
    </wordProcessingML>
    


    <!-- http://www.semanticweb.org/ontologies/2008/7/XCLOntology1.5.owl#control -->

    <wordProcessingML rdf:about="#control">
        <rdfs:comment
            >control (Floating /Inline Embedded Control) 
Floating: This element specifies that the parent VML object is a representation of an embedded control at the current location in the document. This element shall be used to associate the VML data with the appropriate embedded control settings and properties when the document is displayed. 
If the embedded control is not present, cannot be loaded due to application settings, or is not supported, then the VML data shall be used to provide an image representation of the control at the appropriate location in the document. 
Example: Consider a run which consists of an embedded control. That run would be specified using the following WordprocessingML: 
&lt;w:r&gt; 
  &lt;w:pict&gt; 
    &#8230; 
    &lt;w:control r:id=&#8221;rId99&#8221; w:shapeid=&#8221;shape01&#8221; &#8230; /&gt; 
  &lt;/w:pict&gt; 
&lt;/w:r&gt; 
The control element indicates that the parent VML object contains the positioning and last known image representation of an embedded control, whose settings and properties are stored on this element. 

Inline Embedded Control:
This element specifies that the parent embedded object is a representation of an embedded control at the current location in the document. This element shall be used to associate the appropriate embedded control settings and properties when the document is displayed. 
If the embedded control is not present, cannot be loaded due to application settings, or is not supported, then a suitable placeholder image shall be used to provide a representation of the presence of an embedded control at the appropriate location in the document. 
Example: Consider a run which consists of an embedded control. That run would be specified using the following WordprocessingML: 
&lt;w:r&gt; 
  &lt;w:object&gt; 
    &#8230; 
    &lt;w:control r:id=&#8221;rId99&#8221; w:shapeid=&#8221;shape01&#8221; &#8230; /&gt; 
  &lt;/w:object&gt; 
&lt;/w:r&gt; 
The control element indicates that the parent embedded object is an embedded control, whose settings and properties are stored on this element and the (optional) target of the relationship specified using the id 23 attribute. 
[cit. OOXML spec.]</rdfs:comment>
    </wordProcessingML>
    


    <!-- http://www.semanticweb.org/ontologies/2008/7/XCLOntology1.5.owl#copyrightNote -->

    <generalInformation rdf:about="#copyrightNote">
        <ID>id35</ID>
        <rdfs:comment xml:lang="en"
            >defines the holder of the copyright</rdfs:comment>
        <is_same_as rdf:resource="#copyrightTiff"/>
    </generalInformation>
    


    <!-- http://www.semanticweb.org/ontologies/2008/7/XCLOntology1.5.owl#copyrightTiff -->

    <Tiff_Properties rdf:about="#copyrightTiff">
        <is_same_as rdf:resource="#copyrightNote"/>
    </Tiff_Properties>
    


    <!-- http://www.semanticweb.org/ontologies/2008/7/XCLOntology1.5.owl#cr -->

    <wordProcessingML rdf:about="#cr">
        <rdfs:comment
            >cr (Carriage Return) 
This element specifies that a carriage return shall be placed at the current location in the run content. A carriage return is the equivalent of Unicode character 000D, and is used to end the current line of text in WordprocessingML.  
The behavior of a carriage return in run content shall be identical to a break character with null type and clear attributes, which shall end the current line and find the next available line on which to continue. 
Example: Consider the following sentence in a WordprocessingML document: 
This is another simple sentence.
Normally, just as shown above, this sentence would be displayed on a single line as it is not long enough to 
require line breaking (given the width of the current page). However, if a carriage return were inserted after the word another, as follows: 
&lt;w:r&gt; 
  &lt;w:t&gt;This is another&lt;/w:t&gt; 
  &lt;w:cr/&gt; 
  &lt;w:t xml:space=&quot;preserve&quot;&gt; simple sentence.&lt;/w:t&gt; 
&lt;/w:r&gt; 
This would imply that this carriage return character shall force a line break, and break the line after that word: 
This is another 
 simple sentence. 
The carriage return character forced the following text to be restarted on the next available line in the document.
[cit. OOXML spec.]</rdfs:comment>
        <Datatype rdf:resource="#bool"/>
    </wordProcessingML>
    


    <!-- http://www.semanticweb.org/ontologies/2008/7/XCLOntology1.5.owl#creationSoftware -->

    <generalInformation rdf:about="#creationSoftware">
        <ID xml:lang="">id3</ID>
        <Unit rdf:resource="#NULL"/>
        <is_same_as rdf:resource="#Software"/>
        <Datatype rdf:resource="#string"/>
    </generalInformation>
    


    <!-- http://www.semanticweb.org/ontologies/2008/7/XCLOntology1.5.owl#cs -->

    <wordProcessingML rdf:about="#cs">
        <rdfs:comment
            >Use Complex Script Formatting on Run
This element specifies whether the contents of this run shall be treated as complex script text regardless of their Unicode character values when determining the formatting for this run. 
This means that a consumer shall use the complex script formatting applied to the run [Example: The bCs value (&#167;2.3.2.2), not the b value (&#167;2.3.2.1). end example] when determining the resulting formatting properties. 
If this element is not present, the default value is to leave the formatting applied at previous level in the style hierarchy. If this element is never applied in the style hierarchy, then the run contents are set to complex script based on the Unicode character positions of the content. 
Example: Consider the following run of English text in a WordprocessingML document:
&lt;w:r&gt; 
  &lt;w:rPr&gt; 
    &lt;w:bCs/&gt; 
    &lt;w:i/&gt; 
    &lt;w:cs/&gt; 
  &lt;/w:rPr&gt; 
  &lt;w:t&gt;some English text&lt;/w:t&gt; 
&lt;/w:r&gt; 
[cit. OOXML spec.]</rdfs:comment>
        <Datatype rdf:resource="#bool"/>
    </wordProcessingML>
    


    <!-- http://www.semanticweb.org/ontologies/2008/7/XCLOntology1.5.owl#customPageSize -->

    <textInformation rdf:about="#customPageSize">
        <rdfs:comment xml:lang="en"
            >Size of a Text-Page in unit W x H</rdfs:comment>
        <ID>id264</ID>
        <Datatype rdf:resource="#int"/>
    </textInformation>
    


    <!-- http://www.semanticweb.org/ontologies/2008/7/XCLOntology1.5.owl#dayLong -->

    <wordProcessingML rdf:about="#dayLong">
        <rdfs:comment
            >dayLong (Date Block - Long Day Format) 
This element specifies the presence of a date block at the current location in the run content. A date block is a non-editable region of text which shall display the current date filtered through the specified date picture (see following paragraphs) . [Note: The date block is a legacy construct used for compatibility with older word processors, and should not be produced unless it was consumed while reading a document &#8211; it is recommended that the DATE field is used in its place. end note] 
A date block shall be displayed using the primary editing language of the host application, regardless of the languages specified in the parent run&#8217;s lang property (&#167;2.3.2.18). 
The long day format date block shall use a date picture of DDDD, retrieving the long day format for the primary editing language. 
Example: Consider a WordprocessingML run with the following run content: 
&lt;w:r&gt; 
  &lt;w:t xml:space=&quot;preserve&quot;&gt;This is a long date: &lt;/w:t&gt; 
  &lt;w:dayLong /&gt; 
&lt;/w:r&gt;
This run specifies that a long day format date block shall be placed after the text string literal This is a long 
date: in the document. Assuming that the host application&#8217;s primary editing language is French (Canada) and today&#8217;s date is 04/12/2006 (a Wednesday), this run would be displayed as follows: 
This is a long date: mercredi 4 
[cit. OOXML spec.]</rdfs:comment>
    </wordProcessingML>
    


    <!-- http://www.semanticweb.org/ontologies/2008/7/XCLOntology1.5.owl#dayShort -->

    <wordProcessingML rdf:about="#dayShort">
        <rdfs:comment
            >dayShort (Date Block - Short Day Format) 
This element specifies the presence of a date block at the current location in the run content. A date block is a non-editable region of text which shall display the current date filtered through the specified date picture (see following paragraphs) . [Note: The date block is a legacy construct used for compatibility with older word processors, and should not be produced unless it was consumed while reading a document &#8211; it is recommended that the DATE field is used in its place. end note] 
A date block shall be displayed using the primary editing language of the host application, regardless of the languages specified in the parent run&#8217;s lang property (&#167;2.3.2.18). 
The short day format date block shall use a date picture of DD, retrieving the short day format for the primary editing language. 
Example: Consider a WordprocessingML run with the following run content: 
&lt;w:r&gt; 
  &lt;w:t xml:space=&quot;preserve&quot;&gt;This is a short date: &lt;/w:t&gt; 
  &lt;w:dayShort /&gt; 
&lt;/w:r&gt; 
This run specifies that a short day format date block shall be placed after the text string literal This is a short date: in the document. Assuming that the host application&#8217;s primary editing language is English (Canada) and today&#8217;s date is 04/12/2006 (a Wednesday), this run would be displayed as follows: 
This is a short date: 1226 
[cit. OOXML spec.]</rdfs:comment>
        <Datatype rdf:resource="#int"/>
    </wordProcessingML>
    


    <!-- http://www.semanticweb.org/ontologies/2008/7/XCLOntology1.5.owl#defaultColorSpace -->

    <PDF1.3_Properties rdf:about="#defaultColorSpace">
        <rdfs:comment xml:lang="en"
            >PDF 1.1 can be mapped to device-independent ICC ColorSpaces</rdfs:comment>
    </PDF1.3_Properties>
    


    <!-- http://www.semanticweb.org/ontologies/2008/7/XCLOntology1.5.owl#defaultFont -->

    <textInformation rdf:about="#defaultFont">
        <ID>id268</ID>
        <Datatype rdf:resource="#string"/>
    </textInformation>
    


    <!-- http://www.semanticweb.org/ontologies/2008/7/XCLOntology1.5.owl#deflate_Zlib -->

    <textInformation rdf:about="#deflate_Zlib">
        <rdfs:comment xml:lang="en"
            >compression algorithm for textfiles</rdfs:comment>
        <ID>id228</ID>
        <is_same_as rdf:resource="#zTXt"/>
    </textInformation>
    


    <!-- http://www.semanticweb.org/ontologies/2008/7/XCLOntology1.5.owl#delText -->

    <wordProcessingML rdf:about="#delText">
        <rdfs:comment
            >delText (Deleted Text) 
This element specifies that this run contains literal text which shall be displayed in the document. The delText element shall be used for all text runs which are part of a region of text that is contained in a deleted region using the del element (&#167;2.13.5.12). 
Example: Consider a paragraph of WordprocessingML content which reads This is deleted text, where the words deleted text are part of a deleted region of the document. This paragraph would therefore be represented as follows: 
&lt;w:p&gt; 
  &lt;w:r&gt; 
    &lt;w:t xml:space=&quot;preserve&quot;&gt;This is &lt;/w:t&gt; 
  &lt;/w:r&gt; 
  &lt;w:del&gt; 
    &lt;w:r&gt; 
      &lt;w:delText&gt;deleted text&lt;/w:delText&gt; 
    &lt;/w:r&gt; 
  &lt;/w:del&gt; 
&lt;/w:p&gt; 
The deleted text is contained in a delText node, while the regular text is contained in a t node. 
[cit. OOXML spec.]</rdfs:comment>
        <Datatype rdf:resource="#bool"/>
    </wordProcessingML>
    


    <!-- http://www.semanticweb.org/ontologies/2008/7/XCLOntology1.5.owl#dinA4 -->

    <textInformation rdf:about="#dinA4">
        <ID>id265</ID>
        <rdfs:comment xml:lang="en"
            >PageSize in 210 x 297 cm in a TextFile</rdfs:comment>
        <Datatype rdf:resource="#ISO216"/>
    </textInformation>
    


    <!-- http://www.semanticweb.org/ontologies/2008/7/XCLOntology1.5.owl#dinA5 -->

    <textInformation rdf:about="#dinA5">
        <rdfs:comment xml:lang="en"
            >PageSize in 148 x 210 cm in a TextFile</rdfs:comment>
        <ID>id266</ID>
        <Datatype rdf:resource="#ISO216"/>
    </textInformation>
    


    <!-- http://www.semanticweb.org/ontologies/2008/7/XCLOntology1.5.owl#dinA6 -->

    <textInformation rdf:about="#dinA6">
        <ID>id267</ID>
        <rdfs:comment xml:lang="en"
            >PageSize in 105 x 148 cm in a TextFile</rdfs:comment>
        <Datatype rdf:resource="#ISO216"/>
    </textInformation>
    


    <!-- http://www.semanticweb.org/ontologies/2008/7/XCLOntology1.5.owl#dirty -->

    <wordProcessingML rdf:about="#dirty">
        <rdfs:comment
            >dirty (Invalidated Field Cache) 
This element specifies that the field has been changed and the results shall be updated on open in a conforming consumer. 
[cit. OOXML spec.]</rdfs:comment>
        <Datatype rdf:resource="#bool"/>
    </wordProcessingML>
    


    <!-- http://www.semanticweb.org/ontologies/2008/7/XCLOntology1.5.owl#divId -->

    <wordProcessingML rdf:about="#divId">
        <rdfs:comment
            >Associated HTML div ID
This element specifies that this paragraph should be located within the specified HTML div tag when this document is saved in HTML format. This ID is then used to look up the associated div stored in the divs (&#167;2.15.2.8) element. [Note: This element is used to preserve the fidelity of existing HTML documents when saved in the WordprocessingML format. end note]. 
If the paragraph does not specify this element, then any div referenced by the previous paragraph is closed, and this paragraph shall not belong to any div when saved as HTML. If this specified id does not exist in the collection of divs the current document, then any div referenced by the previous paragraph is closed, and this paragraph shall not belong to any div when saved as HTML. 
[Example: Consider the following WordprocessingML paragraph fragment: 
&lt;w:p&gt; 
  &lt;w:pPr&gt; 
    &lt;w:divId w:val=&quot;1512645511&quot; /&gt;  
  &lt;/w:pPr&gt; 
&lt;/w:p&gt;</rdfs:comment>
        <Datatype rdf:resource="#int"/>
    </wordProcessingML>
    


    <!-- http://www.semanticweb.org/ontologies/2008/7/XCLOntology1.5.owl#documentCreationDate -->

    <generalInformation rdf:about="#documentCreationDate">
        <ID>id36</ID>
        <is_same_as rdf:resource="#CreationDate"/>
        <is_same_as rdf:resource="#DateTimeCreated_NISO"/>
        <Datatype rdf:resource="#timeISO8601"/>
    </generalInformation>
    


    <!-- http://www.semanticweb.org/ontologies/2008/7/XCLOntology1.5.owl#documentKeywords -->

    <PDF1.3_Properties rdf:about="#documentKeywords">
        <is_same_as rdf:resource="#textualAnnotation"/>
    </PDF1.3_Properties>
    


    <!-- http://www.semanticweb.org/ontologies/2008/7/XCLOntology1.5.owl#documentLanguage -->

    <generalInformation rdf:about="#documentLanguage">
        <rdfs:comment
            >Language of the Document</rdfs:comment>
        <rdfs:comment>id190</rdfs:comment>
        <Datatype rdf:resource="#string"/>
        <is_same_as rdf:resource="#textualDataLanguage"/>
    </generalInformation>
    


    <!-- http://www.semanticweb.org/ontologies/2008/7/XCLOntology1.5.owl#documentModificationDate -->

    <generalInformation rdf:about="#documentModificationDate">
        <ID>id82</ID>
        <Datatype rdf:resource="#timeISO8601"/>
        <is_same_as rdf:resource="#timeLastMod"/>
    </generalInformation>
    


    <!-- http://www.semanticweb.org/ontologies/2008/7/XCLOntology1.5.owl#documentProducer -->

    <PDF1.3_Properties rdf:about="#documentProducer">
        <is_same_as rdf:resource="#Artist_Tiff"/>
        <is_same_as rdf:resource="#artist"/>
    </PDF1.3_Properties>
    


    <!-- http://www.semanticweb.org/ontologies/2008/7/XCLOntology1.5.owl#documentTitle -->

    <generalInformation rdf:about="#documentTitle">
        <ID>id78</ID>
        <rdfs:comment xml:lang="en"
            >title of the document, if different of fileName (possibly only accuring in pdf-files)</rdfs:comment>
        <is_same_as rdf:resource="#outlinesEntryTitle"/>
        <Datatype rdf:resource="#string"/>
    </generalInformation>
    


    <!-- http://www.semanticweb.org/ontologies/2008/7/XCLOntology1.5.owl#doubleStrike -->

    <textInformation rdf:about="#doubleStrike">
        <ID>id165</ID>
        <rdfs:comment
            >text-property doubleStrike</rdfs:comment>
        <Datatype rdf:resource="#bool"/>
    </textInformation>
    


    <!-- http://www.semanticweb.org/ontologies/2008/7/XCLOntology1.5.owl#drawing -->

    <wordProcessingML rdf:about="#drawing">
        <rdfs:comment
            >drawing (DrawingML Object) 
This element specifies that a DrawingML object is located at this position in the run&#8217;s contents. The layout properties of this DrawingML object are specified using the WordprocessingML Drawing syntax (&#167;5.5). 
Example: Consider a run which consists of a picture which is in line with the text in that paragraph (i.e. on the line and affects the line height). That run would be specified using the following WordprocessingML:
&lt;w:r&gt; 
  &lt;w:drawing&gt; 
    &lt;wp:inline&gt; 
      &#8230; 
    &lt;/wp:inline&gt; 
  &lt;/w:drawing&gt; 
&lt;/w:r&gt; 
The drawing element indicates that a DrawingML object and its WordprocessingML Drawing positioning data are located at the current position in the run (e.g. a picture or a chart). 
[cit. OOXML spec.]</rdfs:comment>
    </wordProcessingML>
    


    <!-- http://www.semanticweb.org/ontologies/2008/7/XCLOntology1.5.owl#dstrike -->

    <wordProcessingML rdf:about="#dstrike">
        <rdfs:comment
            >Double Strikethrough
This element specifies that the contents of this run shall be displayed with two horizontal lines through each character displayed on the line.
If this element is not present, the default value is to leave the formatting applied at previous level in the style hierarchy. If this element is never applied in the style hierarchy, then double strikethrough shall not be applied to the contents of this run. 
This element shall not be present with the strike (&#167;2.3.2.35) property on the same run, since they are mutually exclusive in terms of appearance. 
Example: Consider a run of text which shall have the dstrike property explicitly turned on for the contents of the run. This constraint is specified using the following WordprocessingML: 
&lt;w:rPr&gt; 
  &lt;w:dstrike w:val=&quot;true&quot;/&gt; 
&lt;/w:rPr&gt; 
This run explicitly declares that the dstrike property is true, so the contents of this run will have two horizontal strikethrough lines.
[cit. OOXML spec.]</rdfs:comment>
        <Datatype rdf:resource="#bool"/>
    </wordProcessingML>
    


    <!-- http://www.semanticweb.org/ontologies/2008/7/XCLOntology1.5.owl#eastAsianLayout -->

    <wordProcessingML rdf:about="#eastAsianLayout">
        <rdfs:comment
            >East Asian Typography Settings
This element specifies any East Asian typography settings which shall be applied to the contents of the run. 
The specific typography settings represented by this element include the two lines in one and horizontal in vertical text options. 
The two lines in one setting specifies that the characters in this run should be written out on a single line in the document by creating two sub-lines within the regular line, and laying out this text equally between those sub lines. 
Example: Consider a paragraph with the text two lines in one, which shall be displayed within a single logical line in the document. This constraint would be specified as follows in the WordprocessingML: 
&lt;w:r&gt; 
  &lt;w:rPr&gt; 
    &lt;w:eastAsianLayout w:id=&quot;1&quot; w:combine=&quot;on&quot; /&gt; 
  &lt;/w:rPr&gt; 
  &lt;w:t&gt;two lines in one&lt;/w:t&gt; 
&lt;/w:r&gt;</rdfs:comment>
        <Datatype rdf:resource="#bool"/>
    </wordProcessingML>
    


    <!-- http://www.semanticweb.org/ontologies/2008/7/XCLOntology1.5.owl#effect -->

    <wordProcessingML rdf:about="#effect">
        <rdfs:comment
            >Animated Text Effect
This element specifies an animated text effect which should be displayed when rendering the contents of this run. This effect is rendered around the extents of the text in the run in the same location as a run border with zero pixels of padding would be rendered (if such a run border was present). 
If this element is not present, the default value is to leave the formatting applied at previous level in the style hierarchy. If this element is never applied in the style hierarchy, then no text effect shall be applied to the contents of this run. 
Example: Consider a run of text which shall have an animated text effect consisting of multiple colored flashing lights (see possible attribute values for descriptions of each effect). This constraint is specified using the following WordprocessingML: 
&lt;w:rPr&gt;  
  &lt;w:effect w:val=&quot;lights&quot;/&gt; 
&lt;/w:rPr&gt; 
This run explicitly declares that the effect property is lights, so the contents of this run will have an animated lights text effect.
Possible values are:
&quot;blinkBackground&quot;,
&quot;lights&quot;,
&quot;antsBlack&quot;,
&quot;antsRed&quot;,
&quot;shimmer&quot;,
sparkle&quot;,
&quot;none&quot;
[cit. OOXML spec.]</rdfs:comment>
        <Datatype rdf:resource="#string"/>
    </wordProcessingML>
    


    <!-- http://www.semanticweb.org/ontologies/2008/7/XCLOntology1.5.owl#em -->

    <wordProcessingML rdf:about="#em">
        <rdfs:comment
            >Emphasis Mark
This element specifies the emphasis mark which shall be displayed for each non-space character in this run. An emphasis mark is an additional character that is rendered above or below the main character glyph as specified by the contents of the val attribute. 
If this element is not present, the default value is to leave the formatting applied at previous level in the style hierarchy. If this element is never applied in the style hierarchy, then no emphasis mark shall be added to each character in the contents of this run. 
Example: Consider a run of text which shall have a dot underneath each character as an emphasis mark. This constraint is specified using the following WordprocessingML: 
&lt;w:rPr&gt; 
  &lt;w:em w:val=&quot;dot&quot;/&gt; 
&lt;/w:rPr&gt; 
This run explicitly declares that the emphasis mark type is dot, so the contents of this run will have a dot emphasis mark above each character.
Possible Values:
&quot;none&quot;
&quot;dot&quot;
&quot;comma&quot;
&quot;circle&quot;
&quot;underDot&quot;
[cit. OOXML spec.]</rdfs:comment>
        <Datatype rdf:resource="#string"/>
    </wordProcessingML>
    


    <!-- http://www.semanticweb.org/ontologies/2008/7/XCLOntology1.5.owl#embeddedImage -->

    <PDF1.3_Properties rdf:about="#embeddedImage">
        <is_same_as rdf:resource="#imageData"/>
    </PDF1.3_Properties>
    


    <!-- http://www.semanticweb.org/ontologies/2008/7/XCLOntology1.5.owl#embeddedObject -->

    <generalInformation rdf:about="#embeddedObject">
        <ID>id146</ID>
    </generalInformation>
    


    <!-- http://www.semanticweb.org/ontologies/2008/7/XCLOntology1.5.owl#emboss -->

    <wordProcessingML rdf:about="#emboss">
        <rdfs:comment
            >Embossing
This element specifies that the contents of this run should be displayed as if embossed, which makes text appear as if it is raised off the page in relief. 
This formatting property is a toggle property, which specifies that its behavior differs between its use within a style definition and its use as direct formatting. When used as part of a style definition, setting this property shall toggle the current state of that property as specified up to this point in the hierarchy (i.e. applied to not applied, and vice versa). Setting it to false (or an equivalent) shall result in the current setting remaining unchanged. However, when used as direct formatting, setting this property to true or false shall set the absolute state of the resulting property.  
If this element is not present, the default value is to leave the formatting applied at previous level in the style hierarchy. If this element is never applied in the style hierarchy, then embossing shall not be applied to the contents of this run. 
This element shall not be present with either the imprint (&#167;2.3.2.16) or outline (&#167;2.3.2.21) properties on the same run, since they are mutually exclusive in terms of appearance. 
Example: Consider a run of text which shall have the emboss property explicitly turned on for the contents of the run. This constraint is specified using the following WordprocessingML: 
&lt;w:rPr&gt;
  &lt;w:emboss w:val=&quot;true&quot;/&gt; 
&lt;/w:rPr&gt; 
This run explicitly declares that the emboss property is true, so the contents of this run will appear embossed.
[cit. OOXML spec.]</rdfs:comment>
        <Datatype rdf:resource="#bool"/>
    </wordProcessingML>
    


    <!-- http://www.semanticweb.org/ontologies/2008/7/XCLOntology1.5.owl#exifAudioMetadata -->

    <audioInformation rdf:about="#exifAudioMetadata">
        <ID>id301</ID>
        <Unit rdf:resource="#NULL"/>
        <Datatype rdf:resource="#string"/>
    </audioInformation>
    


    <!-- http://www.semanticweb.org/ontologies/2008/7/XCLOntology1.5.owl#exifPhotoMetadata -->

    <videoinformation rdf:about="#exifPhotoMetadata">
        <rdf:type rdf:resource="#rasterInformation"/>
    </videoinformation>
    


    <!-- http://www.semanticweb.org/ontologies/2008/7/XCLOntology1.5.owl#extraSamples -->

    <rasterInformation rdf:about="#extraSamples">
        <is_same_as rdf:resource="#Extrasamples_NISO"/>
        <is_same_as rdf:resource="#extraSamples_Tiff"/>
        <Datatype rdf:resource="#int"/>
    </rasterInformation>
    


    <!-- http://www.semanticweb.org/ontologies/2008/7/XCLOntology1.5.owl#extraSamples_Tiff -->

    <Tiff_Properties rdf:about="#extraSamples_Tiff">
        <rdfs:comment xml:lang="en"
            >Description of extra components.

Specifies that each pixel has N extra components whose interpretation is defined by one of the values listed below. When this field is used, the SamplesPerPixel field has a value greater than the PhotometricInterpretation field suggests.

For example, full-color RGB data normally has SamplesPerPixel=3. If SamplesPerPixel is greater than 3, then the ExtraSamples field describes the meaning of the extra samples. If SamplesPerPixel is, say, 5 then ExtraSamples will contain 2 values, one for each extra sample. ExtraSamples is typically used to include non-color information, such as opacity, in an image. The possible values for each item in the field&#39;s value are:

0 = Unspecified data
1 = Associated alpha data (with pre-multiplied color)
2 = Unassociated alpha data [cit. TIFF 6.0] [Compatibility: TIFF 6.0]</rdfs:comment>
        <is_same_as rdf:resource="#Extrasamples_NISO"/>
        <is_same_as rdf:resource="#extraSamples"/>
        <Datatype rdf:resource="#int"/>
    </Tiff_Properties>
    


    <!-- http://www.semanticweb.org/ontologies/2008/7/XCLOntology1.5.owl#fileName -->

    <generalInformation rdf:about="#fileName">
        <ID>id205</ID>
        <Restriction rdf:resource="#mandatory"/>
        <Datatype rdf:resource="#string"/>
    </generalInformation>
    


    <!-- http://www.semanticweb.org/ontologies/2008/7/XCLOntology1.5.owl#fileSize -->

    <generalInformation rdf:about="#fileSize">
        <ID>id120</ID>
        <Unit rdf:resource="#byte"/>
        <is_same_as rdf:resource="#fileSize_NISO"/>
        <Restriction rdf:resource="#mandatory"/>
        <Datatype rdf:resource="#uint32Rational"/>
    </generalInformation>
    


    <!-- http://www.semanticweb.org/ontologies/2008/7/XCLOntology1.5.owl#fileSize_NISO -->

    <NISO rdf:about="#fileSize_NISO">
        <Unit rdf:resource="#byte"/>
        <is_same_as rdf:resource="#fileSize"/>
        <Datatype rdf:resource="#int"/>
    </NISO>
    


    <!-- http://www.semanticweb.org/ontologies/2008/7/XCLOntology1.5.owl#fillColour -->

    <vectorInformation rdf:about="#fillColour">
        <ID>id241</ID>
        <rdfs:comment
            >fill-colour for vector-object</rdfs:comment>
        <Datatype rdf:resource="#int"/>
    </vectorInformation>
    


    <!-- http://www.semanticweb.org/ontologies/2008/7/XCLOntology1.5.owl#fillOrder -->

    <rasterInformation rdf:about="#fillOrder">
        <ID>id21</ID>
        <Unit rdf:resource="#NULL"/>
        <Datatype rdf:resource="#int"/>
    </rasterInformation>
    


    <!-- http://www.semanticweb.org/ontologies/2008/7/XCLOntology1.5.owl#fillOrderTiff -->

    <Tiff_Properties rdf:about="#fillOrderTiff">
        <rdfs:comment
            >IFD		Image
Code		266 (hex 0x010A)
Name		FillOrder
LibTiff name		TIFFTAG_FILLORDER
Type		SHORT
Count		1
Default		1 (lower column values in higher order bits)
Description:
The logical order of bits within a byte.
The specification defines these values:
1 = pixels with lower column values are stored in the higher-order bits of the byte. 2 = pixels with lower column values are stored in the lower-order bits of the byte.
The specification goes on to warn that FillOrder=2 should not be used in some cases to avoid ambigouty, and that support for FillOrder=2 is not required in Baseline TIFF compliant readers.
LibTiff defines these values:
FILLORDER_MSB2LSB = 1;
FILLORDER_LSB2MSB = 2;
In practice, the use of FillOrder=2 is very uncommon, and is not recommended.</rdfs:comment>
        <Datatype rdf:resource="#int"/>
    </Tiff_Properties>
    


    <!-- http://www.semanticweb.org/ontologies/2008/7/XCLOntology1.5.owl#fillcolor -->

    <wordProcessingML rdf:about="#fillcolor">
        <rdfs:comment xml:lang="en"
            >same as themecolor. Used for OOXML-objects to specify their color...</rdfs:comment>
        <Datatype rdf:resource="#hex"/>
    </wordProcessingML>
    


    <!-- http://www.semanticweb.org/ontologies/2008/7/XCLOntology1.5.owl#filter -->

    <PNG_Properties rdf:about="#filter">
        <rdfs:comment xml:lang="en"
            >transformation applied to an array of scanlines with the aim of improving their compressibility [Compatibility: PNG 1.1]</rdfs:comment>
    </PNG_Properties>
    


    <!-- http://www.semanticweb.org/ontologies/2008/7/XCLOntology1.5.owl#firstChar -->

    <fontDescriptor rdf:about="#firstChar">
        <rdfs:comment xml:lang="en"
            >(Required except for the standard 14 fonts) The first character code defined in the font&#8217;s Widths array. Note: Beginning with PDF 1.5, the special treatment given to the standard 14 fonts is deprecated. All fonts used in a PDF document should be represented using a complete font descriptor. For backwards capability, viewer applications must still provide the special treatment identified for the standard 14 fonts.</rdfs:comment>
    </fontDescriptor>
    


    <!-- http://www.semanticweb.org/ontologies/2008/7/XCLOntology1.5.owl#fitText -->

    <wordProcessingML rdf:about="#fitText">
        <rdfs:comment
            >Manual Run Width
This element specifies that the contents of this run shall not be automatically displayed based on the width of its contents, rather its contents shall be resized to fit the width specified by the val attribute. This expansion/contraction shall be performed by equally increasing/decreasing the size of each character in this run&#39;s contents when displayed. 
If this element is omitted, then the contents of this run shall be displayed based on the size of its contents. 
Example: Consider a document with a run which shall be displayed in exactly one-half inch of space, regardless of its contents. This constraint would be specified using the following WordprocessingML: 
&lt;w:r&gt; 
  &lt;w:rPr&gt; 
    &lt;w:fitText w:id=&quot;50&quot; w:val=&quot;720&quot; /&gt; 
  &lt;/w:rPr&gt; 
  &lt;w:t&gt;This text shall be displayed in one-half of an inch.&lt;/w:t&gt; 
&lt;/w:r&gt; 
The resulting run contents shall be displayed in exactly 720 twentieths of a point (one half of an inch) when displayed in a document. 
fitText=unique ID for run
val= exact width of space which this run shall be fit into when 
displayed in the document.
[cit. OOXML spec.]</rdfs:comment>
        <Datatype rdf:resource="#int"/>
    </wordProcessingML>
    


    <!-- http://www.semanticweb.org/ontologies/2008/7/XCLOntology1.5.owl#floatArray -->

    <xcl_propertyDatatypes rdf:about="#floatArray"/>
    


    <!-- http://www.semanticweb.org/ontologies/2008/7/XCLOntology1.5.owl#font -->

    <wordProcessingML rdf:about="#font">
        <ID>id159</ID>
        <rdfs:comment xml:lang="en"
            >namevalue of the font used in an OOXML-document</rdfs:comment>
        <is_same_as rdf:resource="#fontName"/>
        <Datatype rdf:resource="#string"/>
    </wordProcessingML>
    


    <!-- http://www.semanticweb.org/ontologies/2008/7/XCLOntology1.5.owl#fontBBox -->

    <fontDescriptor rdf:about="#fontBBox">
        <rdfs:comment xml:lang="en"
            >(Required) A rectangle (see Section 3.8.4, &#8220;Rectangles&#8221;) expressed in the 
glyph coordinate system, specifying the font bounding box. This is the smallest rectangle enclosing the shape that would result if all of the glyphs of the font were placed with their origins coincident and then filled. 
If all four elements of the rectangle are zero, no assumptions are made based on the font bounding box. If any element is nonzero, it is essential that the font bounding box be accurate. If any glyph&#8217;s marks fall outside this bounding box, incorrect behavior may result.</rdfs:comment>
        <Datatype rdf:resource="#matrix"/>
    </fontDescriptor>
    


    <!-- http://www.semanticweb.org/ontologies/2008/7/XCLOntology1.5.owl#fontCapHeight -->

    <fontDescriptor rdf:about="#fontCapHeight">
        <is_same_as rdf:resource="#fontSize"/>
    </fontDescriptor>
    


    <!-- http://www.semanticweb.org/ontologies/2008/7/XCLOntology1.5.owl#fontColour -->

    <textInformation rdf:about="#fontColour">
        <ID>id160</ID>
        <rdfs:comment
            >font color in text formats</rdfs:comment>
        <Datatype rdf:resource="#int"/>
    </textInformation>
    


    <!-- http://www.semanticweb.org/ontologies/2008/7/XCLOntology1.5.owl#fontDescriptorFlag -->

    <PDF1.3_Properties rdf:about="#fontDescriptorFlag">
        <rdfs:comment
            >1 FixedPitch All glyphs have the same width (as opposed to proportional or variable-pitch fonts, which have different widths). 
2 Serif Glyphs have serifs, which are short strokes drawn at an angle on the top and bottom of glyph stems (as opposed to sans serif fonts, which do not). 
3 Symbolic Font contains characters outside the Adobe standard Latin character set. Bits 3 and 6 cannot both be 0 or both be 1 (see below). 
4 Script Glyphs resemble cursive handwriting. 
6 Nonsymbolic Font uses the Adobe standard Latin character set or a subset of it (see below). 
7 Italic Glyphs have dominant vertical strokes that are slanted. 
17 AllCap Font contains no lowercase letters; typically used for display purposes such as titles or headlines. 
18 SmallCap Font contains both uppercase and lowercase letters. The uppercase letters are similar to ones in the regular version of the same typeface family. The glyphs for the lowercase letters have the same shapes as the corresponding uppercase letters, but they are sized and their 
proportions adjusted so that they have the same size and stroke weight as lowercase glyphs in the same typeface family. 
19 ForceBold See below.
[cit. Pdf 1.3]</rdfs:comment>
        <Unit rdf:resource="#bit"/>
        <Datatype rdf:resource="#int"/>
    </PDF1.3_Properties>
    


    <!-- http://www.semanticweb.org/ontologies/2008/7/XCLOntology1.5.owl#fontEncodingType -->

    <textInformation rdf:about="#fontEncodingType">
        <ID>id321</ID>
        <rdfs:comment
            >can be StandardEncoding, MacRomanEncoding, WinAnsiEncoding, and PDF- DocEncoding.</rdfs:comment>
        <is_same_as rdf:resource="#EncodingType"/>
        <Datatype rdf:resource="#string"/>
    </textInformation>
    


    <!-- http://www.semanticweb.org/ontologies/2008/7/XCLOntology1.5.owl#fontFiletype -->

    <textInformation rdf:about="#fontFiletype">
        <ID>id211</ID>
        <rdfs:comment
            >containes which filetype the font is: i.e.: truetype (type 1 or 3), postscript, openType</rdfs:comment>
        <Datatype rdf:resource="#string"/>
    </textInformation>
    


    <!-- http://www.semanticweb.org/ontologies/2008/7/XCLOntology1.5.owl#fontName -->

    <textInformation rdf:about="#fontName">
        <ID>id159</ID>
        <is_same_as rdf:resource="#FontName_PDF"/>
        <Datatype rdf:resource="#string"/>
    </textInformation>
    


    <!-- http://www.semanticweb.org/ontologies/2008/7/XCLOntology1.5.owl#fontSize -->

    <textInformation rdf:about="#fontSize">
        <ID>id158</ID>
        <is_same_as rdf:resource="#FontSize_Pdf"/>
        <Datatype rdf:resource="#int"/>
    </textInformation>
    


    <!-- http://www.semanticweb.org/ontologies/2008/7/XCLOntology1.5.owl#fontTrueType -->

    <PDF1.3_Properties rdf:about="#fontTrueType">
        <rdfs:comment xml:lang="en"
            >The value of Subtype is TrueType.
A TrueType font program can be embedded directly in a PDF file as a stream object. The Type 42 font format that is defined for PostScript does not apply to PDF[cit.]</rdfs:comment>
    </PDF1.3_Properties>
    


    <!-- http://www.semanticweb.org/ontologies/2008/7/XCLOntology1.5.owl#fontType3 -->

    <PDF1.3_Properties rdf:about="#fontType3"/>
    


    <!-- http://www.semanticweb.org/ontologies/2008/7/XCLOntology1.5.owl#fontident -->

    <PDF1.3_Properties rdf:about="#fontident">
        <rdfs:comment xml:lang="en"
            >enables the identification of a font in pdf-file by matching it to installed fonts on the operationsytem...</rdfs:comment>
    </PDF1.3_Properties>
    


    <!-- http://www.semanticweb.org/ontologies/2008/7/XCLOntology1.5.owl#footnote -->

    <textInformation rdf:about="#footnote">
        <ID>id170</ID>
        <rdfs:comment xml:lang="en"
            >marks up a certain position in normdata to specify them as a footnote related to other normdata</rdfs:comment>
        <Datatype rdf:resource="#bool"/>
    </textInformation>
    


    <!-- http://www.semanticweb.org/ontologies/2008/7/XCLOntology1.5.owl#footnoteReference -->

    <wordProcessingML rdf:about="#footnoteReference">
        <rdfs:comment xml:lang="en"
            >All footnotes for a WordprocessingML document are contained in the same Footnotes part. Let&#8217;s look at how the Main Document refers to the footnote. At the point at which the footnote reference is inserted, the following XML is present: 
&lt;w:r&gt; 
   &lt;w:footnoteReference w:id=&quot;2&quot;/&gt; 
&lt;/w:r&gt;26 
The reference to the footnote with id=2 is &#8220;understood&#8221; to be in the Footnotes part that must always exist if there are any footnotes in the document. 
[cit.: OOXML spec]</rdfs:comment>
    </wordProcessingML>
    


    <!-- http://www.semanticweb.org/ontologies/2008/7/XCLOntology1.5.owl#formField -->

    <textInformation rdf:about="#formField">
        <rdfs:comment xml:lang="en"
            >defines some normdata to be content in a formfield.
Defines the position and size of this rectangular field on the page</rdfs:comment>
        <ID>id186</ID>
        <Datatype rdf:resource="#matrix"/>
    </textInformation>
    


    <!-- http://www.semanticweb.org/ontologies/2008/7/XCLOntology1.5.owl#fpsVideo -->

    <videoinformation rdf:about="#fpsVideo">
        <ID>id172</ID>
        <Datatype rdf:resource="#uint32Rational"/>
    </videoinformation>
    


    <!-- http://www.semanticweb.org/ontologies/2008/7/XCLOntology1.5.owl#framePr -->

    <wordProcessingML rdf:about="#framePr">
        <rdfs:comment xml:lang="en"
            >Text Frame Properties
This element specifies information about the current paragraph with regard to text frames. Text frames are paragraphs of text in a document which are positioned in a separate region or frame in the document, and can be positioned with a specific size and position relative to non-frame paragraphs in the current document. The first piece of information specified by the framePr element is that the current paragraph is actually part of a text frame in the document. This information is specified simply by the presence of the framePr element in paragraph&#39;s properties. If the framePr element is omitted, the paragraph shall not be part of any text frame in the document. 
The second piece of information concerns the set of paragraphs which are part of the current text frame in the document. This is determined based on the attributes on the framePr element. If the set of attribute values specified on two adjacent paragraphs is identical, then those two paragraphs shall be considered to be part of the same text frame and rendered within the same frame in the document.
Example:
&lt;w:pPr&gt; 
    &lt;w:framePr w:w=&quot;2191&quot; w:h=&quot;811&quot; w:hRule=&quot;exact&quot; w:hSpace=&quot;180&quot; 
w:wrap=&quot;around&quot; w:vAnchor=&quot;text&quot; w:hAnchor=&quot;page&quot; w:x=&quot;1921&quot;/&gt; 
  &lt;/w:pPr&gt; 
[cit. OOXMl. Spec.]</rdfs:comment>
        <Datatype rdf:resource="#int"/>
    </wordProcessingML>
    


    <!-- http://www.semanticweb.org/ontologies/2008/7/XCLOntology1.5.owl#freeByteCounts -->

    <Tiff_Properties rdf:about="#freeByteCounts">
        <rdfs:comment
            >For each string of contiguous unused bytes in a TIFF file, the number of bytes in the string. 
Tag = 289  (121.H) 
Type = LONG 
Not recommended for general interchange. See also FreeOffsets.</rdfs:comment>
        <Datatype rdf:resource="#int"/>
    </Tiff_Properties>
    


    <!-- http://www.semanticweb.org/ontologies/2008/7/XCLOntology1.5.owl#freeOffsets -->

    <Tiff_Properties rdf:about="#freeOffsets">
        <rdfs:comment rdf:datatype="&xsd;int"
            >For each string of contiguous unused bytes in a TIFF file, the byte offset of the string. 
Tag = 288  (120.H) 
Type = LONG 
Not recommended for general interchange. See also FreeByteCounts.</rdfs:comment>
        <Datatype rdf:resource="#int"/>
    </Tiff_Properties>
    


    <!-- http://www.semanticweb.org/ontologies/2008/7/XCLOntology1.5.owl#freestyleShape -->

    <vectorInformation rdf:about="#freestyleShape">
        <ID>id250</ID>
        <rdfs:comment
            >free defined shape of closed vector path (messured through markers and lines/bezier-curves)</rdfs:comment>
        <Datatype rdf:resource="#int"/>
    </vectorInformation>
    


    <!-- http://www.semanticweb.org/ontologies/2008/7/XCLOntology1.5.owl#gAMA -->

    <PNG_Properties rdf:about="#gAMA">
        <rdfs:comment xml:lang="en"
            >describes the gamma-values in a PNG-file.
&quot;...Specifies the relationship between the image samples and the desired display output intensity. ...It is also necessary to specify the viewing conditions under which the output is desired. For gAMA these are the reference viewing conditions of the sRGB specifications.
The value is encoded as a four-byte PNG unsigned integer, representing gamma times 100000.
EXAMPLE A gamma of 1/2.2 would be stored as the integer 45455&quot;</rdfs:comment>
        <is_same_as rdf:resource="#gammaValue"/>
        <Datatype rdf:resource="#int"/>
    </PNG_Properties>
    


    <!-- http://www.semanticweb.org/ontologies/2008/7/XCLOntology1.5.owl#gIFt -->

    <GIF_Properties rdf:about="#gIFt">
        <rdfs:comment xml:lang="en"
            >Plain Text Extension:
&quot;GIF&#39;s Plain Text Extension is a way to define an image composed entirely of text without actually storing the text as a bitmapped image. It defines a rectangular grid of character cells into which text characters of the specified foreground and background colours are placed, starting from the upper left and proceeding left to right and top to bottom; the decoder chooses the font that is the closest match to the specified size.&quot;
Not very often supported by software</rdfs:comment>
    </GIF_Properties>
    


    <!-- http://www.semanticweb.org/ontologies/2008/7/XCLOntology1.5.owl#gammaValue -->

    <rasterInformation rdf:about="#gammaValue">
        <ID>id41</ID>
        <rdfs:comment xml:lang="en"
            >Level of brightness for pixels ranging from black (0) to white (1). These pixel values serve as the input for the computer monitor. 
The sRGB and Adobe RGB colour spaces are also based on a gamma of 2.2.
Gamma-encoding is supported by certain image-fileformats</rdfs:comment>
        <is_same_as rdf:resource="#gAMA"/>
        <Datatype rdf:resource="#int"/>
    </rasterInformation>
    


    <!-- http://www.semanticweb.org/ontologies/2008/7/XCLOntology1.5.owl#gpsAltitude -->

    <NISO rdf:about="#gpsAltitude"/>
    


    <!-- http://www.semanticweb.org/ontologies/2008/7/XCLOntology1.5.owl#gpsAltitudeRef -->

    <NISO rdf:about="#gpsAltitudeRef"/>
    


    <!-- http://www.semanticweb.org/ontologies/2008/7/XCLOntology1.5.owl#gpsAreaInformation -->

    <NISO rdf:about="#gpsAreaInformation"/>
    


    <!-- http://www.semanticweb.org/ontologies/2008/7/XCLOntology1.5.owl#gpsDOP -->

    <NISO rdf:about="#gpsDOP"/>
    


    <!-- http://www.semanticweb.org/ontologies/2008/7/XCLOntology1.5.owl#gpsDateStamp -->

    <NISO rdf:about="#gpsDateStamp"/>
    


    <!-- http://www.semanticweb.org/ontologies/2008/7/XCLOntology1.5.owl#gpsDestBearing -->

    <NISO rdf:about="#gpsDestBearing"/>
    


    <!-- http://www.semanticweb.org/ontologies/2008/7/XCLOntology1.5.owl#gpsDestBearingRef -->

    <NISO rdf:about="#gpsDestBearingRef"/>
    


    <!-- http://www.semanticweb.org/ontologies/2008/7/XCLOntology1.5.owl#gpsDestDistance -->

    <NISO rdf:about="#gpsDestDistance"/>
    


    <!-- http://www.semanticweb.org/ontologies/2008/7/XCLOntology1.5.owl#gpsDestDistanceRef -->

    <NISO rdf:about="#gpsDestDistanceRef"/>
    


    <!-- http://www.semanticweb.org/ontologies/2008/7/XCLOntology1.5.owl#gpsDestLatitude -->

    <NISO rdf:about="#gpsDestLatitude"/>
    


    <!-- http://www.semanticweb.org/ontologies/2008/7/XCLOntology1.5.owl#gpsDestLatitudeRef -->

    <NISO rdf:about="#gpsDestLatitudeRef"/>
    


    <!-- http://www.semanticweb.org/ontologies/2008/7/XCLOntology1.5.owl#gpsDestLongitude -->

    <NISO rdf:about="#gpsDestLongitude"/>
    


    <!-- http://www.semanticweb.org/ontologies/2008/7/XCLOntology1.5.owl#gpsDestLongitudeRef -->

    <NISO rdf:about="#gpsDestLongitudeRef"/>
    


    <!-- http://www.semanticweb.org/ontologies/2008/7/XCLOntology1.5.owl#gpsDifferential -->

    <NISO rdf:about="#gpsDifferential"/>
    


    <!-- http://www.semanticweb.org/ontologies/2008/7/XCLOntology1.5.owl#gpsImgDirection -->

    <NISO rdf:about="#gpsImgDirection"/>
    


    <!-- http://www.semanticweb.org/ontologies/2008/7/XCLOntology1.5.owl#gpsImgDirectionRef -->

    <NISO rdf:about="#gpsImgDirectionRef"/>
    


    <!-- http://www.semanticweb.org/ontologies/2008/7/XCLOntology1.5.owl#gpsInformation -->

    <otherInformation rdf:about="#gpsInformation">
        <ID>id282</ID>
        <rdfs:comment xml:lang="en"
            >satelite-Information about geographical coordinates (useful for GIS-Objects)</rdfs:comment>
        <Datatype rdf:resource="#uint16"/>
    </otherInformation>
    


    <!-- http://www.semanticweb.org/ontologies/2008/7/XCLOntology1.5.owl#gpsLatitude -->

    <NISO rdf:about="#gpsLatitude"/>
    


    <!-- http://www.semanticweb.org/ontologies/2008/7/XCLOntology1.5.owl#gpsLatitudeRef -->

    <NISO rdf:about="#gpsLatitudeRef"/>
    


    <!-- http://www.semanticweb.org/ontologies/2008/7/XCLOntology1.5.owl#gpsLongitude -->

    <NISO rdf:about="#gpsLongitude"/>
    


    <!-- http://www.semanticweb.org/ontologies/2008/7/XCLOntology1.5.owl#gpsLongitudeRef -->

    <NISO rdf:about="#gpsLongitudeRef"/>
    


    <!-- http://www.semanticweb.org/ontologies/2008/7/XCLOntology1.5.owl#gpsMapDatum -->

    <NISO rdf:about="#gpsMapDatum"/>
    


    <!-- http://www.semanticweb.org/ontologies/2008/7/XCLOntology1.5.owl#gpsMeasureMode -->

    <NISO rdf:about="#gpsMeasureMode"/>
    


    <!-- http://www.semanticweb.org/ontologies/2008/7/XCLOntology1.5.owl#gpsProcessingMethod -->

    <NISO rdf:about="#gpsProcessingMethod"/>
    


    <!-- http://www.semanticweb.org/ontologies/2008/7/XCLOntology1.5.owl#gpsSatellites -->

    <NISO rdf:about="#gpsSatellites"/>
    


    <!-- http://www.semanticweb.org/ontologies/2008/7/XCLOntology1.5.owl#gpsSpeed -->

    <NISO rdf:about="#gpsSpeed"/>
    


    <!-- http://www.semanticweb.org/ontologies/2008/7/XCLOntology1.5.owl#gpsSpeedRef -->

    <NISO rdf:about="#gpsSpeedRef"/>
    


    <!-- http://www.semanticweb.org/ontologies/2008/7/XCLOntology1.5.owl#gpsStatus -->

    <NISO rdf:about="#gpsStatus"/>
    


    <!-- http://www.semanticweb.org/ontologies/2008/7/XCLOntology1.5.owl#gpsTimeStamp -->

    <NISO rdf:about="#gpsTimeStamp"/>
    


    <!-- http://www.semanticweb.org/ontologies/2008/7/XCLOntology1.5.owl#gpsTrack -->

    <NISO rdf:about="#gpsTrack"/>
    


    <!-- http://www.semanticweb.org/ontologies/2008/7/XCLOntology1.5.owl#gpsTrackRef -->

    <NISO rdf:about="#gpsTrackRef"/>
    


    <!-- http://www.semanticweb.org/ontologies/2008/7/XCLOntology1.5.owl#gpsVersionID -->

    <NISO rdf:about="#gpsVersionID"/>
    


    <!-- http://www.semanticweb.org/ontologies/2008/7/XCLOntology1.5.owl#gradientAngle -->

    <vectorInformation rdf:about="#gradientAngle">
        <rdfs:comment
            >Angle of a linear gradient</rdfs:comment>
        <ID>id243</ID>
        <Datatype rdf:resource="#int"/>
    </vectorInformation>
    


    <!-- http://www.semanticweb.org/ontologies/2008/7/XCLOntology1.5.owl#gray -->

    <imageInformation rdf:about="#gray">
        <rdfs:comment xml:lang="en"
            >8 Bit ColourInformation (1 Channel) for the whole image</rdfs:comment>
        <ID>id233</ID>
        <is_same_as rdf:resource="#Gray_ICC"/>
    </imageInformation>
    


    <!-- http://www.semanticweb.org/ontologies/2008/7/XCLOntology1.5.owl#grayResponseCurve -->

    <rasterInformation rdf:about="#grayResponseCurve">
        <ID>id283</ID>
        <rdfs:comment
            >For grayscale data, the optical density of each possible pixel value</rdfs:comment>
        <is_same_as rdf:resource="#GrayResponseCurve_NISO"/>
        <is_same_as rdf:resource="#grayResponseCurveTiff"/>
        <Datatype rdf:resource="#int"/>
    </rasterInformation>
    


    <!-- http://www.semanticweb.org/ontologies/2008/7/XCLOntology1.5.owl#grayResponseCurveTiff -->

    <Tiff_Properties rdf:about="#grayResponseCurveTiff">
        <rdfs:comment xml:lang="en"
            >For greyscale data, the optical density of each possible pixel value [cit. TIFF 6.0] [Compatibility: TIFF 6.0]</rdfs:comment>
        <is_same_as rdf:resource="#GrayResponseCurve_NISO"/>
        <is_same_as rdf:resource="#grayResponseCurve"/>
        <Datatype rdf:resource="#int"/>
    </Tiff_Properties>
    


    <!-- http://www.semanticweb.org/ontologies/2008/7/XCLOntology1.5.owl#grayResponseUnit -->

    <rasterInformation rdf:about="#grayResponseUnit">
        <rdfs:comment rdf:datatype="&xsd;int"
            >The precision of the information contained in the GrayResponseCurve.
Because optical density is specified in terms of fractional numbers, this field is necessary to interpret the stored integer information.</rdfs:comment>
        <ID>id284</ID>
        <is_same_as rdf:resource="#GrayResponseUnit_NISO"/>
        <is_same_as rdf:resource="#grayResponseUnitTiff"/>
        <Datatype rdf:resource="#string"/>
    </rasterInformation>
    


    <!-- http://www.semanticweb.org/ontologies/2008/7/XCLOntology1.5.owl#grayResponseUnitTiff -->

    <Tiff_Properties rdf:about="#grayResponseUnitTiff">
        <rdfs:comment
            >The precision of the information contained in the GrayResponseCurve. 
Tag = 290 (122.H) 
Type = SHORT 
N = 1 
Because optical density is specified in terms of fractional numbers, this field is necessary to interpret the stored integer information. For example, if
GrayScaleResponseUnits is set to 4 (ten-thousandths of a unit), and a  GrayScaleResponseCurve number for gray level 4 is 3455, then the resulting
actual value is 0.3455. 
Optical densitometers typically measure densities within the range of 0.0 to 2.0.
TIFF 6.0 Specification Final&#8212;June 3, 1992 
1 = Number represents tenths of a unit. 
2 = Number represents hundredths of a unit. 
3 = Number represents thousandths of a unit. 
4 =  Number represents ten-thousandths of a unit. 
5 = Number represents hundred-thousandths of a unit.</rdfs:comment>
        <is_same_as rdf:resource="#GrayResponseUnit_NISO"/>
        <is_same_as rdf:resource="#grayResponseUnit"/>
        <Datatype rdf:resource="#int"/>
    </Tiff_Properties>
    


    <!-- http://www.semanticweb.org/ontologies/2008/7/XCLOntology1.5.owl#hIST -->

    <PNG_Properties rdf:about="#hIST">
        <rdfs:comment xml:lang="en"
            >Histogramme chunk for PNGs</rdfs:comment>
        <is_same_as rdf:resource="#histogram"/>
        <is_same_as rdf:resource="#paletteHistogram"/>
    </PNG_Properties>
    


    <!-- http://www.semanticweb.org/ontologies/2008/7/XCLOntology1.5.owl#halftone -->

    <PDF1.3_Properties rdf:about="#halftone">
        <rdfs:comment
            >(PDF 1.2) A halftone screen for gray and color rendering, speci&#64257;ed as a halftone dictionary or stream (see Section 6.4, &#8220;Halftones&#8221;). 
Initial value: installation-dependent. [cit. Pdf 1.3]</rdfs:comment>
        <Datatype rdf:resource="#string"/>
    </PDF1.3_Properties>
    


    <!-- http://www.semanticweb.org/ontologies/2008/7/XCLOntology1.5.owl#headerSize -->

    <generalInformation rdf:about="#headerSize">
        <ID>id122</ID>
        <is_same_as rdf:resource="#headerSizeBmp"/>
        <Datatype rdf:resource="#int"/>
    </generalInformation>
    


    <!-- http://www.semanticweb.org/ontologies/2008/7/XCLOntology1.5.owl#headerSizeBmp -->

    <BMP_Properties rdf:about="#headerSizeBmp">
        <is_same_as rdf:resource="#headerSize"/>
    </BMP_Properties>
    


    <!-- http://www.semanticweb.org/ontologies/2008/7/XCLOntology1.5.owl#hex -->

    <xcl_propertyDatatypes rdf:about="#hex"/>
    


    <!-- http://www.semanticweb.org/ontologies/2008/7/XCLOntology1.5.owl#hidden -->

    <textInformation rdf:about="#hidden">
        <rdfs:comment>text is hidden</rdfs:comment>
        <ID>id169</ID>
        <Datatype rdf:resource="#bool"/>
        <is_same_as rdf:resource="#hidden_OOXML"/>
    </textInformation>
    


    <!-- http://www.semanticweb.org/ontologies/2008/7/XCLOntology1.5.owl#hidden_OOXML -->

    <wordProcessingML rdf:about="#hidden_OOXML"/>
    


    <!-- http://www.semanticweb.org/ontologies/2008/7/XCLOntology1.5.owl#highlight -->

    <wordProcessingML rdf:about="#highlight">
        <rdfs:comment
            >This element specifies a highlighting color which is applied as a background behind the contents of this run. 
If this run has any background shading specified using the shd element (&#167;2.3.2.30), then the background shading shall be superseded by the highlighting color when the contents of this run are displayed. 
If this element is not present, the default value is to leave the formatting applied at previous level in the style hierarchy. If this element is never applied in the style hierarchy, then text highlighting shall not be applied to the contents of this run. 
Example: Consider a run within a paragraph which has run shading applied as well as yellow text highlighting using the highlight element. This formatting is specified using the following WordprocessingML: 
&lt;w:rPr&gt; 
  &lt;w:highlight w:val=&quot;yellow&quot; /&gt;  
  &lt;w:shd w:themeFill=&quot;accent2&quot; w:themeFillTint=&quot;66&quot; /&gt;  
&lt;/w:rPr&gt; 
The resulting run would have yellow highlighting visible over its contents, as the highlighting supersedes the shading for the contents of the run.
Possibile Values are:
black&quot; &quot;blue&quot; &quot;cyan&quot; &quot;green&quot; &quot;magenta&quot; &quot;red&quot; &quot;yellow&quot; &quot;white&quot; &quot;darkBlue&quot; &quot;darkCyan&quot; &quot;darkGreen&quot; &quot;darkMagenta&quot; &quot;darkRed&quot; &quot;darkYellow&quot; &quot;darkGray&quot; lightGray&quot; &quot;none&quot;
[cit. OOXML spec.]</rdfs:comment>
        <Datatype rdf:resource="#string"/>
    </wordProcessingML>
    


    <!-- http://www.semanticweb.org/ontologies/2008/7/XCLOntology1.5.owl#histogram -->

    <rasterInformation rdf:about="#histogram">
        <ID>id42</ID>
        <rdfs:comment
            >approximate usage frequency of each colour in the image</rdfs:comment>
        <is_same_as rdf:resource="#hIST"/>
        <Datatype rdf:resource="#int"/>
        <is_same_as rdf:resource="#paletteHistogram"/>
    </rasterInformation>
    


    <!-- http://www.semanticweb.org/ontologies/2008/7/XCLOntology1.5.owl#horizontalSizeVector -->

    <vectorInformation rdf:about="#horizontalSizeVector">
        <rdfs:comment
            >horizontal size of vectorImage in defined vector-unit</rdfs:comment>
        <ID>id257</ID>
        <Datatype rdf:resource="#uint32Rational"/>
    </vectorInformation>
    


    <!-- http://www.semanticweb.org/ontologies/2008/7/XCLOntology1.5.owl#hostCompOS -->

    <Tiff_Properties rdf:about="#hostCompOS">
        <rdfs:comment xml:lang="en"
            >The computer and/or operating system in use at the time of image creation [cit. TIFF 6.0] [Compatibility: TIFF 6.0]</rdfs:comment>
        <is_same_as rdf:resource="#hostComputer_TIff"/>
        <is_same_as rdf:resource="#hostMachineOS"/>
        <Datatype rdf:resource="#string"/>
    </Tiff_Properties>
    


    <!-- http://www.semanticweb.org/ontologies/2008/7/XCLOntology1.5.owl#hostComputer_TIff -->

    <Tiff_Properties rdf:about="#hostComputer_TIff">
        <rdfs:comment rdf:datatype="&xsd;int"
            >&quot; The computer and/or operating system in use at the time of image creation. &quot;</rdfs:comment>
        <is_same_as rdf:resource="#hostCompOS"/>
        <is_same_as rdf:resource="#hostMachineOS"/>
        <Datatype rdf:resource="#string"/>
    </Tiff_Properties>
    


    <!-- http://www.semanticweb.org/ontologies/2008/7/XCLOntology1.5.owl#hostMachineOS -->

    <generalInformation rdf:about="#hostMachineOS">
        <rdfs:comment xml:lang="en"
            >The computer and/or operating system in use at the time of object creation</rdfs:comment>
        <ID>id140</ID>
        <is_same_as rdf:resource="#HostComputer_NISO"/>
        <is_same_as rdf:resource="#hostComputer_TIff"/>
        <is_same_as rdf:resource="#hostMachineOS"/>
        <Datatype rdf:resource="#string"/>
    </generalInformation>
    


    <!-- http://www.semanticweb.org/ontologies/2008/7/XCLOntology1.5.owl#hps -->

    <wordProcessingML rdf:about="#hps">
        <rdfs:comment
            >hps (Phonetic Guide Text Font Size)
This element specifies the font size which shall be applied to the phonetic guide text in the contents of this run when displayed. 
If this element disagrees with the run properties on the phonetic guide text rt element (&#167;2.3.3.23), then those properties shall be ignored and this element shall determine the size of the phonetic guide text. 
Example: Consider a run of phonetic guide text which shall have an explicit font size of 13.5 points. This constraint is specified using the following WordprocessingML: 
&lt;w:rubyPr&gt; 
  &#8230; 
  &lt;w:hps w:val=&quot;27&quot;/&gt; 
  &#8230; 
&lt;/w:rubyPr&gt; 
The hps property is 27 half-points for the ruby text in this run, so the phonetic guide text will be displayed in 13.5 point font size.
Val specifies a positive measurement specified in half-points (1/144 of an inch).
[cit. OOXML spec.]</rdfs:comment>
        <Datatype rdf:resource="#int"/>
        <Restriction rdf:resource="#relevant"/>
    </wordProcessingML>
    


    <!-- http://www.semanticweb.org/ontologies/2008/7/XCLOntology1.5.owl#hpsBaseText -->

    <wordProcessingML rdf:about="#hpsBaseText">
        <rdfs:comment
            >hpsBaseText (Phonetic Guide Base Text Font Size) 
This element specifies the font size which shall be applied to the base text of this phonetic guide text when displayed. If this element disagrees with the run properties on the phonetic guide base text rubyBase element (&#167;2.3.3.26), then this property shall be ignored and the sz element (&#167;2.3.2.36) in that run shall determine the size of the phonetic guide base text. 
Example: Consider a run of phonetic guide base text which shall have an explicit font size of 30 points. This constraint is specified using the following WordprocessingML: WordprocessingML Reference Material - Paragraphs and Rich Formatting 
&lt;w:rubyPr&gt; 
  &#8230; 
  &lt;w:hpsBaseText w:val=&quot;60&quot;/&gt; 
  &#8230; 
&lt;/w:rubyPr&gt; 
The hpsBaseText property is 60 half-points for the base text in this phonetic guide, so the phonetic guide base text will be displayed in 30 point font size.</rdfs:comment>
    </wordProcessingML>
    


    <!-- http://www.semanticweb.org/ontologies/2008/7/XCLOntology1.5.owl#hypertextLink -->

    <textInformation rdf:about="#hypertextLink">
        <rdfs:comment xml:lang="en"
            >defines that some textdata contain a hyperlink</rdfs:comment>
        <ID>id184</ID>
        <Datatype rdf:resource="#string"/>
    </textInformation>
    


    <!-- http://www.semanticweb.org/ontologies/2008/7/XCLOntology1.5.owl#i -->

    <wordProcessingML rdf:about="#i">
        <rdfs:comment
            >italics:
This element specifies whether the italic property should be applied to all non-complex script characters in the contents of this run when displayed in a document. 
This formatting property is a toggle property, which specifies that its behavior differs between its use within a style definition and its use as direct formatting. When used as part of a style definition, setting this property shall toggle the current state of that property as specified up to this point in the hierarchy (i.e. applied to not applied, and vice versa). Setting it to false (or an equivalent) shall result in the current setting remaining unchanged. However, when used as direct formatting, setting this property to true or false shall set the absolute state of the resulting property.  
If this element is not present, the default value is to leave the formatting applied at previous level in the style hierarchy .If this element is never applied in the style hierarchy, then italics shall not be applied to non-complex script characters. 
Example: Consider a run of text which shall have the i property explicitly turned on for the non-complex script contents of the run. This constraint is specified using the following WordprocessingML: 
&lt;w:rPr&gt; 
  &lt;w:i /&gt; 
&lt;/w:rPr&gt;
[cit. OOXML spec.]</rdfs:comment>
        <Datatype rdf:resource="#bool"/>
    </wordProcessingML>
    


    <!-- http://www.semanticweb.org/ontologies/2008/7/XCLOntology1.5.owl#iCCP -->

    <PNG_Properties rdf:about="#iCCP">
        <rdfs:comment xml:lang="en"
            >Containes ICC-Profile-Data.
Profile name: 1-79 bytes (character string)
Null separator: 1 byte (null character)
Compression method: 1 byte
Compressed profile: n bytes

If the iCCP chunk is present, the image samples conform to the colour space represented by the embedded ICC profile as defined by the International colour Consortium [ICC]. The colour space of the ICC profile shall be an RGB colour space for colour images (PNG colour types 2, 3, and 6), or a greyscale colour space for greyscale images (PNG colour types 0 and 4).</rdfs:comment>
        <is_same_as rdf:resource="#ICCProfileName"/>
    </PNG_Properties>
    


    <!-- http://www.semanticweb.org/ontologies/2008/7/XCLOntology1.5.owl#iCs -->

    <wordProcessingML rdf:about="#iCs">
        <rdfs:comment
            >Complex Script Italics
This element specifies whether the italic property should be applied to all complex script characters in the contents of this run when displayed in a document. 
This formatting property is a toggle property, which specifies that its behavior differs between its use within a style definition and its use as direct formatting. When used as part of a style definition, setting this property shall toggle the current state of that property as specified up to this point in the hierarchy (i.e. applied to not applied, and vice versa). Setting it to false (or an equivalent) shall result in the current setting remaining unchanged. However, when used as direct formatting, setting this property to true or false shall set the absolute state of the resulting property.
If this element is not present, the default value is to leave the formatting applied at previous level in the style hierarchy. If this element is never applied in the style hierarchy, then italics shall not be applied to complex script characters. 
Example: Consider a run of text which shall have the iCs property explicitly turned on for the complex script contents of the run. This constraint is specified using the following WordprocessingML: 
&lt;w:rPr&gt; 
  &lt;w:iCs w:val=&quot;true&quot;/&gt; 
&lt;/w:rPr&gt; 
This run explicitly declares that the iCs property is true, so italics are turned on for the complex script contents of this run. 
[cit. OOXML spec.]</rdfs:comment>
        <Datatype rdf:resource="#bool"/>
    </wordProcessingML>
    


    <!-- http://www.semanticweb.org/ontologies/2008/7/XCLOntology1.5.owl#iTXt -->

    <PNG_Properties rdf:about="#iTXt">
        <rdfs:comment xml:lang="en"
            >text compression</rdfs:comment>
        <is_same_as rdf:resource="#deflate_Zlib"/>
        <is_same_as rdf:resource="#zTXt"/>
    </PNG_Properties>
    


    <!-- http://www.semanticweb.org/ontologies/2008/7/XCLOntology1.5.owl#imageData -->

    <otherInformation rdf:about="#imageData">
        <ID>id19</ID>
        <is_same_as rdf:resource="#ImageData_NISO"/>
        <is_same_as rdf:resource="#embeddedImage"/>
        <Datatype rdf:resource="#string"/>
    </otherInformation>
    


    <!-- http://www.semanticweb.org/ontologies/2008/7/XCLOntology1.5.owl#imageDescription -->

    <Tiff_Properties rdf:about="#imageDescription">
        <Datatype rdf:resource="#string"/>
        <is_same_as rdf:resource="#textualAnnotation"/>
    </Tiff_Properties>
    


    <!-- http://www.semanticweb.org/ontologies/2008/7/XCLOntology1.5.owl#imageHeight -->

    <rasterInformation rdf:about="#imageHeight">
        <ID xml:lang="">id2</ID>
        <is_same_as rdf:resource="#Height_Gif"/>
        <is_same_as rdf:resource="#ImageLength_NISO"/>
        <is_same_as rdf:resource="#ImageLength_tiff"/>
        <Unit rdf:resource="#NULL"/>
        <Datatype rdf:resource="#int"/>
    </rasterInformation>
    


    <!-- http://www.semanticweb.org/ontologies/2008/7/XCLOntology1.5.owl#imageLeftPosition -->

    <GIF_Properties rdf:about="#imageLeftPosition">
        <rdfs:comment xml:lang="en"
            >position of an image in a gif file</rdfs:comment>
    </GIF_Properties>
    


    <!-- http://www.semanticweb.org/ontologies/2008/7/XCLOntology1.5.owl#imageOrientation -->

    <imageInformation rdf:about="#imageOrientation">
        <ID>id316</ID>
        <rdfs:comment xml:lang="en"
            >Orientation of the image e.g., landscape or portrait.</rdfs:comment>
        <is_same_as rdf:resource="#Orientation_NISO"/>
        <is_same_as rdf:resource="#orientation_TIFF"/>
    </imageInformation>
    


    <!-- http://www.semanticweb.org/ontologies/2008/7/XCLOntology1.5.owl#imageReference -->

    <wordProcessingML rdf:about="#imageReference"/>
    


    <!-- http://www.semanticweb.org/ontologies/2008/7/XCLOntology1.5.owl#imageTopPosition -->

    <GIF_Properties rdf:about="#imageTopPosition">
        <rdfs:comment xml:lang="en"
            >position of an image in a gif file</rdfs:comment>
    </GIF_Properties>
    


    <!-- http://www.semanticweb.org/ontologies/2008/7/XCLOntology1.5.owl#imageType -->

    <imageInformation rdf:about="#imageType">
        <ID>id20</ID>
        <rdfs:comment xml:lang="en"
            >Interpretation of image pixels representing the colour type of an image</rdfs:comment>
        <Datatype rdf:resource="#string"/>
    </imageInformation>
    


    <!-- http://www.semanticweb.org/ontologies/2008/7/XCLOntology1.5.owl#imageWidth -->

    <rasterInformation rdf:about="#imageWidth">
        <ID>id30</ID>
        <is_same_as rdf:resource="#ImageWidth_NISO"/>
        <is_same_as rdf:resource="#ImageWidth_tiff"/>
        <is_same_as rdf:resource="#Width_Gif"/>
        <Datatype rdf:resource="#int"/>
    </rasterInformation>
    


    <!-- http://www.semanticweb.org/ontologies/2008/7/XCLOntology1.5.owl#importantColours -->

    <BMP_Properties rdf:about="#importantColours"/>
    


    <!-- http://www.semanticweb.org/ontologies/2008/7/XCLOntology1.5.owl#imprint -->

    <wordProcessingML rdf:about="#imprint">
        <rdfs:comment
            >(Imprinting)
This element specifies that the contents of this run should be displayed as if imprinted, which makes text appear to be imprinted or pressed into page (also referred to as &#39;engrave&#39;).
This formatting property is a toggle property, which specifies that its behavior differs between its use within a style definition and its use as direct formatting. When used as part of a style definition, setting this property shall toggle the current state of that property as specified up to this point in the hierarchy (i.e. applied to not applied, and vice versa). Setting it to false (or an equivalent) shall result in the current setting remaining unchanged. However, when used as direct formatting, setting this property to true or false shall set the absolute state of the resulting property.  
If this element is not present, the default value is to leave the formatting applied at previous level in the style hierarchy. If this element is never applied in the style hierarchy, then imprinting shall not be applied to the contents of this run. 
This element shall not be present with either the emboss (&#167;2.3.2.11) or outline (&#167;2.3.2.21) properties on the same run, since they are mutually exclusive in terms of appearance. 
Example: Consider a run of text which shall have the imprint property explicitly turned on for the contents of the run. This constraint is specified using the following WordprocessingML: 
&lt;w:rPr&gt; 
  &lt;w:imprint w:val=&quot;true&quot;/&gt; 
&lt;/w:rPr&gt; 
This run explicitly declares that the imprint property is true, so the contents of this run will appear imprinted.
[cit. OOXML spec.]</rdfs:comment>
        <Datatype rdf:resource="#bool"/>
    </wordProcessingML>
    


    <!-- http://www.semanticweb.org/ontologies/2008/7/XCLOntology1.5.owl#ind -->

    <wordProcessingML rdf:about="#ind">
        <rdfs:comment xml:lang="en"
            >Paragraph Indentation
This element specifies the set of indentation properties applied to the current paragraph. Indentation settings are overriden on an individual basis - if any single attribute on this element is omitted on a given paragraph, its value is determined by the setting previously set at any level of the style hierarchy (i.e. that previous setting remains unchanged). If any single attribute on this element is never specified in the style hierarchy, then no indentation of that type is applied to the paragraph. 
[Example: Consider a paragraph which should have a one inch indentation from the text margins on both the left and the right sides, except for the first line in each paragraph, which should only be indented one quarter of an inch from the text margin (on the side which begins the flow of text for this paragraph). This set of indentations is specified using the following WordprocessingML: 
&lt;w:pPr&gt; 
  &lt;w:ind w:left=&quot;1440&quot; w:right=&quot;1440&quot; w:hanging=&quot;1080&quot; /&gt;  
&lt;/w:pPr&gt; 
Explanation: This set of indentations specifies that the first line should be indented 1440 twentieths of a point (one inch) from the indentation specified for all remaining paragraphs, which is the 1440 twentieths of a point, as specified by the left attribute. This gives the first line a two inch indentation from the text margin. end example] 
[cit. OOXML spec.]</rdfs:comment>
        <Datatype rdf:resource="#int"/>
    </wordProcessingML>
    


    <!-- http://www.semanticweb.org/ontologies/2008/7/XCLOntology1.5.owl#int -->

    <xcl_propertyDatatypes rdf:about="#int"/>
    


    <!-- http://www.semanticweb.org/ontologies/2008/7/XCLOntology1.5.owl#int16 -->

    <xcl_propertyDatatypes rdf:about="#int16"/>
    


    <!-- http://www.semanticweb.org/ontologies/2008/7/XCLOntology1.5.owl#int32 -->

    <xcl_propertyDatatypes rdf:about="#int32"/>
    


    <!-- http://www.semanticweb.org/ontologies/2008/7/XCLOntology1.5.owl#int64 -->

    <xcl_propertyDatatypes rdf:about="#int64"/>
    


    <!-- http://www.semanticweb.org/ontologies/2008/7/XCLOntology1.5.owl#int8 -->

    <xcl_propertyDatatypes rdf:about="#int8"/>
    


    <!-- http://www.semanticweb.org/ontologies/2008/7/XCLOntology1.5.owl#interlace -->

    <rasterInformation rdf:about="#interlace">
        <rdfs:comment
            >algorithm for encoding raster image data in multiple layers with the purpose of improved transmission and image built up [Compatibility: PNG 1.1]</rdfs:comment>
        <ID>id45</ID>
        <is_same_as rdf:resource="#Interlace_1"/>
        <Datatype rdf:resource="#int"/>
    </rasterInformation>
    


    <!-- http://www.semanticweb.org/ontologies/2008/7/XCLOntology1.5.owl#iso8859_1 -->

    <textInformation rdf:about="#iso8859_1">
        <rdfs:comment
            >westeuropean (iso)</rdfs:comment>
        <ID>id296</ID>
    </textInformation>
    


    <!-- http://www.semanticweb.org/ontologies/2008/7/XCLOntology1.5.owl#iso8859_15 -->

    <textInformation rdf:about="#iso8859_15">
        <ID>id288</ID>
        <rdfs:comment>latin 9 iso</rdfs:comment>
    </textInformation>
    


    <!-- http://www.semanticweb.org/ontologies/2008/7/XCLOntology1.5.owl#iso8859_2 -->

    <textInformation rdf:about="#iso8859_2">
        <ID>id291</ID>
        <rdfs:comment
            >centraleuropean iso</rdfs:comment>
    </textInformation>
    


    <!-- http://www.semanticweb.org/ontologies/2008/7/XCLOntology1.5.owl#iso8859_3 -->

    <textInformation rdf:about="#iso8859_3">
        <rdfs:comment>latin3 iso</rdfs:comment>
        <ID>id289</ID>
    </textInformation>
    


    <!-- http://www.semanticweb.org/ontologies/2008/7/XCLOntology1.5.owl#iso8859_4 -->

    <textInformation rdf:about="#iso8859_4">
        <ID>id290</ID>
        <rdfs:comment>baltic iso</rdfs:comment>
    </textInformation>
    


    <!-- http://www.semanticweb.org/ontologies/2008/7/XCLOntology1.5.owl#iso8859_5 -->

    <textInformation rdf:about="#iso8859_5">
        <rdfs:comment>cyrillic iso</rdfs:comment>
        <ID>id293</ID>
    </textInformation>
    


    <!-- http://www.semanticweb.org/ontologies/2008/7/XCLOntology1.5.owl#iso8859_6 -->

    <textInformation rdf:about="#iso8859_6">
        <rdfs:comment>arrabic iso</rdfs:comment>
        <ID>id292</ID>
    </textInformation>
    


    <!-- http://www.semanticweb.org/ontologies/2008/7/XCLOntology1.5.owl#iso8859_7 -->

    <textInformation rdf:about="#iso8859_7">
        <rdfs:comment>greek iso</rdfs:comment>
        <ID>id294</ID>
    </textInformation>
    


    <!-- http://www.semanticweb.org/ontologies/2008/7/XCLOntology1.5.owl#iso8859_8 -->

    <textInformation rdf:about="#iso8859_8">
        <rdfs:comment>hebrew iso</rdfs:comment>
        <ID>id295</ID>
    </textInformation>
    


    <!-- http://www.semanticweb.org/ontologies/2008/7/XCLOntology1.5.owl#iso8859_9 -->

    <textInformation rdf:about="#iso8859_9">
        <rdfs:comment>turkish iso</rdfs:comment>
        <ID>id287</ID>
    </textInformation>
    


    <!-- http://www.semanticweb.org/ontologies/2008/7/XCLOntology1.5.owl#isoCoatedV2 -->

    <imageInformation rdf:about="#isoCoatedV2">
        <ID>id236</ID>
    </imageInformation>
    


    <!-- http://www.semanticweb.org/ontologies/2008/7/XCLOntology1.5.owl#isoUncoated -->

    <imageInformation rdf:about="#isoUncoated">
        <ID>id237</ID>
    </imageInformation>
    


    <!-- http://www.semanticweb.org/ontologies/2008/7/XCLOntology1.5.owl#isoWebCoatedECI -->

    <imageInformation rdf:about="#isoWebCoatedECI">
        <ID>id238</ID>
    </imageInformation>
    


    <!-- http://www.semanticweb.org/ontologies/2008/7/XCLOntology1.5.owl#italic -->

    <textInformation rdf:about="#italic">
        <rdfs:comment
            >text-property italic</rdfs:comment>
        <ID>id162</ID>
        <Datatype rdf:resource="#bool"/>
        <is_same_as rdf:resource="#i"/>
    </textInformation>
    


    <!-- http://www.semanticweb.org/ontologies/2008/7/XCLOntology1.5.owl#jc -->

    <wordProcessingML rdf:about="#jc">
        <rdfs:comment xml:lang="en"
            >Paragraph Alignment
This element specifies the paragraph alignment which shall be applied to text in this paragraph. If this element is omitted on a given paragraph, its value is determined by the setting previously set at any level of the style hierarchy (i.e. that previous setting remains unchanged). If this setting is never specified in the style hierarchy, then no alignment is applied to the paragraph. 
[Example: Consider a paragraph which should be right justified to the right page side paragraph extents within a document. This constraint is specified in the following WordprocessingML content: 
&lt;w:pPr&gt; 
  &lt;w:jc w:val=&quot;right&quot; /&gt; 
&lt;/w:pPr&gt; 
Explanation:
Specifies the justification which should be applied to the parent object within a document. 
The possible values (see below) for this attribute are always specified relative to the page, and do not change semantic from right-to-left and left-to-right documents. 
[Example: Consider the following WordprocessingML fragment for a paragraph in a document: 
&lt;w:pPr&gt; 
  &lt;w:jc w:val=&quot;right&quot; /&gt; 
&lt;/w:pPr&gt; 
This paragraph is now right justified on the page, regardless of the paragraph or section setting. The possible values for this attribute are defined by the ST_Jc simple type.
[cit. OOXML spec.]</rdfs:comment>
    </wordProcessingML>
    


    <!-- http://www.semanticweb.org/ontologies/2008/7/XCLOntology1.5.owl#justifyAdjustment -->

    <textInformation rdf:about="#justifyAdjustment">
        <ID>id272</ID>
        <Datatype rdf:resource="#bool"/>
    </textInformation>
    


    <!-- http://www.semanticweb.org/ontologies/2008/7/XCLOntology1.5.owl#keepLines -->

    <wordProcessingML rdf:about="#keepLines">
        <rdfs:comment xml:lang="en"
            >Keep All Lines On One Page
This element specifies that when rendering this document in a page view, all lines for this page are maintained on a single page whenever possible. 
This means that if the contents of the current paragraph would normally span across two pages due to the placement of the paragraph&#39;s text, all lines in this paragraph shall be moved onto the next page to ensure they are displayed together. If this is not possible because all lines in the paragraph would exceed a single page in any case, then lines in this paragraph shall start on a new page, with page breaks as needed afterwards. If this element is omitted on a given paragraph, its value is determined by the setting previously set at any level of the style hierarchy (i.e. that previous setting remains unchanged). If this setting is never specified in the style hierarchy, then this property shall not be applied. 
[Example: Consider a WordprocessingML document in which a code fragment (such as the schema fragments in this document) are defined such that they should never be broken across a page boundary in order to improve readability. This constraint would be specified using the following paragraph properties in WordprocessingML: 
&lt;w:pPr&gt; 
  &lt;w:keepLines /&gt; 
  ... 
&lt;/w:pPr&gt;17 
Values: on/off
[cit. OOXML Spec.]</rdfs:comment>
        <Datatype rdf:resource="#bool"/>
    </wordProcessingML>
    


    <!-- http://www.semanticweb.org/ontologies/2008/7/XCLOntology1.5.owl#keepNext -->

    <wordProcessingML rdf:about="#keepNext">
        <rdfs:comment xml:lang="en"
            >Keep Paragraph With Next Paragraph
This element specifies that when rendering this document in a paginated view, the contents of this paragraph are at least partly rendered on the same page as the following paragraph whenever possible. 
This means that if the contents of the current paragraph would normally be completely rendered on a different page than the following paragraph (because only one of the two paragraphs would fit on the remaining space on the first page), then both paragraphs shall be rendered on a single page. This property can be chained between multiple paragraphs to ensure that all paragraphs are rendered on a single page without any intervening page boundaries. If this is not possible the entire set of paragraphs that are grouped together using this property would exceed a single page in any case, then the set of &quot;keep with next&quot; paragraphs shall start on a new page, with page breaks as needed afterwards. 
If this element is omitted on a given paragraph, its value is determined by the setting previously set at any level of the style hierarchy (i.e. that previous setting remains unchanged). If this setting is never specified in the style hierarchy, then this property shall not be applied. 
Values: on/off
[cit. OOXML Spec.]</rdfs:comment>
        <Datatype rdf:resource="#bool"/>
    </wordProcessingML>
    


    <!-- http://www.semanticweb.org/ontologies/2008/7/XCLOntology1.5.owl#kern -->

    <wordProcessingML rdf:about="#kern">
        <rdfs:comment xml:lang="en"
            >Font Kerning 
This element specifies whether font kerning shall be applied to the contents of this run. If it is specified, then kerning shall be automatically adjusted when displaying characters in this run as needed. 
The val attribute specifies the smallest font size which shall have its kerning automatically adjusted if this setting is specified. If the font size in the sz element (&#167;2.3.2.36) is smaller than this value, then no font kerning shall be performed. 
If this element is not present, the default value is to leave the formatting applied at previous level in the style hierarchy. If this element is never applied in the style hierarchy, then font kerning shall not be applied to the contents of this run. 
Example: Consider the following WordprocessingML run which has font kerning properties specified: 
&lt;w:r&gt; 
  &lt;w:rPr&gt; 
   &lt;w:sz w:val=&quot;22&quot; /&gt; 
    &lt;w:kern w:val=&quot;28&quot; /&gt; 
  &lt;/w:rPr&gt; 
&lt;/w:r&gt; 
Even though font kerning is turned on via the kern element, the contents of this run shall not be kerned because that settings only applied to font sizes of 14 points (28 half-points) or larger. If the kern element&#39;s val attribute was less than or equal to the sz element&#39;s val attribute, then kerning would be applied:  
&lt;w:r&gt; 
  &lt;w:rPr&gt; 
    &lt;w:sz w:val=&quot;22&quot; /&gt; 
    &lt;w:kern w:val=&quot;22&quot; /&gt; 
  &lt;/w:rPr&gt; 
&lt;/w:r&gt;
[cit. OOXML spec.]</rdfs:comment>
        <Datatype rdf:resource="#int"/>
    </wordProcessingML>
    


    <!-- http://www.semanticweb.org/ontologies/2008/7/XCLOntology1.5.owl#kinsoku -->

    <wordProcessingML rdf:about="#kinsoku">
        <rdfs:comment xml:lang="en"
            >Use East Asian Typography Rules for First and Last Character per Line
This element specifies whether East Asian typography and line-breaking rules shall be applied to text in this paragraph to determine which characters may begin and end each line. This property only applies to Chinese PRC, Chinese Taiwan, and Japanese text in this paragraph.  
If this element is omitted on a given paragraph, its value is determined by the setting previously set at any level of the style hierarchy (i.e. that previous setting remains unchanged). If this setting is never specified in the style hierarchy, then this property shall be applied to Chinese PRC, Chinese Taiwan, and Japanese text in this paragraph. [cit. OOXMl Spec.]</rdfs:comment>
        <Datatype rdf:resource="#bool"/>
    </wordProcessingML>
    


    <!-- http://www.semanticweb.org/ontologies/2008/7/XCLOntology1.5.owl#lang_ooxml -->

    <wordProcessingML rdf:about="#lang_ooxml">
        <rdfs:comment
            >Languages for Run Content
This element specifies the languages which shall be used to check spelling and grammar (if requested) when processing the contents of this run.  
If this element is not present, the default value is to leave the formatting applied at previous level in the style hierarchy. If this element is never applied in the style hierarchy, then the languages for the contents of this run shall be automatically determined based on their contents using any method desired. 
Example: Consider a run which contains both Latin and complex script characters in its contents. If those contents should be interpreted as French (Canada) and Hebrew, respectively, that requirement would be specified as follows in the resulting WordprocessingML: 
&lt;w:r&gt; 
  &lt;w:rPr&gt;
    &lt;w:lang w:val=&quot;fr-CA&quot; w:bidi=&quot;he-IL&quot; /&gt; 
  &lt;/w:rPr&gt; 
&lt;/w:r&gt; 
The resulting run specifies that any complex script contents shall be spell and grammar checked as if they were Hebrew, and any Latin character contents shall be spell and grammar checked as if they were French (Canada).
[cit. OOXML spec.]</rdfs:comment>
        <is_same_as rdf:resource="#documentLanguage"/>
        <Datatype rdf:resource="#string"/>
    </wordProcessingML>
    


    <!-- http://www.semanticweb.org/ontologies/2008/7/XCLOntology1.5.owl#lastChar -->

    <fontDescriptor rdf:about="#lastChar"/>
    


    <!-- http://www.semanticweb.org/ontologies/2008/7/XCLOntology1.5.owl#lastModifiedBy -->

    <generalInformation rdf:about="#lastModifiedBy">
        <ID>id188</ID>
        <rdfs:comment xml:lang="en"
            >name of the person/user who modified the file last</rdfs:comment>
        <Datatype rdf:resource="#string"/>
    </generalInformation>
    


    <!-- http://www.semanticweb.org/ontologies/2008/7/XCLOntology1.5.owl#leading -->

    <PDF1.3_Properties rdf:about="#leading">
        <rdfs:comment
            >Set the text leading, T l, to leading, which is a number expressed in unscaled text space units. Text leading is used only by the T*, &#39;, and &quot; operators. Default value: 0. 
[cit. Pdf 1.3]</rdfs:comment>
        <Datatype rdf:resource="#int"/>
    </PDF1.3_Properties>
    


    <!-- http://www.semanticweb.org/ontologies/2008/7/XCLOntology1.5.owl#left -->

    <wordProcessingML rdf:about="#left">
        <rdfs:comment xml:lang="en"
            >Left Paragraph Border
This element specifies the border which shall be displayed on the left side of the page around the specified paragraph. 
To determine if any two adjoining paragraphs should have a left border which spans the full line height or not, the left border shall be drawn between the top border or between border at the top (whichever would be rendered for the current paragraph), and the bottom border or between border at the bottom (whichever would be rendered for the current paragraph). 
If this element is omitted on a given paragraph, its value is determined by the setting previously set at any level of the style hierarchy (i.e. that previous setting remains unchanged). If this setting is never specified in the style hierarchy, then no left border shall be applied.
[cit. OOXML Spec.]</rdfs:comment>
        <Datatype rdf:resource="#bool"/>
    </wordProcessingML>
    


    <!-- http://www.semanticweb.org/ontologies/2008/7/XCLOntology1.5.owl#leftAdjustment -->

    <textInformation rdf:about="#leftAdjustment">
        <ID>id270</ID>
        <Datatype rdf:resource="#bool"/>
    </textInformation>
    


    <!-- http://www.semanticweb.org/ontologies/2008/7/XCLOntology1.5.owl#lineBreak -->

    <textInformation rdf:about="#lineBreak">
        <ID>id183</ID>
        <rdfs:comment
            >Content-property describing if a string content breaks to a new line</rdfs:comment>
        <Datatype rdf:resource="#bool"/>
    </textInformation>
    


    <!-- http://www.semanticweb.org/ontologies/2008/7/XCLOntology1.5.owl#lineColour -->

    <vectorInformation rdf:about="#lineColour">
        <ID>id244</ID>
        <rdfs:comment
            >Colour of a line-/path-object</rdfs:comment>
        <Datatype rdf:resource="#int"/>
    </vectorInformation>
    


    <!-- http://www.semanticweb.org/ontologies/2008/7/XCLOntology1.5.owl#lineJoin -->

    <PDF1.3_Properties rdf:about="#lineJoin">
        <rdfs:comment
            >A code specifying the shape of joints between connected segments of a stroked path (see &#8220;Line Join Style&#8221; on page 140). 
Initial value: 0, for mitered joins. 
[cit. Pdf 1.3]</rdfs:comment>
        <Datatype rdf:resource="#int"/>
    </PDF1.3_Properties>
    


    <!-- http://www.semanticweb.org/ontologies/2008/7/XCLOntology1.5.owl#lineJoinBevel -->

    <vectorInformation rdf:about="#lineJoinBevel">
        <ID>id319</ID>
        <is_same_as rdf:resource="#LineJoinStyle3"/>
        <Datatype rdf:resource="#int"/>
    </vectorInformation>
    


    <!-- http://www.semanticweb.org/ontologies/2008/7/XCLOntology1.5.owl#lineJoinMiter -->

    <vectorInformation rdf:about="#lineJoinMiter">
        <ID>id318</ID>
        <is_same_as rdf:resource="#LineJoinStyle1"/>
        <Datatype rdf:resource="#int"/>
    </vectorInformation>
    


    <!-- http://www.semanticweb.org/ontologies/2008/7/XCLOntology1.5.owl#lineJoinRound -->

    <vectorInformation rdf:about="#lineJoinRound">
        <ID>id251</ID>
        <is_same_as rdf:resource="#LineJoinStyle2"/>
        <Datatype rdf:resource="#int"/>
    </vectorInformation>
    


    <!-- http://www.semanticweb.org/ontologies/2008/7/XCLOntology1.5.owl#lineSpacing -->

    <textInformation rdf:about="#lineSpacing">
        <rdfs:comment
            >Space between lines in textdocument.</rdfs:comment>
        <ID>id192</ID>
        <Datatype rdf:resource="#uint32Rational"/>
    </textInformation>
    


    <!-- http://www.semanticweb.org/ontologies/2008/7/XCLOntology1.5.owl#lineStyle -->

    <vectorInformation rdf:about="#lineStyle">
        <ID>id252</ID>
        <rdfs:comment
            >style of vectorLine (dashed, dotted etc...)</rdfs:comment>
        <Datatype rdf:resource="#string"/>
    </vectorInformation>
    


    <!-- http://www.semanticweb.org/ontologies/2008/7/XCLOntology1.5.owl#lineWidth -->

    <vectorInformation rdf:about="#lineWidth">
        <ID>id253</ID>
        <rdfs:comment
            >Length of a line/path in a vector-object</rdfs:comment>
        <is_same_as rdf:resource="#lineWidth_Pdf"/>
        <Datatype rdf:resource="#uint32Rational"/>
    </vectorInformation>
    


    <!-- http://www.semanticweb.org/ontologies/2008/7/XCLOntology1.5.owl#lineWidth_Pdf -->

    <PDF1.3_Properties rdf:about="#lineWidth_Pdf">
        <rdfs:comment
            >The thickness, in user space units, of paths to be stroked (see &#8220;Line 
Width&#8221; on page 139). Initial value: 1.0. [cit. Pdf 1.3]</rdfs:comment>
        <is_same_as rdf:resource="#lineWidth"/>
    </PDF1.3_Properties>
    


    <!-- http://www.semanticweb.org/ontologies/2008/7/XCLOntology1.5.owl#linearPath -->

    <vectorInformation rdf:about="#linearPath">
        <ID>id256</ID>
        <rdfs:comment xml:lang="en"
            >defines a vectorline between two markerPositions (in Opposition to B&#233;zier-Curves it is linear)</rdfs:comment>
        <Datatype rdf:resource="#int"/>
    </vectorInformation>
    


    <!-- http://www.semanticweb.org/ontologies/2008/7/XCLOntology1.5.owl#listPr -->

    <wordProcessingML rdf:about="#listPr">
        <rdfs:comment xml:lang="en"
            >indicates that a paragraph is marked as a list</rdfs:comment>
    </wordProcessingML>
    


    <!-- http://www.semanticweb.org/ontologies/2008/7/XCLOntology1.5.owl#littleEndian -->

    <generalInformation rdf:about="#littleEndian">
        <ID>id225</ID>
        <rdfs:comment xml:lang="en"
            >The Kind of Byte-Order</rdfs:comment>
        <is_same_as rdf:resource="#littleEndian_NISO"/>
    </generalInformation>
    


    <!-- http://www.semanticweb.org/ontologies/2008/7/XCLOntology1.5.owl#littleEndian_NISO -->

    <NISO rdf:about="#littleEndian_NISO">
        <Unit rdf:resource="#NULL"/>
        <is_same_as rdf:resource="#littleEndian"/>
    </NISO>
    


    <!-- http://www.semanticweb.org/ontologies/2008/7/XCLOntology1.5.owl#logicalScreenBackroundColour -->

    <GIF_Properties rdf:about="#logicalScreenBackroundColour"/>
    


    <!-- http://www.semanticweb.org/ontologies/2008/7/XCLOntology1.5.owl#logicalScreenHeight -->

    <GIF_Properties rdf:about="#logicalScreenHeight">
        <rdfs:comment xml:lang="en"
            >Size of area in which the picture or pictures are displayed (it can be bigger than the size of the classical image).</rdfs:comment>
    </GIF_Properties>
    


    <!-- http://www.semanticweb.org/ontologies/2008/7/XCLOntology1.5.owl#logicalScreenWidth -->

    <GIF_Properties rdf:about="#logicalScreenWidth">
        <rdfs:comment xml:lang="en"
            >Size of area in which the picture or pictureS are displayed (it can be bigger than the size of the classical image).</rdfs:comment>
    </GIF_Properties>
    


    <!-- http://www.semanticweb.org/ontologies/2008/7/XCLOntology1.5.owl#lookup -->

    <PDF1.3_Properties rdf:about="#lookup">
        <rdfs:comment
            >dictionary entry for lookup-tables in PDF.
The Entry looks like this: &lt;000000 FF0000 00FF000000FF B57342 &#8230;&gt;</rdfs:comment>
        <is_same_as rdf:resource="#Backgroundcolour_Gif"/>
        <is_same_as rdf:resource="#backgroundColour_PNG"/>
        <Datatype rdf:resource="#int"/>
    </PDF1.3_Properties>
    


    <!-- http://www.semanticweb.org/ontologies/2008/7/XCLOntology1.5.owl#macOsEncoding -->

    <textInformation rdf:about="#macOsEncoding">
        <ID>id286</ID>
        <rdfs:comment
            >encodingType for MacOs Operationsystem</rdfs:comment>
        <owl:sameAs rdf:resource="#MacRomanEncoding"/>
        <Datatype rdf:resource="#bool"/>
    </textInformation>
    


    <!-- http://www.semanticweb.org/ontologies/2008/7/XCLOntology1.5.owl#mandatory -->

    <property_restriction rdf:about="#mandatory"/>
    


    <!-- http://www.semanticweb.org/ontologies/2008/7/XCLOntology1.5.owl#marginBottom -->

    <textInformation rdf:about="#marginBottom">
        <rdfs:comment xml:lang="en"
            >distance between text and margin in a formatted text-document</rdfs:comment>
        <Datatype rdf:resource="#int"/>
    </textInformation>
    


    <!-- http://www.semanticweb.org/ontologies/2008/7/XCLOntology1.5.owl#marginLeft -->

    <textInformation rdf:about="#marginLeft">
        <rdfs:comment xml:lang="en"
            >distance between text and margin in a formatted text-document</rdfs:comment>
        <ID>id262</ID>
        <Datatype rdf:resource="#int"/>
    </textInformation>
    


    <!-- http://www.semanticweb.org/ontologies/2008/7/XCLOntology1.5.owl#marginRight -->

    <textInformation rdf:about="#marginRight">
        <rdfs:comment xml:lang="en"
            >distance between text and margin in a formatted text-document</rdfs:comment>
        <ID>id263</ID>
        <Datatype rdf:resource="#int"/>
    </textInformation>
    


    <!-- http://www.semanticweb.org/ontologies/2008/7/XCLOntology1.5.owl#marginTop -->

    <textInformation rdf:about="#marginTop">
        <rdfs:comment xml:lang="en"
            >distance between text and margin in a formatted text-document</rdfs:comment>
        <ID>id261</ID>
        <Datatype rdf:resource="#int"/>
    </textInformation>
    


    <!-- http://www.semanticweb.org/ontologies/2008/7/XCLOntology1.5.owl#markerPosition -->

    <vectorInformation rdf:about="#markerPosition">
        <rdfs:comment xml:lang="en"
            >Position of a point in  vector-file. Is defined by it x- and y-achsis distance</rdfs:comment>
        <ID>id254</ID>
        <Datatype rdf:resource="#int"/>
    </vectorInformation>
    


    <!-- http://www.semanticweb.org/ontologies/2008/7/XCLOntology1.5.owl#matrix -->

    <xcl_propertyDatatypes rdf:about="#matrix"/>
    


    <!-- http://www.semanticweb.org/ontologies/2008/7/XCLOntology1.5.owl#maxSampleValue -->

    <Tiff_Properties rdf:about="#maxSampleValue">
        <rdfs:comment
            >The maximum component value used [cit. TIFF 6.0] [Compatibility: TIFF 6.0]</rdfs:comment>
        <Datatype rdf:resource="#int"/>
    </Tiff_Properties>
    


    <!-- http://www.semanticweb.org/ontologies/2008/7/XCLOntology1.5.owl#mediabox -->

    <PDF1.3_Properties rdf:about="#mediabox">
        <rdfs:comment
            >(Required; inheritable) A rectangle (example: [0 0 612 792]), expressed in default user space units, de&#64257;ning the maximum imageable area of the physical medium on which the page is to be printed (see 
Section 8.6.1, &#8220;Page Boundaries&#8221;).[cit. Pdf 1.3]</rdfs:comment>
        <Datatype rdf:resource="#floatArray"/>
    </PDF1.3_Properties>
    


    <!-- http://www.semanticweb.org/ontologies/2008/7/XCLOntology1.5.owl#mimeType -->

    <generalInformation rdf:about="#mimeType">
        <is_same_as rdf:resource="#mimeType_NISO"/>
        <Datatype rdf:resource="#string"/>
    </generalInformation>
    


    <!-- http://www.semanticweb.org/ontologies/2008/7/XCLOntology1.5.owl#mimeType_NISO -->

    <NISO rdf:about="#mimeType_NISO">
        <is_same_as rdf:resource="#mimeType"/>
        <Datatype rdf:resource="#string"/>
    </NISO>
    


    <!-- http://www.semanticweb.org/ontologies/2008/7/XCLOntology1.5.owl#minSampleValue -->

    <Tiff_Properties rdf:about="#minSampleValue">
        <rdfs:comment
            >The minimum component value used [cit. TIFF 6.0] [Compatibility: TIFF 6.0]</rdfs:comment>
        <Datatype rdf:resource="#int"/>
    </Tiff_Properties>
    


    <!-- http://www.semanticweb.org/ontologies/2008/7/XCLOntology1.5.owl#mirrorIndents -->

    <wordProcessingML rdf:about="#mirrorIndents">
        <rdfs:comment xml:lang="en"
            >Use Left/Right Indents as Inside/Outside Indents
This element specifies whether the paragraph indents should be interpreted as mirrored indents. When this element is present, the left indent shall become the inside indent and the right indent shall become the outside indent. 
If the mirrorIndents property is specified for this paragraph, then the inside page edge is the right page edge odd numbered pages and the left page edge for even numbered pages. Conversely, the outside page edge is the left page edge for odd numbered pages and the right page edge for even numbered pages. 
If this element is omitted on a given paragraph, its value is determined by the setting previously set at any level of the style hierarchy (i.e. that previous setting remains unchanged). If this setting is never specified in the style hierarchy, then this property shall not be applied. 
[cit. OOXML Spec.]</rdfs:comment>
        <Datatype rdf:resource="#bool"/>
    </wordProcessingML>
    


    <!-- http://www.semanticweb.org/ontologies/2008/7/XCLOntology1.5.owl#mp3_Codec -->

    <audioInformation rdf:about="#mp3_Codec">
        <rdfs:comment xml:lang="en"
            >Audio CompressionAlgorithm, equals MPEG1 Layer3</rdfs:comment>
    </audioInformation>
    


    <!-- http://www.semanticweb.org/ontologies/2008/7/XCLOntology1.5.owl#newSubfileType -->

    <Tiff_Properties rdf:about="#newSubfileType">
        <rdfs:comment
            >A general indication of the kind of data contained in this subfile. 
Tag = 254  (FE.H) 
Type = LONG 
N = 1 
Replaces the old SubfileType field, due to limitations in the definition of that field. NewSubfileType is mainly useful when there are multiple subfiles in a single TIFF file. 
This field is made up of a set of 32 flag bits. Unused bits are expected to be 0. Bit 0 is the low-order bit. 
Currently defined values are: 
Bit 0 is 1 if the image is a reduced-resolution version of another image in this TIFF file; else the bit is 0. 
Bit 1 is 1 if the image is a single page of a multi-page image (see the PageNumber field description); else the bit is 0. 
Bit 2 is 1 if the image defines a transparency mask for another image in this TIFF file. The PhotometricInterpretation value must be 4, designating a transparency mask. These values are defined as bit flags because they are independent of each other. Default is 0.</rdfs:comment>
        <Datatype rdf:resource="#int"/>
    </Tiff_Properties>
    


    <!-- http://www.semanticweb.org/ontologies/2008/7/XCLOntology1.5.owl#noProof -->

    <wordProcessingML rdf:about="#noProof">
        <rdfs:comment
            >noProof (Do Not Check Spelling or Grammar)
This element specifies that the contents of this run shall not report any errors when the document is scanned for spelling and grammar. [Note: It is entirely at the consumer&#39;s/producer&#39;s discretion whether this is done by not checking the region for spelling and grammar, or simply by suppressing the results. end note] 
If this element is not present, the default value is to leave the formatting applied at previous level in the style hierarchy. If this element is never applied in the style hierarchy, then spelling and grammar error shall not be suppressed on the contents of this run. 
Example: Consider a run of text which shall not ever have spelling or grammar errors reported for the contents of the run, for example, the XML fragments included in this Specification. This constraint is specified using the following WordprocessingML: 
&lt;w:rPr&gt; 
  &lt;w:noProof w:val=&quot;true&quot;/&gt; 
&lt;/w:rPr&gt; 
This run explicitly declares that the noProof property is true, so the contents of this run will never report spelling or grammar errors. 
[cit. OOXML spec.]</rdfs:comment>
        <Datatype rdf:resource="#bool"/>
    </wordProcessingML>
    


    <!-- http://www.semanticweb.org/ontologies/2008/7/XCLOntology1.5.owl#normData -->

    <generalInformation rdf:about="#normData">
        <ID>id7</ID>
        <Unit rdf:resource="#NULL"/>
        <Datatype rdf:resource="#string"/>
    </generalInformation>
    


    <!-- http://www.semanticweb.org/ontologies/2008/7/XCLOntology1.5.owl#normDataOffset -->

    <Tiff_Properties rdf:about="#normDataOffset">
        <rdfs:comment xml:lang="en"
            >A general indication of the kind of data contained in this subfile [cit. TIFF 6.0] [Compatibility: TIFF 6.0]</rdfs:comment>
        <is_same_as rdf:resource="#normData"/>
    </Tiff_Properties>
    


    <!-- http://www.semanticweb.org/ontologies/2008/7/XCLOntology1.5.owl#numPr -->

    <wordProcessingML rdf:about="#numPr">
        <rdfs:comment xml:lang="en"
            >Numbering Definition Instance Reference
This element specifies that the current paragraph references a numbering definition instance in the current document. 
The presence of this element specifies that the paragraph will inherit the properties specified by the numbering definition in the num element (&#167;2.9.16) at the level specified by the level specified in the lvl element (&#167;2.9.7) and shall have an associated number positioned before the beginning of the text flow in this paragraph. When this element appears as part of the paragraph formatting for a paragraph style, then any numbering level defined using the ilvl element shall be ignored, and the pStyle element (&#167;2.9.25) on the associated abstract numbering definition shall be used instead. 
[cit. OOXML Spec.]</rdfs:comment>
        <Datatype rdf:resource="#bool"/>
    </wordProcessingML>
    


    <!-- http://www.semanticweb.org/ontologies/2008/7/XCLOntology1.5.owl#numberOfAudioChannels -->

    <audioInformation rdf:about="#numberOfAudioChannels">
        <rdfs:comment
            >2=stereo, 1=mono...</rdfs:comment>
        <ID>id208</ID>
        <Datatype rdf:resource="#int"/>
    </audioInformation>
    


    <!-- http://www.semanticweb.org/ontologies/2008/7/XCLOntology1.5.owl#numberOfCharacters -->

    <textInformation rdf:about="#numberOfCharacters">
        <ID>id189</ID>
        <rdfs:comment xml:lang="en"
            >defines the number of characters</rdfs:comment>
        <Datatype rdf:resource="#int"/>
    </textInformation>
    


    <!-- http://www.semanticweb.org/ontologies/2008/7/XCLOntology1.5.owl#numberOfInks -->

    <imageInformation rdf:about="#numberOfInks">
        <ID>id197</ID>
        <rdfs:comment xml:lang="en"
            >numberOfInks (=number of Channels). SHould be only interesting if bitDepth/ColourSpace is different than the usual ones...</rdfs:comment>
        <is_same_as rdf:resource="#N"/>
        <Datatype rdf:resource="#int"/>
        <is_same_as rdf:resource="#numberOfInks_Tiff"/>
        <is_same_as rdf:resource="#samplesPerPixel"/>
    </imageInformation>
    


    <!-- http://www.semanticweb.org/ontologies/2008/7/XCLOntology1.5.owl#numberOfInks_Tiff -->

    <Tiff_Properties rdf:about="#numberOfInks_Tiff">
        <rdfs:comment
            >The number of inks.
Usually equal to SamplesPerPixel, unless there are extra samples. [cit. Tiff]</rdfs:comment>
        <Datatype rdf:resource="#int"/>
        <is_same_as rdf:resource="#numberOfInks"/>
        <is_same_as rdf:resource="#samplesPerPixel"/>
        <is_same_as rdf:resource="#samplesPerPixelTIff"/>
    </Tiff_Properties>
    


    <!-- http://www.semanticweb.org/ontologies/2008/7/XCLOntology1.5.owl#numberOfPages -->

    <textInformation rdf:about="#numberOfPages">
        <ID>id84</ID>
        <rdfs:comment xml:lang="en">number of Pages</rdfs:comment>
        <Datatype rdf:resource="#int"/>
    </textInformation>
    


    <!-- http://www.semanticweb.org/ontologies/2008/7/XCLOntology1.5.owl#oMath -->

    <wordProcessingML rdf:about="#oMath">
        <rdfs:comment
            >oMath (Office Open XML Math)
This element specifies that this run contains WordprocessingML which shall be handled as though it was Office Open XML Math. 
Rationale: Like other run properties may be applied to the glyph representing the paragraph mark, it is possible to create an Office Open XML Math equation on an empty paragraph as well. Since that paragraph mark must be defined by WordprocessingML, it is not possible to store the paragraph using the Office Open XML Math markup. Instead, this run property is stored on the paragraph mark&#39;s run properties to indicate that the paragraph mark is part of an Office Open XML Math equation. 
If this element is not present, the default value is to leave the formatting applied at previous level in the style hierarchy. If this element is never applied in the style hierarchy, then this run shall not be treated as Office Open XML Math. 
This property may be applied to any run, but that should only introduce the semantic that the run is math in the user interface, and shall not change the appearance of the text. 
XML Math syntax, and must be written out as a property on the actual run as follows: 
&lt;w:pPr&gt; 
  &lt;w:rPr&gt; 
    &lt;w:oMath /&gt; 
  &lt;/w:rPr&gt; 
&lt;/w:pPr&gt; 
[cit. OOXML spec.]</rdfs:comment>
        <Datatype rdf:resource="#bool"/>
    </wordProcessingML>
    


    <!-- http://www.semanticweb.org/ontologies/2008/7/XCLOntology1.5.owl#opacity -->

    <vectorInformation rdf:about="#opacity">
        <rdfs:comment
            >defines the value of opacity in a vector-object (default is 100%)</rdfs:comment>
        <ID>id245</ID>
        <Datatype rdf:resource="#int"/>
    </vectorInformation>
    


    <!-- http://www.semanticweb.org/ontologies/2008/7/XCLOntology1.5.owl#openTypeFont -->

    <textInformation rdf:about="#openTypeFont">
        <ID>id221</ID>
    </textInformation>
    


    <!-- http://www.semanticweb.org/ontologies/2008/7/XCLOntology1.5.owl#orientation_TIFF -->

    <Tiff_Properties rdf:about="#orientation_TIFF">
        <rdfs:comment
            >The orientation of the image with respect to the rows and columns [cit. TIFF 6.0] [Compatibility: TIFF 6.0]</rdfs:comment>
        <is_same_as rdf:resource="#imageOrientation"/>
        <Datatype rdf:resource="#int"/>
    </Tiff_Properties>
    


    <!-- http://www.semanticweb.org/ontologies/2008/7/XCLOntology1.5.owl#outline -->

    <wordProcessingML rdf:about="#outline">
        <rdfs:comment
            >outline (Display Character Outline) 
This element specifies that the contents of this run should be displayed as if they have an outline, by drawing a one pixel wide border around the inside and outside borders of each character glyph in the run.  
This formatting property is a toggle property, which specifies that its behavior differs between its use within a style definition and its use as direct formatting. When used as part of a style definition, setting this property shall toggle the current state of that property as specified up to this point in the hierarchy (i.e. applied to not applied, and vice versa). Setting it to false (or an equivalent) shall result in the current setting remaining unchanged. However, when used as direct formatting, setting this property to true or false shall set the absolute state of the resulting property.
If this element is not present, the default value is to leave the formatting applied at previous level in the style hierarchy. If this element is never applied in the style hierarchy, then outline shall not be applied to the contents of this run. 
This element shall not be present with either the emboss (&#167;2.3.2.11) or imprint (&#167;2.3.2.16) properties on the same run, since they are mutually exclusive in terms of appearance. Example:
&lt;w:rPr&gt; 
  &lt;w:outline w:val=&quot;false&quot;/&gt; 
&lt;/w:rPr&gt;
[cit. OOXML spec.]</rdfs:comment>
        <Datatype rdf:resource="#bool"/>
    </wordProcessingML>
    


    <!-- http://www.semanticweb.org/ontologies/2008/7/XCLOntology1.5.owl#outlineLvl -->

    <wordProcessingML rdf:about="#outlineLvl">
        <rdfs:comment xml:lang="en"
            >Associated Outline Level
This element specifies the outline level which shall be associated with the current paragraph in the document. The outline level specifies an integer which defines the level of the associated text. This level shall not affect the appearance of the text in the document, but shall be used to calculate the TOC field (&#167;2.16.5.75) if the appropriate field switches have been set, and may be used by consumers to provide additional application behavior. 
[cit. OOXML Spec.]</rdfs:comment>
        <Datatype rdf:resource="#int"/>
    </wordProcessingML>
    


    <!-- http://www.semanticweb.org/ontologies/2008/7/XCLOntology1.5.owl#outlinesEntryTitle -->

    <PDF1.3_Properties rdf:about="#outlinesEntryTitle">
        <rdfs:comment xml:lang="en"
            >Title text string (Required) The text to be displayed on the screen for this item. OR: Title text string (Optional; PDF 1.1) The document&#8217;s title.</rdfs:comment>
        <is_same_as rdf:resource="#documentTitle"/>
    </PDF1.3_Properties>
    


    <!-- http://www.semanticweb.org/ontologies/2008/7/XCLOntology1.5.owl#overflowPunct -->

    <wordProcessingML rdf:about="#overflowPunct">
        <rdfs:comment xml:lang="en"
            >Allow Punctuation to Extent Past Text Extents
This element specifies that punctuation characters which appear at the end of text in any line in this paragraph shall be allowed to extend one character past the text extents (indents/margins) as needed in order to ensure that they are not displayed as hanging punctuation. Hanging punctuation is defined as punctuation which appears on a different line than the text which it logically would appear with. Omitting this element sets its value to true. [cit. OOXML Spec]</rdfs:comment>
        <Datatype rdf:resource="#bool"/>
    </wordProcessingML>
    


    <!-- http://www.semanticweb.org/ontologies/2008/7/XCLOntology1.5.owl#overprintMode_pdf -->

    <PDF1.3_Properties rdf:about="#overprintMode_pdf">
        <rdfs:comment
            >(PDF 1.3) A code specifying whether a color component value of 0 in a DeviceCMYK color space should erase that component (0) or leave it unchanged (1) when overprinting (see Section 4.5.6, &#8220;Overprint Control&#8221;). Initial value: 0. [cit. Pdf 1.3]</rdfs:comment>
        <Datatype rdf:resource="#int"/>
    </PDF1.3_Properties>
    


    <!-- http://www.semanticweb.org/ontologies/2008/7/XCLOntology1.5.owl#overprint_Pdf -->

    <PDF1.3_Properties rdf:about="#overprint_Pdf">
        <rdfs:comment
            >(PDF 1.2) A &#64258;ag specifying (on output devices that support the overprint control feature) whether painting in one set of colorants should cause the corresponding areas of other colorants to be erased (false) or left unchanged (true); see Section 4.5.6, &#8220;Overprint Control.&#8221; In PDF 1.3, there are two separate overprint parameters: 
one for stroking and one for all other painting operations. Initial value: false. 
[cit. Pdf 1.3]</rdfs:comment>
        <Datatype rdf:resource="#bool"/>
    </PDF1.3_Properties>
    


    <!-- http://www.semanticweb.org/ontologies/2008/7/XCLOntology1.5.owl#p(OOXML) -->

    <wordProcessingML rdf:about="#p(OOXML)">
        <rdfs:comment xml:lang="en"
            >Paragraph
This element specifies a paragraph of content in the document. 
The contents of a paragraph in a WordprocessingML document shall consist of any combination of the following 
four types of content: 
 Paragraph properties 
 Annotations (bookmarks, comments, revisions) 
 Custom markup 
 Run level content (fields, hyperlinks, runs) 
[cit. OOXML Spec.]</rdfs:comment>
    </wordProcessingML>
    


    <!-- http://www.semanticweb.org/ontologies/2008/7/XCLOntology1.5.owl#pBdr -->

    <wordProcessingML rdf:about="#pBdr">
        <rdfs:comment xml:lang="en"
            >Paragraph Borders
This element specifies the borders for the parent paragraph. Each child element shall specify a specific type of border (left, right, bottom, top, and between). If this element is omitted on a given paragraph, its value is determined by the setting previously set at any level of the style hierarchy (i.e. that previous setting remains unchanged). If this setting is never specified in the style hierarchy, then no paragraph borders shall be applied. 
[Example: Consider a pairing of paragraphs which have a three point red border around them, and a six point border between them. These paragraphs would each have the following set of paragraph borders: 
&lt;w:pBdr&gt; 
  &lt;w:top w:val=&quot;single&quot; w:sz=&quot;24&quot; w:space=&quot;1&quot; w:color=&quot;FF0000&quot; /&gt;  
  &lt;w:left w:val=&quot;single&quot; w:sz=&quot;24&quot; w:space=&quot;4&quot; w:color=&quot;FF0000&quot; /&gt;  
  &lt;w:bottom w:val=&quot;single&quot; w:sz=&quot;24&quot; w:space=&quot;1&quot; w:color=&quot;FF0000&quot; /&gt;  
  &lt;w:right w:val=&quot;single&quot; w:sz=&quot;24&quot; w:space=&quot;4&quot; w:color=&quot;FF0000&quot; /&gt;
  &lt;w:between w:val=&quot;single&quot; w:sz=&quot;48&quot; w:space=&quot;1&quot; w:color=&quot;4D5D2C&quot; /&gt;  
&lt;/w:pBdr&gt;
[cit. OOXML Spec.]</rdfs:comment>
        <Datatype rdf:resource="#int"/>
    </wordProcessingML>
    


    <!-- http://www.semanticweb.org/ontologies/2008/7/XCLOntology1.5.owl#pHYs -->

    <PNG_Properties rdf:about="#pHYs">
        <rdfs:comment xml:lang="en"
            >intended pixel-size or aspect-ratio for the image</rdfs:comment>
    </PNG_Properties>
    


    <!-- http://www.semanticweb.org/ontologies/2008/7/XCLOntology1.5.owl#pPr -->

    <wordProcessingML rdf:about="#pPr">
        <rdfs:comment xml:lang="en"
            >Previous Paragraph Properties
This element specifies a set of paragraph properties which shall be attributed to a revision by a particular author and at a particular time. This element contains the set of properties which have been tracked as a secific set of revisions by one author. 
[Example: Consider a paragraph which should have a set of paragraph formatting properties that were added with revision tracking turned on. This set of revised properties is specified in the paragraph properties as follows: 
&lt;w:p&gt; 
  &lt;w:pPr&gt; 
    &lt;w:pBdr&gt; 
      &lt;w:bottom w:val=&quot;single&quot; w:sz=&quot;8&quot; w:space=&quot;4&quot; w:color=&quot;4F81BD&quot; /&gt;
[cit. OOXML Spec.]</rdfs:comment>
        <Datatype rdf:resource="#bool"/>
    </wordProcessingML>
    


    <!-- http://www.semanticweb.org/ontologies/2008/7/XCLOntology1.5.owl#pPr_Paragraph_Properties -->

    <wordProcessingML rdf:about="#pPr_Paragraph_Properties">
        <rdfs:comment xml:lang="en"
            >Paragraph Properties
This element specifies a set of paragraph properties which shall be applied to the contents of the parent paragraph after all style/numbering/table properties have been applied to the text. These properties are defined as direct formatting, since they are directly applied to the paragraph and supersede any formatting from styles. [cit. OOXML Spec.]</rdfs:comment>
        <Datatype rdf:resource="#int"/>
    </wordProcessingML>
    


    <!-- http://www.semanticweb.org/ontologies/2008/7/XCLOntology1.5.owl#pStyle -->

    <wordProcessingML rdf:about="#pStyle">
        <rdfs:comment xml:lang="en"
            >Referenced Paragraph Style
This element specifies the style ID of the paragraph style which shall be used to format the contents of this 
paragraph. 
This formatting is applied at the following location in the style hierarchy: 
 Document defaults 
 Table styles 
 Numbering styles 
 Paragraph styles (this element) 
 Character styles 
 Direct Formatting</rdfs:comment>
        <Datatype rdf:resource="#string"/>
    </wordProcessingML>
    


    <!-- http://www.semanticweb.org/ontologies/2008/7/XCLOntology1.5.owl#package&#39;sPackageRelationshipZIP_Item -->

    <DOCX_Properties rdf:about="#package&#39;sPackageRelationshipZIP_Item">
        <rdfs:comment xml:lang="en"
            >Information about the relationships between a package and its parts is stored in the package&#39;s package-relationship ZIP item [cit. OOXML spec]</rdfs:comment>
    </DOCX_Properties>
    


    <!-- http://www.semanticweb.org/ontologies/2008/7/XCLOntology1.5.owl#pageBackroundColour -->

    <textInformation rdf:about="#pageBackroundColour">
        <rdfs:comment xml:lang="en"
            >Colourvalue of the Page in a formatted text-document</rdfs:comment>
        <ID>id206</ID>
        <Datatype rdf:resource="#int"/>
    </textInformation>
    


    <!-- http://www.semanticweb.org/ontologies/2008/7/XCLOntology1.5.owl#pageBreak -->

    <textInformation rdf:about="#pageBreak">
        <rdfs:comment
            >Property describing if a textual content breaks to a new page (Unit not yet decided)</rdfs:comment>
        <ID>id182</ID>
        <Datatype rdf:resource="#bool"/>
    </textInformation>
    


    <!-- http://www.semanticweb.org/ontologies/2008/7/XCLOntology1.5.owl#pageBreakBefore -->

    <wordProcessingML rdf:about="#pageBreakBefore">
        <rdfs:comment xml:lang="en"
            >Start Paragraph on Next Page
This element specifies that when rendering this document in a paginated view, the contents of this paragraph are rendered on the start of a new page in the document. 
This means that if the contents of the current paragraph would normally be rendered on the middle of a page in the host document, then the paragraph shall be rendered on a new page as if the paragraph was preceded by a page break in the WordprocessingML contents of the document. This property supersedes any use of the keepNext property, so that if any paragraph wishes to be on the same page as this paragraph, they will still be separated by a page break. 
If this element is omitted on a given paragraph, its value is determined by the setting previously set at any level of the style hierarchy (i.e. that previous setting remains unchanged). If this setting is never specified in the style hierarchy, then this property shall not be applied. 
[cit. OOXML Spec.]</rdfs:comment>
        <Datatype rdf:resource="#bool"/>
    </wordProcessingML>
    


    <!-- http://www.semanticweb.org/ontologies/2008/7/XCLOntology1.5.owl#pageLayoutDisplay -->

    <textInformation rdf:about="#pageLayoutDisplay">
        <ID>id77</ID>
        <is_same_as rdf:resource="#PageLayout"/>
    </textInformation>
    


    <!-- http://www.semanticweb.org/ontologies/2008/7/XCLOntology1.5.owl#pageNumber -->

    <textInformation rdf:about="#pageNumber">
        <rdfs:comment
            >The number of the page on which the content is from (either scanned pages for image-objects but also text documents)</rdfs:comment>
        <ID>id195</ID>
        <Datatype rdf:resource="#int"/>
    </textInformation>
    


    <!-- http://www.semanticweb.org/ontologies/2008/7/XCLOntology1.5.owl#paletteHistogram -->

    <rasterInformation rdf:about="#paletteHistogram">
        <ID>240</ID>
        <rdfs:comment xml:lang="en"
            >approximate usage frequency of each colour in the palette index (rgbPalette)</rdfs:comment>
        <is_same_as rdf:resource="#hIST"/>
        <is_same_as rdf:resource="#histogram"/>
        <Datatype rdf:resource="#int"/>
    </rasterInformation>
    


    <!-- http://www.semanticweb.org/ontologies/2008/7/XCLOntology1.5.owl#palettePlanarConfig -->

    <rasterInformation rdf:about="#palettePlanarConfig">
        <ID>id54</ID>
        <rdfs:comment
            >planarConfiguration of the paletteColourValues</rdfs:comment>
        <Datatype rdf:resource="#int"/>
    </rasterInformation>
    


    <!-- http://www.semanticweb.org/ontologies/2008/7/XCLOntology1.5.owl#paragraph -->

    <textInformation rdf:about="#paragraph">
        <rdfs:comment
            >describes structured continuous text data</rdfs:comment>
        <ID>id207</ID>
        <Datatype rdf:resource="#bool"/>
    </textInformation>
    


    <!-- http://www.semanticweb.org/ontologies/2008/7/XCLOntology1.5.owl#partRelationshipZIP_Item -->

    <DOCX_Properties rdf:about="#partRelationshipZIP_Item">
        <rdfs:comment xml:lang="en"
            >Information about the relationships between two parts is stored in the part- relationship ZIP item for the source part [cit.: OOXML spec.]</rdfs:comment>
    </DOCX_Properties>
    


    <!-- http://www.semanticweb.org/ontologies/2008/7/XCLOntology1.5.owl#passwordProtectedAction -->

    <generalInformation rdf:about="#passwordProtectedAction">
        <ID>id187</ID>
    </generalInformation>
    


    <!-- http://www.semanticweb.org/ontologies/2008/7/XCLOntology1.5.owl#pdfBaseFont -->

    <PDF1.3_Properties rdf:about="#pdfBaseFont">
        <rdfs:comment xml:lang="en"
            >fontcapheight return maximum capheight for specified font and size</rdfs:comment>
    </PDF1.3_Properties>
    


    <!-- http://www.semanticweb.org/ontologies/2008/7/XCLOntology1.5.owl#pdfFontName -->

    <generalInformation rdf:about="#pdfFontName"/>
    


    <!-- http://www.semanticweb.org/ontologies/2008/7/XCLOntology1.5.owl#pdfObjectType -->

    <PDF1.3_Properties rdf:about="#pdfObjectType">
        <rdfs:comment xml:lang="en"
            >can be something like image</rdfs:comment>
    </PDF1.3_Properties>
    


    <!-- http://www.semanticweb.org/ontologies/2008/7/XCLOntology1.5.owl#pdfVersion -->

    <PDF1.3_Properties rdf:about="#pdfVersion">
        <rdfs:comment
            >notates the version of the pdf-file</rdfs:comment>
    </PDF1.3_Properties>
    


    <!-- http://www.semanticweb.org/ontologies/2008/7/XCLOntology1.5.owl#pel -->

    <block rdf:about="#pel">
        <rdfs:comment xml:lang="en"
            >An 8-bit sample of luminance or chrominance data (image/videodata) in a MPEG</rdfs:comment>
    </block>
    


    <!-- http://www.semanticweb.org/ontologies/2008/7/XCLOntology1.5.owl#photometricInterpretation -->

    <Tiff_Properties rdf:about="#photometricInterpretation">
        <rdfs:comment
            >The color space of the image data.
The specification considers these values baseline:
0 = WhiteIsZero. For bilevel and grayscale images: 0 is imaged as white.
1 = BlackIsZero. For bilevel and grayscale images: 0 is imaged as black.
2 = RGB. RGB value of (0,0,0) represents black, and (255,255,255) represents white, assuming 8-bit components. The components are stored in the indicated order: first Red, then Green, then Blue.
3 = Palette color. In this model, a color is described with a single component. The value of the component is used as an index into the red, green and blue curves in the ColorMap field to retrieve an RGB triplet that defines the color. When PhotometricInterpretation=3 is used, ColorMap must be present and SamplesPerPixel must be 1.
4 = Transparency Mask. This means that the image is used to define an irregularly shaped region of another image in the same TIFF file. SamplesPerPixel and BitsPerSample must be 1. PackBits compression is recommended. The 1-bits define the interior of the region; the 0-bits define the exterior of the region. [cit. Tiff]</rdfs:comment>
    </Tiff_Properties>
    


    <!-- http://www.semanticweb.org/ontologies/2008/7/XCLOntology1.5.owl#photoshopLayerName -->

    <rasterInformation rdf:about="#photoshopLayerName">
        <ID>id199</ID>
        <rdfs:comment
            >photoshop-layer in a psd- or tiff-file. Should be linked with imagedata</rdfs:comment>
        <Datatype rdf:resource="#string"/>
    </rasterInformation>
    


    <!-- http://www.semanticweb.org/ontologies/2008/7/XCLOntology1.5.owl#pixelAspectRatio -->

    <rasterInformation rdf:about="#pixelAspectRatio">
        <rdfs:comment
            >Defines Pixelheight/Pixelwidth - in gif 89a , also useful for video and other picture-formats</rdfs:comment>
        <ID>id75</ID>
        <is_same_as rdf:resource="#PAR"/>
        <Datatype rdf:resource="#uint16"/>
    </rasterInformation>
    


    <!-- http://www.semanticweb.org/ontologies/2008/7/XCLOntology1.5.owl#planarConfiguration -->

    <rasterInformation rdf:about="#planarConfiguration">
        <rdfs:comment xml:lang="en"
            >How the components of each pixel are stored</rdfs:comment>
        <ID>id49</ID>
        <is_same_as rdf:resource="#PlanarConfiguration_NISO"/>
        <Datatype rdf:resource="#int"/>
        <is_same_as rdf:resource="#planarConfigurationTiff"/>
    </rasterInformation>
    


    <!-- http://www.semanticweb.org/ontologies/2008/7/XCLOntology1.5.owl#planarConfigurationTiff -->

    <Tiff_Properties rdf:about="#planarConfigurationTiff">
        <rdfs:comment xml:lang="en"
            >How the components of each pixel are stored</rdfs:comment>
        <is_same_as rdf:resource="#PlanarConfiguration_NISO"/>
        <Datatype rdf:resource="#int"/>
        <is_same_as rdf:resource="#planarConfiguration"/>
    </Tiff_Properties>
    


    <!-- http://www.semanticweb.org/ontologies/2008/7/XCLOntology1.5.owl#position -->

    <wordProcessingML rdf:about="#position">
        <rdfs:comment
            >position (Vertically Raised or Lowered Text) 
This element specifies the amount by which text shall be raised or lowered for this run in relation to the default baseline of the surrounding non-positioned text. This allows the text to be repositioned without altering the font size of the contents. 
If the val attribute is positive, then the parent run shall be raised above the baseline of the surrounding text by the specified number of half-points. If the val attribute is negative, then the parent run shall be lowered below the baseline of the surrounding text by the specified number of half-points.
If this element is not present, the default value is to leave the formatting applied at previous level in the style hierarchy. If this element is never applied in the style hierarchy, then the text shall not be raised or lowered relative to the default baseline location for the contents of this run. Example: Consider a run which shall be positioned 12 points above the default baseline location when displaying its contents. This requirement would be specified using the following WordprocessingML: 
&lt;w:rPr&gt; 
  &lt;w:position w:val=&quot;24&quot; /&gt; 
&lt;/w:rPr&gt; 
val: Point Measurement) 
Specifies a positive or negative measurement in half-points (1/144 of an inch). 
The contents of this attribute value are interpreted based on the context of the parent XML element. 
Example: Consider the following WordprocessingML fragment: 
&lt;w:rPr&gt; 
  &lt;w:position w:val=&quot;-12&quot; /&gt;  
&lt;/w:rPr&gt; 
In this case, the value in the val attribute is amount by which the specified run shall be raised or lowered compared to the baseline of the surrounding text.
[cit. OOXML spec.]</rdfs:comment>
        <Datatype rdf:resource="#int"/>
    </wordProcessingML>
    


    <!-- http://www.semanticweb.org/ontologies/2008/7/XCLOntology1.5.owl#postscriptFont -->

    <textInformation rdf:about="#postscriptFont">
        <rdfs:comment
            >filetype for font</rdfs:comment>
        <ID>id222</ID>
        <Datatype rdf:resource="#XCLLabel"/>
    </textInformation>
    


    <!-- http://www.semanticweb.org/ontologies/2008/7/XCLOntology1.5.owl#procSet -->

    <PDF1.3_Properties rdf:about="#procSet">
        <rdfs:comment xml:lang="en"
            >The ProcSet entry in a content stream&#8217;s resource dictionary (see Section 3.7.2, &#8220;Resource Dictionaries&#8221;) holds an array consisting of the names of the procedure sets used in that content stream. These procedure sets are used only when the content stream is printed to a PostScript output device. The names identify PostScript procedure sets that must be sent to the device to interpret the PDF operators in the content stream. Each element of this array must be one of the predefined names shown in Table 10.1. (See implementation note 159 in Appendix H.)

Devided in: procSetPdf, procSetText, procSetImageB, procSetImageC, procSetImageI</rdfs:comment>
    </PDF1.3_Properties>
    


    <!-- http://www.semanticweb.org/ontologies/2008/7/XCLOntology1.5.owl#r -->

    <wordProcessingML rdf:about="#r">
        <rdfs:comment
            >r (Text Run) 
This element specifies a run of content in the parent field, hyperlink, custom XML element, structured document tag, smart tag, or paragraph. 
The contents of a run in a WordprocessingML document shall consist of any combination of run content. 
Example: Consider a basic WordprocessingML paragraph with a pair of runs. This run would be expressed as follows: 
&lt;w:document&gt; 
  &lt;w:body&gt; 
    &lt;w:p&gt; 
      &lt;w:r&gt; 
        &lt;w:t&gt;Text&lt;/w:t&gt; 
      &lt;/w:r&gt; 
      &lt;w:fldSimple w:instr=&quot;AUTHOR&quot;&gt; 
        &lt;w:r&gt; 
          &lt;w:t&gt;Author Name&lt;/w:t&gt; 
        &lt;/w:r&gt; 
      &lt;/w:fldSimple&gt; 
    &lt;/w:p&gt; 
  &lt;/w:body&gt; 
&lt;/w:document&gt; 
The r element is the container for all of the content in the run, which in this example includes both a run in the paragraph and a run within a simple field.
[cit. OOXML spec.]</rdfs:comment>
    </wordProcessingML>
    


    <!-- http://www.semanticweb.org/ontologies/2008/7/XCLOntology1.5.owl#rFonts -->

    <wordProcessingML rdf:about="#rFonts">
        <rdfs:comment
            >rFonts (Run Fonts) 
This element specifies the fonts which shall be used to display the text contents of this run. Within a single run, there may be up to four types of content present which shall each be allowed to use a unique font:
 ASCII 
 High ANSI 
 Complex Script 
 East Asian 
The use of each of these fonts shall be determined by the Unicode character values of the run content, unless manually overridden via use of the cs element (&#167;2.3.2.6). 
If this element is not present, the default value is to leave the formatting applied at previous level in the style hierarchy. If this element is never applied in the style hierarchy, then the text shall be displayed in any default font which supports each type of content.  
Example: Consider a single text run with both Arabic and English text, as follows: 
English &#1577;&#1610; &#1576;&#1585;&#1593; &#1604;&#1575; 
This content may be expressed in a single WordprocessingML run: 
&lt;w:r&gt; 
  &lt;w:t&gt;English &#1577;&#1610;&#1576;&#1585;&#1593;&#1604;&#1575;&lt;/w:t&gt; 
&lt;/w:r&gt; 
Although it is in the same run, the contents are in different font faces by specifying a different font for ASCII and CS characters in the run: 
&lt;w:r&gt; 
  &lt;w:rPr&gt; 
    &lt;w:rFonts w:ascii=&quot;Courier New&quot; w:cs=&quot;Times New Roman&quot; /&gt; 
  &lt;/w:rPr&gt; 
  &lt;w:t&gt;English &#1577;&#1610;&#1576;&#1585;&#1593;&#1604;&#1575;&lt;/w:t&gt; 
&lt;/w:r&gt; 
[cit. OOXML spec.]</rdfs:comment>
        <Datatype rdf:resource="#string"/>
    </wordProcessingML>
    


    <!-- http://www.semanticweb.org/ontologies/2008/7/XCLOntology1.5.owl#rPr -->

    <wordProcessingML rdf:about="#rPr">
        <rdfs:comment xml:lang="en"
            >Run Properties for the Paragraph Mark
This element specifies the set of run properties applied to the glyph used to represent the physical location of the paragraph mark for this paragraph. This paragraph mark, being a physical character in the document, can be formatted, and therefore must be capable of representing this formatting like any other character in the document. 
If this element is not present, the paragraph mark is unformatted, as with any other run of text. 
[Example: Consider a run of text displayed as follows, including a display format using the pilcrow sign &#182; for the paragraph mark glyph: 
This is some text and the paragraph mark.&#182;
[cit. OOXML Spec.]</rdfs:comment>
        <Datatype rdf:resource="#bool"/>
    </wordProcessingML>
    


    <!-- http://www.semanticweb.org/ontologies/2008/7/XCLOntology1.5.owl#rPr(Previous_Run_Properties_for_the_Paragraph_Mark) -->

    <wordProcessingML rdf:about="#rPr(Previous_Run_Properties_for_the_Paragraph_Mark)">
        <rdfs:comment xml:lang="en"
            >Previous Run Properties for the Paragraph Mark
This element specifies a set of run properties applied to the glyph used to represent the physical location of the paragraph mark for this paragraph which shall be attributed to a revision by a particular author and at a particular time. This element contains the set of properties which have been tracked as a specific set of revisions by one author.
[cit. OOXML Spec.]</rdfs:comment>
        <Datatype rdf:resource="#bool"/>
    </wordProcessingML>
    


    <!-- http://www.semanticweb.org/ontologies/2008/7/XCLOntology1.5.owl#rStyle -->

    <wordProcessingML rdf:about="#rStyle">
        <rdfs:comment
            >rStyle (Referenced Character Style) 
This element specifies the style ID of the character style which shall be used to format the contents of this paragraph. 
This formatting is applied at the following location in the style hierarchy: Document defaults 
Table styles 
Numbering styles 
Paragraph styles 
Character styles (this element) 
Direct Formatting 
This means that all properties specified in the style element (&#167;2.7.3.17) with a styleId which corresponds to the value in this element&#39;s val attribute are applied to the run at the appropriate level in the hierarchy. 
If this element is omitted, or it references a style which does not exist, then no character style shall be applied to the current paragraph. As well, this property is ignored if the run properties are part of a character style. Example: Consider the following WordprocessingML fragment: 
&lt;w:rPr&gt; 
  &lt;w:pStyle w:val=&#8221;TestCharacterStyle&#8221; /&gt; 
  &lt;w:b /&gt; 
  &lt;w:i /&gt; 
&lt;/w:rPr&gt; 
This run specifies that it will inherit all of the run properties specified by the paragraph style with a styleId of TestCharacterStyle, which will then have any bold or italics settings overridden and set to be applied to the run.
[cit. OOXML spec.]</rdfs:comment>
        <Datatype rdf:resource="#string"/>
    </wordProcessingML>
    


    <!-- http://www.semanticweb.org/ontologies/2008/7/XCLOntology1.5.owl#rational -->

    <xcl_propertyDatatypes rdf:about="#rational"/>
    


    <!-- http://www.semanticweb.org/ontologies/2008/7/XCLOntology1.5.owl#rectangleValues -->

    <vectorInformation rdf:about="#rectangleValues">
        <rdfs:comment
            >Length of sides in a rectangular vecor-object</rdfs:comment>
        <ID>id248</ID>
        <Datatype rdf:resource="#int"/>
    </vectorInformation>
    


    <!-- http://www.semanticweb.org/ontologies/2008/7/XCLOntology1.5.owl#relevant -->

    <property_restriction rdf:about="#relevant"/>
    


    <!-- http://www.semanticweb.org/ontologies/2008/7/XCLOntology1.5.owl#renderingIntent_PNG -->

    <PNG_Properties rdf:about="#renderingIntent_PNG">
        <rdfs:comment xml:lang="en"
            >0=Perceptual
1=Relative colourimetric
2=Saturation
3=Absolute colourimetric</rdfs:comment>
        <is_same_as rdf:resource="#RenderingIntent_Pdf"/>
        <Datatype rdf:resource="#int"/>
    </PNG_Properties>
    


    <!-- http://www.semanticweb.org/ontologies/2008/7/XCLOntology1.5.owl#resPDFFontAlias -->

    <PDF1.3_Properties rdf:about="#resPDFFontAlias">
        <rdfs:comment xml:lang="en"
            >Resource location of the font-alias file in the system</rdfs:comment>
    </PDF1.3_Properties>
    


    <!-- http://www.semanticweb.org/ontologies/2008/7/XCLOntology1.5.owl#resolutionUnit -->

    <rasterInformation rdf:about="#resolutionUnit">
        <rdfs:comment
            >Name of the Unit, that messures the resolution of the Image.
If none it is none: default is generally inch</rdfs:comment>
        <is_same_as rdf:resource="#resolutionUnitTiff"/>
        <Datatype rdf:resource="#string"/>
    </rasterInformation>
    


    <!-- http://www.semanticweb.org/ontologies/2008/7/XCLOntology1.5.owl#resolutionUnitTiff -->

    <Tiff_Properties rdf:about="#resolutionUnitTiff">
        <is_same_as rdf:resource="#resolutionUnit"/>
        <Datatype rdf:resource="#string"/>
    </Tiff_Properties>
    


    <!-- http://www.semanticweb.org/ontologies/2008/7/XCLOntology1.5.owl#resolutionX -->

    <rasterInformation rdf:about="#resolutionX">
        <rdfs:comment
            >The number of pixels per ResolutionUnit in the ImageWidth direction.</rdfs:comment>
        <ID>id23</ID>
        <Datatype rdf:resource="#int"/>
        <is_same_as rdf:resource="#resolutionX_Tiff"/>
    </rasterInformation>
    


    <!-- http://www.semanticweb.org/ontologies/2008/7/XCLOntology1.5.owl#resolutionX_Tiff -->

    <Tiff_Properties rdf:about="#resolutionX_Tiff">
        <Datatype rdf:resource="#int"/>
        <is_same_as rdf:resource="#resolutionX"/>
    </Tiff_Properties>
    


    <!-- http://www.semanticweb.org/ontologies/2008/7/XCLOntology1.5.owl#resolutionY -->

    <rasterInformation rdf:about="#resolutionY">
        <ID>id24</ID>
        <rdfs:comment
            >The number of pixels per ResolutionUnit in the ImageHeigth direction.</rdfs:comment>
        <Datatype rdf:resource="#int"/>
        <is_same_as rdf:resource="#resolutionY_Tiff"/>
    </rasterInformation>
    


    <!-- http://www.semanticweb.org/ontologies/2008/7/XCLOntology1.5.owl#resolutionY_Tiff -->

    <Tiff_Properties rdf:about="#resolutionY_Tiff">
        <Datatype rdf:resource="#int"/>
        <is_same_as rdf:resource="#resolutionY"/>
    </Tiff_Properties>
    


    <!-- http://www.semanticweb.org/ontologies/2008/7/XCLOntology1.5.owl#rgb -->

    <imageInformation rdf:about="#rgb">
        <rdfs:comment xml:lang="en"
            >ColourSpace: RGB triple</rdfs:comment>
        <ID>id132</ID>
        <Datatype rdf:resource="#uint16"/>
    </imageInformation>
    


    <!-- http://www.semanticweb.org/ontologies/2008/7/XCLOntology1.5.owl#rgbPalette -->

    <rasterInformation rdf:about="#rgbPalette">
        <ID>id25</ID>
        <is_same_as rdf:resource="#PLTE"/>
        <is_same_as rdf:resource="#colourMapTiff"/>
        <Datatype rdf:resource="#int"/>
        <is_same_as rdf:resource="#lookup"/>
    </rasterInformation>
    


    <!-- http://www.semanticweb.org/ontologies/2008/7/XCLOntology1.5.owl#rgbPaletteWithFiller -->

    <rasterInformation rdf:about="#rgbPaletteWithFiller">
        <rdfs:comment
            >means a rgb-palette which is not completed and has some values of 0,0,0 at the end</rdfs:comment>
        <ID>id70</ID>
        <Datatype rdf:resource="#uint32Rational"/>
    </rasterInformation>
    


    <!-- http://www.semanticweb.org/ontologies/2008/7/XCLOntology1.5.owl#right -->

    <wordProcessingML rdf:about="#right">
        <rdfs:comment xml:lang="en"
            >Right Paragraph Border
This element specifies the border which shall be displayed on the right side of the page around the specified paragraph. 
To determine if any two adjoining paragraphs should have a right border which spans the full line height or not, the right border shall be drawn between the top border or between border at the top (whichever would be rendered for the current paragraph), and the bottom border or between border at the bottom (whichever would be rendered for the current paragraph). 
If this element is omitted on a given paragraph, its value is determined by the setting previously set at any level of the style hierarchy (i.e. that previous setting remains unchanged). If this setting is never specified in the style hierarchy, then no right border shall be applied.
Example: &lt;w:right w:val=&quot;single&quot; w:sz=&quot;24&quot; w:space=&quot;4&quot; w:color=&quot;C3D69B&quot; w:themeColor=&quot;accent3&quot; w:themeTint=&quot;99&quot; /&gt;
[cit. OOXML Spec.]</rdfs:comment>
        <Datatype rdf:resource="#bool"/>
        <is_same_as rdf:resource="#rightAdjustment"/>
    </wordProcessingML>
    


    <!-- http://www.semanticweb.org/ontologies/2008/7/XCLOntology1.5.owl#rightAdjustment -->

    <textInformation rdf:about="#rightAdjustment">
        <ID>id271</ID>
        <Datatype rdf:resource="#bool"/>
        <Restriction rdf:resource="#relevant"/>
    </textInformation>
    


    <!-- http://www.semanticweb.org/ontologies/2008/7/XCLOntology1.5.owl#rotationDisplay -->

    <textInformation rdf:about="#rotationDisplay">
        <rdfs:comment
            >The number of degrees by which the page should be rotated clockwise when displayed</rdfs:comment>
        <is_same_as rdf:resource="#Rotate"/>
        <Datatype rdf:resource="#int"/>
    </textInformation>
    


    <!-- http://www.semanticweb.org/ontologies/2008/7/XCLOntology1.5.owl#rotationPrint -->

    <textInformation rdf:about="#rotationPrint">
        <rdfs:comment
            >The number of degrees by which the page should be rotated clockwise when printed</rdfs:comment>
        <Datatype rdf:resource="#int"/>
    </textInformation>
    


    <!-- http://www.semanticweb.org/ontologies/2008/7/XCLOntology1.5.owl#rowNumber -->

    <textInformation rdf:about="#rowNumber">
        <ID>id277</ID>
        <rdfs:comment
            >n-th row in a table</rdfs:comment>
    </textInformation>
    


    <!-- http://www.semanticweb.org/ontologies/2008/7/XCLOntology1.5.owl#rowsPerStrip_Tiff -->

    <Tiff_Properties rdf:about="#rowsPerStrip_Tiff">
        <rdfs:comment
            >The number of rows per strip.
TIFF image data can be organized into strips for faster random access and efficient I/O buffering.
RowsPerStrip and ImageLength together tell us the number of strips in the entire image. The equation is:
StripsPerImage = floor ((ImageLength + RowsPerStrip - 1) / RowsPerStrip).</rdfs:comment>
        <is_same_as rdf:resource="#RowsPerStrip_NISO"/>
        <Datatype rdf:resource="#int"/>
    </Tiff_Properties>
    


    <!-- http://www.semanticweb.org/ontologies/2008/7/XCLOntology1.5.owl#rtl -->

    <wordProcessingML rdf:about="#rtl">
        <rdfs:comment
            >rtl (Right To Left Text) 
This element specifies that the alignment and reading order for this run shall be right to left. This setting determines the way in which the run contents are presented in the document when punctuation characters are part of the run&#39;s contents. When this property is specified, each part of the run between a punctuation mark shall be laid out right to left on the line. 
If this element is not present, the default value is to leave the formatting applied at previous level in the style hierarchy. If this element is never applied in the style hierarchy, then right to left alignment shall not be applied to the contents of this run. 
Example: Consider the following run of English text: This is a list: one, two, three. Typically, each region of text between a punctuation mark is presented in a left to right reading order in the document (as 
shown above). If the right to left property is set on this text, as follows: 
&lt;w:rPr&gt; 
  &lt;w:rtl v:val=&quot;on&quot;/&gt; 
&lt;/w:rPr&gt; 
This run shall now have a right to left reading order, as follows: 
.three ,two ,one :This is a list In a right to left language, this would result in the correct placement of the punctuation with respect to each region of right to left text. 
[cit. OOXML spec.]</rdfs:comment>
        <Datatype rdf:resource="#bool"/>
    </wordProcessingML>
    


    <!-- http://www.semanticweb.org/ontologies/2008/7/XCLOntology1.5.owl#sPLT -->

    <PNG_Properties rdf:about="#sPLT">
        <rdfs:comment xml:lang="en"
            >Palette-Chunk recomended for colour_types: 0 and 4...
look it up</rdfs:comment>
    </PNG_Properties>
    


    <!-- http://www.semanticweb.org/ontologies/2008/7/XCLOntology1.5.owl#sRGB -->

    <imageInformation rdf:about="#sRGB">
        <ID>id235</ID>
        <is_same_as rdf:resource="#sRGB_PNG"/>
        <is_same_as rdf:resource="#sRGB_Tiff"/>
    </imageInformation>
    


    <!-- http://www.semanticweb.org/ontologies/2008/7/XCLOntology1.5.owl#sRGB_PNG -->

    <PNG_Properties rdf:about="#sRGB_PNG">
        <rdfs:comment xml:lang="en"
            >indicates that the standard sRGB colour space is used.
The sRGB chunk contains:
Rendering intent: 1 byte
The following values are defined for rendering intent:
0: Perceptual, for images preferring good adaptation to the output device gamut at the expense of colourimetric accuracy, such as photographs.

1: Relative colourimetric, for images requiring colour appearance matching (relative to the output device white point), such as logos.

2: Saturation, for images preferring preservation of saturation at the expense of hue and lightness, such as charts and graphs.
3: Absolute colourimetric, for images requiring preservation of absolute colourimetry, such as previews of images destined for a different output device (proofs).</rdfs:comment>
        <Datatype rdf:resource="#hex"/>
        <is_same_as rdf:resource="#sRGB"/>
    </PNG_Properties>
    


    <!-- http://www.semanticweb.org/ontologies/2008/7/XCLOntology1.5.owl#sRGB_Tiff -->

    <Tiff_Properties rdf:about="#sRGB_Tiff">
        <rdfs:comment
            >sRGB specification</rdfs:comment>
        <Datatype rdf:resource="#int"/>
        <is_same_as rdf:resource="#sRGB"/>
    </Tiff_Properties>
    


    <!-- http://www.semanticweb.org/ontologies/2008/7/XCLOntology1.5.owl#sample -->

    <xcl_units rdf:about="#sample"/>
    


    <!-- http://www.semanticweb.org/ontologies/2008/7/XCLOntology1.5.owl#samplerateAudio -->

    <audioInformation rdf:about="#samplerateAudio">
        <ID>id173</ID>
        <Datatype rdf:resource="#int"/>
    </audioInformation>
    


    <!-- http://www.semanticweb.org/ontologies/2008/7/XCLOntology1.5.owl#samplesPerPixel -->

    <rasterInformation rdf:about="#samplesPerPixel">
        <ID>id217</ID>
        <rdfs:comment
            >The number of components per pixel.</rdfs:comment>
        <is_same_as rdf:resource="#SamplesPerPixel_NISO"/>
        <Datatype rdf:resource="#int"/>
        <is_same_as rdf:resource="#samplesPerPixelTIff"/>
    </rasterInformation>
    


    <!-- http://www.semanticweb.org/ontologies/2008/7/XCLOntology1.5.owl#samplesPerPixelTIff -->

    <Tiff_Properties rdf:about="#samplesPerPixelTIff">
        <rdfs:comment
            >The number of components per pixel.
SamplesPerPixel is usually 1 for bilevel, grayscale, and palette-colour images. SamplesPerPixel is usually 3 for RGB images. If this value is higher, ExtraSamples should give an indication of the meaning of the additional channels.</rdfs:comment>
        <is_same_as rdf:resource="#SamplesPerPixel_NISO"/>
        <Datatype rdf:resource="#int"/>
        <is_same_as rdf:resource="#samplesPerPixel"/>
    </Tiff_Properties>
    


    <!-- http://www.semanticweb.org/ontologies/2008/7/XCLOntology1.5.owl#scale -->

    <PDF1.3_Properties rdf:about="#scale">
        <rdfs:comment
            >Horizontal Text scaling:
Set the horizontal scaling, T h, to (scale &#247; 100). scale is a number specifying the percentage of the normal width. Default value: 100 (normal width). 
[cit. pdf 1.3]</rdfs:comment>
        <Datatype rdf:resource="#int"/>
    </PDF1.3_Properties>
    


    <!-- http://www.semanticweb.org/ontologies/2008/7/XCLOntology1.5.owl#scanDocName -->

    <Tiff_Properties rdf:about="#scanDocName">
        <rdfs:comment xml:lang="en"
            >The name of the document from which this image was scanned [cit. TIFF 6.0] [Compatibility: TIFF 6.0]</rdfs:comment>
    </Tiff_Properties>
    


    <!-- http://www.semanticweb.org/ontologies/2008/7/XCLOntology1.5.owl#scanlineTiff -->

    <Tiff_Properties rdf:about="#scanlineTiff">
        <Datatype rdf:resource="#string"/>
    </Tiff_Properties>
    


    <!-- http://www.semanticweb.org/ontologies/2008/7/XCLOntology1.5.owl#scannerInformation -->

    <Tiff_Properties rdf:about="#scannerInformation">
        <rdfs:comment
            >Name and Information about the scanner, used to digitize the Image</rdfs:comment>
        <is_same_as rdf:resource="#scannerName"/>
        <Datatype rdf:resource="#string"/>
    </Tiff_Properties>
    


    <!-- http://www.semanticweb.org/ontologies/2008/7/XCLOntology1.5.owl#scannerName -->

    <rasterInformation rdf:about="#scannerName">
        <ID>id281</ID>
        <rdfs:comment
            >Name of the scanner, that digized the image</rdfs:comment>
        <is_same_as rdf:resource="#scannerInformation"/>
        <Datatype rdf:resource="#string"/>
    </rasterInformation>
    


    <!-- http://www.semanticweb.org/ontologies/2008/7/XCLOntology1.5.owl#semimajorEllipseDiameter -->

    <vectorInformation rdf:about="#semimajorEllipseDiameter">
        <ID>id320</ID>
        <rdfs:comment
            >length of the major diamter in a ellipse-shaped vector-object</rdfs:comment>
        <Datatype rdf:resource="#uint32Rational"/>
    </vectorInformation>
    


    <!-- http://www.semanticweb.org/ontologies/2008/7/XCLOntology1.5.owl#semiminorEllipseDiameter -->

    <vectorInformation rdf:about="#semiminorEllipseDiameter">
        <ID>id247</ID>
        <rdfs:comment
            >length of the minor diamter in a ellipse-shaped vector-object</rdfs:comment>
        <Datatype rdf:resource="#uint32Rational"/>
    </vectorInformation>
    


    <!-- http://www.semanticweb.org/ontologies/2008/7/XCLOntology1.5.owl#shadow -->

    <textInformation rdf:about="#shadow">
        <ID>id166</ID>
        <rdfs:comment
            >text-property shadow</rdfs:comment>
        <Datatype rdf:resource="#bool"/>
        <is_same_as rdf:resource="#shadow_OOXML"/>
    </textInformation>
    


    <!-- http://www.semanticweb.org/ontologies/2008/7/XCLOntology1.5.owl#shadow_OOXML -->

    <wordProcessingML rdf:about="#shadow_OOXML">
        <rdfs:comment
            >Example: Consider a top border which shall appear with a shadow effect, resulting in the following WordprocessingML: 
&lt;w:bottom w:shadow=&quot;true&quot; ... /&gt; 
This frame&#39;s val is true, indicating that the shadow effect shall be applied to the border. [cit. OOXML spec.]</rdfs:comment>
        <Datatype rdf:resource="#bool"/>
    </wordProcessingML>
    


    <!-- http://www.semanticweb.org/ontologies/2008/7/XCLOntology1.5.owl#shd -->

    <wordProcessingML rdf:about="#shd">
        <rdfs:comment xml:lang="en"
            >Paragraph &amp; Run Shading
This element specifies the shading applied to the contents of the run or paragraph. 
This shading consists of three components: 
 Background Color 
 (optional) Pattern 
 (optional) Pattern Color 
The resulting shading is applied by setting the background color behind the paragraph, then applying the pattern color using the mask supplied by the pattern over that background.  
If this element is not present, the default value is to leave the formatting applied at previous level in the style hierarchy. If this element is never applied in the style hierarchy, then run shading shall not be applied to the contents of this run. 
Example: Consider a run which shall have a background consisting of a theme color accent6 with a theme color text2 overlaid using a 20% fill pattern. This requirement is specified using the following WordprocessingML: 
&lt;w:pPr&gt; 
  &lt;w:shd w:val=&quot;pct20&quot; w:themeColor=&quot;text2&quot; w:themeFill=&quot;accent6&quot; /&gt;  
&lt;/w:pPr&gt; 
The resulting run will use the background color accent6 under the foreground pattern color text2 as specified by the pct20 pattern mask.
This shading val is pct20, indicating that the border style is a 20 percent foreground fill mask. 
[cit. OOXML Spec.]</rdfs:comment>
        <Datatype rdf:resource="#int"/>
    </wordProcessingML>
    


    <!-- http://www.semanticweb.org/ontologies/2008/7/XCLOntology1.5.owl#signature -->

    <generalInformation rdf:about="#signature">
        <ID xml:lang="">id4</ID>
        <is_same_as rdf:resource="#GIF_Signature"/>
        <Unit rdf:resource="#NULL"/>
        <Datatype rdf:resource="#string"/>
    </generalInformation>
    


    <!-- http://www.semanticweb.org/ontologies/2008/7/XCLOntology1.5.owl#significantBits -->

    <PNG_Properties rdf:about="#significantBits">
        <rdfs:comment xml:lang="en"
            >number of bits that are significant in the samples [Compatibility: PNG 1.1]</rdfs:comment>
    </PNG_Properties>
    


    <!-- http://www.semanticweb.org/ontologies/2008/7/XCLOntology1.5.owl#simpleTransparency -->

    <rasterInformation rdf:about="#simpleTransparency">
        <ID>id181</ID>
        <rdfs:comment
            >simple Transparency in opposite to alpha-transparency (and the RGB-value for the colour which is set to be transparent)</rdfs:comment>
        <rdfs:isDefinedBy rdf:resource="#uint32Rational"/>
    </rasterInformation>
    


    <!-- http://www.semanticweb.org/ontologies/2008/7/XCLOntology1.5.owl#smallCaps -->

    <textInformation rdf:about="#smallCaps">
        <ID>id167</ID>
        <rdfs:comment
            >text-property smallCaps</rdfs:comment>
        <Datatype rdf:resource="#bool"/>
        <is_same_as rdf:resource="#smallCaps_OOXML"/>
    </textInformation>
    


    <!-- http://www.semanticweb.org/ontologies/2008/7/XCLOntology1.5.owl#smallCaps_OOXML -->

    <wordProcessingML rdf:about="#smallCaps_OOXML">
        <rdfs:comment
            >SmallCaps:
This element specifies that all small letter characters in this text run shall be formatted for display only as their capital letter character equivalents in a font size two points smaller than the actual font size specified for this text. This property does not affect any non-alphabetic character in this run, and does not change the Unicode character for lowercase text, only the method in which it is displayed. If this font cannot be made two point smaller than the current size, then it shall be displayed as the smallest possible font size in capital letters. 
This formatting property is a toggle property, which specifies that its behavior differs between its use within a style definition and its use as direct formatting. When used as part of a style definition, setting this property shall toggle the current state of that property as specified up to this point in the hierarchy (i.e. applied to not applied, and vice versa). Setting it to false (or an equivalent) shall result in the current setting remaining unchanged. However, when used as direct formatting, setting this property to true or false shall set the absolute state of the resulting property.  
If this element is not present, the default value is to leave the formatting applied at previous level in the style hierarchy. If this element is never applied in the style hierarchy, then the characters are not formatted as capital letters.
Example:
&lt;w:r&gt; 
    &lt;w:sz w:val=&quot;24&quot; /&gt; 
    &lt;w:smallCaps w:val=&quot;true&quot; /&gt; 
  &lt;/w:rPr&gt; 
  &lt;w:t&gt;Hello World&lt;/w:t&gt; 
&lt;/w:r&gt; 
[cit. OOXML spec.]</rdfs:comment>
        <Datatype rdf:resource="#bool"/>
    </wordProcessingML>
    


    <!-- http://www.semanticweb.org/ontologies/2008/7/XCLOntology1.5.owl#smoothness -->

    <PDF1.3_Properties rdf:about="#smoothness">
        <rdfs:comment
            >(PDF 1.3) The precision with which color gradients are to be rendered on the output device (see Section 6.5.2, &#8220;Smoothness Tolerance&#8221;). The value of this parameter gives the maximum error tolerance, expressed as a fraction of the range of each color component; smaller numbers give smoother color transitions at the expense of more computation and memory use. Initial value: installation-dependent. [cit. Pdf 1.3]</rdfs:comment>
        <Datatype rdf:resource="#string"/>
    </PDF1.3_Properties>
    


    <!-- http://www.semanticweb.org/ontologies/2008/7/XCLOntology1.5.owl#snapToGrid -->

    <wordProcessingML rdf:about="#snapToGrid">
        <rdfs:comment xml:lang="en"
            >Use Document Grid Settings for Inter-Line Paragraph Spacing
This element specifies whether the current paragraph should use the document grid lines per page settings defined in the docGrid element (&#167;2.6.5) when laying out the contents in the paragraph. This setting determines whether the additional line pitch specified in the document grid shall be added to each line in this paragraph as specified by the document grid. 
If this element is omitted on a given paragraph, its value is determined by the setting previously set at any level of the style hierarchy (i.e. that previous setting remains unchanged). If this setting is never specified in the style hierarchy, then the paragraph shall use the document grid to lay out text when a document grid is defined for this document. 
[Example: Consider two single-spaced paragraphs in a section with a document grid set to allow 15 lines per page. This document grid would effectively specifies that an additional line pitch of 45.6 points shall be added to each line in order to ensure that the resulting page contains only 15 lines of text. 
Values: off/on
[cit. OOXML Spec.]</rdfs:comment>
        <Datatype rdf:resource="#bool"/>
    </wordProcessingML>
    


    <!-- http://www.semanticweb.org/ontologies/2008/7/XCLOntology1.5.owl#sort -->

    <GIF_Properties rdf:about="#sort">
        <rdfs:comment xml:lang="en"
            >Sorted (local or global) ColourMap ordered by the frequency of colour-fields (descending).
0=unsorted (normally)</rdfs:comment>
    </GIF_Properties>
    


    <!-- http://www.semanticweb.org/ontologies/2008/7/XCLOntology1.5.owl#sourceXDimensionUnit -->

    <NISO rdf:about="#sourceXDimensionUnit">
        <rdfs:comment
            >Definition a data element that specifies the unit of measure used in 8.1.3.1.1
enumerated type, restricted to list 
[cit. NISO MIX]</rdfs:comment>
        <Datatype rdf:resource="#string"/>
    </NISO>
    


    <!-- http://www.semanticweb.org/ontologies/2008/7/XCLOntology1.5.owl#sourceXDimensionValue -->

    <NISO rdf:about="#sourceXDimensionValue">
        <rdfs:comment
            >Definition a data element that specifies the width of the imaged object 
Type non-negative real [cit. NISO MIX]</rdfs:comment>
        <Datatype rdf:resource="#int"/>
    </NISO>
    


    <!-- http://www.semanticweb.org/ontologies/2008/7/XCLOntology1.5.owl#space -->

    <wordProcessingML rdf:about="#space">
        <rdfs:comment
            >Specifies the spacing offset that shall be used to place this border on the parent object. 
When a document has a page border that is relative to the page edges (using a value of page in the offsetFrom attribute on pgBorders (&#167;2.6.10)), it shall specify the distance between the edge of the page and the beginning of this border in points. 
When a document has a page border that is relative to the text extents (using a value of text in the offsetFrom attribute on pgBorders (&#167;2.6.10)), or any other border type, it shall specify the distance between the edge of the object and the beginning of this border in points. 
Example: Consider a document with a set of page borders all specified to appear 24 points from the edge of the page. The resulting WordprocessingML would be as follows: 
&lt;w:pgBorders w:offsetFrom=&quot;page&quot;&gt; 
  &lt;w:bottom &#8230; w:space=&quot;24/&gt;
&lt;/w:pgBorders 
The offsetFrom attribute specifies that the space value will provide the offset of the page border from the page edge, and the value of the space attribute specifies that the page offset shall be 24 points. 
[cit. OOXML spec.]</rdfs:comment>
        <Datatype rdf:resource="#int"/>
    </wordProcessingML>
    


    <!-- http://www.semanticweb.org/ontologies/2008/7/XCLOntology1.5.owl#spacing -->

    <wordProcessingML rdf:about="#spacing">
        <rdfs:comment xml:lang="en"
            >Spacing Between Lines and Above/Below Paragraph
This element specifies the inter-line and inter-paragraph spacing which shall be applied to the contents of this paragraph when it is displayed by a consumer. 
If this element is omitted on a given paragraph, each of its values is determined by the setting previously set at any level of the style hierarchy (i.e. that previous setting remains unchanged). If this setting is never specified in the style hierarchy, then the paragraph shall have no spacing applied to its lines, or above and below its contents. 
[Example: Consider the following WordprocessingML paragraph: 
&lt;w:pPr&gt; 
  &lt;w:spacing w:after=&quot;200&quot; w:line=&quot;276&quot; w:lineRule=&quot;auto&quot; /&gt;  
&lt;/w:pPr&gt;
This paragraph specifies that it shall have at least 200 twentieths of a point after the last line in each paragraph, and that the spacing in each line should be automatically calculated based on a 1.15 times (276 divided by 240) the normal single spacing calculation. end example] 
[cit. OOXML Spec.]</rdfs:comment>
        <Datatype rdf:resource="#bool"/>
    </wordProcessingML>
    


    <!-- http://www.semanticweb.org/ontologies/2008/7/XCLOntology1.5.owl#spacingAfter -->

    <wordProcessingML rdf:about="#spacingAfter">
        <rdfs:comment xml:lang="en"
            >spacing after a letter in ooxml bodytext</rdfs:comment>
        <Datatype rdf:resource="#int"/>
    </wordProcessingML>
    


    <!-- http://www.semanticweb.org/ontologies/2008/7/XCLOntology1.5.owl#spacingBefore -->

    <wordProcessingML rdf:about="#spacingBefore">
        <rdfs:comment xml:lang="en"
            >spacing before a letter in ooxml bodytext</rdfs:comment>
        <Datatype rdf:resource="#int"/>
    </wordProcessingML>
    


    <!-- http://www.semanticweb.org/ontologies/2008/7/XCLOntology1.5.owl#specVanish -->

    <wordProcessingML rdf:about="#specVanish">
        <rdfs:comment
            >specVanish (Paragraph Mark Is Always Hidden) 
This element specifies that the given run shall always behave as if it is hidden, even when hidden text is being  displayed in the current document. 
This property shall only be used to specify that a paragraph mark shall never be used to break the end of a paragraph for display, even if it is being shown on the document, as would be the case if a regularly hidden paragraph was not being displayed in the document. [Note: This property was typically used to ensure that a paragraph style can be applied to a part of a paragraph, and still appear as in the Table of Contents (which in previous word processors would ignore the use of the style if it were being used as a character style. end note] If this element is applied to any other run, it may be ignored. 
If this element is not present, the default value is to leave the formatting applied at previous level in the style hierarchy. If this element is never applied in the style hierarchy, then the run properties for the paragraph mark shall not always be treated as if hidden. 
Example: Consider a paragraph mark which never be used to break the end of the paragraph in the document. 
This constraint is specified using the following WordprocessingML: 
&lt;w:pPr&gt; 
  &lt;w:rPr&gt; 
    &lt;w:specVanish /&gt;  
  &lt;/w:rPr&gt; 
&lt;/w:pPr&gt; 
The presence of the specVanish element means that this paragraph mark shall always be treated as hidden (shall never be used to end the paragraph for display), but may be used to mark the end of use of a paragraph style.
[cit. OOXML spec.]</rdfs:comment>
        <Datatype rdf:resource="#bool"/>
    </wordProcessingML>
    


    <!-- http://www.semanticweb.org/ontologies/2008/7/XCLOntology1.5.owl#spotColour -->

    <imageInformation rdf:about="#spotColour">
        <ID>id196</ID>
        <rdfs:comment xml:lang="en"
            >Name of the SpotColour</rdfs:comment>
        <Datatype rdf:resource="#string"/>
    </imageInformation>
    


    <!-- http://www.semanticweb.org/ontologies/2008/7/XCLOntology1.5.owl#squareSideLength -->

    <vectorInformation rdf:about="#squareSideLength">
        <ID>id249</ID>
        <rdfs:comment
            >Length of the side in a square-shaped vector-object</rdfs:comment>
        <Datatype rdf:resource="#int"/>
    </vectorInformation>
    


    <!-- http://www.semanticweb.org/ontologies/2008/7/XCLOntology1.5.owl#stemH -->

    <fontDescriptor rdf:about="#stemH">
        <rdfs:comment xml:lang="en"
            >The thickness, measured vertically, of the dominant horizontal stems of glyphs in the font. Default value: 0. [cit.]</rdfs:comment>
    </fontDescriptor>
    


    <!-- http://www.semanticweb.org/ontologies/2008/7/XCLOntology1.5.owl#stemV -->

    <fontDescriptor rdf:about="#stemV">
        <rdfs:comment xml:lang="en"
            >The thickness, measured horizontally, of the dominant vertical stems of glyphs in the font - required.[cit.]</rdfs:comment>
    </fontDescriptor>
    


    <!-- http://www.semanticweb.org/ontologies/2008/7/XCLOntology1.5.owl#strike -->

    <textInformation rdf:about="#strike">
        <ID>id164</ID>
        <rdfs:comment
            >text-property strike</rdfs:comment>
        <Datatype rdf:resource="#bool"/>
    </textInformation>
    


    <!-- http://www.semanticweb.org/ontologies/2008/7/XCLOntology1.5.owl#strike_OOXML -->

    <wordProcessingML rdf:about="#strike_OOXML">
        <rdfs:comment
            >strike (Single Strikethrough) 
This element specifies that the contents of this run shall be displayed with a single horizontal line through the center of the line. 
This formatting property is a toggle property, which specifies that its behavior differs between its use within a style definition and its use as direct formatting. When used as part of a style definition, setting this property shall toggle the current state of that property as specified up to this point in the hierarchy (i.e. applied to not applied, and vice versa). Setting it to false (or an equivalent) shall result in the current setting remaining unchanged. However, when used as direct formatting, setting this property to true or false shall set the absolute state of the resulting property.  
If this element is not present, the default value is to leave the formatting applied at previous level in the style hierarchy. If this element is never applied in the style hierarchy, then strikethrough shall not be applied to the contents of this run. 
This element shall not be present with the dstrike (&#167;2.3.2.7) property on the same run, since they are mutually exclusive in terms of appearance. 
Example: Consider a run of text which shall have the strike property explicitly turned on for the contents of the 
run. This constraint is specified using the following WordprocessingML: 
&lt;w:rPr&gt; 
  &lt;w:strike w:val=&quot;true&quot;/&gt; 
&lt;/w:rPr&gt; 
This run explicitly declares that the strike property is true, so the contents of this run will have a single horizontal strikethrough line.
[cit. OOXML spec.]</rdfs:comment>
        <Datatype rdf:resource="#bool"/>
    </wordProcessingML>
    


    <!-- http://www.semanticweb.org/ontologies/2008/7/XCLOntology1.5.owl#string -->

    <xcl_propertyDatatypes rdf:about="#string"/>
    


    <!-- http://www.semanticweb.org/ontologies/2008/7/XCLOntology1.5.owl#stripByteCount_Tiff -->

    <Tiff_Properties rdf:about="#stripByteCount_Tiff">
        <rdfs:comment
            >Tag = 279  (117.H) 
Type = SHORT or LONG 
For each strip, the number of bytes in that strip after any compression.
Putting it all together (along with a couple of less-important fields that are discussed later), a sample bilevel image file might contain the following fields</rdfs:comment>
        <is_same_as rdf:resource="#StripByteCounts_NISO"/>
        <Datatype rdf:resource="#int"/>
    </Tiff_Properties>
    


    <!-- http://www.semanticweb.org/ontologies/2008/7/XCLOntology1.5.owl#strokeAdjustment -->

    <PDF1.3_Properties rdf:about="#strokeAdjustment">
        <rdfs:comment
            >(PDF 1.2) A &#64258;ag specifying whether to compensate for possible rasterization effects when stroking a path with a line width that is small relative to the pixel resolution of the output device (see Section 6.5.4, &#8220;Automatic Stroke Adjustment&#8221;). Note that this is considered a device-independent parameter, even though the details of its effects are device-dependent. Initial value: false. [cit. Pdf 1.3]</rdfs:comment>
        <Datatype rdf:resource="#bool"/>
    </PDF1.3_Properties>
    


    <!-- http://www.semanticweb.org/ontologies/2008/7/XCLOntology1.5.owl#strokeDasharray -->

    <vectorInformation rdf:about="#strokeDasharray">
        <rdfs:comment xml:lang="en"
            >length of strokes and gaps in a vector-Dash-Line</rdfs:comment>
        <is_same_as rdf:resource="#LineDashPattern"/>
        <Datatype rdf:resource="#int"/>
    </vectorInformation>
    


    <!-- http://www.semanticweb.org/ontologies/2008/7/XCLOntology1.5.owl#strokeLinecapButt -->

    <vectorInformation rdf:about="#strokeLinecapButt">
        <rdfs:comment xml:lang="en"
            >kind of cap at the end of a vector_line</rdfs:comment>
    </vectorInformation>
    


    <!-- http://www.semanticweb.org/ontologies/2008/7/XCLOntology1.5.owl#strokeLinecapRound -->

    <vectorInformation rdf:about="#strokeLinecapRound">
        <rdfs:comment xml:lang="en"
            >kind of cap at the end of a vector_line</rdfs:comment>
    </vectorInformation>
    


    <!-- http://www.semanticweb.org/ontologies/2008/7/XCLOntology1.5.owl#strokeLinecapSquare -->

    <vectorInformation rdf:about="#strokeLinecapSquare">
        <rdfs:comment xml:lang="en"
            >kind of cap at the end of a vector_line</rdfs:comment>
    </vectorInformation>
    


    <!-- http://www.semanticweb.org/ontologies/2008/7/XCLOntology1.5.owl#subfileType -->

    <Tiff_Properties rdf:about="#subfileType">
        <rdfs:comment
            >A general indication of the kind of data contained in this subfile.
 The specification defines these values:

1 = full-resolution image data
2 = reduced-resolution image data
3 = a single page of a multi-page image (see the PageNumber field description).  [cit. TIFF 6.0] [Compatibility: TIFF 6.0]</rdfs:comment>
        <Datatype rdf:resource="#int"/>
    </Tiff_Properties>
    


    <!-- http://www.semanticweb.org/ontologies/2008/7/XCLOntology1.5.owl#suggestedPaletteAlpha -->

    <rasterInformation rdf:about="#suggestedPaletteAlpha">
        <ID>id56</ID>
        <rdfs:comment xml:lang="en"
            >alpha value for suggested palette</rdfs:comment>
        <Datatype rdf:resource="#int"/>
        <is_same_as rdf:resource="#suggestedPaletteAlphaPNG"/>
    </rasterInformation>
    


    <!-- http://www.semanticweb.org/ontologies/2008/7/XCLOntology1.5.owl#suggestedPaletteAlphaPNG -->

    <PNG_Properties rdf:about="#suggestedPaletteAlphaPNG">
        <is_same_as rdf:resource="#suggestedPaletteAlpha"/>
    </PNG_Properties>
    


    <!-- http://www.semanticweb.org/ontologies/2008/7/XCLOntology1.5.owl#suggestedPaletteFrequency -->

    <rasterInformation rdf:about="#suggestedPaletteFrequency">
        <ID>id57</ID>
        <rdfs:comment xml:lang="en"
            >frequency of suggested palette</rdfs:comment>
        <Datatype rdf:resource="#int"/>
        <is_same_as rdf:resource="#suggestedPaletteFrequencyPNG"/>
    </rasterInformation>
    


    <!-- http://www.semanticweb.org/ontologies/2008/7/XCLOntology1.5.owl#suggestedPaletteFrequencyPNG -->

    <PNG_Properties rdf:about="#suggestedPaletteFrequencyPNG">
        <rdfs:comment xml:lang="en"
            >frequency of suggested palette</rdfs:comment>
        <is_same_as rdf:resource="#suggestedPaletteFrequency"/>
    </PNG_Properties>
    


    <!-- http://www.semanticweb.org/ontologies/2008/7/XCLOntology1.5.owl#suggestedPaletteNamePNG -->

    <PNG_Properties rdf:about="#suggestedPaletteNamePNG">
        <rdfs:comment xml:lang="en"
            >name of a reduced palette that may be used when the display device is not capable of displaying the full range of colours in the image [Compatibility: PNG 1.1]</rdfs:comment>
    </PNG_Properties>
    


    <!-- http://www.semanticweb.org/ontologies/2008/7/XCLOntology1.5.owl#suggestedPaletteRGB -->

    <rasterInformation rdf:about="#suggestedPaletteRGB">
        <rdfs:comment
            >name of a reduced palette that may be used when the display device is not capable of displaying the full range of colours in the image</rdfs:comment>
        <Datatype rdf:resource="#string"/>
    </rasterInformation>
    


    <!-- http://www.semanticweb.org/ontologies/2008/7/XCLOntology1.5.owl#suggestedPaletteSampleDepth -->

    <PNG_Properties rdf:about="#suggestedPaletteSampleDepth">
        <rdfs:comment xml:lang="en"
            >sample depth of a suggested palette [Compatibility: PNG 1.1]</rdfs:comment>
    </PNG_Properties>
    


    <!-- http://www.semanticweb.org/ontologies/2008/7/XCLOntology1.5.owl#suppressAutoHyphens -->

    <wordProcessingML rdf:about="#suppressAutoHyphens">
        <rdfs:comment xml:lang="en"
            >Suppress Hyphenation for Paragraph
This element specifies whether any hyphenation shall be performed on this paragraph by the consumer when requested using the autoHyphenation element (&#167;2.15.1.10) in the document&#39;s settings. This element specifies whether the current paragraph should be exempted from any hyphenation which is applied by the consumer on this document. 
If this element is omitted on a given paragraph, its value is determined by the setting previously set at any level of the style hierarchy (i.e. that previous setting remains unchanged). If this setting is never specified in the style hierarchy, then the default hyphenation settings for the document, as specified in the autoHyphenation element, shall apply to the contents of this paragraph. 
[Example: Consider a document which shall be hyphenated automatically by a consumer, since it has the autoHyphenation element set to true in its document settings. If this paragraph should be exempted from that hyphenation pass, this requirement would be specified using the following WordprocessingML: 
&lt;w:pPr&gt; 
  &lt;w:suppressAutoHyphens /&gt; 
&lt;/w:pPr&gt; 
The paragraph would then be exempted from hyphenation by a consumer at display time, regardless of the hyphenation settings for the document. end example] 
[cit. OOXML Spec.]
Values: On/Off</rdfs:comment>
        <Datatype rdf:resource="#bool"/>
    </wordProcessingML>
    


    <!-- http://www.semanticweb.org/ontologies/2008/7/XCLOntology1.5.owl#suppressLineNumbers -->

    <wordProcessingML rdf:about="#suppressLineNumbers">
        <rdfs:comment xml:lang="en"
            >Suppress Line Numbers for Paragraph
This element specifies whether line numbers shall be calculated for lines in this paragraph by the consumer when line numbering is requested using the lnNumType element (&#167;2.6.8) in the paragraph&#39;s parent section settings. This element specifies whether the current paragraph&#39;s lines should be exempted from line numbering which is applied by the consumer on this document, not just suppressing the display of the numbering, but removing these lines from the line numbering calculation. 
If this element is omitted on a given paragraph, its value is determined by the setting previously set at any level of the style hierarchy (i.e. that previous setting remains unchanged). If this setting is never specified in the style hierarchy, then the default line number settings for the section, as specified in the lnNumType element shall apply to each line of this paragraph. 
[Example: Consider a document with three paragraphs, each of which are displayed on five lines , all contained in a section which has  the lnNumType element specified. If the second paragraph should be exempted from that line numbering, this requirement would be specified using the following WordprocessingML: 
&lt;w:pPr&gt; 
  &lt;w:suppressLineNumbers /&gt; 
&lt;/w:pPr&gt; 
The paragraph would then be exempted from line by a consumer at display time, which would result in paragraph one using line numbers one through five, the second paragraph having no line numbers, and the third paragraph using line numbers six through ten. end example]
Values: On/Off
[cit. OOXML Spec.]</rdfs:comment>
        <Datatype rdf:resource="#bool"/>
    </wordProcessingML>
    


    <!-- http://www.semanticweb.org/ontologies/2008/7/XCLOntology1.5.owl#suppressOverlap -->

    <wordProcessingML rdf:about="#suppressOverlap">
        <rdfs:comment xml:lang="en"
            >This element specifies whether a text frame which intersects another text frame at display time shall be allowed to overlap the contents of the other text frame. If a text frame cannot overlap other text frames, it shall be repositioned when displayed to prevent this overlap as needed. 
If this element is omitted on a given paragraph, its value is determined by the setting previously set at any level of the style hierarchy (i.e. that previous setting remains unchanged). If this setting is never specified in the style hierarchy, then overlap shall be allowed between a text frame which intersects another text frame displayed at the same location. 
[cit. OOXMl spec.]</rdfs:comment>
        <Unit rdf:resource="#NULL"/>
        <Datatype rdf:resource="#bool"/>
    </wordProcessingML>
    


    <!-- http://www.semanticweb.org/ontologies/2008/7/XCLOntology1.5.owl#swop -->

    <imageInformation rdf:about="#swop">
        <rdfs:comment
            >ICC Colour Profile</rdfs:comment>
        <ID>id239</ID>
    </imageInformation>
    


    <!-- http://www.semanticweb.org/ontologies/2008/7/XCLOntology1.5.owl#sz -->

    <wordProcessingML rdf:about="#sz">
        <rdfs:comment xml:lang="en"
            >size of characters in ooxml
Example:
&lt;w:rPr&gt; 
  &lt;w:sz w:val=&quot;27&quot;/&gt; 
&lt;/w:rPr&gt; 
[cit. OOXML spec.]</rdfs:comment>
        <Datatype rdf:resource="#int"/>
    </wordProcessingML>
    


    <!-- http://www.semanticweb.org/ontologies/2008/7/XCLOntology1.5.owl#szCs -->

    <wordProcessingML rdf:about="#szCs">
        <rdfs:comment
            >szCs (Complex Script Font Size) 
This element specifies the font size which shall be applied to all complex script characters in the contents of this run when displayed. 
If this element is not present, the default value is to leave the value applied at previous level in the style hierarchy. If this element is never applied in the style hierarchy, then any appropriate font size may be used for complex script characters. 
Example: Consider a run of text which shall have an explicit font size of 10 points for the complex script contents of the run. This constraint is specified using the following WordprocessingML: 
&lt;w:rPr&gt; 
  &lt;w:szCs w:val=&quot;20&quot;/&gt; 
&lt;/w:rPr&gt; 
This run explicitly declares that the sz property is 20 half-point for the non-complex script contents of this run, so the text will be displayed in 10 point font size.
Val: Specifies a positive measurement specified in half-points (1/144 of an inch). 
[cit. OOXML spec.]</rdfs:comment>
        <Datatype rdf:resource="#int"/>
    </wordProcessingML>
    


    <!-- http://www.semanticweb.org/ontologies/2008/7/XCLOntology1.5.owl#tEXt -->

    <PNG_Properties rdf:about="#tEXt">
        <rdfs:comment xml:lang="en"
            >PNG-Chunk containing Latin-1-encoded Text.
can be compressed textual data (with deflate of zlib). The flag is then 0, uncompressed is 1</rdfs:comment>
        <is_same_as rdf:resource="#textData"/>
    </PNG_Properties>
    


    <!-- http://www.semanticweb.org/ontologies/2008/7/XCLOntology1.5.owl#tIME -->

    <PNG_Properties rdf:about="#tIME">
        <rdfs:comment xml:lang="en"
            >chunk that containes the time, the file was last changed.
It contains:
Year 	2 bytes (complete; for example, 1995, not 95)
Month 	1 byte (1-12)
Day 	1 byte (1-31)
Hour 	1 byte (0-23)
Minute 	1 byte (0-59)
Second 	1 byte (0-60) (to allow for leap seconds)

Universal Time (UTC) should be specified rather than local time.</rdfs:comment>
        <is_same_as rdf:resource="#timeLastMod"/>
    </PNG_Properties>
    


    <!-- http://www.semanticweb.org/ontologies/2008/7/XCLOntology1.5.owl#tRNS -->

    <PNG_Properties rdf:about="#tRNS">
        <rdfs:comment xml:lang="en"
            >PNG-Chunk that containes the value for a simple transparency-colour (in opposite to alpha-channels).
For indexed images, it stores alpha channel values for one or more palette entries. For truecolour and greyscale images (greyscale) and colour_type2 (simple true-colour), it stores a single pixel value that is to be regarded as fully transparent.</rdfs:comment>
    </PNG_Properties>
    


    <!-- http://www.semanticweb.org/ontologies/2008/7/XCLOntology1.5.owl#tab -->

    <wordProcessingML rdf:about="#tab">
        <rdfs:comment xml:lang="en"
            >tab (Custom Tab Stop) 
This element specifies a single custom tab stop within a set of custom tab stops applied as part of a set of customized paragraph properties in a document. 
[Example: Consider a custom tab stops at 1.5&quot; in a WordprocessingML document. This tab stop would be contained within a tab element defining the tab stop as follows: 
&lt;w:tab w:val=&quot;left&quot; w:pos=&quot;2160&quot; /&gt;
[cit. OOCML spec.]</rdfs:comment>
        <Datatype rdf:resource="#int"/>
    </wordProcessingML>
    


    <!-- http://www.semanticweb.org/ontologies/2008/7/XCLOntology1.5.owl#tableBorder -->

    <textInformation rdf:about="#tableBorder">
        <ID>id278</ID>
        <rdfs:comment
            >width of outline in a table (messured in documentUnit)</rdfs:comment>
        <Datatype rdf:resource="#int"/>
    </textInformation>
    


    <!-- http://www.semanticweb.org/ontologies/2008/7/XCLOntology1.5.owl#tableBorderColour -->

    <textInformation rdf:about="#tableBorderColour">
        <ID>id279</ID>
        <rdfs:comment
            >Colour of tableBorder in ColourSpace of Document</rdfs:comment>
        <Datatype rdf:resource="#int"/>
    </textInformation>
    


    <!-- http://www.semanticweb.org/ontologies/2008/7/XCLOntology1.5.owl#tableNumberOfColumns -->

    <textInformation rdf:about="#tableNumberOfColumns">
        <rdfs:comment
            >Number of Columns in a Table</rdfs:comment>
        <ID>id202</ID>
        <Datatype rdf:resource="#int"/>
    </textInformation>
    


    <!-- http://www.semanticweb.org/ontologies/2008/7/XCLOntology1.5.owl#tableNumberOfRows -->

    <textInformation rdf:about="#tableNumberOfRows">
        <ID>id201</ID>
        <rdfs:comment
            >Number of Rows in a Table</rdfs:comment>
        <Datatype rdf:resource="#int"/>
    </textInformation>
    


    <!-- http://www.semanticweb.org/ontologies/2008/7/XCLOntology1.5.owl#tabs -->

    <wordProcessingML rdf:about="#tabs">
        <rdfs:comment xml:lang=""
            >tabs (Set of Custom Tab Stops) 
Specifies the type of vertical alignment which shall be used to align the characters on each line in the current paragraph. 
[Example: Consider a paragraph of text of different font sizes which shall be aligned based on the baseline point of each character in each line. This requirement would be specified as follows in the WordprocessingML: 
&lt;w:pPr&gt; 
  &lt;w:textAlignment w:val=&quot;baseLine&quot; /&gt; 
&lt;/w:pPr&gt; 
The resulting text would be aligned to the baseline for each character on the line. [cit. OOXML spec.]</rdfs:comment>
        <Datatype rdf:resource="#int"/>
    </wordProcessingML>
    


    <!-- http://www.semanticweb.org/ontologies/2008/7/XCLOntology1.5.owl#textAdjustment -->

    <textInformation rdf:about="#textAdjustment">
        <ID>id191</ID>
        <rdfs:comment
            >Adjustment of text in document (left, center, right, justification)</rdfs:comment>
        <Datatype rdf:resource="#string"/>
    </textInformation>
    


    <!-- http://www.semanticweb.org/ontologies/2008/7/XCLOntology1.5.owl#textAlignment -->

    <wordProcessingML rdf:about="#textAlignment">
        <rdfs:comment
            >textAlignment (Vertical Character Alignment on Line) 
This element specifies the vertical alignment of all text on each line displayed within a paragraph. If the line height (before any added spacing) is larger than one or more characters on the line, all characters will be aligned to each other as specified by this element. 
If this element is omitted on a given paragraph, its value is determined by the setting previously set at any level of the style hierarchy (i.e. that previous setting remains unchanged). If this setting is never specified in the style hierarchy, then the vertical alignment of all characters on the line shall be automatically determined by the consumer.
example: 
&lt;w:pPr&gt; 
  &lt;w:textAlignment w:val=&quot;top&quot; /&gt; 
&lt;/w:pPr&gt; 
possible values:
buttom/center/top/auto/baseline
[cit. OOXML spec.]</rdfs:comment>
        <Datatype rdf:resource="#string"/>
    </wordProcessingML>
    


    <!-- http://www.semanticweb.org/ontologies/2008/7/XCLOntology1.5.owl#textData -->

    <otherInformation rdf:about="#textData">
        <ID>id214</ID>
        <Datatype rdf:resource="#string"/>
        <is_same_as rdf:resource="#tEXt"/>
        <is_same_as rdf:resource="#textualDataString"/>
    </otherInformation>
    


    <!-- http://www.semanticweb.org/ontologies/2008/7/XCLOntology1.5.owl#textDirection -->

    <wordProcessingML rdf:about="#textDirection">
        <rdfs:comment
            >This element specifies the direction of the text flow for this paragraph. 
If this element is omitted on a given paragraph, its value is determined by the setting previously set at any level of the style hierarchy (i.e. that previous setting remains unchanged). If this setting is never specified in the style hierarchy, then the paragraph shall inherit the text flow settings from the parent section. 
Possible values:
btLr (Bottom to Top, Left to Right)
lrTb (Left to Right, Top to Bottom)
lrTbV (Left to Right, Top to Bottom Rotated)
tbLrV (Top to Bottom, Left to Right Rotated)
tbRl (Top to Bottom, Right to Left)
tbRlV (Top to Bottom, Right to Left Rotated)
[cit. OOXMl spec.]</rdfs:comment>
        <Datatype rdf:resource="#string"/>
    </wordProcessingML>
    


    <!-- http://www.semanticweb.org/ontologies/2008/7/XCLOntology1.5.owl#textboxTightWrap -->

    <wordProcessingML rdf:about="#textboxTightWrap">
        <rdfs:comment xml:lang=""
            >textboxTightWrap (Allow Surrounding Paragraphs to Tight Wrap to Text Box Contents):
This element specifies whether, for paragraphs in a text box, the surrounding text shall be allowed to overlap with the empty text box boundaries and tight wrap to the extents of the text within the text box. This element shall only be read for paragraphs which are contained within a text box (have a txbxContent ancestor), ignored otherwise.  
If the parent text box does not meet the following three criteria, then this property has no effect: 
The text box wrapping must be set to tight 
The text box border must not be set 
The text box shading must not be set 
If this element is omitted on a given paragraph, its value is determined by the setting previously set at any level of the style hierarchy (i.e. that previous setting remains unchanged). If this setting is never specified in the style hierarchy, then paragraphs in a text box have no tight wrapping overrides, and text shall wrap to the extents of the text box. The possible values for this attribute are defined by the ST_TextboxTightWrap simple 
type
Example: 
&lt;w:pPr&gt; 
  &lt;w:textboxTightWrap w:val=&quot;all&quot; /&gt; 
&lt;/w:pPr&gt;</rdfs:comment>
        <Datatype rdf:resource="#string"/>
    </wordProcessingML>
    


    <!-- http://www.semanticweb.org/ontologies/2008/7/XCLOntology1.5.owl#textualAnnotation -->

    <generalInformation rdf:about="#textualAnnotation">
        <rdfs:comment xml:lang="en"
            >general textual Annotation - not formatted in any kind of metadata-standards like METS</rdfs:comment>
        <ID>id58</ID>
        <is_same_as rdf:resource="#documentKeywords"/>
        <is_same_as rdf:resource="#imageDescription"/>
        <Datatype rdf:resource="#string"/>
        <is_same_as rdf:resource="#textualDataKeyword"/>
    </generalInformation>
    


    <!-- http://www.semanticweb.org/ontologies/2008/7/XCLOntology1.5.owl#textualDataKeyword -->

    <PNG_Properties rdf:about="#textualDataKeyword">
        <is_same_as rdf:resource="#textualAnnotation"/>
    </PNG_Properties>
    


    <!-- http://www.semanticweb.org/ontologies/2008/7/XCLOntology1.5.owl#textualDataLanguage -->

    <Tiff_Properties rdf:about="#textualDataLanguage">
        <is_same_as rdf:resource="#documentLanguage"/>
    </Tiff_Properties>
    


    <!-- http://www.semanticweb.org/ontologies/2008/7/XCLOntology1.5.owl#textualDataString -->

    <PNG_Properties rdf:about="#textualDataString">
        <is_same_as rdf:resource="#textData"/>
    </PNG_Properties>
    


    <!-- http://www.semanticweb.org/ontologies/2008/7/XCLOntology1.5.owl#themeColor -->

    <wordProcessingML rdf:about="#themeColor">
        <rdfs:comment xml:lang="en"
            >This simple type specifies a theme color to be applied to the current object. The specified theme color is a reference to one of the predefined theme colors, located in the document&#39;s Theme part, which allows color information to be set centrally in the document. 
[Example: Consider a set of borders configured to use the accent2 theme color, resulting in the following WordprocessingML markup: 
&lt;w:top &#8230; w:color=&quot;FFA8A0&quot; w:themeColor=&quot;accent2&quot; w:themeTint=&quot;99&quot; /&gt;
&lt;w:bottom &#8230; w:color=&quot;FFA8A0&quot; w:themeColor=&quot;accent2&quot; w:themeTint=&quot;99&quot; /&gt; 
&lt;w:left &#8230; w:color=&quot;FFA8A0&quot; w:themeColor=&quot;accent2&quot; w:themeTint=&quot;99&quot; /&gt;
&lt;w:right &#8230; w:color=&quot;FFA8A0&quot; w:themeColor=&quot;accent2&quot; w:themeTint=&quot;99&quot; /&gt;
The borders have a themeColor attribute of type ST_ThemeColor that when specified, imports the accent2 theme color specified for this document. end example] This simple type&#39;s contents are a restriction of the XML Schema string datatype. [cit. OOXML spec.]</rdfs:comment>
        <Datatype rdf:resource="#hex"/>
    </wordProcessingML>
    


    <!-- http://www.semanticweb.org/ontologies/2008/7/XCLOntology1.5.owl#themeTint -->

    <wordProcessingML rdf:about="#themeTint">
        <rdfs:comment
            >Specifies the tint value applied to the supplied theme color (if any).
If the themeTint is supplied, then it is applied to the RGB value of the theme color (from the theme part) to determine the final color applied to this border. 
The themeTint value is stored as a hex encoding of the tint value (from 0&#8211;255) applied to the current border. 
Example: Consider a tint of 60% applied to a border in a document. This tint is calculated as follows: 
Txml=0.6+255=153=99(hex)
The resulting themeTint value in the file format would be 99. 
[cit. OOXML spec.]</rdfs:comment>
        <Datatype rdf:resource="#hex"/>
    </wordProcessingML>
    


    <!-- http://www.semanticweb.org/ontologies/2008/7/XCLOntology1.5.owl#thresholding -->

    <Tiff_Properties rdf:about="#thresholding">
        <rdfs:comment
            >For black and white TIFF files that represent shades of gray, the technique used to convert from gray to black and white pixels [TIFF 6.0]</rdfs:comment>
        <Datatype rdf:resource="#int"/>
    </Tiff_Properties>
    


    <!-- http://www.semanticweb.org/ontologies/2008/7/XCLOntology1.5.owl#tileByteCounts_Tiff -->

    <Tiff_Properties rdf:about="#tileByteCounts_Tiff">
        <rdfs:comment
            >For each tile, the number of (compressed) bytes in that tile. (325)</rdfs:comment>
        <is_same_as rdf:resource="#TileByteCounts_NISO"/>
        <Datatype rdf:resource="#int"/>
    </Tiff_Properties>
    


    <!-- http://www.semanticweb.org/ontologies/2008/7/XCLOntology1.5.owl#tileLength_Tiff -->

    <Tiff_Properties rdf:about="#tileLength_Tiff">
        <rdfs:comment
            >The tile length (height) in pixels. This is the number of rows in each tile. (323)</rdfs:comment>
        <Datatype rdf:resource="#int"/>
    </Tiff_Properties>
    


    <!-- http://www.semanticweb.org/ontologies/2008/7/XCLOntology1.5.owl#tileOffset_Tiff -->

    <Tiff_Properties rdf:about="#tileOffset_Tiff">
        <rdfs:comment
            >For each tile, the byte offset of that tile, as compressed and stored on disk (324)</rdfs:comment>
        <is_same_as rdf:resource="#TileOffsets_NISO"/>
        <Datatype rdf:resource="#int"/>
    </Tiff_Properties>
    


    <!-- http://www.semanticweb.org/ontologies/2008/7/XCLOntology1.5.owl#tileWidth_Tiff -->

    <Tiff_Properties rdf:about="#tileWidth_Tiff">
        <rdfs:comment
            >The tile width in pixels. This is the number of columns in each tile (322)</rdfs:comment>
        <is_same_as rdf:resource="#TileWidth_NISO"/>
        <Datatype rdf:resource="#int"/>
    </Tiff_Properties>
    


    <!-- http://www.semanticweb.org/ontologies/2008/7/XCLOntology1.5.owl#timeISO8601 -->

    <xcl_propertyDatatypes rdf:about="#timeISO8601"/>
    


    <!-- http://www.semanticweb.org/ontologies/2008/7/XCLOntology1.5.owl#timeLastMod -->

    <PNG_Properties rdf:about="#timeLastMod">
        <rdfs:comment xml:lang="en"
            >Date of last modification</rdfs:comment>
        <is_same_as rdf:resource="#documentModificationDate"/>
    </PNG_Properties>
    


    <!-- http://www.semanticweb.org/ontologies/2008/7/XCLOntology1.5.owl#timeStamp -->

    <videoinformation rdf:about="#timeStamp">
        <ID>id280</ID>
        <Datatype rdf:resource="#timeISO8601"/>
    </videoinformation>
    


    <!-- http://www.semanticweb.org/ontologies/2008/7/XCLOntology1.5.owl#top -->

    <wordProcessingML rdf:about="#top">
        <rdfs:comment
            >(Top Border):
This element specifies the presentation and display of the page border displayed at the top of each page in this section. 
Example: 
&lt;w:sectPr&gt; 
  &#8230; 
  &lt;w:pgBorders&gt; 
    &lt;w:top w:val=&quot;balloons&quot;
&#8230; w:color=&quot;FFA8A0&quot; w:themeColor=&quot;accent2&quot; 
w:themeTint=&quot;99&quot; /&gt;
  &lt;/w:pgBorders&gt; 
  &#8230; 
&lt;/w:sectPr&gt;
[cit. OOXML spec.]</rdfs:comment>
        <Unit rdf:resource="#NULL"/>
    </wordProcessingML>
    


    <!-- http://www.semanticweb.org/ontologies/2008/7/XCLOntology1.5.owl#topLinePunct -->

    <wordProcessingML rdf:about="#topLinePunct">
        <rdfs:comment
            >topLinePunct (Compress Punctuation at Start of a Line) 
This element specifies whether punctuation shall be compressed when it appears as the first character in a line, allowing subsequent characters on the line to be move in accordingly. 
If this element is omitted on a given paragraph, its value is determined by the setting previously set at any level of the style hierarchy (i.e. that previous setting remains unchanged). If this setting is never specified in the style hierarchy, then punctuation shall not be compressed in this paragraph, even when it appears at the start of a line. 
Example: Consider a paragraph which should allow punctuation at the start of a line to be compressed, in order to prevent it from taking up unnecessary space. This constraint is specified using the following 
WordprocessingML: 
&lt;w:pPr&gt; 
  &lt;w:topLinePunct w:val=&quot;on&quot; /&gt; 
&lt;/w:pPr&gt; 
The topLinePunct element specifies that this compression shall be allowed when displaying this paragraph.
[cit. OOXML spec.]</rdfs:comment>
        <Datatype rdf:resource="#bool"/>
    </wordProcessingML>
    


    <!-- http://www.semanticweb.org/ontologies/2008/7/XCLOntology1.5.owl#transfer -->

    <PDF1.3_Properties rdf:about="#transfer">
        <rdfs:comment
            >(PDF 1.2) A function that adjusts device gray or color component levels to compensate for nonlinear response in a particular output device (see Section 6.3, &#8220;Transfer Functions&#8221;). Initial value: installation-dependent. [cit. Pdf 1.3]</rdfs:comment>
        <Datatype rdf:resource="#string"/>
    </PDF1.3_Properties>
    


    <!-- http://www.semanticweb.org/ontologies/2008/7/XCLOntology1.5.owl#trueType1 -->

    <textInformation rdf:about="#trueType1">
        <ID>id219</ID>
        <is_same_as rdf:resource="#TrueType_pdf"/>
        <Datatype rdf:resource="#XCLLabel"/>
    </textInformation>
    


    <!-- http://www.semanticweb.org/ontologies/2008/7/XCLOntology1.5.owl#trueType3 -->

    <textInformation rdf:about="#trueType3">
        <ID>id220</ID>
        <Datatype rdf:resource="#XCLLabel"/>
    </textInformation>
    


    <!-- http://www.semanticweb.org/ontologies/2008/7/XCLOntology1.5.owl#u -->

    <wordProcessingML rdf:about="#u">
        <rdfs:comment
            >u (Underline) 
This element specifies that the contents of this run should be displayed along with an underline appearing directly below the character height (less all spacing above and below the characters on the line).  
If this element is not present, the default value is to leave the formatting applied at previous level in the style hierarchy. If this element is never applied in the style hierarchy, then an underline shall not be applied to the contents of this run. 
Example: Consider a run of text which shall have a double underline explicitly turned on for the contents of the run. This constraint is specified using the following WordprocessingML: 
&lt;w:rPr&gt; 
  &lt;w:u w:val=&quot;double&quot;/&gt; 
&lt;/w:rPr&gt; 
The val of the underline on this run is double, so the style of the underline on this run shall be a double line
This run explicitly declares an underline using the u property. The val of that underline is double, so the style of the underline on this run shall be a double line.
Possible Values:
&quot;single&quot; &quot;words&quot; &quot;double&quot; &quot;thick&quot; &quot;dotted&quot; &quot;dottedHeavy&quot; &quot;dash&quot; &quot;dashedHeavy&quot; &quot;dashLong&quot; &quot;dashLongHeavy&quot; &quot;dotDash&quot; &quot;dashDotHeavy&quot; &quot;dotDotDash&quot; &quot;dashDotDotHeavy&quot; &quot;wave&quot; &quot;wavyHeavy&quot; &quot;wavyDouble&quot; &quot;none&quot;
[cit. OOXML spec.]</rdfs:comment>
        <Datatype rdf:resource="#string"/>
    </wordProcessingML>
    


    <!-- http://www.semanticweb.org/ontologies/2008/7/XCLOntology1.5.owl#uiName -->

    <wordProcessingML rdf:about="#uiName">
        <rdfs:comment xml:lang="en"
            >User-given name of the Paragraph-/character-Style in OOXML</rdfs:comment>
        <Datatype rdf:resource="#string"/>
    </wordProcessingML>
    


    <!-- http://www.semanticweb.org/ontologies/2008/7/XCLOntology1.5.owl#uint16 -->

    <xcl_propertyDatatypes rdf:about="#uint16"/>
    


    <!-- http://www.semanticweb.org/ontologies/2008/7/XCLOntology1.5.owl#uint32 -->

    <xcl_propertyDatatypes rdf:about="#uint32"/>
    


    <!-- http://www.semanticweb.org/ontologies/2008/7/XCLOntology1.5.owl#uint32Rational -->

    <xcl_propertyDatatypes rdf:about="#uint32Rational"/>
    


    <!-- http://www.semanticweb.org/ontologies/2008/7/XCLOntology1.5.owl#uint8 -->

    <xcl_propertyDatatypes rdf:about="#uint8"/>
    


    <!-- http://www.semanticweb.org/ontologies/2008/7/XCLOntology1.5.owl#uncolouredTilling -->

    <PDF1.3_Properties rdf:about="#uncolouredTilling">
        <rdfs:comment xml:lang="en"
            >PDF-Pattern Property</rdfs:comment>
    </PDF1.3_Properties>
    


    <!-- http://www.semanticweb.org/ontologies/2008/7/XCLOntology1.5.owl#undercolorRemoval -->

    <PDF1.3_Properties rdf:about="#undercolorRemoval">
        <rdfs:comment
            >(PDF 1.2) A function that calculates the reduction in the levels of cyan, magenta, and yellow colorants to compensate for the amount of black added by black generation (see Section 6.2.3, &#8220;Conversion from DeviceRGB to DeviceCMYK&#8221;). Initial value: installation dependent. [cit. Pdf 1.3]</rdfs:comment>
        <Datatype rdf:resource="#string"/>
    </PDF1.3_Properties>
    


    <!-- http://www.semanticweb.org/ontologies/2008/7/XCLOntology1.5.owl#underline -->

    <textInformation rdf:about="#underline">
        <rdfs:comment
            >text-property underline</rdfs:comment>
        <ID>id163</ID>
        <Datatype rdf:resource="#bool"/>
        <is_same_as rdf:resource="#u"/>
    </textInformation>
    


    <!-- http://www.semanticweb.org/ontologies/2008/7/XCLOntology1.5.owl#uppercaseLetters -->

    <textInformation rdf:about="#uppercaseLetters">
        <ID>id212</ID>
        <is_same_as rdf:resource="#AllCap"/>
    </textInformation>
    


    <!-- http://www.semanticweb.org/ontologies/2008/7/XCLOntology1.5.owl#utf16 -->

    <textInformation rdf:about="#utf16">
        <rdfs:comment
            >Defines the text_Encoding type of the normdata</rdfs:comment>
        <ID>id299</ID>
    </textInformation>
    


    <!-- http://www.semanticweb.org/ontologies/2008/7/XCLOntology1.5.owl#utf32 -->

    <textInformation rdf:about="#utf32">
        <ID>id300</ID>
    </textInformation>
    


    <!-- http://www.semanticweb.org/ontologies/2008/7/XCLOntology1.5.owl#utf7 -->

    <textInformation rdf:about="#utf7">
        <ID>id297</ID>
    </textInformation>
    


    <!-- http://www.semanticweb.org/ontologies/2008/7/XCLOntology1.5.owl#utf8 -->

    <textInformation rdf:about="#utf8">
        <ID>id298</ID>
    </textInformation>
    


    <!-- http://www.semanticweb.org/ontologies/2008/7/XCLOntology1.5.owl#vAlign -->

    <wordProcessingML rdf:about="#vAlign">
        <rdfs:comment
            >vAlign (Vertical Text Alignment on Page) 
This element specifies the vertical alignment for text on pages in the current section, relative to the top and bottom margins in the main document story on each page. 
Consider a section used as a title page on which text shall be vertically centered. In order to center the text vertically on the page, the following WordprocessingML is used: 
&lt;w:sectPr&gt; 
  &#8230; 
  &lt;w:vAlign w:val=&quot;center&quot; /&gt; 
&lt;/w:sectPr&gt; 
The vAlign value of center specifies that text shall be laid out in the center of the top and bottom text margins for all pages in this section.
[cit. OOXML spec.]</rdfs:comment>
        <Datatype rdf:resource="#string"/>
    </wordProcessingML>
    


    <!-- http://www.semanticweb.org/ontologies/2008/7/XCLOntology1.5.owl#vanish -->

    <wordProcessingML rdf:about="#vanish">
        <rdfs:comment
            >vanish (Hidden Text) 
This element specifies whether the contents of this run shall be hidden from display at display time in a document. [Note: The setting should affect the normal display of text, but an application may have settings to force hidden text to be displayed. end note] 
This formatting property is a toggle property, which specifies that its behavior differs between its use within a style definition and its use as direct formatting. When used as part of a style definition, setting this property shall toggle the current state of that property as specified up to this point in the hierarchy (i.e. applied to not applied, and vice versa). Setting it to false (or an equivalent) shall result in the current setting remaining unchanged. However, when used as direct formatting, setting this property to true or false shall set the absolute state of the resulting property.  
If this element is not present, the default value is to leave the formatting applied at previous level in the style hierarchy .If this element is never applied in the style hierarchy, then this text shall not be hidden when displayed in a document. 
Example: Consider a run of text which shall have the hidden text property turned on for the contents of the run. 
This constraint is specified using the following WordprocessingML: 
&lt;w:rPr&gt; 
  &lt;w:vanish /&gt; 
&lt;/w:rPr&gt; 
This run declares that the vanish property is set for the contents of this run, so the contents of this run will be hidden when the document contents are displayed.
[cit. OOXML spec.]</rdfs:comment>
        <Datatype rdf:resource="#bool"/>
    </wordProcessingML>
    


    <!-- http://www.semanticweb.org/ontologies/2008/7/XCLOntology1.5.owl#vectorUnit -->

    <vectorInformation rdf:about="#vectorUnit">
        <ID>id259</ID>
        <rdfs:comment
            >Unit which defines objects in a vectorImage</rdfs:comment>
        <Datatype rdf:resource="#string"/>
    </vectorInformation>
    


    <!-- http://www.semanticweb.org/ontologies/2008/7/XCLOntology1.5.owl#vert -->

    <wordProcessingML rdf:about="#vert">
        <rdfs:comment
            >vert (Horizontal in Vertical (Rotate Text)) 
Specifies that characters in this run should be rendered with a 270 degree rotation to the left from all other contents of the line when displayed in the document as described If this attribute is omitted, then the contents of this run shall not be rotated with respect to the normal text flow.  
Example: Consider a paragraph with the text this word is vertical, of which the word vertical shall be displayed vertically within the document. This constraint would be specified as follows in the WordprocessingML: 
&lt;w:r&gt; 
  &lt;w:rPr&gt; 
    &lt;w:eastAsianLayout w:id=&quot;2&quot; w:vert=&quot;on&quot; /&gt; 
  &lt;/w:rPr&gt; 
  &lt;w:t&gt;vertical&lt;/w:t&gt; 
&lt;/w:r&gt; 
The resulting text would be displayed with a 270 degree rotation from the other text content. 
[cit. OOXML spec.]</rdfs:comment>
        <Datatype rdf:resource="#bool"/>
    </wordProcessingML>
    


    <!-- http://www.semanticweb.org/ontologies/2008/7/XCLOntology1.5.owl#vertAlign -->

    <wordProcessingML rdf:about="#vertAlign">
        <rdfs:comment
            >vertAlign (Subscript/Superscript Text)
This element specifies the alignment which shall be applied to the contents of this run in relation to the default appearance of the run&#39;s text. This allows the text to be repositioned as subscript or superscript without altering the font size of the run properties. 
If this element is not present, the default value is to leave the formatting applied at previous level in the style hierarchy. If this element is never applied in the style hierarchy, then the text shall not be subscript or superscript relative to the default baseline location for the contents of this run. 
Example: Consider a run which shall be positioning as superscript when displaying its contents. This requirement would be specified using the following WordprocessingML: 
&lt;w:rPr&gt; 
  &lt;w:vertAlign w:val=&quot;superscript&quot; /&gt; 
&lt;/w:rPr&gt; 
The resulting run is positioned as superscript, therefore it is rendered in a smaller size above the default baseline location for the contents of the run.
Possbile Values:
&quot;baseline&quot; &quot;superscript&quot; &quot;subscript&quot;
[cit. OOXML spec.]</rdfs:comment>
        <Datatype rdf:resource="#string"/>
    </wordProcessingML>
    


    <!-- http://www.semanticweb.org/ontologies/2008/7/XCLOntology1.5.owl#verticalSizeVector -->

    <vectorInformation rdf:about="#verticalSizeVector">
        <rdfs:comment
            >vertical size of vectorImage in defined vector-unit</rdfs:comment>
        <ID>id258</ID>
        <Datatype rdf:resource="#uint32Rational"/>
    </vectorInformation>
    


    <!-- http://www.semanticweb.org/ontologies/2008/7/XCLOntology1.5.owl#videoCodec -->

    <videoinformation rdf:about="#videoCodec">
        <ID>id177</ID>
        <Datatype rdf:resource="#string"/>
    </videoinformation>
    


    <!-- http://www.semanticweb.org/ontologies/2008/7/XCLOntology1.5.owl#videoData -->

    <otherInformation rdf:about="#videoData"/>
    


    <!-- http://www.semanticweb.org/ontologies/2008/7/XCLOntology1.5.owl#view -->

    <wordProcessingML rdf:about="#view"/>
    


    <!-- http://www.semanticweb.org/ontologies/2008/7/XCLOntology1.5.owl#w -->

    <wordProcessingML rdf:about="#w">
        <rdfs:comment
            >w (Expanded/Compressed Text) 
This element specifies the amount by which each character shall be expanded or when the character is rendered in the document. This property has an of stretching or compressing each character in the run, as opposed to the spacing element (&#167;2.3.2.33) which expands/compresses the text by adding additional character pitch but not changing the width of the actual characters displayed on the line. 
If this element is not present, the default value is to leave the formatting applied at previous level in the style hierarchy. If this element is never applied in the style hierarchy, then the run shall be displayed at 100% of its normal width. 
Example: Consider a run of text which shall be expanded to 200% of its normal width when displaying each character within the contents of the run. This constraint is specified using the following WordprocessingML: 
&lt;w:rPr&gt; 
  &lt;w:w w:val=&quot;200&quot;/&gt; 
&lt;/w:rPr&gt;
[cit. OOXML spec.]</rdfs:comment>
        <Datatype rdf:resource="#int"/>
    </wordProcessingML>
    


    <!-- http://www.semanticweb.org/ontologies/2008/7/XCLOntology1.5.owl#watermark -->

    <generalInformation rdf:about="#watermark">
        <ID>id285</ID>
        <rdfs:comment xml:lang="en"
            >type of watermark to be used in file (digimark, stirmark etc...)</rdfs:comment>
        <Datatype rdf:resource="#string"/>
    </generalInformation>
    


    <!-- http://www.semanticweb.org/ontologies/2008/7/XCLOntology1.5.owl#webHidden -->

    <wordProcessingML rdf:about="#webHidden">
        <rdfs:comment
            >webHidden (Web Hidden Text) 
This element specifies whether the contents of this run shall be hidden from display at display time in a document when the document is being displayed in a web page view. [Note: The setting should affect the normal display of text in a web page view, but an application may have settings to force hidden text to be displayed. end note] As well, this setting should not affect a normal paginated view of the document. 
If this element is not present, the default value is to leave the formatting applied at previous level in the style hierarchy .If this element is never applied in the style hierarchy, then this text shall not be hidden when 
displayed in a document in a web page view.
Example: Consider a run of text which shall have the hidden text property turned on for the contents of the run. 
This constraint is specified using the following WordprocessingML: 
&lt;w:rPr&gt; 
  &lt;w:webHidden /&gt; 
&lt;/w:rPr&gt; 
This run declares that the webHidden property is set for the contents of this run, so the contents of this run will be hidden when the document contents are displayed in a web page view.
[cit. OOXML spec.]</rdfs:comment>
        <Datatype rdf:resource="#bool"/>
    </wordProcessingML>
    


    <!-- http://www.semanticweb.org/ontologies/2008/7/XCLOntology1.5.owl#whitePointX -->

    <rasterInformation rdf:about="#whitePointX">
        <rdfs:comment
            >chromaticity of a computer display&#39;s nominal white...</rdfs:comment>
        <ID>id28</ID>
        <is_same_as rdf:resource="#WhitePoint_Tiff"/>
        <Datatype rdf:resource="#uint32Rational"/>
    </rasterInformation>
    


    <!-- http://www.semanticweb.org/ontologies/2008/7/XCLOntology1.5.owl#whitePointY -->

    <rasterInformation rdf:about="#whitePointY">
        <rdfs:comment
            >chromaticity of a computer display&#39;s nominal white...</rdfs:comment>
        <ID>id29</ID>
        <Datatype rdf:resource="#uint32Rational"/>
    </rasterInformation>
    


    <!-- http://www.semanticweb.org/ontologies/2008/7/XCLOntology1.5.owl#widowControl -->

    <wordProcessingML rdf:about="#widowControl">
        <rdfs:comment
            >widowControl (Allow First/Last Line to Display on a Separate Page)
This element specifies whether a consumer shall prevent a single line of this paragraph from being displayed on a separate page from the remaining content at display time by moving the line onto the following page. 
When displaying a paragraph in a page, it is sometimes the case that the first line of that paragraph would display as the last line on one page, and all subsequent lines would display on the following page. This property ensures that a consumer shall move the single line to the following page as well to prevent having one line on its own page. As well, if a single line appears at the top of a page, a consumer shall move the preceding line onto the following page as well, to prevent a single line from being displayed on a separate page. 
If this element is omitted on a given paragraph, its value is determined by the setting previously set at any level of the style hierarchy (i.e. that previous setting remains unchanged). If this setting is never specified in the style hierarchy, then this paragraph shall prevent a single line from being shown on a separate page whenever it would normally occur. 
&lt;w:pPr&gt; 
  &lt;w:widowControl w:val=&quot;off&quot; /&gt;
&lt;/w:pPr&gt; 
[cit. OOXML spec.]</rdfs:comment>
        <Datatype rdf:resource="#bool"/>
    </wordProcessingML>
    


    <!-- http://www.semanticweb.org/ontologies/2008/7/XCLOntology1.5.owl#wordSpace -->

    <PDF1.3_Properties rdf:about="#wordSpace">
        <rdfs:comment
            >Set the word spacing, T w, to wordSpace, which is a number expressed in unscaled text space units. Word spacing is used by the Tj, TJ, and &#39; operators. Default value: 0. 
[cit. Pdf 1.3]</rdfs:comment>
        <Datatype rdf:resource="#int"/>
        <is_same_as rdf:resource="#wordSpacing"/>
    </PDF1.3_Properties>
    


    <!-- http://www.semanticweb.org/ontologies/2008/7/XCLOntology1.5.owl#wordSpacing -->

    <textInformation rdf:about="#wordSpacing">
        <Datatype rdf:resource="#int"/>
        <is_same_as rdf:resource="#wordSpace"/>
    </textInformation>
    


    <!-- http://www.semanticweb.org/ontologies/2008/7/XCLOntology1.5.owl#wordWrap -->

    <wordProcessingML rdf:about="#wordWrap">
        <rdfs:comment
            >wordWrap (Allow Line Breaking At Character Level) 
This element specifies whether a consumer shall break Latin text which exceeds the text extents of a line by breaking the word across two lines (breaking on the character level) or by moving the word to the following line (breaking on the word level). 
If this element is omitted on a given paragraph, its value is determined by the setting previously set at any level of the style hierarchy (i.e. that previous setting remains unchanged). If this setting is never specified in the style hierarchy, then this paragraph shall break Latin words at the word level, not the character level when it is displayed. 
[Example: Consider a paragraph whose first line ends with the word world, where the text extents for that line would normally fall between the letter o and the letter r. If this element is omitted, a producer would normally move the entire word world to the following line, since the word does not fit within the first line&#39;s text extents. 
However, if this document should allow words to be broken at the character level, that constraint would be specified as follows: 
&lt;w:pPr&gt; 
  &lt;w:wordWrap w:val=&quot;off&quot; /&gt; 
&lt;/w:pPr&gt; 
[cit. OOXML spec.]</rdfs:comment>
        <Datatype rdf:resource="#bool"/>
    </wordProcessingML>
    


    <!-- http://www.semanticweb.org/ontologies/2008/7/XCLOntology1.5.owl#xmp_Metadata -->

    <imageInformation rdf:about="#xmp_Metadata">
        <ID>id66</ID>
        <rdfs:comment xml:lang="en"
            >XML packet containing XMP metadata. (700) XMP is an extensible way to include metadata such as meaningful descriptions and titles, searchable keywords, and up-to-date author and copyright information</rdfs:comment>
        <Datatype rdf:resource="#string"/>
    </imageInformation>
    


    <!-- http://www.semanticweb.org/ontologies/2008/7/XCLOntology1.5.owl#xyPositionOfImage -->

    <otherInformation rdf:about="#xyPositionOfImage">
        <ID>id218</ID>
        <rdfs:comment xml:lang="en"
            >describes the absolute XY-Position of an Image in an animated Gif (and formats with similar features)</rdfs:comment>
        <Datatype rdf:resource="#int"/>
    </otherInformation>
    


    <!-- http://www.semanticweb.org/ontologies/2008/7/XCLOntology1.5.owl#zTXt -->

    <PNG_Properties rdf:about="#zTXt">
        <rdfs:comment xml:lang="en"
            >Text Compression</rdfs:comment>
        <is_same_as rdf:resource="#iTXt"/>
    </PNG_Properties>
    


    <!-- http://www.semanticweb.org/ontologies/2008/7/XCLOntology1.5.owl#zoomPercentage -->

    <wordProcessingML rdf:about="#zoomPercentage">
        <Unit rdf:resource="#NULL"/>
        <Datatype rdf:resource="#int"/>
    </wordProcessingML>
    


    <!-- http://www.semanticweb.org/ontologies/2008/7/XCLOntology1.5.owl#&#64258;atness -->

    <PDF1.3_Properties rdf:about="#&#64258;atness">
        <rdfs:comment
            >The precision with which curves are to be rendered on the output device (see Section 6.5.1, &#8220;Flatness Tolerance&#8221;). The value of this parameter gives the maximum error tolerance, measured in output device pixels; smaller numbers give smoother curves at the expense of more computation and memory use. Initial value: 1.0. 
[cit. Pdf 1.3]</rdfs:comment>
        <Datatype rdf:resource="#int"/>
    </PDF1.3_Properties>
    


    <!-- 
    ///////////////////////////////////////////////////////////////////////////////////////
    //
    // General axioms
    //
    ///////////////////////////////////////////////////////////////////////////////////////
     -->

    <rdf:Description>
        <rdf:type rdf:resource="&owl;AllDisjointClasses"/>
        <owl:members rdf:parseType="Collection">
            <rdf:Description rdf:about="#DOCX"/>
            <rdf:Description rdf:about="#PPTX"/>
            <rdf:Description rdf:about="#XLSX"/>
        </owl:members>
    </rdf:Description>
    <rdf:Description>
        <rdf:type rdf:resource="&owl;AllDisjointClasses"/>
        <owl:members rdf:parseType="Collection">
            <rdf:Description rdf:about="#AI_CS"/>
            <rdf:Description rdf:about="#AI_until_Version_9"/>
            <rdf:Description rdf:about="#EPS"/>
            <rdf:Description rdf:about="#SVG"/>
        </owl:members>
    </rdf:Description>
</rdf:RDF>



<!-- Generated by the OWL API (version 2.2.1.842) http://owlapi.sourceforge.net -->

